@prefix dc: <http://purl.org/dc/elements/1.1/> .
@prefix rdfs: <http://www.w3.org/2000/01/rdf-schema#> .
@prefix skos: <http://www.w3.org/2004/02/skos/core#> .

<https://vocabs.acdh.oeaw.ac.at/archeaccessrestrictions/academic> a skos:Concept ;
    dc:source "CLARIN" ;
    skos:definition "Akademischer Zugang bedeutet, dass die Zugehörigkeit an eine akademische Institution mittels Shibboleth-Login geprüft wird."@de,
        "Academic access means that an affiliation with an academic institution is checked via Shibboleth login."@en ;
    skos:inScheme <https://vocabs.acdh.oeaw.ac.at/archeaccessrestrictions/Schema> ;
    skos:prefLabel "akademisch"@de,
        "academic"@en ;
    skos:topConceptOf <https://vocabs.acdh.oeaw.ac.at/archeaccessrestrictions/Schema> .

<https://vocabs.acdh.oeaw.ac.at/archeaccessrestrictions/public> a skos:Concept ;
    dc:source "CLARIN" ;
    skos:definition "Öffentliche Ressourcen sind ohne Einschränkungen zugänglich."@de,
        "Public resources are accessible without any further restrictions."@en ;
    skos:inScheme <https://vocabs.acdh.oeaw.ac.at/archeaccessrestrictions/Schema> ;
    skos:prefLabel "öffentlich"@de,
        "public"@en ;
    skos:topConceptOf <https://vocabs.acdh.oeaw.ac.at/archeaccessrestrictions/Schema> .

<https://vocabs.acdh.oeaw.ac.at/archeaccessrestrictions/restricted> a skos:Concept ;
    dc:source "CLARIN" ;
    skos:definition "Beschränkter Zugang erfordert eine Registrierung und die Erlaubnis des Dateninhabers."@de,
        "Restricted access requires registration and an a permission from the owner."@en ;
    skos:inScheme <https://vocabs.acdh.oeaw.ac.at/archeaccessrestrictions/Schema> ;
    skos:prefLabel "eingeschränkt"@de,
        "restricted"@en ;
    skos:topConceptOf <https://vocabs.acdh.oeaw.ac.at/archeaccessrestrictions/Schema> .

<https://vocabs.acdh.oeaw.ac.at/archeaccessrestrictions/Schema> a skos:ConceptScheme ;
    rdfs:label "ARCHE Zugriffsbeschränkungen"@de,
        "ARCHE access restrictions"@en ;
    dc:creator "Martina Trognitz" ;
    dc:description "Eine Liste mit Typen von Zugriffsmöglichkeiten für ARCHE"@de,
        "A list of access restriction types for ARCHE."@en ;
    dc:format "application/rdf+xml" ;
    dc:language "English",
        "German" ;
    dc:relation <https://arche.acdh.oeaw.ac.at/browser/> ;
    dc:rights "https://creativecommons.org/licenses/by/4.0/" ;
    dc:subject "Zugriffsbeschränkung"@de,
        "access restriction"@en ;
    dc:title "ARCHE Zugriffsbeschränkungen"@de,
        "ARCHE access restrictions"@en ;
    skos:hasTopConcept <https://vocabs.acdh.oeaw.ac.at/archeaccessrestrictions/academic>,
        <https://vocabs.acdh.oeaw.ac.at/archeaccessrestrictions/public>,
        <https://vocabs.acdh.oeaw.ac.at/archeaccessrestrictions/restricted> .

