<?xml version="1.0" encoding="UTF-8"?>
<rdf:RDF
    xmlns:dct="http://purl.org/dc/terms/"
    xmlns:rdf="http://www.w3.org/1999/02/22-rdf-syntax-ns#"
    xmlns:dc="http://purl.org/dc/elements/1.1/"
    xmlns:j.0="https://vocabs.dariah.eu/bbt/"
    xmlns:owl="http://www.w3.org/2002/07/owl#"
    xmlns:skos="http://www.w3.org/2004/02/skos/core#"
    xmlns:rdfs="http://www.w3.org/2000/01/rdf-schema#"
    xmlns:xsd="http://www.w3.org/2001/XMLSchema#">
  <skos:Collection rdf:about="https://vocabs.dariah.eu/bbt/Facet/000002">
    <skos:member>
      <skos:Concept rdf:about="https://vocabs.dariah.eu/bbt/Concept/000016">
        <rdfs:type rdf:resource="http://www.w3.org/2004/02/skos/core#Concept"/>
        <dct:modified>2016-02-09T09:16:59Z</dct:modified>
        <skos:narrowMatch rdf:resource="http://www.eionet.europa.eu/gemet/concept/812"/>
        <skos:notation>000016</skos:notation>
        <skos:inScheme>
          <skos:ConceptScheme rdf:about="https://vocabs.dariah.eu/bbt/ConceptScheme/Backbone_Thesaurus">
            <dct:rights>https://creativecommons.org/licenses/by/4.0/</dct:rights>
            <dct:creator xml:lang="en">Lida Charami</dct:creator>
            <dct:issued>2017-09-01T12:00:00Z</dct:issued>
            <skos:hasTopConcept>
              <skos:Concept rdf:about="https://vocabs.dariah.eu/bbt/Concept/000008">
                <dct:dateSubmitted>2015-08-13T07:33:06Z</dct:dateSubmitted>
                <skos:scopeNote xml:lang="en">This term classifies attitudes and/or social behaviors that are expected of a person and which result from or are acquired through the relation of that person with other individuals or social groups.</skos:scopeNote>
                <skos:narrower>
                  <skos:Concept rdf:about="https://vocabs.dariah.eu/bbt/Concept/000026">
                    <dct:creator>BBT maintenance WG</dct:creator>
                    <skos:prefLabel xml:lang="en">roles of interpersonal relations</skos:prefLabel>
                    <dct:dateSubmitted>2015-08-13T07:18:40Z</dct:dateSubmitted>
                    <rdfs:type rdf:resource="http://www.w3.org/2004/02/skos/core#Concept"/>
                    <dct:modified>2016-02-09T09:16:59Z</dct:modified>
                    <skos:broader rdf:resource="https://vocabs.dariah.eu/bbt/Concept/000008"/>
                    <skos:narrowMatch rdf:resource="http://83.212.173.34:8080/THEMAS-EL-DEMOS/HUMANITIES/Concept/198"/>
                    <skos:scopeNote xml:lang="en">This term classifies attitudes and/ or behaviors that characterize the interpersonal relations of people who are linked through kinship, marriage or adoption. It also comprises the types of attitudes and/ or behaviors of people linked through religious, spiritual, friendly, rivalrous and/ or antagonistic relations.</skos:scopeNote>
                    <skos:inScheme rdf:resource="https://vocabs.dariah.eu/bbt/ConceptScheme/Backbone_Thesaurus"/>
                    <skos:notation>000026</skos:notation>
                  </skos:Concept>
                </skos:narrower>
                <skos:prefLabel xml:lang="en">roles</skos:prefLabel>
                <skos:topConceptOf rdf:resource="https://vocabs.dariah.eu/bbt/ConceptScheme/Backbone_Thesaurus"/>
                <dct:modified>2016-02-09T08:44:59Z</dct:modified>
                <skos:notation>000008</skos:notation>
                <dct:creator>BBT maintenance WG</dct:creator>
                <skos:narrower>
                  <skos:Concept rdf:about="https://vocabs.dariah.eu/bbt/Concept/000025">
                    <skos:scopeNote xml:lang="en">This term classifies official roles attributed to persons or social groups which grant rights and/or dictate obligations in relation to either the functioning of these rights and/or to the performing of administrative and management duties of institutional bodies. These properties are institutionally and socially recognized and acquire meaning only in the context of an organized community.</skos:scopeNote>
                    <skos:prefLabel xml:lang="en">offices</skos:prefLabel>
                    <skos:broader rdf:resource="https://vocabs.dariah.eu/bbt/Concept/000008"/>
                    <skos:inScheme rdf:resource="https://vocabs.dariah.eu/bbt/ConceptScheme/Backbone_Thesaurus"/>
                    <dct:creator>BBT maintenance WG</dct:creator>
                    <dct:modified>2016-02-09T09:16:59Z</dct:modified>
                    <dct:dateSubmitted>2015-08-13T07:18:40Z</dct:dateSubmitted>
                    <skos:notation>000025</skos:notation>
                  </skos:Concept>
                </skos:narrower>
                <skos:inScheme rdf:resource="https://vocabs.dariah.eu/bbt/ConceptScheme/Backbone_Thesaurus"/>
              </skos:Concept>
            </skos:hasTopConcept>
            <dct:created>2015-07-01T12:00:00Z</dct:created>
            <dct:creator xml:lang="en">Helen Goulis</dct:creator>
            <skos:hasTopConcept>
              <skos:Concept rdf:about="https://vocabs.dariah.eu/bbt/Concept/000006">
                <rdfs:type rdf:resource="http://www.w3.org/2004/02/skos/core#Concept"/>
                <skos:inScheme rdf:resource="https://vocabs.dariah.eu/bbt/ConceptScheme/Backbone_Thesaurus"/>
                <skos:exactMatch rdf:resource="http://thesauri.dainst.org/_588a9c73"/>
                <skos:narrower>
                  <skos:Concept rdf:about="https://vocabs.dariah.eu/bbt/Concept/000021">
                    <dct:creator>BBT maintenance WG</dct:creator>
                    <skos:prefLabel xml:lang="en">symbolic objects</skos:prefLabel>
                    <rdfs:type rdf:resource="http://www.w3.org/2004/02/skos/core#Concept"/>
                    <dct:modified>2016-02-09T09:16:59Z</dct:modified>
                    <skos:narrowMatch rdf:resource="http://83.212.173.34:8080/PARTHENOS-DEMO/PARTHENOS/Concept/8"/>
                    <skos:scopeNote xml:lang="en">This term classifies identifiable symbols and/or any aggregation of symbols, that have an objectively recognizable structure and that are documented as single units (sets or arrays of signs). Symbolic objects may serve to designate something, or to communicate some propositional content, but they don’t depend on what they designate or communicate. They can exist on one or more carriers simultaneously without this feature adding to or removing from the identity of the symbols. Being objectively recognizable and documented as single units, symbolic objects are independent of the material carrier and the symbolized content as well. Consequently symbolic objects may or may not have a specific meaning.</skos:scopeNote>
                    <skos:narrowMatch rdf:resource="http://83.212.173.34:8080/PARTHENOS-DEMO/PARTHENOS/Concept/10"/>
                    <skos:inScheme rdf:resource="https://vocabs.dariah.eu/bbt/ConceptScheme/Backbone_Thesaurus"/>
                    <skos:notation>000021</skos:notation>
                    <skos:narrowMatch rdf:resource="http://83.212.173.34:8080/THEMAS-EL-DEMOS/HUMANITIES/Concept/361"/>
                    <skos:note xml:lang="en">Narrower term examples: "information objects ","structural parts of information objects"</skos:note>
                    <dct:dateSubmitted>2015-08-13T07:18:40Z</dct:dateSubmitted>
                    <skos:broader rdf:resource="https://vocabs.dariah.eu/bbt/Concept/000006"/>
                  </skos:Concept>
                </skos:narrower>
                <dct:modified>2016-02-09T08:44:59Z</dct:modified>
                <skos:prefLabel xml:lang="en">conceptual objects</skos:prefLabel>
                <dct:creator>BBT maintenance WG</dct:creator>
                <dct:dateSubmitted>2015-08-13T07:33:06Z</dct:dateSubmitted>
                <skos:narrower>
                  <skos:Concept rdf:about="https://vocabs.dariah.eu/bbt/Concept/000024">
                    <skos:notation>000024</skos:notation>
                    <dct:modified>2016-02-09T09:16:59Z</dct:modified>
                    <skos:note xml:lang="en">Narrower term examples: "identity","social identity","gender identity" </skos:note>
                    <dct:creator>BBT maintenance WG</dct:creator>
                    <skos:inScheme rdf:resource="https://vocabs.dariah.eu/bbt/ConceptScheme/Backbone_Thesaurus"/>
                    <skos:scopeNote xml:lang="en">This term classifies concepts for use in categorizing and/ or systematizing aspects of our perceptible reality. These concept types express fundamental ways of viewing reality and are drawn from different conceptual contexts, each expressing a particular standpoint. They arise from the discussion and comparison of the formulation, definition and use of concepts in different disciplines. They are thus, among other things, meant to play a kind of mediating role between various disciplines and are proposed towards the end of establishing a common inter-disciplinary and inter-thematic conceptual framework.</skos:scopeNote>
                    <skos:broader rdf:resource="https://vocabs.dariah.eu/bbt/Concept/000006"/>
                    <skos:prefLabel xml:lang="en">concepts</skos:prefLabel>
                    <skos:narrowMatch rdf:resource="http://83.212.173.34:8080/THEMAS-EL-DEMOS/HUMANITIES/Concept/358"/>
                    <rdfs:type rdf:resource="http://www.w3.org/2004/02/skos/core#Concept"/>
                    <dct:dateSubmitted>2015-08-13T07:18:40Z</dct:dateSubmitted>
                  </skos:Concept>
                </skos:narrower>
                <skos:scopeNote xml:lang="en">This term classifies objects whose essence remains the same regardless of the carrier. They are products of the human activity supported by the use of technical or electronic devices (digital photos, geometric measurements etc.) or without it (concepts, thoughts). The fact that they are materially produced does not determine their identity. Conceptual objects have the ability to exist on more than one particular carrier at the same time (paper, electronic signals, photos, human memories etc.), without the latter changing or altering their identity. On the contrary, any alteration of the conceptual object itself (removal of a part, revision etc.) changes the definition of its identity. Conceptual objects exist as long as they can be found on at least one carrier (human memory included). Their existence ends when the last carrier and the last memory are lost.</skos:scopeNote>
                <skos:narrower>
                  <skos:Concept rdf:about="https://vocabs.dariah.eu/bbt/Concept/000022">
                    <dct:modified>2016-02-09T09:16:59Z</dct:modified>
                    <skos:note xml:lang="en">Narrower term examples: "information objects","structural parts of information objects"</skos:note>
                    <skos:scopeNote xml:lang="en">This term classifies mental contents produced by human activity, representing data of physical, logical or psychological realities or even fiction. These objects, though expressed by the use of symbols, do not depend on them, a fact that allows their transcription to another set of symbols. However a propositional object sometimes cannot be differentiated distinctively from the used symbols (e.g. a poem).</skos:scopeNote>
                    <skos:narrowMatch rdf:resource="http://83.212.173.34:8080/PARTHENOS-DEMO/PARTHENOS/Concept/10"/>
                    <skos:inScheme rdf:resource="https://vocabs.dariah.eu/bbt/ConceptScheme/Backbone_Thesaurus"/>
                    <skos:narrowMatch rdf:resource="http://83.212.173.34:8080/THEMAS-EL-DEMOS/HUMANITIES/Concept/260"/>
                    <skos:narrowMatch rdf:resource="http://83.212.173.34:8080/PARTHENOS-DEMO/PARTHENOS/Concept/5845"/>
                    <skos:notation>000022</skos:notation>
                    <dct:creator>BBT maintenance WG</dct:creator>
                    <skos:prefLabel xml:lang="en">propositional objects</skos:prefLabel>
                    <skos:broader rdf:resource="https://vocabs.dariah.eu/bbt/Concept/000006"/>
                    <rdfs:type rdf:resource="http://www.w3.org/2004/02/skos/core#Concept"/>
                    <dct:dateSubmitted>2015-08-13T07:18:40Z</dct:dateSubmitted>
                  </skos:Concept>
                </skos:narrower>
                <skos:narrowMatch rdf:resource="http://83.212.173.34:8080/PARTHENOS-DEMO/PARTHENOS/Concept/5&quot;"/>
                <skos:notation>000006</skos:notation>
                <skos:topConceptOf rdf:resource="https://vocabs.dariah.eu/bbt/ConceptScheme/Backbone_Thesaurus"/>
                <skos:narrower>
                  <skos:Concept rdf:about="https://vocabs.dariah.eu/bbt/Concept/000023">
                    <rdfs:type rdf:resource="http://www.w3.org/2004/02/skos/core#Concept"/>
                    <dct:dateSubmitted>2015-08-13T07:18:40Z</dct:dateSubmitted>
                    <skos:notation>000023</skos:notation>
                    <skos:inScheme rdf:resource="https://vocabs.dariah.eu/bbt/ConceptScheme/Backbone_Thesaurus"/>
                    <skos:note xml:lang="en">Narrower term examples: "procedures","techniques"</skos:note>
                    <skos:scopeNote xml:lang="en">This term classifies systems of specifications, restrictions and regulations about the design (this involves setting the principles, specifying the requirements and the means for achieving the desired result, estimating the consequences and the expected outcome) and/or the performance of the necessary activities (application of the selected principles and rules, provision and activation of the means and requirements for the realization of the chosen goals,  re-estimation of the consequences) in order to achieve certain results of a specific type.</skos:scopeNote>
                    <skos:narrowMatch rdf:resource="http://www.eionet.europa.eu/gemet/concept/210"/>
                    <dct:creator>BBT maintenance WG</dct:creator>
                    <dct:modified>2016-02-09T09:16:59Z</dct:modified>
                    <skos:narrowMatch rdf:resource="http://83.212.173.34:8080/PARTHENOS-DEMO/PARTHENOS/Concept/6"/>
                    <skos:narrowMatch rdf:resource="http://83.212.173.34:8080/THEMAS-EL-DEMOS/HUMANITIES/Concept/346"/>
                    <skos:prefLabel xml:lang="en">methods</skos:prefLabel>
                    <skos:broader rdf:resource="https://vocabs.dariah.eu/bbt/Concept/000006"/>
                  </skos:Concept>
                </skos:narrower>
              </skos:Concept>
            </skos:hasTopConcept>
            <dct:creator xml:lang="en">Makis Chrisovitsanos</dct:creator>
            <dct:issued>2018-09-12T15:14:34Z</dct:issued>
            <skos:hasTopConcept>
              <skos:Concept rdf:about="https://vocabs.dariah.eu/bbt/Concept/000003">
                <skos:narrowMatch rdf:resource="http://www.eionet.europa.eu/gemet/concept/5184"/>
                <skos:narrowMatch rdf:resource="http://www.eionet.europa.eu/gemet/concept/11791"/>
                <skos:topConceptOf rdf:resource="https://vocabs.dariah.eu/bbt/ConceptScheme/Backbone_Thesaurus"/>
                <skos:narrowMatch rdf:resource="http://www.eionet.europa.eu/gemet/concept/52"/>
                <skos:narrowMatch rdf:resource="http://www.eionet.europa.eu/gemet/concept/5912"/>
                <skos:note xml:lang="en"></skos:note>
                <skos:narrowMatch rdf:resource="http://www.eionet.europa.eu/gemet/concept/7401"/>
                <rdfs:type rdf:resource="http://www.w3.org/2004/02/skos/core#Concept"/>
                <skos:narrowMatch rdf:resource="http://www.eionet.europa.eu/gemet/concept/4839"/>
                <dct:modified>2016-02-09T08:44:59Z</dct:modified>
                <skos:narrowMatch rdf:resource="http://thesauri.dainst.org/_e3a93fec"/>
                <skos:notation>000003</skos:notation>
                <skos:narrowMatch rdf:resource="http://www.eionet.europa.eu/gemet/concept/11792"/>
                <skos:inScheme rdf:resource="https://vocabs.dariah.eu/bbt/ConceptScheme/Backbone_Thesaurus"/>
                <skos:scopeNote xml:lang="en">This term classifies physical substances that  are constituents of material objects or are used in their construction, but whose individual substance is not a factor in the objects’ function (e.g. gold, water, bricks, etc.) The term may include pure raw materials, processed or unprocessed, and also materials that have been modelled and are incorporated into objects. Their main attribute is that they cannot be individualized, that is, they cannot be distinct "units" with clear and distinct boundaries or roles in respect to other units of the same or different kind.</skos:scopeNote>
                <skos:narrowMatch rdf:resource="http://www.eionet.europa.eu/gemet/concept/5756"/>
                <skos:narrowMatch rdf:resource="http://www.eionet.europa.eu/gemet/concept/14619"/>
                <skos:narrowMatch rdf:resource="http://83.212.173.34:8080/THEMAS-EL-DEMOS/HUMANITIES/Concept/130"/>
                <skos:narrowMatch rdf:resource="http://thesauri.dainst.org/c_f8c9d94f"/>
                <dct:creator>BBT maintenance WG</dct:creator>
                <skos:narrowMatch rdf:resource="http://www.eionet.europa.eu/gemet/concept/11793"/>
                <skos:narrowMatch rdf:resource="http://www.eionet.europa.eu/gemet/concept/6918"/>
                <skos:prefLabel xml:lang="en">materials</skos:prefLabel>
                <skos:narrowMatch rdf:resource="http://www.eionet.europa.eu/gemet/concept/4519"/>
                <skos:narrowMatch rdf:resource="http://www.eionet.europa.eu/gemet/concept/4523"/>
                <dct:dateSubmitted>2015-08-13T07:33:06Z</dct:dateSubmitted>
                <skos:narrowMatch rdf:resource="http://www.eionet.europa.eu/gemet/concept/4493"/>
                <skos:narrowMatch rdf:resource="http://www.eionet.europa.eu/gemet/concept/5978"/>
                <skos:narrowMatch rdf:resource="http://www.eionet.europa.eu/gemet/concept/2643"/>
              </skos:Concept>
            </skos:hasTopConcept>
            <skos:hasTopConcept>
              <skos:Concept rdf:about="https://vocabs.dariah.eu/bbt/Concept/000005">
                <skos:scopeNote xml:lang="el">Περιλαμβάνει τύπους πολιτισμικών, κοινωνικών, διανοητικών φαινομένων που χαρακτηρίζονται από συνοχή δημιουργώντας νοητές ενότητες. Η συνοχή αυτή συγκροτείται λόγω της παρουσίασης ενός τουλάχιστον ποιοτικού στοιχείου που εμφανίζουν σύνολα φαινόμενων χωροχρονικά οριοθετημένων. Η χωροχρονική οριοθέτηση αποτελεί μορφικό χαρακτηριστικό του θέματος «Εποχές», δεν αναφέρεται δηλαδή σε συγκεκριμένες πραγματώσεις του θέματος αυτού. Κατά συνέπεια, στο θέμα αυτό δεν περιλαμβάνονται τα στιγμιότυπα εποχώνόπως η Αναγέννηση ή η Ρωμαϊκή περίοδος, ή η περίοδος των βαλκανικών πολέμων κτλ., αλλά οι τύποι κατηγοριοποίησής τους, δηλαδή οι αφηρημένες έννοιες, βάσει των οποίων είναι δυνατός ο εν γένει προσδιορισμός της συνοχής στην εμφάνιση πολιτισμικών, κοινωνικών και διανοητικών φαινομένων.</skos:scopeNote>
                <skos:notation>000005</skos:notation>
                <dct:creator>BBT maintenance WG</dct:creator>
                <dct:modified>2016-02-09T08:44:59Z</dct:modified>
                <skos:topConceptOf rdf:resource="https://vocabs.dariah.eu/bbt/ConceptScheme/Backbone_Thesaurus"/>
                <skos:note xml:lang="en">Narrower term examples: "geological epochs", "epochs of Art", "epochs of technology"</skos:note>
                <dct:dateSubmitted>2015-08-13T07:33:06Z</dct:dateSubmitted>
                <skos:prefLabel xml:lang="el">εποχές</skos:prefLabel>
                <skos:inScheme rdf:resource="https://vocabs.dariah.eu/bbt/ConceptScheme/Backbone_Thesaurus"/>
                <skos:prefLabel xml:lang="en">types of epochs</skos:prefLabel>
                <skos:scopeNote xml:lang="en">This term classifies cultural, social, intellectual phenomena consistent with each other thus creating intelligible unities. These phenomena are spatially and temporally limited and their consistency relies on the appearance of at least one qualitative element that links them in a unity. The spatial and temporal restriction is a formal feature of the facet “types of epochs”. That means that this term has no reference to specific realizations of these types of phenomena. Consequently, this term does not include time periods such as the Renaissance or the Roman period, or the period of the Balkan wars etc., but their categorization, i.e. the abstract concepts by virtue of which it is possible to conceive the cultural, social and intellectual phenomena as coherent.  </skos:scopeNote>
              </skos:Concept>
            </skos:hasTopConcept>
            <dct:title xml:lang="en">Backbone Thesaurus</dct:title>
            <dct:subject xml:lang="en">materials</dct:subject>
            <dct:creator xml:lang="en">BBT maintenance WG</dct:creator>
            <dct:description xml:lang="en">The top-level thesaurus proposed in DARIAH</dct:description>
            <dct:creator xml:lang="en">Maria Daskalaki</dct:creator>
            <dct:creator xml:lang="en">Martin Doerr</dct:creator>
            <owl:versionInfo>v1.2</owl:versionInfo>
            <dct:creator xml:lang="en">Helen Katsiadaki</dct:creator>
            <dct:language>Greek</dct:language>
            <dct:creator xml:lang="en">Chryssoula Bekiari</dct:creator>
            <dct:subject xml:lang="en">activities</dct:subject>
            <dct:creator xml:lang="en">Hella Hollander</dct:creator>
            <dct:creator xml:lang="en">Wolfgang Schmidle</dct:creator>
            <skos:hasTopConcept>
              <skos:Concept rdf:about="https://vocabs.dariah.eu/bbt/Concept/000002">
                <skos:narrower>
                  <skos:Concept rdf:about="https://vocabs.dariah.eu/bbt/Concept/000015">
                    <skos:scopeNote xml:lang="en">This term classifies changes in states, things and entities that can be attributed to activity of natural phenomena and whose effect is such as to cause the dissolution or modification of the subject of these changes to the degree that their identity is destroyed.  </skos:scopeNote>
                    <skos:prefLabel xml:lang="en">natural disasters</skos:prefLabel>
                    <skos:broader rdf:resource="https://vocabs.dariah.eu/bbt/Concept/000002"/>
                    <skos:inScheme rdf:resource="https://vocabs.dariah.eu/bbt/ConceptScheme/Backbone_Thesaurus"/>
                    <dct:creator>BBT maintenance WG</dct:creator>
                    <dct:modified>2016-02-09T09:16:59Z</dct:modified>
                    <dct:dateSubmitted>2015-08-13T07:18:40Z</dct:dateSubmitted>
                    <skos:notation>000015</skos:notation>
                  </skos:Concept>
                </skos:narrower>
                <skos:scopeNote xml:lang="en">This term classifies changes in states of affairs, things and entities that result from natural phenomena (e.g. earthquakes, floods).</skos:scopeNote>
                <skos:topConceptOf rdf:resource="https://vocabs.dariah.eu/bbt/ConceptScheme/Backbone_Thesaurus"/>
                <skos:prefLabel xml:lang="en">natural processes</skos:prefLabel>
                <skos:narrower rdf:resource="https://vocabs.dariah.eu/bbt/Concept/000016"/>
                <skos:inScheme rdf:resource="https://vocabs.dariah.eu/bbt/ConceptScheme/Backbone_Thesaurus"/>
                <dct:dateSubmitted>2015-08-13T07:33:06Z</dct:dateSubmitted>
                <skos:notation>000002</skos:notation>
                <dct:creator>BBT maintenance WG</dct:creator>
                <dct:modified>2016-02-09T08:44:59Z</dct:modified>
              </skos:Concept>
            </skos:hasTopConcept>
            <dct:creator xml:lang="en">Iraklitos Souyioultzoglou</dct:creator>
            <skos:hasTopConcept>
              <skos:Concept rdf:about="https://vocabs.dariah.eu/bbt/Concept/000001">
                <skos:scopeNote xml:lang="en">This term classifies intentional actions that result in the preservation, creation, production, modification or destruction of an entity (living beings, conceptual/material objects, groups, social, intellectual, physical etc. phenomena).</skos:scopeNote>
                <skos:topConceptOf rdf:resource="https://vocabs.dariah.eu/bbt/ConceptScheme/Backbone_Thesaurus"/>
                <dct:modified>2016-02-09T08:44:59Z</dct:modified>
                <skos:narrower>
                  <skos:Concept rdf:about="https://vocabs.dariah.eu/bbt/Concept/000013">
                    <skos:inScheme rdf:resource="https://vocabs.dariah.eu/bbt/ConceptScheme/Backbone_Thesaurus"/>
                    <skos:narrowMatch rdf:resource="http://83.212.173.34:8080/THEMAS-EL-DEMOS/HUMANITIES/Concept/102"/>
                    <dct:dateSubmitted>2015-08-13T07:18:40Z</dct:dateSubmitted>
                    <dct:creator>BBT maintenance WG</dct:creator>
                    <skos:narrowMatch rdf:resource="http://83.212.173.34:8080/PARTHENOS-DEMO/PARTHENOS/Concept/5828"/>
                    <skos:note> Narrower term examples: "governance" </skos:note>
                    <skos:prefLabel xml:lang="en">functions</skos:prefLabel>
                    <dct:modified>2016-02-09T09:16:59Z</dct:modified>
                    <skos:scopeNote xml:lang="en">This term classifies activities that are structural parts of a relatively stable complex system of permanent and self-contained procedures that repeat themselves within this system and thus contribute to its preservation. Although functions are part of a wider system, each function is completely distinct from the rest. As structural parts of a complex system, functions are actions that play a certain role within a system and aim at a specific goal, which they must accomplish. In this respect it is not possible that the purpose which a certain function has to achieve is different from that for which the function is performed. In other words, the purpose of a function is one of its identity criteria. Consequently, the notion of the function univocally relates the actions performed and the target achieved by these actions in such a way that, if some other target is achieved due to external factors, we speak of a different function or activity. </skos:scopeNote>
                    <skos:scopeNote xml:lang="el">Η ιεραρχία αυτή περιλαμβάνει ενέργειες που αποτελούν δομικά μέρη ενός σχετικά σταθερά διαρθρωμένου συστήματος (διαδικασιών, οργανισμών, μηχανισμών) μόνιμων και αλληλοεξαρτώμενων διεργασιών που επαναλαμβάνονται στο πλαίσιο αυτού του συστήματος και συντελούν έτσι στη διατήρησή του. Παρόλο που οι λειτουργίες είναι μέρη ενός ευρύτερου συστήματος, κάθε επιμέρους λειτουργία είναι απολύτως διακριτή από κάθε άλλη.Ως δομικά μέρη ενός διαρθρωμένου συστήματος, οι λειτουργίες είναι ενέργειες που έχουν ένα συγκεκριμένο ρόλο στο εσωτερικό του συστήματος και αποσκοπούν σε έναν ορισμένο σκοπό, τον οποίο πρέπει να εκπληρώσουν. Με αυτή την έννοια, δεν είναι δυνατόν ο σκοπός, τον οποίο εκπληρώνουν αυτές οι ενέργειες, να είναι διαφορετικός από τον σκοπό για τον οποίο επιτελούνται∙ με άλλα λόγια, ένα από τα κριτήρια ταυτότητας της λειτουργίας είναι ο σκοπός της.Η έννοια της λειτουργίας συνδέει, άρα, με μονοσήμαντο τρόπο τις σχέσεις των ενεργειών που επιτελούνται και του στόχου που επιτυγχάνουν οι ενέργειες αυτές, ώστε, όταν προκύψει από την παρεμβολή κάποιου άλλου τυχαίου παράγοντα ένας άλλος σκοπός από τον επιδιωκόμενο, να μιλάμε για άλλη λειτουργία ή για άλλη δραστηριότητα.Στον ορισμό της λειτουργίας δεν ενδιαφέρουν ούτε τα βήματα των δραστηριοτήτων για την εκπλήρωση ενός σκοπού, ούτε η μέθοδος, δηλαδή οι περιορισμοί που επιβάλλονται προκειμένου να επιτευχθεί ο σκοπός αυτός.</skos:scopeNote>
                    <skos:notation>000013</skos:notation>
                    <skos:prefLabel xml:lang="el">λειτουργίες</skos:prefLabel>
                    <rdfs:type rdf:resource="http://www.w3.org/2004/02/skos/core#Concept"/>
                    <skos:broader rdf:resource="https://vocabs.dariah.eu/bbt/Concept/000001"/>
                  </skos:Concept>
                </skos:narrower>
                <skos:narrower>
                  <skos:Concept rdf:about="https://vocabs.dariah.eu/bbt/Concept/000010">
                    <skos:prefLabel xml:lang="el">τομείς απασχόλησης</skos:prefLabel>
                    <skos:inScheme rdf:resource="https://vocabs.dariah.eu/bbt/ConceptScheme/Backbone_Thesaurus"/>
                    <skos:narrowMatch rdf:resource="http://www.eionet.europa.eu/gemet/concept/429"/>
                    <dct:dateSubmitted>2015-08-13T07:18:40Z</dct:dateSubmitted>
                    <skos:scopeNote xml:lang="en">This term classifies professional or potentially professional areas of employment, that are socially and/ or legally recognized on the basis of the criteria of self-coherence, the efficacy of the practices they employ, the adoption of common methods and the ability to transfer knowledge and expertise in the relevant professional sector. Each sector includes types of activities that point to a certain unity of action characteristic of some sort of professional or potentially potential specialization. The specialization may relate to the production or modification of material objects, the conception and understanding of activities or phenomena, the provision /transfer of services, knowledge and know-how and the creation of works and phenomena with aesthetic value. Note: It is important to clarify that the terms classified in the “disciplines” term  should not be confused with the actor who performs an act or the results of his activity or the method used in order to achieve this result. The actor as “the efficient cause”, the result as “the final cause” and the method as the sum of the rules and constraints that an actor follows in order to perform an act, are different terms which belong to different facets and hierarchies. When determining the activities classified in the “Disciplines” hierarchy we should not confuse the history of a specific discipline ie the specific temporal and spatial environment in which this discipline appeared and was perceived with the type of activities characterizing this discipline.</skos:scopeNote>
                    <skos:note xml:lang="en">Narrower term examples: "construction of material objects and installations", "conception and comprehension of phenomena", "provision of knowledge and expertise",  "production of works and/or phenomena of aesthetic value"</skos:note>
                    <skos:broader rdf:resource="https://vocabs.dariah.eu/bbt/Concept/000001"/>
                    <skos:exactMatch rdf:resource="http://thesauri.dainst.org/_6e11e02c"/>
                    <skos:notation>000010</skos:notation>
                    <rdfs:type rdf:resource="http://www.w3.org/2004/02/skos/core#Concept"/>
                    <dct:modified>2016-02-09T09:16:59Z</dct:modified>
                    <skos:narrowMatch rdf:resource="http://83.212.173.34:8080/THEMAS-EL-DEMOS/HUMANITIES/Concept/148"/>
                    <dct:creator>BBT maintenance WG</dct:creator>
                    <skos:scopeNote xml:lang="el">Περιλαμβάνει τομείς επαγγελματικής ή δυνάμει επαγγελματικής απασχόλησης, κοινωνικά ή/και νομικά αποδεκτής βάσει των κριτηρίων της αυτοτέλειας του κάθε τομέα, της αποτελεσματικότητας της πρακτικής που εφαρμόζει, της υιοθέτησης κοινών μεθόδων και της δυνατότητας μεταβίβασης της γνώσης και της τεχνογνωσίας του εκάστοτε επαγγελματικού τομέα. Ο κάθε τομέας περιέχει τύπους ενεργειών που δημιουργούν ενότητες, οι οποίες εκφράζουν μια μορφή επαγγελματικής ή δυνάμει επαγγελματικής εξειδίκευσης. Η εξειδίκευση αυτή μπορεί να αφορά στην κατασκευή ή αλλαγή υλικών αντικειμένων, στη σύλληψη και κατανόηση ενεργειών ή φαινομένων, στην παροχή, στη μεταφορά/ μεταβίβαση υπηρεσιών, γνώσης και τεχνογνωσίας και στην παραγωγή έργων και φαινομένων με αισθητική αξία. Γενικές παρατηρήσεις: α) Θα πρέπει να είναι απολύτως σαφές ότι οι όροι τους οποίους προσδιορίζουμε στην ιεραρχία αυτή αφορούν τύπους ενεργειών και δεν πρέπει να συγχέονται ούτε με τον δράστη, ούτε με το αποτέλεσμα της ενέργειας, ούτε με τη διαδικασία που οδηγεί στο συγκεκριμένο αποτέλεσμα. Ο δράστης, ως το ποιητικό αίτιο, το αποτέλεσμα ως το τελικό αίτιο και η διαδικασία ως το σύνολο των περιορισμών και κανόνων, η εφαρμογή των οποίων κρίνεται ότι οδηγεί σε ένα συγκεκριμένο αποτέλεσμα, αποτελούν ξεχωριστούς όρους που ανήκουν σε διαφορετικές ιεραρχίες και θέματα. β) Στον προσδιορισμό δραστηριοτήτων και την κατάταξή τους στους αντίστοιχους ειδικότερους όρους, θα πρέπει να μην συγχέουμε την ιστορία ενός τομέα απασχόλησης, δηλαδή το συγκεκριμένο πλαίσιο στο οποίο ο τομέας αυτός εμφανίζεται και προσλαμβάνεται, με τον τύπο των ενεργειών που χαρακτηρίζουν τον τομέα αυτόν.</skos:scopeNote>
                    <skos:prefLabel xml:lang="en">disciplines</skos:prefLabel>
                    <skos:narrowMatch rdf:resource="http://83.212.173.34:8080/PARTHENOS-DEMO/PARTHENOS/Concept/5827"/>
                  </skos:Concept>
                </skos:narrower>
                <skos:narrowMatch rdf:resource="http://www.eionet.europa.eu/gemet/concept/1320"/>
                <skos:narrowMatch rdf:resource="http://thesauri.dainst.org/_4dc296b2"/>
                <rdfs:type rdf:resource="http://www.w3.org/2004/02/skos/core#Concept"/>
                <skos:narrower>
                  <skos:Concept rdf:about="https://vocabs.dariah.eu/bbt/Concept/000012">
                    <skos:scopeNote xml:lang="en">This term classifies intentional activities aimed at causing the end of the existence of entities and states of affairs. </skos:scopeNote>
                    <skos:prefLabel xml:lang="en">intentional destructions</skos:prefLabel>
                    <skos:broader rdf:resource="https://vocabs.dariah.eu/bbt/Concept/000001"/>
                    <skos:inScheme rdf:resource="https://vocabs.dariah.eu/bbt/ConceptScheme/Backbone_Thesaurus"/>
                    <dct:creator>BBT maintenance WG</dct:creator>
                    <dct:modified>2016-02-09T09:16:59Z</dct:modified>
                    <dct:dateSubmitted>2015-08-13T07:18:40Z</dct:dateSubmitted>
                    <skos:notation>000012</skos:notation>
                  </skos:Concept>
                </skos:narrower>
                <skos:inScheme rdf:resource="https://vocabs.dariah.eu/bbt/ConceptScheme/Backbone_Thesaurus"/>
                <skos:prefLabel xml:lang="en">activities</skos:prefLabel>
                <skos:narrower>
                  <skos:Concept rdf:about="https://vocabs.dariah.eu/bbt/Concept/000014">
                    <skos:narrowMatch rdf:resource="http://83.212.173.34:8080/THEMAS-EL-DEMOS/HUMANITIES/Concept/145"/>
                    <rdfs:type rdf:resource="http://www.w3.org/2004/02/skos/core#Concept"/>
                    <dct:creator>BBT maintenance WG</dct:creator>
                    <skos:notation>000014</skos:notation>
                    <skos:prefLabel xml:lang="en">other activities</skos:prefLabel>
                    <dct:dateSubmitted>2015-08-13T07:18:40Z</dct:dateSubmitted>
                    <skos:broader rdf:resource="https://vocabs.dariah.eu/bbt/Concept/000001"/>
                    <skos:inScheme rdf:resource="https://vocabs.dariah.eu/bbt/ConceptScheme/Backbone_Thesaurus"/>
                    <dct:modified>2016-02-09T09:16:59Z</dct:modified>
                    <skos:scopeNote xml:lang="en"> </skos:scopeNote>
                  </skos:Concept>
                </skos:narrower>
                <skos:narrowMatch rdf:resource="http://www.eionet.europa.eu/gemet/concept/1874"/>
                <skos:narrowMatch rdf:resource="http://www.eionet.europa.eu/gemet/concept/1899"/>
                <skos:notation>000001</skos:notation>
                <dct:creator>BBT maintenance WG</dct:creator>
                <dct:dateSubmitted>2015-08-13T07:33:06Z</dct:dateSubmitted>
                <skos:narrower>
                  <skos:Concept rdf:about="https://vocabs.dariah.eu/bbt/Concept/000011">
                    <dct:dateSubmitted>2015-08-13T07:18:40Z</dct:dateSubmitted>
                    <skos:narrowMatch rdf:resource="http://83.212.173.34:8080/THEMAS-EL-DEMOS/HUMANITIES/Concept/232"/>
                    <skos:inScheme rdf:resource="https://vocabs.dariah.eu/bbt/ConceptScheme/Backbone_Thesaurus"/>
                    <skos:notation>000011</skos:notation>
                    <rdfs:type rdf:resource="http://www.w3.org/2004/02/skos/core#Concept"/>
                    <dct:creator>BBT maintenance WG</dct:creator>
                    <skos:prefLabel xml:lang="en">human interactions</skos:prefLabel>
                    <dct:modified>2016-02-09T09:16:59Z</dct:modified>
                    <skos:narrowMatch rdf:resource="http://83.212.173.34:8080/THEMAS-EL-DEMOS/HUMANITIES/Concept/643"/>
                    <skos:note xml:lang="en">Narrower term examples: "social events, confrontations or conflicts", "political", "social and economic occurrences", "group management"</skos:note>
                    <skos:scopeNote xml:lang="en">This term classifies intentional activities carried out by at least one actor causing or changing phenomena or states of affairs on the social, political, financial, cultural and intellectual level.</skos:scopeNote>
                    <skos:broader rdf:resource="https://vocabs.dariah.eu/bbt/Concept/000001"/>
                  </skos:Concept>
                </skos:narrower>
              </skos:Concept>
            </skos:hasTopConcept>
            <dct:subject xml:lang="en">conceptual objects</dct:subject>
            <dct:subject xml:lang="en">humanities</dct:subject>
            <dct:language>English</dct:language>
            <skos:hasTopConcept>
              <skos:Concept rdf:about="https://vocabs.dariah.eu/bbt/Concept/000004">
                <skos:prefLabel xml:lang="en">material things</skos:prefLabel>
                <dct:modified>2016-02-09T08:44:59Z</dct:modified>
                <skos:notation>000004</skos:notation>
                <dct:dateSubmitted>2015-08-13T07:33:06Z</dct:dateSubmitted>
                <skos:inScheme rdf:resource="https://vocabs.dariah.eu/bbt/ConceptScheme/Backbone_Thesaurus"/>
                <skos:narrower>
                  <skos:Concept rdf:about="https://vocabs.dariah.eu/bbt/Concept/000020">
                    <dct:creator>BBT maintenance WG</dct:creator>
                    <skos:note xml:lang="en">Narrower term examples: "strings", "bases (object components)"</skos:note>
                    <skos:notation>000020</skos:notation>
                    <skos:scopeNote xml:lang="en">This class classifies objects especially constructed to be parts of a complex material object. These objects have autonomy in relation to the complex object of the appropriate type, to which they are intended to be added. Despite their autonomy, however, they are not independent in terms of their intended function, but are structural parts of the object, ie they have a specific function within the module to which they belong and which they form. Note: The structural parts of the material things are not considered narrower terms of the aggregation to which they belong. </skos:scopeNote>
                    <skos:broader rdf:resource="https://vocabs.dariah.eu/bbt/Concept/000004"/>
                    <skos:narrowMatch rdf:resource="http://83.212.173.34:8080/THEMAS-EL-DEMOS/HUMANITIES/Concept/146"/>
                    <rdfs:type rdf:resource="http://www.w3.org/2004/02/skos/core#Concept"/>
                    <dct:dateSubmitted>2015-08-13T07:18:40Z</dct:dateSubmitted>
                    <skos:inScheme rdf:resource="https://vocabs.dariah.eu/bbt/ConceptScheme/Backbone_Thesaurus"/>
                    <dct:modified>2016-02-09T09:16:59Z</dct:modified>
                    <skos:prefLabel xml:lang="en">structural parts of material objects</skos:prefLabel>
                  </skos:Concept>
                </skos:narrower>
                <dct:creator>BBT maintenance WG</dct:creator>
                <skos:narrower>
                  <skos:Concept rdf:about="https://vocabs.dariah.eu/bbt/Concept/000018">
                    <skos:broader rdf:resource="https://vocabs.dariah.eu/bbt/Concept/000004"/>
                    <dct:modified>2016-02-09T09:16:59Z</dct:modified>
                    <skos:narrowMatch rdf:resource="http://83.212.173.34:8080/THEMAS-EL-DEMOS/HUMANITIES/Concept/725"/>
                    <skos:inScheme rdf:resource="https://vocabs.dariah.eu/bbt/ConceptScheme/Backbone_Thesaurus"/>
                    <rdfs:type rdf:resource="http://www.w3.org/2004/02/skos/core#Concept"/>
                    <skos:narrowMatch rdf:resource="http://83.212.173.34:8080/THEMAS-EL-DEMOS/HUMANITIES/Concept/158"/>
                    <skos:prefLabel xml:lang="en">built environment</skos:prefLabel>
                    <skos:narrowMatch rdf:resource="http://www.eionet.europa.eu/gemet/concept/13193"/>
                    <skos:note xml:lang="en">Narrower term examples: "single built works", "complexes", "infrastructure", "residential areas"</skos:note>
                    <dct:creator>BBT maintenance WG</dct:creator>
                    <skos:scopeNote xml:lang="en">This term classifies structures, simple or complex, regardless of their size, duration of construction or use, that are attached or embedded in the ground and cannot be moved without irreversible damage.</skos:scopeNote>
                    <skos:notation>000018</skos:notation>
                    <dct:dateSubmitted>2015-08-13T07:18:40Z</dct:dateSubmitted>
                    <skos:narrowMatch rdf:resource="http://www.eionet.europa.eu/gemet/concept/13136"/>
                  </skos:Concept>
                </skos:narrower>
                <skos:narrower>
                  <skos:Concept rdf:about="https://vocabs.dariah.eu/bbt/Concept/000017">
                    <dct:creator>BBT maintenance WG</dct:creator>
                    <skos:prefLabel xml:lang="en">mobile objects</skos:prefLabel>
                    <skos:scopeNote xml:lang="en">This term classifies material things that result from human endeavor, have aesthetic, cultural, historical, scientific, or other utilitarian value, and are by design or through collecting portable functional entities. </skos:scopeNote>
                    <skos:inScheme rdf:resource="https://vocabs.dariah.eu/bbt/ConceptScheme/Backbone_Thesaurus"/>
                    <dct:dateSubmitted>2015-08-13T07:18:40Z</dct:dateSubmitted>
                    <skos:narrowMatch rdf:resource="http://83.212.173.34:8080/THEMAS-EL-DEMOS/HUMANITIES/Concept/283"/>
                    <skos:note xml:lang="en">Narrower term examples:"stelae", "anvils"</skos:note>
                    <skos:broader rdf:resource="https://vocabs.dariah.eu/bbt/Concept/000004"/>
                    <skos:notation>000017</skos:notation>
                    <dct:modified>2016-02-09T09:16:59Z</dct:modified>
                    <rdfs:type rdf:resource="http://www.w3.org/2004/02/skos/core#Concept"/>
                  </skos:Concept>
                </skos:narrower>
                <skos:scopeNote xml:lang="en">This term classifies things with physical substance that constitute complete units and have a relatively stable form with identifiable boundaries in at least one dimension. Such units can be natural or man-made (with regard to origin), simple or complex (with regard to composition) or consist of parts. In this latter case it is possible that the parts are either distinct and independent from the unit of which they are a part (e.g. a cave on a mountain) or that they have to be defined with reference to the sum of the parts (e.g. chess-chessmen).</skos:scopeNote>
                <skos:narrower>
                  <skos:Concept rdf:about="https://vocabs.dariah.eu/bbt/Concept/000019">
                    <skos:note xml:lang="en">Narrower term examples: "reliefs ", "granules"</skos:note>
                    <dct:modified>2016-02-09T09:16:59Z</dct:modified>
                    <skos:scopeNote xml:lang="en">This term classifies specific formations that are integrally adapted to certain material objects. They cannot, therefore, be separated from the carrier-object, but they also do not identify with it, since it is only a part of the carrier-object that carries the entire feature. In this sense, the feature is fixed, with respect to the carrier-object, while any attempt to remove it will result in the loss of part of the carrier-object. They may have two- or three-dimensional geometric extent, but there are no natural borders that separate them completely, in an objective way from the carrier-objects. Instances of Physical Features can be features in a narrower sense (scratches, holes, reliefs, surface colours etc.), while in the wider sense, they are portions of particular objects with borders that are not absolutely defined, such as the core of the Earth or the head of a marble statue.</skos:scopeNote>
                    <skos:inScheme rdf:resource="https://vocabs.dariah.eu/bbt/ConceptScheme/Backbone_Thesaurus"/>
                    <dct:creator>BBT maintenance WG</dct:creator>
                    <skos:narrowMatch rdf:resource="http://83.212.173.34:8080/THEMAS-EL-DEMOS/HUMANITIES/Concept/183"/>
                    <dct:dateSubmitted>2015-08-13T07:18:40Z</dct:dateSubmitted>
                    <skos:broader rdf:resource="https://vocabs.dariah.eu/bbt/Concept/000004"/>
                    <skos:prefLabel xml:lang="en">physical features</skos:prefLabel>
                    <skos:notation>000019</skos:notation>
                    <rdfs:type rdf:resource="http://www.w3.org/2004/02/skos/core#Concept"/>
                  </skos:Concept>
                </skos:narrower>
                <skos:topConceptOf rdf:resource="https://vocabs.dariah.eu/bbt/ConceptScheme/Backbone_Thesaurus"/>
              </skos:Concept>
            </skos:hasTopConcept>
            <skos:hasTopConcept>
              <skos:Concept rdf:about="https://vocabs.dariah.eu/bbt/Concept/000009">
                <rdfs:type rdf:resource="http://www.w3.org/2004/02/skos/core#Concept"/>
                <skos:topConceptOf rdf:resource="https://vocabs.dariah.eu/bbt/ConceptScheme/Backbone_Thesaurus"/>
                <skos:notation>000009</skos:notation>
                <skos:prefLabel xml:lang="en">geopolitical units</skos:prefLabel>
                <skos:scopeNote xml:lang="en">This term classifies administrative divisions used by a state or other sovereign or political structure within the boundaries of its jurisdiction. Intrinsic features of these units include, among others, the extent of the area over which they are applied/exercised, the chronological extent during which they are in force, their governing bodies and the degree of autonomy they are granted in relation to managing and exploiting of their resources.</skos:scopeNote>
                <skos:inScheme rdf:resource="https://vocabs.dariah.eu/bbt/ConceptScheme/Backbone_Thesaurus"/>
                <dct:dateSubmitted>2015-08-13T07:33:06Z</dct:dateSubmitted>
                <skos:narrowMatch rdf:resource="http://83.212.173.34:8080/THEMAS-EL-DEMOS/HUMANITIES/Concept/280"/>
                <dct:creator>BBT maintenance WG</dct:creator>
                <dct:modified>2016-02-09T08:44:59Z</dct:modified>
              </skos:Concept>
            </skos:hasTopConcept>
            <skos:hasTopConcept>
              <skos:Concept rdf:about="https://vocabs.dariah.eu/bbt/Concept/000007">
                <skos:inScheme rdf:resource="https://vocabs.dariah.eu/bbt/ConceptScheme/Backbone_Thesaurus"/>
                <dct:creator>BBT maintenance WG</dct:creator>
                <skos:narrowMatch rdf:resource="http://83.212.173.34:8080/THEMAS-EL-DEMOS/HUMANITIES/Concept/309"/>
                <rdfs:type rdf:resource="http://www.w3.org/2004/02/skos/core#Concept"/>
                <skos:topConceptOf rdf:resource="https://vocabs.dariah.eu/bbt/ConceptScheme/Backbone_Thesaurus"/>
                <dct:modified>2016-02-09T08:44:59Z</dct:modified>
                <dct:dateSubmitted>2015-08-13T07:33:06Z</dct:dateSubmitted>
                <skos:notation>000007</skos:notation>
                <skos:narrowMatch rdf:resource="http://83.212.173.34:8080/PARTHENOS-DEMO/PARTHENOS/Concept/5829"/>
                <skos:note xml:lang="en">Narrower term examples: "ethnicities", "political parties", "artistic groups", "groups of demonstrators".</skos:note>
                <skos:prefLabel xml:lang="en">groups and collectivities</skos:prefLabel>
                <skos:scopeNote xml:lang="en">This term classifies relations of whatever character (economic, religious, athletic, political, national etc.) that arise from the joint actions of at least two people. These relations should be based on the adoption of common beliefs, traditions, objectives and/or actions as well as showing organizational features.</skos:scopeNote>
              </skos:Concept>
            </skos:hasTopConcept>
            <dct:creator xml:lang="en">Georgia Papadopoulou</dct:creator>
            <dct:modified>2017-09-01T12:00:00Z</dct:modified>
            <dct:subject xml:lang="en">geopolitical units</dct:subject>
            <dct:subject xml:lang="en">processes</dct:subject>
            <dct:creator xml:lang="en">Vanessa Hannesschläger</dct:creator>
            <dct:format>application/rdf+xml</dct:format>
            <dct:subject xml:lang="en">roles</dct:subject>
          </skos:ConceptScheme>
        </skos:inScheme>
        <skos:prefLabel xml:lang="en">geneses</skos:prefLabel>
        <dct:creator>BBT maintenance WG</dct:creator>
        <dct:dateSubmitted>2015-08-13T07:18:40Z</dct:dateSubmitted>
        <skos:scopeNote xml:lang="en">This term classifies changes in states of affairs, things and entities that result from natural phenomena and lead either to a) the creation of new states of affairs/things/entities or b) to the modification of already existing states of affairs/things/entities with the overall effect that their former identity is lost and they are transformed into new entities with a fundamentally different nature. </skos:scopeNote>
        <skos:broader rdf:resource="https://vocabs.dariah.eu/bbt/Concept/000002"/>
      </skos:Concept>
    </skos:member>
    <skos:member rdf:resource="https://vocabs.dariah.eu/bbt/Concept/000015"/>
    <skos:member rdf:resource="https://vocabs.dariah.eu/bbt/Concept/000002"/>
    <skos:scopeNote xml:lang="en">This facet comprises types of changes in states of affairs, things and entities that result from natural phenomena (e.g. earthquakes, floods).</skos:scopeNote>
    <skos:inScheme rdf:resource="https://vocabs.dariah.eu/bbt/ConceptScheme/Backbone_Thesaurus"/>
    <dct:creator xml:lang="en">BBT maintenance WG</dct:creator>
    <skos:prefLabel xml:lang="en">Natural Processes</skos:prefLabel>
    <rdf:type rdf:resource="https://vocabs.dariah.eu/bbt/Facet"/>
  </skos:Collection>
  <j.0:Facet rdf:about="https://vocabs.dariah.eu/bbt/Facet/000006">
    <skos:scopeNote xml:lang="en">This facet comprises types of objects whose essence remains the same regardless of the carrier. They are products of the human activity supported by the use of technical or electronic devices (digital photos, geometric measurements etc.) or without it (concepts, thoughts). The fact that they are materially produced does not determine their identity. Conceptual objects have the ability to exist on more than one particular carrier at the same time (paper, electronic signals, photos, human memories etc.), without the latter changing or altering their identity. On the contrary, any alteration of the conceptual object itself (removal of a part, revision etc.) changes the definition of its identity. Conceptual objects exist as long as they can be found on at least one carrier (human memory included). Their existence ends when the last carrier and the last memory are lost. </skos:scopeNote>
    <skos:member rdf:resource="https://vocabs.dariah.eu/bbt/Concept/000022"/>
    <skos:prefLabel xml:lang="en">Conceptual Objects</skos:prefLabel>
    <skos:member rdf:resource="https://vocabs.dariah.eu/bbt/Concept/000023"/>
    <skos:member rdf:resource="https://vocabs.dariah.eu/bbt/Concept/000021"/>
    <dct:creator xml:lang="en">BBT maintenance WG</dct:creator>
    <skos:member rdf:resource="https://vocabs.dariah.eu/bbt/Concept/000006"/>
    <rdf:type rdf:resource="http://www.w3.org/2004/02/skos/core#Collection"/>
    <skos:member rdf:resource="https://vocabs.dariah.eu/bbt/Concept/000024"/>
    <skos:inScheme rdf:resource="https://vocabs.dariah.eu/bbt/ConceptScheme/Backbone_Thesaurus"/>
  </j.0:Facet>
  <skos:Collection rdf:about="https://vocabs.dariah.eu/bbt/Facet/000004">
    <skos:inScheme rdf:resource="https://vocabs.dariah.eu/bbt/ConceptScheme/Backbone_Thesaurus"/>
    <skos:member rdf:resource="https://vocabs.dariah.eu/bbt/Concept/000017"/>
    <skos:member rdf:resource="https://vocabs.dariah.eu/bbt/Concept/000018"/>
    <dct:creator xml:lang="en">BBT maintenance WG</dct:creator>
    <skos:member rdf:resource="https://vocabs.dariah.eu/bbt/Concept/000019"/>
    <skos:member rdf:resource="https://vocabs.dariah.eu/bbt/Concept/000020"/>
    <skos:member rdf:resource="https://vocabs.dariah.eu/bbt/Concept/000004"/>
    <rdf:type rdf:resource="https://vocabs.dariah.eu/bbt/Facet"/>
    <skos:prefLabel xml:lang="en">Material Things</skos:prefLabel>
    <skos:scopeNote xml:lang="en">The Material Things facet comprises types of things with physical substance that constitute complete units and have a relatively stable form with identifiable boundaries in at least one dimension. Such units can be natural or man-made (with regard to origin), simple or complex (with regard to composition) or consist of parts. In this latter case it is possible that the parts are either distinct and independent from the unit of which they are a part (e.g. a cave on a mountain) or that they have to be defined with reference to the sum of the parts (e.g. chess-chessmen). </skos:scopeNote>
  </skos:Collection>
  <skos:Collection rdf:about="https://vocabs.dariah.eu/bbt/Facet/000008">
    <skos:member rdf:resource="https://vocabs.dariah.eu/bbt/Concept/000026"/>
    <skos:member rdf:resource="https://vocabs.dariah.eu/bbt/Concept/000025"/>
    <skos:member rdf:resource="https://vocabs.dariah.eu/bbt/Concept/000008"/>
    <skos:scopeNote xml:lang="en">This facet comprises the types of attitudes and/or social behaviors that are expected of a person and which result from or are acquired through the relation of that person with other individuals or social groups.</skos:scopeNote>
    <skos:inScheme rdf:resource="https://vocabs.dariah.eu/bbt/ConceptScheme/Backbone_Thesaurus"/>
    <dct:creator xml:lang="en">BBT maintenance WG</dct:creator>
    <skos:prefLabel xml:lang="en">Roles</skos:prefLabel>
    <rdf:type rdf:resource="https://vocabs.dariah.eu/bbt/Facet"/>
  </skos:Collection>
  <rdf:Description rdf:about="https://vocabs.dariah.eu/bbt/Facet/">
    <rdfs:subClassOf rdf:resource="http://www.w3.org/2004/02/skos/core#Collection"/>
    <skos:scopeNote xml:lang="en"> grouping of concepts of the same inherent category</skos:scopeNote>
  </rdf:Description>
  <skos:Collection rdf:about="https://vocabs.dariah.eu/bbt/Facet/000001">
    <skos:member rdf:resource="https://vocabs.dariah.eu/bbt/Concept/000012"/>
    <skos:member rdf:resource="https://vocabs.dariah.eu/bbt/Concept/000011"/>
    <skos:member rdf:resource="https://vocabs.dariah.eu/bbt/Concept/000014"/>
    <dct:creator xml:lang="en">BBT maintenance WG</dct:creator>
    <skos:member rdf:resource="https://vocabs.dariah.eu/bbt/Concept/000013"/>
    <skos:member rdf:resource="https://vocabs.dariah.eu/bbt/Concept/000001"/>
    <skos:member rdf:resource="https://vocabs.dariah.eu/bbt/Concept/000010"/>
    <skos:prefLabel xml:lang="en">Activities</skos:prefLabel>
    <skos:inScheme rdf:resource="https://vocabs.dariah.eu/bbt/ConceptScheme/Backbone_Thesaurus"/>
    <rdf:type rdf:resource="https://vocabs.dariah.eu/bbt/Facet"/>
    <skos:scopeNote xml:lang="en">The “Activities” facet comprises types of intentional actions that result in the preservation, creation, production, modification or destruction of an entity (living beings, conceptual/material objects, groups, social, intellectual, physical etc. phenomena). Note: It is important to note that actions that are unintentional are excluded from this facet. Such actions may result from natural processes (natural disasters, geneses, changes due to natural causes), the non-conscious actions of subjects (e.g. the actions of people that are under the influence of drugs) as well as coerced actions performed in conditions that deprive persons of their free will. The fundamental criterion for the exclusion of these kinds of actions from the “activity” facet is the will, the ability of a subject to choose his purpose according to his judgment. Insofar as the will is the criterion for the determination of an action, the notion of “purpose” is the starting point for building the hierarchies of the “activity” facet. </skos:scopeNote>
  </skos:Collection>
  <skos:Collection rdf:about="https://vocabs.dariah.eu/bbt/Facet/000005">
    <skos:member rdf:resource="https://vocabs.dariah.eu/bbt/Concept/000005"/>
    <skos:scopeNote xml:lang="el">Περιλαμβάνει τύπους πολιτισμικών, κοινωνικών, διανοητικών φαινομένων που χαρακτηρίζονται από συνοχή δημιουργώντας νοητές ενότητες. Η συνοχή αυτή συγκροτείται λόγω της παρουσίασης ενός τουλάχιστον ποιοτικού στοιχείου που εμφανίζουν σύνολα φαινόμενων χωροχρονικά οριοθετημένων. Η χωροχρονική οριοθέτηση αποτελεί μορφικό χαρακτηριστικό του θέματος «Εποχές», δεν αναφέρεται δηλαδή σε συγκεκριμένες πραγματώσεις του θέματος αυτού. Κατά συνέπεια, στο θέμα αυτό δεν περιλαμβάνονται τα στιγμιότυπα εποχώνόπως η Αναγέννηση ή η Ρωμαϊκή περίοδος, ή η περίοδος των βαλκανικών πολέμων κτλ., αλλά οι τύποι κατηγοριοποίησής τους, δηλαδή οι αφηρημένες έννοιες, βάσει των οποίων είναι δυνατός ο εν γένει προσδιορισμός της συνοχής στην εμφάνιση πολιτισμικών, κοινωνικών και διανοητικών φαινομένων.</skos:scopeNote>
    <skos:scopeNote xml:lang="en">This facet comprises types of cultural, social, intellectual phenomena consistent with each other thus creating intelligible unities. These types of phenomena are spatially and temporally limited and their consistency relies on the appearance of at least one qualitative element that links them in a unity. The spatial and temporal restriction is a formal feature of the facet “types of epochs”. That means that the facet “types of epochs” has no reference to specific realizations of these types of phenomena. Consequently, this facet does not include time periods such as the Renaissance or the Roman period, or the period of the Balkan wars etc., but the types of their categorization, i.e. the abstract concepts by virtue of which it is possible to conceive the cultural, social and intellectual phenomena as coherent. </skos:scopeNote>
    <skos:inScheme rdf:resource="https://vocabs.dariah.eu/bbt/ConceptScheme/Backbone_Thesaurus"/>
    <dct:creator xml:lang="en">BBT maintenance WG</dct:creator>
    <skos:prefLabel xml:lang="el">Εποχές</skos:prefLabel>
    <skos:prefLabel xml:lang="en">Types of Epochs</skos:prefLabel>
    <rdf:type rdf:resource="https://vocabs.dariah.eu/bbt/Facet"/>
  </skos:Collection>
  <skos:Collection rdf:about="https://vocabs.dariah.eu/bbt/Facet/000003">
    <skos:member rdf:resource="https://vocabs.dariah.eu/bbt/Concept/000003"/>
    <skos:scopeNote xml:lang="en">This facet comprises types of physical substances that are constituents of material objects or are used in their construction, but whose individual substance is not a factor in the objects’ function (eg gold, water, bricks, etc.) The facet may include pure raw materials, processed or unprocessed, and also materials that have been modelled and are incorporated into objects. Their main attribute is that they cannot be individualized, that is, they cannot be distinct "units" with clear and distinct boundaries or roles in respect to other units of the same or different kind.</skos:scopeNote>
    <skos:inScheme rdf:resource="https://vocabs.dariah.eu/bbt/ConceptScheme/Backbone_Thesaurus"/>
    <dct:creator xml:lang="en">BBT maintenance WG</dct:creator>
    <skos:prefLabel xml:lang="en">Materials</skos:prefLabel>
    <rdf:type rdf:resource="https://vocabs.dariah.eu/bbt/Facet"/>
  </skos:Collection>
  <skos:Collection rdf:about="https://vocabs.dariah.eu/bbt/Facet/000009">
    <skos:member rdf:resource="https://vocabs.dariah.eu/bbt/Concept/000009"/>
    <skos:scopeNote xml:lang="en">This facet comprises types of administrative divisions used by a state or other sovereign or political structure within the boundaries of its jurisdiction. Intrinsic features of these units include, among others, the extent of the area over which they are applied/exercised, the chronological extent during which they are in force, their governing bodies and the degree of autonomy they are granted in relation to managing and exploiting of their resources.</skos:scopeNote>
    <skos:inScheme rdf:resource="https://vocabs.dariah.eu/bbt/ConceptScheme/Backbone_Thesaurus"/>
    <dct:creator xml:lang="en">BBT maintenance WG</dct:creator>
    <skos:prefLabel xml:lang="en">Geopolitical Units</skos:prefLabel>
    <rdf:type rdf:resource="https://vocabs.dariah.eu/bbt/Facet"/>
  </skos:Collection>
  <skos:Collection rdf:about="https://vocabs.dariah.eu/bbt/Facet/000007">
    <skos:member rdf:resource="https://vocabs.dariah.eu/bbt/Concept/000007"/>
    <skos:scopeNote xml:lang="en">This facet comprises relations of whatever character (economic, religious, athletic, political, national etc.) that arise from the joint actions of at least two people. These relations should be based on the adoption of common beliefs, traditions, objectives and/or actions as well as showing organizational features.</skos:scopeNote>
    <skos:inScheme rdf:resource="https://vocabs.dariah.eu/bbt/ConceptScheme/Backbone_Thesaurus"/>
    <dct:creator xml:lang="en">BBT maintenance WG</dct:creator>
    <skos:prefLabel xml:lang="en">Groups and Collectivities</skos:prefLabel>
    <rdf:type rdf:resource="https://vocabs.dariah.eu/bbt/Facet"/>
  </skos:Collection>
</rdf:RDF>
