<?xml version="1.0" encoding="UTF-8"?>
<rdf:RDF
   xmlns:dcterms="http://purl.org/dc/terms/"
   xmlns:owl="http://www.w3.org/2002/07/owl#"
   xmlns:rdf="http://www.w3.org/1999/02/22-rdf-syntax-ns#"
   xmlns:rdfs="http://www.w3.org/2000/01/rdf-schema#"
   xmlns:skos="http://www.w3.org/2004/02/skos/core#"
>
  <rdf:Description rdf:about="https://vocabs.dariah.eu/bbt/Facet/000004">
    <skos:member rdf:resource="https://vocabs.dariah.eu/bbt/Concept/000004"/>
    <rdf:type rdf:resource="http://www.w3.org/2004/02/skos/core#Collection"/>
    <skos:prefLabel xml:lang="el">Υλικά Αντικείμενα</skos:prefLabel>
    <skos:member rdf:resource="https://vocabs.dariah.eu/bbt/Concept/000017"/>
    <skos:scopeNote xml:lang="fr">Cette facette désigne les types d’entités dotées d’une substance physique qui constitue des unités complètes et qui ont une forme aux contours relativement stables et comportant au moins une dimension. Ces unités peuvent être naturelles ou faites par l’homme (en ce qui concerne leur origine), simples ou complexes (en ce qui concerne leur composition) ou consister en parties. Ces parties peuvent être distinctes et indépendantes de l’unité dont elles font partie (par exemple une grotte dans une montagne) ou peuvent être définies comme la somme de leur parties (les échecs / les pièces du jeu d’échecs).</skos:scopeNote>
    <rdf:type rdf:resource="https://vocabs.dariah.eu/bbt/Facet"/>
    <skos:prefLabel xml:lang="fr">Entités Matérielles</skos:prefLabel>
    <dcterms:creator xml:lang="en">BBT maintenance WG</dcterms:creator>
    <skos:member rdf:resource="https://vocabs.dariah.eu/bbt/Concept/000019"/>
    <skos:prefLabel xml:lang="en">Material Things</skos:prefLabel>
    <skos:scopeNote xml:lang="en">The Material Things facet comprises types of things with physical substance that constitute complete units and have a relatively stable form with identifiable boundaries in at least one dimension. Such units can be natural or man-made (with regard to origin), simple or complex (with regard to composition) or consist of parts. In this latter case it is possible that the parts are either distinct and independent from the unit of which they are a part (e.g. a cave on a mountain) or that they have to be defined with reference to the sum of the parts (e.g. chess-chessmen).</skos:scopeNote>
    <skos:scopeNote xml:lang="el">Το θέμα αυτό περιλαμβάνει οτιδήποτε άψυχο που έχει υλική υπόσταση, αποτελεί μια ολοκληρωμένη μονάδα και έχει μια σχετική σταθερότητα μορφής με αναγνωρίσιμα όρια. Τέτοιες μονάδες μπορεί να είναι φυσικές ή δημιουργημένες (ως προς τη προέλευση), απλές ή σύνθετες (ως προς τη σύσταση) και να αποτελούνται από μέρη. Στην τελευταία περίπτωση, είναι πιθανό τα μέρη να είναι διακριτά και να προσδιορίζονται ανεξάρτητα από τη μονάδα της οποίας είναι μέρος (π.χ. μια σπηλιά σε ένα βουνό) ή να απαιτείται για τον προσδιορισμό τους η αναφορά στο σύνολο των μερών (π.χ. σκάκι-πιόνια).</skos:scopeNote>
    <skos:member rdf:resource="https://vocabs.dariah.eu/bbt/Concept/000020"/>
    <skos:prefLabel xml:lang="de">Materielle Objekte</skos:prefLabel>
    <skos:scopeNote xml:lang="de">Die Facette “Materielle Objekte” beinhaltet Typen von Objekten mit physischer Substanz, die eine vollkommene Einheit bilden, mit einer relativ stabilen Form und identifizierbaren Grenzen in wenigstens einer Dimension. Diese Einheiten können einen natürlichen oder anthropogenen Ursprung haben, können eine einfache oder komplexe Zusammensetzung aufweisen oder aus mehreren Teilen bestehen. In letzterem Fall können die Teile entweder verschieden und unabhängig von der Einheit sein von dem sie Teil sind (z. B. Höhle in einem Berg) oder müssen in Bezug auf die Gesamtheit des Objektes definiert werden (z. B. Schach - Schachfigur).</skos:scopeNote>
    <skos:member rdf:resource="https://vocabs.dariah.eu/bbt/Concept/000018"/>
    <skos:inScheme rdf:resource="https://vocabs.dariah.eu/bbt/ConceptScheme/Backbone_Thesaurus"/>
  </rdf:Description>
  <rdf:Description rdf:about="https://vocabs.dariah.eu/bbt/Concept/000015">
    <dcterms:dateSubmitted>2015-08-13T07:18:40Z</dcterms:dateSubmitted>
    <skos:prefLabel xml:lang="de">Naturkatastrophen</skos:prefLabel>
    <skos:prefLabel xml:lang="el">φυσικές καταστροφές</skos:prefLabel>
    <skos:scopeNote xml:lang="de">Dieser Term umfasst Veränderungen in Zuständen, Dingen und Entitäten, die auf Aktivitäten natürlicher Phänomene zurückzuführen sind und deren Auswirkung die Auflösung oder Modifikation des veränderten Objektes in einem solchen Maße erwirken können, dass das Objekt in seiner Identität vollständig zerstört werden kann.</skos:scopeNote>
    <dcterms:creator xml:lang="en">BBT maintenance WG</dcterms:creator>
    <skos:prefLabel xml:lang="en">natural disasters</skos:prefLabel>
    <skos:prefLabel xml:lang="fr">catastrophes naturelles</skos:prefLabel>
    <skos:scopeNote xml:lang="en">This term classifies changes in states, things and entities that can be attributed to activity of natural phenomena and whose effect is such as to cause the dissolution or modification of the subject of these changes to the degree that their identity is destroyed.</skos:scopeNote>
    <skos:broader rdf:resource="https://vocabs.dariah.eu/bbt/Concept/000002"/>
    <rdf:type rdf:resource="http://www.w3.org/2004/02/skos/core#Concept"/>
    <skos:scopeNote xml:lang="fr">Ce terme désigne les changements de situation, d'objets ou d’entités pouvant être attribués à l’activité de phénomènes naturels et dont l’effet est de causer une dissolution ou une modification telles  que l'identité du sujet des ces changements en est détruite.</skos:scopeNote>
    <skos:scopeNote xml:lang="el">Η ιεραρχία αυτή περιλαμβάνει αλλαγές καταστάσεων, πραγμάτων ή οντοτήτων που αποδίδονται στην επενέργεια φυσικών αιτιών, τα οποία προκαλούν τον αφανισμό τους ή τη μετατροπή τους σε τέτοιο βαθμό, ώστε να χάνουν την ταυτότητά τους.</skos:scopeNote>
    <skos:exactMatch rdf:resource="https://humanitiesthesaurus.academyofathens.gr/dyas-resource/Concept/14"/>
    <rdfs:type rdf:resource="http://www.w3.org/2004/02/skos/core#Concept"/>
    <dcterms:modified>2019-04-10T10:55:10Z</dcterms:modified>
    <skos:narrowMatch rdf:resource="https://ark.frantiq.fr/ark:/26678/pcrtZnKEOuwY05"/>
    <skos:notation>000015</skos:notation>
  </rdf:Description>
  <rdf:Description rdf:about="https://vocabs.dariah.eu/bbt/Facet/000001">
    <skos:scopeNote xml:lang="en">The “Activities” facet comprises types of intentional actions that result in the preservation, creation, production, modification or destruction of an entity (living beings, conceptual/material objects, groups, social, intellectual, physical etc. phenomena). Note: It is important to note that actions that are unintentional are excluded from this facet. Such actions may result from natural processes (natural disasters, geneses, changes due to natural causes), the non-conscious actions of subjects (e.g. the actions of people that are under the influence of drugs) as well as coerced actions performed in conditions that deprive persons of their free will. The fundamental criterion for the exclusion of these kinds of actions from the “activity” facet is the will, the ability of a subject to choose his purpose according to his judgment. Insofar as the will is the criterion for the determination of an action, the notion of “purpose” is the starting point for building the hierarchies of the “activity” facet.</skos:scopeNote>
    <rdf:type rdf:resource="https://vocabs.dariah.eu/bbt/Facet"/>
    <skos:member rdf:resource="https://vocabs.dariah.eu/bbt/Concept/000001"/>
    <dcterms:creator xml:lang="en">BBT maintenance WG</dcterms:creator>
    <skos:member rdf:resource="https://vocabs.dariah.eu/bbt/Concept/000013"/>
    <skos:scopeNote xml:lang="el">Το θέμα αυτό περιλαμβάνει εμπρόθετες ενέργειες, οι οποίες οδηγούν στη διατήρηση, τη δημιουργία, την καταστροφή ή τη μεταβολή μιας κατάστασης ή μιας οντότητας (έμβιων όντων, πνευματικών προϊόντων, φυσικών στοιχείων, ομάδων, συγκροτημάτων, πολιτισμικών, κοινωνικών ή πνευματικών φαινομένων κτλ.), και οι οποίες τεκμηριώνονται.

Παρατηρήσεις: Είναι σημαντικό να τονιστεί ότι από αυτή τη θεματική ενότητα αποκλείονται όλες οι μη-εμπρόθετες ενέργειες είτε αυτές προέρχονται από φυσικές διεργασίες (φυσικές καταστροφές, γενέσεις, αλλαγές που προκύπτουν από φυσικά αίτια) είτε είναι μη-συνειδητές ενέργειες ενός υποκειμένου (ενέργειες που γίνονται υπό την επήρεια παραισθησιογόνων φαρμάκων, ποτών κτλ.) είτε είναι ενέργειες που προκύπτουν από καταναγκασμό (ενέργειες που προκύπτουν από τον εξαναγκασμό του υποκειμένου σε συνθήκες που του στερείται η δυνατότητα να επιλέξει). Ο αποκλεισμός αυτών των περιπτώσεων από το θέμα «Δραστηριότητες» οφείλεται στο γεγονός ότι θεμελιώδες κριτήριο για τον προσδιορισμό της δραστηριότητας θεωρείται η βούληση, η ικανότητα δηλαδή του υποκείμενου να επιλέγει τον σκοπό του σύμφωνα με τη κρίση του. Εφόσον το κριτήριο για τον προσδιορισμό του θέματος «Δραστηριότητες» είναι η πρόθεση, η έννοια «σκοπός» αποτελεί τη βάση για τον ορισμό των ιεραρχιών</skos:scopeNote>
    <skos:member rdf:resource="https://vocabs.dariah.eu/bbt/Concept/000012"/>
    <skos:prefLabel xml:lang="de">Aktivitäten</skos:prefLabel>
    <skos:member rdf:resource="https://vocabs.dariah.eu/bbt/Concept/000010"/>
    <skos:member rdf:resource="https://vocabs.dariah.eu/bbt/Concept/000011"/>
    <skos:prefLabel xml:lang="fr">Activités</skos:prefLabel>
    <skos:scopeNote xml:lang="de">Die „Aktivitäten“ Facette beinhaltet Typen intentioneller Aktionen, die in der Erhaltung, Herstellung, Modifikation oder Zerstörung einer Entität (Lebewesen; konzeptionelle/materielle Objekte; Gruppen; soziale, intellektuelle, physische Phänomene usw.) resultieren.
Notiz: Es ist wichtig festzuhalten, dass unbeabsichtigte Handlungen von dieser Facette ausgenommen sind. Solche Handlungen können sich aus äußeren Faktoren (Naturkatastrophen, Genese usw. aufgrund natürlicher Ursachen), unbewussten Aktionen von Personen (z. B. Handlungen von Personen unter dem Einfluss von Drogen) wie auch aus erzwungenen Aktionen von Personen, die ihres freien Willens entmachten wurden, ergeben. Das grundlegende Kriterium für den Ausschluss dieser Art von Handlungen aus der Facette „Aktivitäten“ ist der Wille und die Möglichkeit des ausführenden Subjekts den Zweck seiner Aktivität aufgrund seines Urteilsvermögens zu erkennen. Da der Wille das Kriterium für die Bestimmung einer Aktion ist, bildet das Konzept der "Absicht" den Ausgangspunkt für den Aufbau der Hierarchien der Facette „Aktivitäten“.</skos:scopeNote>
    <skos:prefLabel xml:lang="en">Activities</skos:prefLabel>
    <rdf:type rdf:resource="http://www.w3.org/2004/02/skos/core#Collection"/>
    <skos:prefLabel xml:lang="el">Δραστηριότητες</skos:prefLabel>
    <skos:inScheme rdf:resource="https://vocabs.dariah.eu/bbt/ConceptScheme/Backbone_Thesaurus"/>
    <skos:scopeNote xml:lang="fr">La facette "Activités" désigne les types d'actions intentionnelles qui entraînent la conservation, la création, la production, la modification ou la destruction d’une entité (être vivant, objet conceptuel ou matériel, groupes, phénomènes sociaux, intellectuels, physiques etc.)
Note : Il est important de noter que les actions non intentionnelles n’entrent pas dans cette catégorie. Ces dernières actions peuvent résulter de processus naturels (catastrophes naturelles, genèses, changements dus à des causes naturelles), d'actions non-conscientes de sujets (par exemples les actions de personnes sous l'influence de drogues), d'actions contraintes accomplies par des personnes privées de leur libre arbitre. Le critère fondamental pour exclure ces types d'action de la facette "Activités" est la volonté, la capacité du sujet à définir son objectif en fonction de son jugement. Dans la mesure où la volonté est le critère pour la détermination d'une action, la notion d’objectif est le point de départ pour la construction des hiérarchies de la facette "Activités"</skos:scopeNote>
  </rdf:Description>
  <rdf:Description rdf:about="https://vocabs.dariah.eu/bbt/Concept/000024">
    <skos:prefLabel xml:lang="de">Konzepte</skos:prefLabel>
    <skos:broader rdf:resource="https://vocabs.dariah.eu/bbt/Concept/000006"/>
    <skos:prefLabel xml:lang="en">concepts</skos:prefLabel>
    <skos:note xml:lang="en">Narrower term examples: "identity","social identity","gender identity"</skos:note>
    <rdf:type rdf:resource="http://www.w3.org/2004/02/skos/core#Concept"/>
    <dcterms:dateSubmitted>2015-08-13T07:18:40Z</dcterms:dateSubmitted>
    <skos:prefLabel xml:lang="fr">concepts</skos:prefLabel>
    <skos:scopeNote xml:lang="el">Η ιεραρχία αυτή περιλαμβάνει τύπους εννοιών ως τρόπων θεώρησης ή/και συστηματοποίησης πλευρών της πραγματικότητας που προσλαμβάνουμε. Οι έννοιες ως τύποι εκφράζουν θεμελιώδεις τρόπους θέασης της πραγματικότητας και συνάγονται από επιμέρους εννοιολογικά πλαίσια, τα οποία εκφράζουν κάθε φορά μια συγκεκριμένη σκοπιά. Οι τύποι εννοιών προκύπτουν από τη συζήτηση και σύγκριση του σχηματισμού, του ορισμού και της χρήσης εννοιών από διαφορετικά επιστημονικά πεδία. Έχουν έτσι, μεταξύ άλλων, ένα είδος διαμεσολαβητικού ρόλου ανάμεσα σε διάφορες επιστήμες και τείνουν με αυτόν τον τρόπο στη διαμόρφωση ενός κοινού διεπιστημονικού και διαθεματικού εννοιολογικού πλαισίου.</skos:scopeNote>
    <skos:scopeNote xml:lang="fr">Ce terme désigne les concepts utilisés pour catégoriser et/ou systématiser les aspects de notre réalité sensible. Ils expriment les façons fondamentales de voir la réalité et sont tirés de différents contextes conceptuels, chacun exprimant un point de vue particulier. Ils résultent de la discussion et de la comparaison de la formulation, définition et utilisation des concepts dans différentes disciplines. Ils sont donc, entre autres, destinés à jouer un rôle de médiation entre les différentes disciplines et sont proposés dans le but d’établir un cadre conceptuel interdisciplinaire et inter-thématique.</skos:scopeNote>
    <skos:notation>000024</skos:notation>
    <rdfs:type rdf:resource="http://www.w3.org/2004/02/skos/core#Concept"/>
    <skos:exactMatch rdf:resource="http://thesauri.dainst.org/_dfdb34ff"/>
    <skos:scopeNote xml:lang="de">Unter diesem Term sind Konzepte klassifiziert, die zur Kategorisierung und/oder Systematisierung von Aspekten unserer wahrnehmbaren Realität dienen. Diese Typen von Konzepten drücken fundamentale Wege der Realitätswahrnehmung aus und rühren von unterschiedlichen konzeptionellen Kontexten, die alle eine eigene Sichtweise vertreten. Sie entstehen aus der Diskussion und aus dem Vergleich mit Formulierungen, Definitionen und dem Gebrauch dieser Konzepte in verschiedenen Disziplinen. Daher spielen sie unter anderem eine Vermittlerrolle zwischen verschiedenen Disziplinen und schaffen einen interdisziplinären und interthematischen konzeptionellen Rahmen.</skos:scopeNote>
    <skos:exactMatch rdf:resource="https://humanitiesthesaurus.academyofathens.gr/dyas-resource/Concept/28"/>
    <skos:prefLabel xml:lang="el">έννοιες</skos:prefLabel>
    <dcterms:modified>2019-04-10T10:55:17Z</dcterms:modified>
    <skos:scopeNote xml:lang="en">This term classifies concepts for use in categorizing and/ or systematizing aspects of our perceptible reality. These concept types express fundamental ways of viewing reality and are drawn from different conceptual contexts, each expressing a particular standpoint. They arise from the discussion and comparison of the formulation, definition and use of concepts in different disciplines. They are thus, among other things, meant to play a kind of mediating role between various disciplines and are proposed towards the end of establishing a common inter-disciplinary and inter-thematic conceptual framework.</skos:scopeNote>
    <dcterms:creator xml:lang="en">BBT maintenance WG</dcterms:creator>
  </rdf:Description>
  <rdf:Description rdf:about="https://vocabs.dariah.eu/bbt/Concept/000019">
    <skos:narrowMatch rdf:resource="https://isl.ics.forth.gr/parthenos_vocabularies/Concept/32813"/>
    <skos:narrowMatch rdf:resource="https://isl.ics.forth.gr/parthenos_vocabularies/Concept/32952"/>
    <skos:narrowMatch rdf:resource="https://isl.ics.forth.gr/parthenos_vocabularies/Concept/32758"/>
    <dcterms:modified>2019-04-10T10:55:14Z</dcterms:modified>
    <skos:narrowMatch rdf:resource="https://isl.ics.forth.gr/parthenos_vocabularies/Concept/32693"/>
    <skos:narrowMatch rdf:resource="https://isl.ics.forth.gr/parthenos_vocabularies/Concept/32908"/>
    <skos:narrowMatch rdf:resource="https://isl.ics.forth.gr/parthenos_vocabularies/Concept/32894"/>
    <skos:narrowMatch rdf:resource="https://isl.ics.forth.gr/parthenos_vocabularies/Concept/32623"/>
    <skos:narrowMatch rdf:resource="https://isl.ics.forth.gr/parthenos_vocabularies/Concept/32411"/>
    <skos:narrowMatch rdf:resource="https://isl.ics.forth.gr/parthenos_vocabularies/Concept/32396"/>
    <skos:narrowMatch rdf:resource="https://isl.ics.forth.gr/parthenos_vocabularies/Concept/32264"/>
    <skos:narrowMatch rdf:resource="https://isl.ics.forth.gr/parthenos_vocabularies/Concept/32701"/>
    <skos:narrowMatch rdf:resource="https://isl.ics.forth.gr/parthenos_vocabularies/Concept/32449"/>
    <skos:narrowMatch rdf:resource="https://isl.ics.forth.gr/parthenos_vocabularies/Concept/32255"/>
    <skos:narrowMatch rdf:resource="https://isl.ics.forth.gr/parthenos_vocabularies/Concept/32509"/>
    <skos:narrowMatch rdf:resource="https://isl.ics.forth.gr/parthenos_vocabularies/Concept/32407"/>
    <skos:narrowMatch rdf:resource="https://isl.ics.forth.gr/parthenos_vocabularies/Concept/32231"/>
    <skos:narrowMatch rdf:resource="https://isl.ics.forth.gr/parthenos_vocabularies/Concept/32490"/>
    <skos:narrowMatch rdf:resource="https://isl.ics.forth.gr/parthenos_vocabularies/Concept/32786"/>
    <skos:narrowMatch rdf:resource="https://isl.ics.forth.gr/parthenos_vocabularies/Concept/32428"/>
    <skos:narrowMatch rdf:resource="https://isl.ics.forth.gr/parthenos_vocabularies/Concept/32933"/>
    <skos:narrowMatch rdf:resource="https://isl.ics.forth.gr/parthenos_vocabularies/Concept/32809"/>
    <skos:narrowMatch rdf:resource="https://isl.ics.forth.gr/parthenos_vocabularies/Concept/32729"/>
    <skos:narrowMatch rdf:resource="https://isl.ics.forth.gr/parthenos_vocabularies/Concept/32905"/>
    <skos:narrowMatch rdf:resource="https://isl.ics.forth.gr/parthenos_vocabularies/Concept/32227"/>
    <skos:narrowMatch rdf:resource="https://isl.ics.forth.gr/parthenos_vocabularies/Concept/32316"/>
    <skos:narrowMatch rdf:resource="https://isl.ics.forth.gr/parthenos_vocabularies/Concept/32728"/>
    <skos:narrowMatch rdf:resource="https://isl.ics.forth.gr/parthenos_vocabularies/Concept/32724"/>
    <skos:narrowMatch rdf:resource="https://isl.ics.forth.gr/parthenos_vocabularies/Concept/32835"/>
    <skos:narrowMatch rdf:resource="https://isl.ics.forth.gr/parthenos_vocabularies/Concept/32622"/>
    <skos:narrowMatch rdf:resource="https://isl.ics.forth.gr/parthenos_vocabularies/Concept/32595"/>
    <skos:narrowMatch rdf:resource="https://isl.ics.forth.gr/parthenos_vocabularies/Concept/32357"/>
    <skos:narrowMatch rdf:resource="https://isl.ics.forth.gr/parthenos_vocabularies/Concept/32722"/>
    <skos:narrowMatch rdf:resource="https://isl.ics.forth.gr/parthenos_vocabularies/Concept/32414"/>
    <skos:narrowMatch rdf:resource="https://isl.ics.forth.gr/parthenos_vocabularies/Concept/32764"/>
    <dcterms:dateSubmitted>2015-08-13T07:18:40Z</dcterms:dateSubmitted>
    <skos:narrowMatch rdf:resource="https://isl.ics.forth.gr/parthenos_vocabularies/Concept/32518"/>
    <skos:narrowMatch rdf:resource="https://isl.ics.forth.gr/parthenos_vocabularies/Concept/32280"/>
    <skos:narrowMatch rdf:resource="https://isl.ics.forth.gr/parthenos_vocabularies/Concept/32964"/>
    <skos:narrowMatch rdf:resource="https://isl.ics.forth.gr/parthenos_vocabularies/Concept/32508"/>
    <skos:narrowMatch rdf:resource="https://isl.ics.forth.gr/parthenos_vocabularies/Concept/32571"/>
    <skos:narrowMatch rdf:resource="https://isl.ics.forth.gr/parthenos_vocabularies/Concept/32935"/>
    <skos:narrowMatch rdf:resource="https://isl.ics.forth.gr/parthenos_vocabularies/Concept/32417"/>
    <skos:narrowMatch rdf:resource="https://isl.ics.forth.gr/parthenos_vocabularies/Concept/32512"/>
    <skos:narrowMatch rdf:resource="https://isl.ics.forth.gr/parthenos_vocabularies/Concept/32736"/>
    <skos:narrowMatch rdf:resource="https://isl.ics.forth.gr/parthenos_vocabularies/Concept/32225"/>
    <skos:narrowMatch rdf:resource="https://isl.ics.forth.gr/parthenos_vocabularies/Concept/32667"/>
    <skos:narrowMatch rdf:resource="https://isl.ics.forth.gr/parthenos_vocabularies/Concept/32338"/>
    <skos:narrowMatch rdf:resource="https://isl.ics.forth.gr/parthenos_vocabularies/Concept/32696"/>
    <skos:narrowMatch rdf:resource="https://isl.ics.forth.gr/parthenos_vocabularies/Concept/32770"/>
    <skos:narrowMatch rdf:resource="https://isl.ics.forth.gr/parthenos_vocabularies/Concept/32618"/>
    <skos:narrowMatch rdf:resource="https://isl.ics.forth.gr/parthenos_vocabularies/Concept/32864"/>
    <skos:narrowMatch rdf:resource="https://isl.ics.forth.gr/parthenos_vocabularies/Concept/32727"/>
    <skos:narrowMatch rdf:resource="https://isl.ics.forth.gr/parthenos_vocabularies/Concept/32539"/>
    <skos:narrowMatch rdf:resource="https://isl.ics.forth.gr/parthenos_vocabularies/Concept/32340"/>
    <skos:narrowMatch rdf:resource="https://isl.ics.forth.gr/parthenos_vocabularies/Concept/32705"/>
    <skos:narrowMatch rdf:resource="https://isl.ics.forth.gr/parthenos_vocabularies/Concept/32637"/>
    <skos:narrowMatch rdf:resource="https://isl.ics.forth.gr/parthenos_vocabularies/Concept/32548"/>
    <skos:narrowMatch rdf:resource="https://isl.ics.forth.gr/parthenos_vocabularies/Concept/32760"/>
    <skos:narrowMatch rdf:resource="https://isl.ics.forth.gr/parthenos_vocabularies/Concept/32590"/>
    <dcterms:creator xml:lang="en">BBT maintenance WG</dcterms:creator>
    <skos:narrowMatch rdf:resource="https://isl.ics.forth.gr/parthenos_vocabularies/Concept/32896"/>
    <skos:narrowMatch rdf:resource="https://isl.ics.forth.gr/parthenos_vocabularies/Concept/32276"/>
    <skos:narrowMatch rdf:resource="https://isl.ics.forth.gr/parthenos_vocabularies/Concept/32536"/>
    <skos:narrowMatch rdf:resource="https://isl.ics.forth.gr/parthenos_vocabularies/Concept/32936"/>
    <skos:narrowMatch rdf:resource="https://isl.ics.forth.gr/parthenos_vocabularies/Concept/32750"/>
    <skos:narrowMatch rdf:resource="https://isl.ics.forth.gr/parthenos_vocabularies/Concept/32658"/>
    <skos:narrowMatch rdf:resource="https://isl.ics.forth.gr/parthenos_vocabularies/Concept/32591"/>
    <skos:narrowMatch rdf:resource="https://isl.ics.forth.gr/parthenos_vocabularies/Concept/32524"/>
    <skos:narrowMatch rdf:resource="https://isl.ics.forth.gr/parthenos_vocabularies/Concept/32268"/>
    <skos:narrowMatch rdf:resource="https://isl.ics.forth.gr/parthenos_vocabularies/Concept/32563"/>
    <skos:narrowMatch rdf:resource="https://isl.ics.forth.gr/parthenos_vocabularies/Concept/32719"/>
    <skos:narrowMatch rdf:resource="https://isl.ics.forth.gr/parthenos_vocabularies/Concept/32440"/>
    <skos:narrowMatch rdf:resource="https://isl.ics.forth.gr/parthenos_vocabularies/Concept/32260"/>
    <skos:narrowMatch rdf:resource="https://isl.ics.forth.gr/parthenos_vocabularies/Concept/32217"/>
    <skos:narrowMatch rdf:resource="https://isl.ics.forth.gr/parthenos_vocabularies/Concept/32597"/>
    <skos:narrowMatch rdf:resource="https://isl.ics.forth.gr/parthenos_vocabularies/Concept/32397"/>
    <skos:narrowMatch rdf:resource="https://isl.ics.forth.gr/parthenos_vocabularies/Concept/32788"/>
    <skos:narrowMatch rdf:resource="https://isl.ics.forth.gr/parthenos_vocabularies/Concept/32940"/>
    <skos:narrowMatch rdf:resource="https://isl.ics.forth.gr/parthenos_vocabularies/Concept/32529"/>
    <skos:narrowMatch rdf:resource="https://isl.ics.forth.gr/parthenos_vocabularies/Concept/32435"/>
    <skos:narrowMatch rdf:resource="https://isl.ics.forth.gr/parthenos_vocabularies/Concept/32243"/>
    <skos:note xml:lang="en">Narrower term examples: "reliefs ", "granules"</skos:note>
    <skos:narrowMatch rdf:resource="https://isl.ics.forth.gr/parthenos_vocabularies/Concept/32326"/>
    <skos:narrowMatch rdf:resource="https://ark.frantiq.fr/ark:/26678/pcrtdakpjJaSz5"/>
    <skos:narrowMatch rdf:resource="https://isl.ics.forth.gr/parthenos_vocabularies/Concept/32783"/>
    <skos:narrowMatch rdf:resource="https://isl.ics.forth.gr/parthenos_vocabularies/Concept/32249"/>
    <skos:narrowMatch rdf:resource="https://isl.ics.forth.gr/parthenos_vocabularies/Concept/32495"/>
    <skos:narrowMatch rdf:resource="https://isl.ics.forth.gr/parthenos_vocabularies/Concept/32735"/>
    <skos:narrowMatch rdf:resource="https://isl.ics.forth.gr/parthenos_vocabularies/Concept/32288"/>
    <skos:narrowMatch rdf:resource="https://isl.ics.forth.gr/parthenos_vocabularies/Concept/32747"/>
    <skos:prefLabel xml:lang="el">υλικά μορφώματα</skos:prefLabel>
    <skos:narrowMatch rdf:resource="https://isl.ics.forth.gr/parthenos_vocabularies/Concept/32205"/>
    <skos:narrowMatch rdf:resource="https://isl.ics.forth.gr/parthenos_vocabularies/Concept/32558"/>
    <skos:narrowMatch rdf:resource="https://isl.ics.forth.gr/parthenos_vocabularies/Concept/32665"/>
    <skos:narrowMatch rdf:resource="https://isl.ics.forth.gr/parthenos_vocabularies/Concept/32278"/>
    <skos:narrowMatch rdf:resource="https://isl.ics.forth.gr/parthenos_vocabularies/Concept/32209"/>
    <skos:narrowMatch rdf:resource="https://isl.ics.forth.gr/parthenos_vocabularies/Concept/32598"/>
    <skos:exactMatch rdf:resource="http://thesauri.dainst.org/_46c2d50b"/>
    <skos:narrowMatch rdf:resource="https://isl.ics.forth.gr/parthenos_vocabularies/Concept/32673"/>
    <skos:narrowMatch rdf:resource="https://isl.ics.forth.gr/parthenos_vocabularies/Concept/32890"/>
    <skos:narrowMatch rdf:resource="https://isl.ics.forth.gr/parthenos_vocabularies/Concept/32862"/>
    <skos:narrowMatch rdf:resource="https://isl.ics.forth.gr/parthenos_vocabularies/Concept/32687"/>
    <skos:narrowMatch rdf:resource="https://isl.ics.forth.gr/parthenos_vocabularies/Concept/32682"/>
    <skos:narrowMatch rdf:resource="https://isl.ics.forth.gr/parthenos_vocabularies/Concept/32257"/>
    <skos:narrowMatch rdf:resource="https://isl.ics.forth.gr/parthenos_vocabularies/Concept/32917"/>
    <skos:narrowMatch rdf:resource="https://isl.ics.forth.gr/parthenos_vocabularies/Concept/32751"/>
    <skos:narrowMatch rdf:resource="https://isl.ics.forth.gr/parthenos_vocabularies/Concept/32854"/>
    <skos:narrowMatch rdf:resource="https://isl.ics.forth.gr/parthenos_vocabularies/Concept/32969"/>
    <skos:narrowMatch rdf:resource="https://isl.ics.forth.gr/parthenos_vocabularies/Concept/32485"/>
    <skos:narrowMatch rdf:resource="https://isl.ics.forth.gr/parthenos_vocabularies/Concept/32294"/>
    <skos:narrowMatch rdf:resource="https://isl.ics.forth.gr/parthenos_vocabularies/Concept/32569"/>
    <skos:narrowMatch rdf:resource="https://isl.ics.forth.gr/parthenos_vocabularies/Concept/32606"/>
    <skos:narrowMatch rdf:resource="https://isl.ics.forth.gr/parthenos_vocabularies/Concept/32456"/>
    <skos:narrowMatch rdf:resource="https://isl.ics.forth.gr/parthenos_vocabularies/Concept/32676"/>
    <skos:narrowMatch rdf:resource="https://isl.ics.forth.gr/parthenos_vocabularies/Concept/32244"/>
    <skos:narrowMatch rdf:resource="https://isl.ics.forth.gr/parthenos_vocabularies/Concept/32976"/>
    <skos:narrowMatch rdf:resource="https://isl.ics.forth.gr/parthenos_vocabularies/Concept/32685"/>
    <skos:prefLabel xml:lang="fr">caractéristiques physiques</skos:prefLabel>
    <skos:narrowMatch rdf:resource="https://isl.ics.forth.gr/parthenos_vocabularies/Concept/32965"/>
    <skos:narrowMatch rdf:resource="https://isl.ics.forth.gr/parthenos_vocabularies/Concept/32741"/>
    <skos:narrowMatch rdf:resource="https://isl.ics.forth.gr/parthenos_vocabularies/Concept/32686"/>
    <skos:scopeNote xml:lang="en">This term classifies specific formations that are integrally adapted to certain material objects. They cannot, therefore, be separated from the carrier-object, but they also do not identify with it, since it is only a part of the carrier-object that carries the entire feature. In this sense, the feature is fixed, with respect to the carrier-object, while any attempt to remove it will result in the loss of part of the carrier-object. They may have two- or three-dimensional geometric extent, but there are no natural borders that separate them completely, in an objective way from the carrier-objects. Instances of Physical Features can be features in a narrower sense (scratches, holes, reliefs, surface colours etc.), while in the wider sense, they are portions of particular objects with borders that are not absolutely defined, such as the core of the Earth or the head of a marble statue.</skos:scopeNote>
    <skos:scopeNote xml:lang="de">Dieser Term beinhaltet spezifische Merkmale eines materiellen Objektes. Diese Merkmale können nicht von dem Trägerobjekt getrennt werden, identifizieren sich aber auch nicht mit ihm, da sie lediglich Teil des Trägerobjektes sind, welches die Gesamtheit der Eigenschaften bildet. Das physische Merkmal ist fester Bestandteil des Trägerobjektes und jeder Versuch, es zu entfernen, führt zum Verlust eines Teiles des Trägerobjektes. Die Merkmale können zwei- oder dreidimensionale geometrische Ausdehnungen aufweisen, aber es gibt keine natürlichen Grenzen, die sie vollständig und objektiv von dem Trägerobjekt trennen. Beispiele von physischen Merkmalen können im engeren Sinne Eigenschaften sein (wie Kratzer, Löcher, Reliefs, Oberflächenfarben usw.), oder im weiteren Sinne Teile von bestimmten Objekten mit nicht klar definierten Grenzen (wie der Kern der Erde oder der Kopf einer Marmorstatue).</skos:scopeNote>
    <skos:broader rdf:resource="https://vocabs.dariah.eu/bbt/Concept/000004"/>
    <skos:narrowMatch rdf:resource="https://isl.ics.forth.gr/parthenos_vocabularies/Concept/32780"/>
    <skos:narrowMatch rdf:resource="https://isl.ics.forth.gr/parthenos_vocabularies/Concept/32805"/>
    <skos:narrowMatch rdf:resource="https://isl.ics.forth.gr/parthenos_vocabularies/Concept/32550"/>
    <skos:narrowMatch rdf:resource="https://isl.ics.forth.gr/parthenos_vocabularies/Concept/32549"/>
    <skos:narrowMatch rdf:resource="https://isl.ics.forth.gr/parthenos_vocabularies/Concept/32850"/>
    <skos:narrowMatch rdf:resource="https://isl.ics.forth.gr/parthenos_vocabularies/Concept/32895"/>
    <skos:narrowMatch rdf:resource="https://isl.ics.forth.gr/parthenos_vocabularies/Concept/32215"/>
    <skos:narrowMatch rdf:resource="https://isl.ics.forth.gr/parthenos_vocabularies/Concept/32401"/>
    <skos:narrowMatch rdf:resource="https://isl.ics.forth.gr/parthenos_vocabularies/Concept/32345"/>
    <skos:narrowMatch rdf:resource="https://isl.ics.forth.gr/parthenos_vocabularies/Concept/32458"/>
    <skos:narrowMatch rdf:resource="https://isl.ics.forth.gr/parthenos_vocabularies/Concept/32594"/>
    <skos:narrowMatch rdf:resource="https://isl.ics.forth.gr/parthenos_vocabularies/Concept/32823"/>
    <skos:narrowMatch rdf:resource="https://isl.ics.forth.gr/parthenos_vocabularies/Concept/32585"/>
    <skos:scopeNote xml:lang="el">Η ιεραρχία αυτή περιλαμβάνει συγκεκριμένους σχηματισμούς που είναι προσαρμοσμένοι με αναπόσπαστο τρόπο σε συγκεκριμένα υλικά αντικείμενα. Δεν μπορούν, επομένως, να χωριστούν από τον φορέα-αντικείμενο, χωρίς όμως να ταυτίζονται με αυτόν, εφόσον ένα τμήμα του φορέα-αντικειμένου μπορεί να φέρει ολόκληρο το μόρφωμα. Με αυτήν την έννοια, το μόρφωμα είναι σταθερό ως προς τον φορέα-αντικείμενο, ενώ η προσπάθεια απομάκρυνσής του συνοδεύεται από απώλεια μέρους του φορέα-αντικειμένου. Ενδέχεται να έχουν δισδιάστατη ή τρισδιάστατη γεωμετρική έκταση, αλλά δεν υπάρχουν φυσικά σύνορα που να τα διαχωρίζουν απόλυτα, με αντικειμενικό τρόπο από τα αντικείμενα-φορείς. Πραγματώσεις υλικών μορφωμάτων μπορεί, για παράδειγμα, να είναι μορφώματα με την στενότερη έννοια του όρου (γρατζουνιές, τρύπες, ανάγλυφα, χρώματα επιφάνειας κ.τ.λ.), ενώ με την ευρύτερη έννοια μορφώματα είναι μέρη συγκεκριμένων αντικειμένων με σύνορα που δεν προσδιορίζονται με απόλυτο τρόπο, όπως είναι ο πυρήνας της γης ή το κεφάλι σε ένα μαρμάρινο άγαλμα.</skos:scopeNote>
    <skos:scopeNote xml:lang="fr">Ce terme désigne des formations spécifiques intégralement adaptées à certains objets matériels. Elles ne peuvent donc être séparées de l’objet qui les porte mais ne s’identifient pas à cet objet puisque seule une partie de l'objet les supporte. En ce sens, la caractéristique est fixe par rapport à cet objet de sorte que toute tentative de la retirer résulterait dans la perte d’une partie de l’objet qui la porte. Elles peuvent avoir une forme bi ou tri dimensionnelle mais il n’existe pas de limite qui les sépare complètement,  de façon objective, de l’objet. Certaines caractéristiques physiques être des caractéristique au sens le plus restreint  (entailles, trous, reliefs, surface colorée) alors qu'au sens large elles sont des parties d'objets aux limites non définies comme le centre de la terre ou la tête d'une statue de marbre.</skos:scopeNote>
    <skos:narrowMatch rdf:resource="https://isl.ics.forth.gr/parthenos_vocabularies/Concept/32370"/>
    <skos:narrowMatch rdf:resource="https://isl.ics.forth.gr/parthenos_vocabularies/Concept/32931"/>
    <skos:narrowMatch rdf:resource="https://isl.ics.forth.gr/parthenos_vocabularies/Concept/32482"/>
    <skos:narrowMatch rdf:resource="https://isl.ics.forth.gr/parthenos_vocabularies/Concept/32351"/>
    <skos:narrowMatch rdf:resource="https://isl.ics.forth.gr/parthenos_vocabularies/Concept/32592"/>
    <skos:narrowMatch rdf:resource="https://isl.ics.forth.gr/parthenos_vocabularies/Concept/32519"/>
    <skos:narrowMatch rdf:resource="https://isl.ics.forth.gr/parthenos_vocabularies/Concept/32534"/>
    <skos:narrowMatch rdf:resource="https://isl.ics.forth.gr/parthenos_vocabularies/Concept/32828"/>
    <skos:narrowMatch rdf:resource="https://isl.ics.forth.gr/parthenos_vocabularies/Concept/32432"/>
    <skos:narrowMatch rdf:resource="https://isl.ics.forth.gr/parthenos_vocabularies/Concept/32500"/>
    <skos:narrowMatch rdf:resource="https://isl.ics.forth.gr/parthenos_vocabularies/Concept/32803"/>
    <skos:narrowMatch rdf:resource="https://ark.frantiq.fr/ark:/26678/pcrt9PJh9aTXv4"/>
    <skos:narrowMatch rdf:resource="https://isl.ics.forth.gr/parthenos_vocabularies/Concept/32365"/>
    <skos:narrowMatch rdf:resource="https://isl.ics.forth.gr/parthenos_vocabularies/Concept/32560"/>
    <skos:narrowMatch rdf:resource="https://isl.ics.forth.gr/parthenos_vocabularies/Concept/32642"/>
    <skos:narrowMatch rdf:resource="https://isl.ics.forth.gr/parthenos_vocabularies/Concept/32564"/>
    <skos:narrowMatch rdf:resource="https://isl.ics.forth.gr/parthenos_vocabularies/Concept/32614"/>
    <skos:narrowMatch rdf:resource="https://isl.ics.forth.gr/parthenos_vocabularies/Concept/32634"/>
    <skos:narrowMatch rdf:resource="https://isl.ics.forth.gr/parthenos_vocabularies/Concept/32285"/>
    <skos:narrowMatch rdf:resource="https://isl.ics.forth.gr/parthenos_vocabularies/Concept/32951"/>
    <skos:narrowMatch rdf:resource="https://isl.ics.forth.gr/parthenos_vocabularies/Concept/32888"/>
    <skos:narrowMatch rdf:resource="https://isl.ics.forth.gr/parthenos_vocabularies/Concept/32635"/>
    <skos:narrowMatch rdf:resource="https://isl.ics.forth.gr/parthenos_vocabularies/Concept/32830"/>
    <skos:narrowMatch rdf:resource="https://isl.ics.forth.gr/parthenos_vocabularies/Concept/32341"/>
    <skos:narrowMatch rdf:resource="https://isl.ics.forth.gr/parthenos_vocabularies/Concept/32628"/>
    <skos:narrowMatch rdf:resource="https://isl.ics.forth.gr/parthenos_vocabularies/Concept/32953"/>
    <skos:narrowMatch rdf:resource="https://isl.ics.forth.gr/parthenos_vocabularies/Concept/32431"/>
    <skos:narrowMatch rdf:resource="https://isl.ics.forth.gr/parthenos_vocabularies/Concept/32332"/>
    <skos:narrowMatch rdf:resource="https://isl.ics.forth.gr/parthenos_vocabularies/Concept/32328"/>
    <skos:narrowMatch rdf:resource="https://isl.ics.forth.gr/parthenos_vocabularies/Concept/32901"/>
    <skos:narrowMatch rdf:resource="https://isl.ics.forth.gr/parthenos_vocabularies/Concept/32603"/>
    <skos:narrowMatch rdf:resource="https://isl.ics.forth.gr/parthenos_vocabularies/Concept/32282"/>
    <skos:narrowMatch rdf:resource="https://isl.ics.forth.gr/parthenos_vocabularies/Concept/32975"/>
    <skos:narrowMatch rdf:resource="https://isl.ics.forth.gr/parthenos_vocabularies/Concept/32914"/>
    <rdfs:type rdf:resource="http://www.w3.org/2004/02/skos/core#Concept"/>
    <skos:narrowMatch rdf:resource="https://isl.ics.forth.gr/parthenos_vocabularies/Concept/32589"/>
    <skos:narrowMatch rdf:resource="https://isl.ics.forth.gr/parthenos_vocabularies/Concept/32273"/>
    <skos:exactMatch rdf:resource="http://w3id.org/lob/concept/2272"/>
    <skos:narrowMatch rdf:resource="https://isl.ics.forth.gr/parthenos_vocabularies/Concept/32317"/>
    <skos:narrowMatch rdf:resource="https://isl.ics.forth.gr/parthenos_vocabularies/Concept/32318"/>
    <skos:narrowMatch rdf:resource="https://isl.ics.forth.gr/parthenos_vocabularies/Concept/32447"/>
    <skos:narrowMatch rdf:resource="https://isl.ics.forth.gr/parthenos_vocabularies/Concept/32629"/>
    <skos:narrowMatch rdf:resource="https://isl.ics.forth.gr/parthenos_vocabularies/Concept/32241"/>
    <skos:notation>000019</skos:notation>
    <skos:narrowMatch rdf:resource="https://isl.ics.forth.gr/parthenos_vocabularies/Concept/32516"/>
    <skos:narrowMatch rdf:resource="https://isl.ics.forth.gr/parthenos_vocabularies/Concept/32849"/>
    <skos:narrowMatch rdf:resource="https://isl.ics.forth.gr/parthenos_vocabularies/Concept/32777"/>
    <skos:narrowMatch rdf:resource="https://isl.ics.forth.gr/parthenos_vocabularies/Concept/32324"/>
    <skos:narrowMatch rdf:resource="https://isl.ics.forth.gr/parthenos_vocabularies/Concept/32769"/>
    <skos:narrowMatch rdf:resource="https://isl.ics.forth.gr/parthenos_vocabularies/Concept/32763"/>
    <skos:narrowMatch rdf:resource="https://isl.ics.forth.gr/parthenos_vocabularies/Concept/32994"/>
    <skos:narrowMatch rdf:resource="https://isl.ics.forth.gr/parthenos_vocabularies/Concept/32974"/>
    <skos:narrowMatch rdf:resource="https://isl.ics.forth.gr/parthenos_vocabularies/Concept/32970"/>
    <skos:narrowMatch rdf:resource="https://isl.ics.forth.gr/parthenos_vocabularies/Concept/32959"/>
    <skos:narrowMatch rdf:resource="https://isl.ics.forth.gr/parthenos_vocabularies/Concept/32985"/>
    <skos:narrowMatch rdf:resource="https://isl.ics.forth.gr/parthenos_vocabularies/Concept/32601"/>
    <skos:narrowMatch rdf:resource="https://isl.ics.forth.gr/parthenos_vocabularies/Concept/32234"/>
    <skos:narrowMatch rdf:resource="https://isl.ics.forth.gr/parthenos_vocabularies/Concept/32389"/>
    <skos:narrowMatch rdf:resource="https://isl.ics.forth.gr/parthenos_vocabularies/Concept/32847"/>
    <skos:narrowMatch rdf:resource="https://isl.ics.forth.gr/parthenos_vocabularies/Concept/32546"/>
    <skos:narrowMatch rdf:resource="https://isl.ics.forth.gr/parthenos_vocabularies/Concept/32463"/>
    <skos:narrowMatch rdf:resource="https://isl.ics.forth.gr/parthenos_vocabularies/Concept/32515"/>
    <skos:narrowMatch rdf:resource="https://isl.ics.forth.gr/parthenos_vocabularies/Concept/32670"/>
    <skos:narrowMatch rdf:resource="https://isl.ics.forth.gr/parthenos_vocabularies/Concept/32547"/>
    <skos:narrowMatch rdf:resource="https://isl.ics.forth.gr/parthenos_vocabularies/Concept/32689"/>
    <skos:narrowMatch rdf:resource="https://isl.ics.forth.gr/parthenos_vocabularies/Concept/32891"/>
    <skos:narrowMatch rdf:resource="https://isl.ics.forth.gr/parthenos_vocabularies/Concept/32486"/>
    <skos:narrowMatch rdf:resource="https://isl.ics.forth.gr/parthenos_vocabularies/Concept/32322"/>
    <skos:narrowMatch rdf:resource="https://isl.ics.forth.gr/parthenos_vocabularies/Concept/32723"/>
    <rdf:type rdf:resource="http://www.w3.org/2004/02/skos/core#Concept"/>
    <skos:narrowMatch rdf:resource="https://isl.ics.forth.gr/parthenos_vocabularies/Concept/32960"/>
    <skos:narrowMatch rdf:resource="https://isl.ics.forth.gr/parthenos_vocabularies/Concept/32941"/>
    <skos:narrowMatch rdf:resource="https://isl.ics.forth.gr/parthenos_vocabularies/Concept/32394"/>
    <skos:exactMatch rdf:resource="https://humanitiesthesaurus.academyofathens.gr/dyas-resource/Concept/29"/>
    <skos:narrowMatch rdf:resource="https://isl.ics.forth.gr/parthenos_vocabularies/Concept/32868"/>
    <skos:narrowMatch rdf:resource="https://isl.ics.forth.gr/parthenos_vocabularies/Concept/32284"/>
    <skos:narrowMatch rdf:resource="https://isl.ics.forth.gr/parthenos_vocabularies/Concept/32281"/>
    <skos:narrowMatch rdf:resource="https://isl.ics.forth.gr/parthenos_vocabularies/Concept/32961"/>
    <skos:narrowMatch rdf:resource="https://isl.ics.forth.gr/parthenos_vocabularies/Concept/32926"/>
    <skos:narrowMatch rdf:resource="https://isl.ics.forth.gr/parthenos_vocabularies/Concept/32342"/>
    <skos:narrowMatch rdf:resource="https://isl.ics.forth.gr/parthenos_vocabularies/Concept/32694"/>
    <skos:narrowMatch rdf:resource="https://isl.ics.forth.gr/parthenos_vocabularies/Concept/32503"/>
    <skos:narrowMatch rdf:resource="https://isl.ics.forth.gr/parthenos_vocabularies/Concept/32912"/>
    <skos:prefLabel xml:lang="en">physical features</skos:prefLabel>
    <skos:narrowMatch rdf:resource="https://isl.ics.forth.gr/parthenos_vocabularies/Concept/32306"/>
    <skos:narrowMatch rdf:resource="https://isl.ics.forth.gr/parthenos_vocabularies/Concept/32478"/>
    <skos:narrowMatch rdf:resource="https://isl.ics.forth.gr/parthenos_vocabularies/Concept/32426"/>
    <skos:narrowMatch rdf:resource="https://isl.ics.forth.gr/parthenos_vocabularies/Concept/32587"/>
    <skos:narrowMatch rdf:resource="https://isl.ics.forth.gr/parthenos_vocabularies/Concept/32202"/>
    <skos:narrowMatch rdf:resource="https://isl.ics.forth.gr/parthenos_vocabularies/Concept/32801"/>
    <skos:narrowMatch rdf:resource="https://isl.ics.forth.gr/parthenos_vocabularies/Concept/32872"/>
    <skos:narrowMatch rdf:resource="https://isl.ics.forth.gr/parthenos_vocabularies/Concept/32987"/>
    <skos:prefLabel xml:lang="de">Physische Merkmale</skos:prefLabel>
    <skos:narrowMatch rdf:resource="https://ark.frantiq.fr/ark:/26678/pcrtySs2lWdI4z"/>
    <skos:narrowMatch rdf:resource="https://isl.ics.forth.gr/parthenos_vocabularies/Concept/32690"/>
    <skos:narrowMatch rdf:resource="https://isl.ics.forth.gr/parthenos_vocabularies/Concept/32373"/>
    <skos:narrowMatch rdf:resource="https://isl.ics.forth.gr/parthenos_vocabularies/Concept/32600"/>
  </rdf:Description>
  <rdf:Description rdf:about="https://vocabs.dariah.eu/bbt/Concept/000022">
    <rdfs:type rdf:resource="http://www.w3.org/2004/02/skos/core#Concept"/>
    <skos:narrowMatch rdf:resource="https://ark.frantiq.fr/ark:/26678/pcrtGEWgO8RzhI"/>
    <skos:narrowMatch rdf:resource="https://ark.frantiq.fr/ark:/26678/pcrtzdEfDOOga9"/>
    <skos:notation>000022</skos:notation>
    <skos:scopeNote xml:lang="de">Dieser Term umfasst durch menschliche Aktivität entstandene, mentale Inhalte, welche Daten physischer, logischer oder psychologischer Realität oder auch Fiktion darstellen. Obwohl sie mit Hilfe von Symbolen ausgedrückt werden, sind diese Objekte davon unabhängig, was ihre Transformation in andere Symbole ermöglicht. Trotzdem kann ein Aussageobjekt manchmal nicht klar von dem genutzten Symbol getrennt werden (z. B. Gedicht).</skos:scopeNote>
    <dcterms:dateSubmitted>2015-08-13T07:18:40Z</dcterms:dateSubmitted>
    <skos:exactMatch rdf:resource="https://humanitiesthesaurus.academyofathens.gr/dyas-resource/Concept/25"/>
    <dcterms:modified>2019-04-10T10:55:19Z</dcterms:modified>
    <skos:prefLabel xml:lang="de">Aussageobjekte</skos:prefLabel>
    <skos:prefLabel xml:lang="fr">objets propositionnels</skos:prefLabel>
    <skos:scopeNote xml:lang="fr">Ce terme désigne les contenus mentaux produit par l’activité humaine représentant des données de la réalité physique, logique, psychologique ou même de la fiction. Ces objets, bien qu’exprimés au moyen de symboles, ne dépendent pas de ces symboles, ce qui permet leur transcription aux moyens d’un autre système de symboles. Cependant un objet propositionnel ne peut parfois pas être dissocié des symboles utilisés, par exemple un poème.</skos:scopeNote>
    <skos:narrowMatch rdf:resource="https://ark.frantiq.fr/ark:/26678/pcrt7q7SOMjW4B"/>
    <skos:prefLabel xml:lang="el">προτασιακά αντικείμενα</skos:prefLabel>
    <skos:prefLabel xml:lang="en">propositional objects</skos:prefLabel>
    <skos:narrowMatch rdf:resource="https://ark.frantiq.fr/ark:/26678/pcrtZnKEOuwY05"/>
    <skos:narrowMatch rdf:resource="https://ark.frantiq.fr/ark:/26678/pcrtPqhdPEr4nl"/>
    <skos:exactMatch rdf:resource="http://thesauri.dainst.org/_d9a01ada"/>
    <skos:scopeNote xml:lang="el">Περιλαμβάνει περιεχόμενα του νου που είναι δημιουργήματα της ανθρώπινης δραστηριότητας και αναπαριστούν δεδομένα της φυσικής, λογικής ή ψυχολογικής πραγματικότητας ή ακόμα και προϊόντα της φαντασίας. Τα περιεχόμενα αυτά, ενώ εκφέρονται μέσω της χρήσης συμβόλων, είναι ανεξάρτητα από αυτά, γεγονός που καθιστά δυνατή τη μεταγραφή τους σε άλλο σύστημα συμβόλων. Το γεγονός αυτό δεν αποκλείει την περίπτωση, ένα προτασιακό περιεχόμενο να μην μπορεί να χωριστεί με σαφήνεια από τα σύμβολα, με τα οποία εκφέρεται (π.χ. ένα ποίημα).Επίσης, τα περιεχόμενα αυτά είναι ανεξάρτητα από το υλικό – χαρτί, ηλεκτρονικά μέσα κτλ. – του εκάστοτε φορέα εκφοράς τους.</skos:scopeNote>
    <skos:narrowMatch rdf:resource="https://ark.frantiq.fr/ark:/26678/pcrtweM71fK5x5"/>
    <rdf:type rdf:resource="http://www.w3.org/2004/02/skos/core#Concept"/>
    <skos:broader rdf:resource="https://vocabs.dariah.eu/bbt/Concept/000006"/>
    <skos:note xml:lang="en">Narrower term examples: "information objects","structural parts of information objects"</skos:note>
    <skos:scopeNote xml:lang="en">This term classifies mental contents produced by human activity, representing data of physical, logical or psychological realities or even fiction. These objects, though expressed by the use of symbols, do not depend on them, a fact that allows their transcription to another set of symbols. However a propositional object sometimes cannot be differentiated distinctively from the used symbols (e.g. a poem).</skos:scopeNote>
    <dcterms:creator xml:lang="en">BBT maintenance WG</dcterms:creator>
  </rdf:Description>
  <rdf:Description rdf:about="https://vocabs.dariah.eu/bbt/ConceptScheme/Backbone_Thesaurus">
    <dcterms:creator xml:lang="en">Chryssoula Bekiari</dcterms:creator>
    <dcterms:creator xml:lang="en">Maria Daskalaki</dcterms:creator>
    <dcterms:creator xml:lang="en">Vanessa Hannesschläger</dcterms:creator>
    <dcterms:creator xml:lang="en">BBT maintenance WG</dcterms:creator>
    <dcterms:creator xml:lang="en">Lida Charami</dcterms:creator>
    <dcterms:subject xml:lang="en">humanities</dcterms:subject>
    <rdfs:label>Backbone Thesaurus</rdfs:label>
    <dcterms:subject xml:lang="en">geopolitical units</dcterms:subject>
    <owl:versionInfo>1.2.3</owl:versionInfo>
    <dcterms:creator xml:lang="en">Martin Doerr</dcterms:creator>
    <dcterms:format>application/rdf+xml</dcterms:format>
    <dcterms:subject xml:lang="en">activities</dcterms:subject>
    <skos:hasTopConcept rdf:resource="https://vocabs.dariah.eu/bbt/Concept/000009"/>
    <dcterms:created>2015-07-01T12:00:00Z</dcterms:created>
    <dcterms:rights>https://creativecommons.org/licenses/by/4.0/</dcterms:rights>
    <dcterms:description xml:lang="en">The BBT is the research outcome of work undertaken by the DARIAH Thesaurus Maintenance WG in an effort to design and establish a coherent overarching thesaurus for the humanities, under which specialist thesauri and structured vocabularies used across scholarly communities can be aligned and form a thesaurus federation.  It aims at enabling cross-disciplinary resource discovery while ensuring compatibility with thesauri that cover highly specific scientific domains and areas of knowledge in development.  The BBT was created and funded by the DARIAH GR Developing a Greek Research Infrastructure for the Humanities project (2013-2015). Currently it receives funding by the APOLLONIS Greek Infrastructure for Humanities, Arts and Language Research and Innovation project (2017-2020).</dcterms:description>
    <dcterms:language>German</dcterms:language>
    <skos:hasTopConcept rdf:resource="https://vocabs.dariah.eu/bbt/Concept/000001"/>
    <dcterms:language>Greek</dcterms:language>
    <dcterms:creator xml:lang="en">Helen Goulis</dcterms:creator>
    <skos:hasTopConcept rdf:resource="https://vocabs.dariah.eu/bbt/Concept/000007"/>
    <dcterms:title xml:lang="en">Backbone Thesaurus</dcterms:title>
    <rdf:type rdf:resource="http://www.w3.org/2004/02/skos/core#ConceptScheme"/>
    <skos:hasTopConcept rdf:resource="https://vocabs.dariah.eu/bbt/Concept/0000049"/>
    <dcterms:creator xml:lang="en">Makis Chrisovitsanos</dcterms:creator>
    <skos:hasTopConcept rdf:resource="https://vocabs.dariah.eu/bbt/Concept/000004"/>
    <dcterms:issued>2020-01-21T11:20:37Z</dcterms:issued>
    <skos:hasTopConcept rdf:resource="https://vocabs.dariah.eu/bbt/Concept/000003"/>
    <dcterms:modified>2020-10-23T07:35:11Z</dcterms:modified>
    <dcterms:subject xml:lang="en">roles</dcterms:subject>
    <dcterms:subject xml:lang="en">processes</dcterms:subject>
    <skos:hasTopConcept rdf:resource="https://vocabs.dariah.eu/bbt/Concept/000006"/>
    <dcterms:creator xml:lang="en">Hella Hollander</dcterms:creator>
    <skos:hasTopConcept rdf:resource="https://vocabs.dariah.eu/bbt/Concept/000005"/>
    <dcterms:creator xml:lang="en">Helen Katsiadaki</dcterms:creator>
    <skos:hasTopConcept rdf:resource="https://vocabs.dariah.eu/bbt/Concept/000008"/>
    <dcterms:language>French</dcterms:language>
    <dcterms:subject xml:lang="en">materials</dcterms:subject>
    <skos:hasTopConcept rdf:resource="https://vocabs.dariah.eu/bbt/Concept/000002"/>
    <dcterms:creator xml:lang="en">Iraklitos Souyioultzoglou</dcterms:creator>
    <dcterms:creator xml:lang="en">Wolfgang Schmidle</dcterms:creator>
    <dcterms:language>English</dcterms:language>
    <dcterms:subject xml:lang="en">conceptual objects</dcterms:subject>
    <dcterms:creator xml:lang="en">Georgia Papadopoulou</dcterms:creator>
  </rdf:Description>
  <rdf:Description rdf:about="https://vocabs.dariah.eu/bbt/Facet/000002">
    <skos:scopeNote xml:lang="en">This facet comprises types of changes in states of affairs, things and entities that result from natural phenomena (e.g. earthquakes, floods).</skos:scopeNote>
    <skos:member rdf:resource="https://vocabs.dariah.eu/bbt/Concept/000002"/>
    <skos:prefLabel xml:lang="en">Natural Processes</skos:prefLabel>
    <skos:scopeNote xml:lang="el">Το θέμα αυτό περιλαμβάνει αλλαγές καταστάσεων, πραγμάτων και οντοτήτων που αποδίδονται στην επενέργεια φυσικών αιτιών (σεισμών, πλημμύρων κτλ.).</skos:scopeNote>
    <skos:scopeNote xml:lang="fr">Cette facette désigne tous les types de changements de situations, d'objets ou d’entités résultant d’un phénomène naturel, par exemple tremblements de terre, inondations.</skos:scopeNote>
    <rdf:type rdf:resource="http://www.w3.org/2004/02/skos/core#Collection"/>
    <rdf:type rdf:resource="https://vocabs.dariah.eu/bbt/Facet"/>
    <skos:scopeNote xml:lang="de">Diese Facette beinhaltet Typen von Veränderungen von Sachverhalten, Dingen und Entitäten, die eine natürliche Ursache haben (z. B. Erdbeben, Fluten).</skos:scopeNote>
    <skos:prefLabel xml:lang="el">Φυσικές Μεταβολές</skos:prefLabel>
    <skos:prefLabel xml:lang="fr">Processus Naturel</skos:prefLabel>
    <dcterms:creator xml:lang="en">BBT maintenance WG</dcterms:creator>
    <skos:prefLabel xml:lang="de">Natürliche Prozesse</skos:prefLabel>
    <skos:inScheme rdf:resource="https://vocabs.dariah.eu/bbt/ConceptScheme/Backbone_Thesaurus"/>
    <skos:member rdf:resource="https://vocabs.dariah.eu/bbt/Concept/000016"/>
    <skos:member rdf:resource="https://vocabs.dariah.eu/bbt/Concept/000015"/>
  </rdf:Description>
  <rdf:Description rdf:about="https://vocabs.dariah.eu/bbt/Concept/000009">
    <skos:narrowMatch rdf:resource="https://isl.ics.forth.gr/parthenos_vocabularies/Concept/32250"/>
    <skos:narrowMatch rdf:resource="https://isl.ics.forth.gr/parthenos_vocabularies/Concept/32497"/>
    <skos:narrowMatch rdf:resource="https://isl.ics.forth.gr/parthenos_vocabularies/Concept/32819"/>
    <skos:narrowMatch rdf:resource="https://isl.ics.forth.gr/parthenos_vocabularies/Concept/32604"/>
    <skos:narrowMatch rdf:resource="https://isl.ics.forth.gr/parthenos_vocabularies/Concept/32654"/>
    <skos:narrowMatch rdf:resource="https://isl.ics.forth.gr/parthenos_vocabularies/Concept/32277"/>
    <skos:narrowMatch rdf:resource="https://isl.ics.forth.gr/parthenos_vocabularies/Concept/32376"/>
    <skos:prefLabel xml:lang="el">γεωπολιτικές μονάδες</skos:prefLabel>
    <skos:narrowMatch rdf:resource="https://isl.ics.forth.gr/parthenos_vocabularies/Concept/32988"/>
    <skos:narrowMatch rdf:resource="https://isl.ics.forth.gr/parthenos_vocabularies/Concept/32541"/>
    <skos:narrowMatch rdf:resource="https://isl.ics.forth.gr/parthenos_vocabularies/Concept/32506"/>
    <skos:narrowMatch rdf:resource="https://isl.ics.forth.gr/parthenos_vocabularies/Concept/32574"/>
    <skos:narrowMatch rdf:resource="https://isl.ics.forth.gr/parthenos_vocabularies/Concept/32749"/>
    <skos:narrowMatch rdf:resource="https://isl.ics.forth.gr/parthenos_vocabularies/Concept/32796"/>
    <skos:scopeNote xml:lang="en">This term classifies administrative divisions used by a state or other sovereign or political structure within the boundaries of its jurisdiction. Intrinsic features of these units include, among others, the extent of the area over which they are applied/exercised, the chronological extent during which they are in force, their governing bodies and the degree of autonomy they are granted in relation to managing and exploiting of their resources.</skos:scopeNote>
    <skos:narrowMatch rdf:resource="https://isl.ics.forth.gr/parthenos_vocabularies/Concept/32978"/>
    <skos:narrowMatch rdf:resource="https://isl.ics.forth.gr/parthenos_vocabularies/Concept/32493"/>
    <skos:narrowMatch rdf:resource="https://isl.ics.forth.gr/parthenos_vocabularies/Concept/32532"/>
    <skos:narrowMatch rdf:resource="https://isl.ics.forth.gr/parthenos_vocabularies/Concept/32928"/>
    <skos:narrowMatch rdf:resource="https://isl.ics.forth.gr/parthenos_vocabularies/Concept/32346"/>
    <skos:narrowMatch rdf:resource="https://isl.ics.forth.gr/parthenos_vocabularies/Concept/32739"/>
    <skos:narrowMatch rdf:resource="https://isl.ics.forth.gr/parthenos_vocabularies/Concept/32726"/>
    <skos:narrowMatch rdf:resource="https://isl.ics.forth.gr/parthenos_vocabularies/Concept/32391"/>
    <skos:narrowMatch rdf:resource="https://isl.ics.forth.gr/parthenos_vocabularies/Concept/32436"/>
    <skos:narrowMatch rdf:resource="https://isl.ics.forth.gr/parthenos_vocabularies/Concept/32361"/>
    <skos:prefLabel xml:lang="en">geopolitical units</skos:prefLabel>
    <skos:narrowMatch rdf:resource="https://isl.ics.forth.gr/parthenos_vocabularies/Concept/32815"/>
    <skos:narrowMatch rdf:resource="https://isl.ics.forth.gr/parthenos_vocabularies/Concept/32661"/>
    <skos:topConceptOf rdf:resource="https://vocabs.dariah.eu/bbt/ConceptScheme/Backbone_Thesaurus"/>
    <skos:narrowMatch rdf:resource="https://isl.ics.forth.gr/parthenos_vocabularies/Concept/32232"/>
    <skos:narrowMatch rdf:resource="https://isl.ics.forth.gr/parthenos_vocabularies/Concept/32494"/>
    <skos:narrowMatch rdf:resource="https://isl.ics.forth.gr/parthenos_vocabularies/Concept/32455"/>
    <skos:narrowMatch rdf:resource="https://isl.ics.forth.gr/parthenos_vocabularies/Concept/32530"/>
    <rdfs:type rdf:resource="http://www.w3.org/2004/02/skos/core#Concept"/>
    <skos:narrowMatch rdf:resource="https://isl.ics.forth.gr/parthenos_vocabularies/Concept/32385"/>
    <skos:narrowMatch rdf:resource="https://isl.ics.forth.gr/parthenos_vocabularies/Concept/32405"/>
    <skos:narrowMatch rdf:resource="https://isl.ics.forth.gr/parthenos_vocabularies/Concept/32706"/>
    <skos:narrowMatch rdf:resource="https://isl.ics.forth.gr/parthenos_vocabularies/Concept/32907"/>
    <skos:narrowMatch rdf:resource="https://isl.ics.forth.gr/parthenos_vocabularies/Concept/32887"/>
    <skos:narrowMatch rdf:resource="https://isl.ics.forth.gr/parthenos_vocabularies/Concept/32586"/>
    <skos:prefLabel xml:lang="fr">unités géopolitiques</skos:prefLabel>
    <skos:narrowMatch rdf:resource="https://isl.ics.forth.gr/parthenos_vocabularies/Concept/32925"/>
    <skos:narrowMatch rdf:resource="https://isl.ics.forth.gr/parthenos_vocabularies/Concept/32881"/>
    <skos:narrowMatch rdf:resource="https://isl.ics.forth.gr/parthenos_vocabularies/Concept/32242"/>
    <skos:narrowMatch rdf:resource="https://isl.ics.forth.gr/parthenos_vocabularies/Concept/32927"/>
    <skos:narrowMatch rdf:resource="https://isl.ics.forth.gr/parthenos_vocabularies/Concept/32884"/>
    <skos:narrowMatch rdf:resource="https://isl.ics.forth.gr/parthenos_vocabularies/Concept/32713"/>
    <skos:narrowMatch rdf:resource="https://isl.ics.forth.gr/parthenos_vocabularies/Concept/32489"/>
    <skos:narrowMatch rdf:resource="https://isl.ics.forth.gr/parthenos_vocabularies/Concept/32934"/>
    <skos:narrowMatch rdf:resource="https://isl.ics.forth.gr/parthenos_vocabularies/Concept/32883"/>
    <skos:narrowMatch rdf:resource="https://isl.ics.forth.gr/parthenos_vocabularies/Concept/32827"/>
    <skos:narrowMatch rdf:resource="https://isl.ics.forth.gr/parthenos_vocabularies/Concept/32716"/>
    <skos:narrowMatch rdf:resource="https://isl.ics.forth.gr/parthenos_vocabularies/Concept/32834"/>
    <skos:narrowMatch rdf:resource="https://isl.ics.forth.gr/parthenos_vocabularies/Concept/32649"/>
    <dcterms:modified>2019-04-10T11:12:59Z</dcterms:modified>
    <skos:narrowMatch rdf:resource="https://isl.ics.forth.gr/parthenos_vocabularies/Concept/32266"/>
    <skos:narrowMatch rdf:resource="https://isl.ics.forth.gr/parthenos_vocabularies/Concept/32909"/>
    <skos:narrowMatch rdf:resource="https://isl.ics.forth.gr/parthenos_vocabularies/Concept/32983"/>
    <skos:narrowMatch rdf:resource="https://isl.ics.forth.gr/parthenos_vocabularies/Concept/32885"/>
    <skos:narrowMatch rdf:resource="https://isl.ics.forth.gr/parthenos_vocabularies/Concept/32395"/>
    <skos:narrowMatch rdf:resource="https://isl.ics.forth.gr/parthenos_vocabularies/Concept/32829"/>
    <skos:narrowMatch rdf:resource="https://isl.ics.forth.gr/parthenos_vocabularies/Concept/32295"/>
    <skos:narrowMatch rdf:resource="https://isl.ics.forth.gr/parthenos_vocabularies/Concept/32545"/>
    <skos:narrowMatch rdf:resource="https://isl.ics.forth.gr/parthenos_vocabularies/Concept/32256"/>
    <skos:narrowMatch rdf:resource="https://isl.ics.forth.gr/parthenos_vocabularies/Concept/32383"/>
    <skos:narrowMatch rdf:resource="https://isl.ics.forth.gr/parthenos_vocabularies/Concept/32388"/>
    <skos:exactMatch rdf:resource="http://thesauri.dainst.org/_8cb35559"/>
    <skos:narrowMatch rdf:resource="https://isl.ics.forth.gr/parthenos_vocabularies/Concept/32441"/>
    <skos:narrowMatch rdf:resource="https://isl.ics.forth.gr/parthenos_vocabularies/Concept/32448"/>
    <skos:narrowMatch rdf:resource="https://isl.ics.forth.gr/parthenos_vocabularies/Concept/32443"/>
    <skos:narrowMatch rdf:resource="https://isl.ics.forth.gr/parthenos_vocabularies/Concept/32210"/>
    <skos:narrowMatch rdf:resource="https://isl.ics.forth.gr/parthenos_vocabularies/Concept/32309"/>
    <skos:narrowMatch rdf:resource="https://isl.ics.forth.gr/parthenos_vocabularies/Concept/32466"/>
    <skos:notation>000009</skos:notation>
    <skos:scopeNote xml:lang="fr">Ce terme désigne les types de divisions administratives utilisées par un État ou toute autre structure politique souveraine au sein de ses limites de juridiction. Les caractéristiques intrinsèques de ses unités incluent, entre autres, l'étendue de la zone sur laquelle elles sont appliquées/exercées, l'étendue chronologique pendant laquelle elles sont en vigueur, leurs corps gouvernants et le degré d'autonomie qui leur est attribué par rapport à la gestion et à l'exploitation de leurs ressources.</skos:scopeNote>
    <skos:narrowMatch rdf:resource="https://isl.ics.forth.gr/parthenos_vocabularies/Concept/32451"/>
    <skos:narrowMatch rdf:resource="https://isl.ics.forth.gr/parthenos_vocabularies/Concept/32853"/>
    <skos:narrowMatch rdf:resource="https://isl.ics.forth.gr/parthenos_vocabularies/Concept/32794"/>
    <skos:narrowMatch rdf:resource="https://isl.ics.forth.gr/parthenos_vocabularies/Concept/32602"/>
    <skos:narrowMatch rdf:resource="https://isl.ics.forth.gr/parthenos_vocabularies/Concept/32265"/>
    <skos:narrowMatch rdf:resource="https://isl.ics.forth.gr/parthenos_vocabularies/Concept/32544"/>
    <skos:narrowMatch rdf:resource="https://isl.ics.forth.gr/parthenos_vocabularies/Concept/32214"/>
    <skos:narrowMatch rdf:resource="https://isl.ics.forth.gr/parthenos_vocabularies/Concept/32556"/>
    <skos:narrowMatch rdf:resource="https://isl.ics.forth.gr/parthenos_vocabularies/Concept/32817"/>
    <skos:narrowMatch rdf:resource="https://isl.ics.forth.gr/parthenos_vocabularies/Concept/32703"/>
    <skos:narrowMatch rdf:resource="https://isl.ics.forth.gr/parthenos_vocabularies/Concept/32311"/>
    <skos:narrowMatch rdf:resource="https://isl.ics.forth.gr/parthenos_vocabularies/Concept/32567"/>
    <skos:narrowMatch rdf:resource="https://isl.ics.forth.gr/parthenos_vocabularies/Concept/32498"/>
    <skos:narrowMatch rdf:resource="https://isl.ics.forth.gr/parthenos_vocabularies/Concept/32675"/>
    <skos:narrowMatch rdf:resource="https://isl.ics.forth.gr/parthenos_vocabularies/Concept/32692"/>
    <skos:narrowMatch rdf:resource="https://isl.ics.forth.gr/parthenos_vocabularies/Concept/32616"/>
    <skos:narrowMatch rdf:resource="https://isl.ics.forth.gr/parthenos_vocabularies/Concept/32305"/>
    <skos:narrowMatch rdf:resource="https://isl.ics.forth.gr/parthenos_vocabularies/Concept/32752"/>
    <skos:narrowMatch rdf:resource="https://isl.ics.forth.gr/parthenos_vocabularies/Concept/32916"/>
    <skos:narrowMatch rdf:resource="https://isl.ics.forth.gr/parthenos_vocabularies/Concept/32708"/>
    <skos:narrowMatch rdf:resource="https://isl.ics.forth.gr/parthenos_vocabularies/Concept/32773"/>
    <skos:narrowMatch rdf:resource="https://isl.ics.forth.gr/parthenos_vocabularies/Concept/32743"/>
    <skos:narrowMatch rdf:resource="https://isl.ics.forth.gr/parthenos_vocabularies/Concept/32510"/>
    <skos:narrowMatch rdf:resource="https://isl.ics.forth.gr/parthenos_vocabularies/Concept/32307"/>
    <skos:narrowMatch rdf:resource="https://isl.ics.forth.gr/parthenos_vocabularies/Concept/32254"/>
    <dcterms:dateSubmitted>2015-08-13T07:33:06Z</dcterms:dateSubmitted>
    <skos:scopeNote xml:lang="de">Dieser Term beinhaltet Typen von administrativen Einheiten, die von staatlichen oder anderen souveränen/unabhängigen oder politischen Körperschaften innerhalb der Grenzen ihrer Jurisdiktion genutzt werden. Wesentliche Eigenschaften dieser Einheiten sind u. a. ihre geographische Ausdehnung, ihre chronologische Ausdehnung, ihre Regierungsgremien und der Grad ihrer Autonomie, die ihnen in Bezug auf die Verwaltung ihrer Ressourcen zugesprochen sind.</skos:scopeNote>
    <skos:narrowMatch rdf:resource="https://isl.ics.forth.gr/parthenos_vocabularies/Concept/32838"/>
    <skos:narrowMatch rdf:resource="https://isl.ics.forth.gr/parthenos_vocabularies/Concept/32967"/>
    <skos:narrowMatch rdf:resource="https://isl.ics.forth.gr/parthenos_vocabularies/Concept/32954"/>
    <skos:narrowMatch rdf:resource="https://isl.ics.forth.gr/parthenos_vocabularies/Concept/32387"/>
    <skos:scopeNote xml:lang="el">Ο όρος περιγράφει τύπους διοικητικών διαιρέσεων τους οποίους εφαρμόζει ένα κράτος ή άλλο κρατικό ή πολιτικό μόρφωμα στην επικράτεια δικαιοδοσίας του. Εγγενή χαρακτηριστικά των τύπων αυτών αποτελούν, μεταξύ άλλων, η εδαφική έκταση στην οποία υλοποιούνται/ ασκούνται, η χρονική διάρκεια που είναι σε ισχύ, οι φορείς άσκησης εξουσίας που έχουν στη διάθεσή τους και ο βαθμός αυτονομίας τους σε θέματα διοίκησης και εκμετάλλευσης των πόρων τους.</skos:scopeNote>
    <dcterms:creator xml:lang="en">BBT maintenance WG</dcterms:creator>
    <skos:narrowMatch rdf:resource="https://isl.ics.forth.gr/parthenos_vocabularies/Concept/32329"/>
    <skos:narrowMatch rdf:resource="https://isl.ics.forth.gr/parthenos_vocabularies/Concept/32792"/>
    <skos:narrowMatch rdf:resource="https://isl.ics.forth.gr/parthenos_vocabularies/Concept/32413"/>
    <skos:narrowMatch rdf:resource="https://isl.ics.forth.gr/parthenos_vocabularies/Concept/32269"/>
    <skos:narrowMatch rdf:resource="https://isl.ics.forth.gr/parthenos_vocabularies/Concept/32859"/>
    <skos:narrowMatch rdf:resource="https://isl.ics.forth.gr/parthenos_vocabularies/Concept/32555"/>
    <skos:narrowMatch rdf:resource="https://isl.ics.forth.gr/parthenos_vocabularies/Concept/32593"/>
    <skos:narrowMatch rdf:resource="https://isl.ics.forth.gr/parthenos_vocabularies/Concept/32488"/>
    <skos:narrowMatch rdf:resource="https://isl.ics.forth.gr/parthenos_vocabularies/Concept/32213"/>
    <skos:narrowMatch rdf:resource="https://isl.ics.forth.gr/parthenos_vocabularies/Concept/32468"/>
    <skos:narrowMatch rdf:resource="https://isl.ics.forth.gr/parthenos_vocabularies/Concept/32348"/>
    <skos:prefLabel xml:lang="de">Geopolitische Einheiten</skos:prefLabel>
    <skos:narrowMatch rdf:resource="https://isl.ics.forth.gr/parthenos_vocabularies/Concept/32733"/>
    <skos:narrowMatch rdf:resource="https://isl.ics.forth.gr/parthenos_vocabularies/Concept/32984"/>
    <skos:narrowMatch rdf:resource="https://isl.ics.forth.gr/parthenos_vocabularies/Concept/32538"/>
    <skos:narrowMatch rdf:resource="https://isl.ics.forth.gr/parthenos_vocabularies/Concept/32248"/>
    <skos:narrowMatch rdf:resource="https://isl.ics.forth.gr/parthenos_vocabularies/Concept/32753"/>
    <skos:narrowMatch rdf:resource="https://isl.ics.forth.gr/parthenos_vocabularies/Concept/32354"/>
    <skos:narrowMatch rdf:resource="https://isl.ics.forth.gr/parthenos_vocabularies/Concept/32298"/>
    <skos:narrowMatch rdf:resource="https://isl.ics.forth.gr/parthenos_vocabularies/Concept/32577"/>
    <skos:narrowMatch rdf:resource="https://isl.ics.forth.gr/parthenos_vocabularies/Concept/32806"/>
    <skos:narrowMatch rdf:resource="https://isl.ics.forth.gr/parthenos_vocabularies/Concept/32471"/>
    <skos:narrowMatch rdf:resource="https://isl.ics.forth.gr/parthenos_vocabularies/Concept/32335"/>
    <skos:narrowMatch rdf:resource="https://isl.ics.forth.gr/parthenos_vocabularies/Concept/32445"/>
    <skos:narrowMatch rdf:resource="https://isl.ics.forth.gr/parthenos_vocabularies/Concept/32802"/>
    <skos:narrowMatch rdf:resource="https://isl.ics.forth.gr/parthenos_vocabularies/Concept/32224"/>
    <skos:narrowMatch rdf:resource="https://isl.ics.forth.gr/parthenos_vocabularies/Concept/32691"/>
    <skos:narrowMatch rdf:resource="https://isl.ics.forth.gr/parthenos_vocabularies/Concept/32730"/>
    <skos:narrowMatch rdf:resource="https://isl.ics.forth.gr/parthenos_vocabularies/Concept/32699"/>
    <skos:narrowMatch rdf:resource="https://isl.ics.forth.gr/parthenos_vocabularies/Concept/32523"/>
    <skos:exactMatch rdf:resource="https://humanitiesthesaurus.academyofathens.gr/dyas-resource/Concept/32"/>
    <skos:narrowMatch rdf:resource="https://isl.ics.forth.gr/parthenos_vocabularies/Concept/32446"/>
    <rdf:type rdf:resource="http://www.w3.org/2004/02/skos/core#Concept"/>
    <skos:narrowMatch rdf:resource="https://isl.ics.forth.gr/parthenos_vocabularies/Concept/32573"/>
    <skos:narrowMatch rdf:resource="https://isl.ics.forth.gr/parthenos_vocabularies/Concept/32406"/>
    <skos:narrowMatch rdf:resource="https://isl.ics.forth.gr/parthenos_vocabularies/Concept/32785"/>
    <skos:narrowMatch rdf:resource="https://isl.ics.forth.gr/parthenos_vocabularies/Concept/32246"/>
    <skos:narrowMatch rdf:resource="https://isl.ics.forth.gr/parthenos_vocabularies/Concept/32932"/>
    <skos:narrowMatch rdf:resource="https://isl.ics.forth.gr/parthenos_vocabularies/Concept/32856"/>
    <skos:narrowMatch rdf:resource="https://isl.ics.forth.gr/parthenos_vocabularies/Concept/32271"/>
    <skos:narrowMatch rdf:resource="https://isl.ics.forth.gr/parthenos_vocabularies/Concept/32505"/>
    <skos:narrowMatch rdf:resource="https://isl.ics.forth.gr/parthenos_vocabularies/Concept/32734"/>
    <skos:narrowMatch rdf:resource="https://isl.ics.forth.gr/parthenos_vocabularies/Concept/32611"/>
  </rdf:Description>
  <rdf:Description rdf:about="https://vocabs.dariah.eu/bbt/Concept/000004">
    <rdfs:type rdf:resource="http://www.w3.org/2004/02/skos/core#Concept"/>
    <skos:exactMatch rdf:resource="http://thesauri.dainst.org/_1c0fa2d2"/>
    <skos:narrower rdf:resource="https://vocabs.dariah.eu/bbt/Concept/000020"/>
    <skos:narrower rdf:resource="https://vocabs.dariah.eu/bbt/Concept/000017"/>
    <skos:prefLabel xml:lang="en">material things</skos:prefLabel>
    <skos:prefLabel xml:lang="de">Materielle Objekte</skos:prefLabel>
    <dcterms:dateSubmitted>2015-08-13T07:33:06Z</dcterms:dateSubmitted>
    <skos:scopeNote xml:lang="el">Ο όρος περιγράφει οτιδήποτε άψυχο που έχει υλική υπόσταση, αποτελεί μια ολοκληρωμένη μονάδα και έχει μια σχετική σταθερότητα μορφής με αναγνωρίσιμα όρια. Τέτοιες μονάδες μπορεί να είναι φυσικές ή δημιουργημένες (ως προς τη προέλευση), απλές ή σύνθετες (ως προς τη σύσταση) και να αποτελούνται από μέρη. Στην τελευταία περίπτωση, είναι πιθανό τα μέρη να είναι διακριτά και να προσδιορίζονται ανεξάρτητα από τη μονάδα της οποίας είναι μέρος (π.χ. μια σπηλιά σε ένα βουνό) ή να απαιτείται για τον προσδιορισμό τους η αναφορά στο σύνολο των μερών (π.χ. σκάκι-πιόνια).</skos:scopeNote>
    <dcterms:creator xml:lang="en">BBT maintenance WG</dcterms:creator>
    <skos:scopeNote xml:lang="en">This term classifies things with physical substance that constitute complete units and have a relatively stable form with identifiable boundaries in at least one dimension. Such units can be natural or man-made (with regard to origin), simple or complex (with regard to composition) or consist of parts. In this latter case it is possible that the parts are either distinct and independent from the unit of which they are a part (e.g. a cave on a mountain) or that they have to be defined with reference to the sum of the parts (e.g. chess-chessmen).</skos:scopeNote>
    <dcterms:modified>2019-04-10T11:13:46Z</dcterms:modified>
    <skos:prefLabel xml:lang="el">υλικά αντικείμενα</skos:prefLabel>
    <rdf:type rdf:resource="http://www.w3.org/2004/02/skos/core#Concept"/>
    <skos:scopeNote xml:lang="de">Dieser Term beinhaltet Typen von Objekten mit physischer Substanz, die eine vollkommene Einheit bilden, mit einer relativ stabilen Form und identifizierbaren Grenzen in wenigstens einer Dimension. Diese Einheiten können einen natürlichen oder anthropogenen Ursprung haben, können eine einfache oder komplexe Zusammensetzung aufweisen oder aus mehreren Teilen bestehen. In letzterem Fall können die Teile entweder verschieden und unabhängig von der Einheit sein von dem sie Teil sind (z. B. Höhle in einem Berg) oder müssen in Bezug auf die Gesamtheit des Objektes definiert werden (z. B. Schach - Schachfigur).</skos:scopeNote>
    <skos:prefLabel xml:lang="fr">entités matérielles</skos:prefLabel>
    <skos:narrower rdf:resource="https://vocabs.dariah.eu/bbt/Concept/000018"/>
    <skos:notation>000004</skos:notation>
    <skos:scopeNote xml:lang="fr">Ce terme désigne les types d’entités dotées d’une substance physique qui constitue des unités complètes et qui ont une forme aux contours relativement stables et comportant au moins une dimension. Ces unités peuvent être naturelles ou faites par l’homme (en ce qui concerne leur origine), simples ou complexes (en ce qui concerne leur composition) ou consister en parties. Ces parties peuvent être distinctes et indépendantes de l’unité dont elles font partie (par exemple une grotte dans une montagne) ou peuvent être définies comme la somme de leur parties (les échecs / les pièces du jeu d’échecs).</skos:scopeNote>
    <skos:narrower rdf:resource="https://vocabs.dariah.eu/bbt/Concept/000019"/>
    <skos:topConceptOf rdf:resource="https://vocabs.dariah.eu/bbt/ConceptScheme/Backbone_Thesaurus"/>
  </rdf:Description>
  <rdf:Description rdf:about="https://vocabs.dariah.eu/bbt/Concept/000018">
    <skos:narrowMatch rdf:resource="https://isl.ics.forth.gr/parthenos_vocabularies/Concept/32620"/>
    <skos:narrowMatch rdf:resource="https://isl.ics.forth.gr/parthenos_vocabularies/Concept/32759"/>
    <skos:narrowMatch rdf:resource="https://isl.ics.forth.gr/parthenos_vocabularies/Concept/32848"/>
    <skos:narrowMatch rdf:resource="https://isl.ics.forth.gr/parthenos_vocabularies/Concept/32430"/>
    <skos:narrowMatch rdf:resource="https://isl.ics.forth.gr/parthenos_vocabularies/Concept/32400"/>
    <skos:narrowMatch rdf:resource="https://isl.ics.forth.gr/parthenos_vocabularies/Concept/32992"/>
    <skos:narrowMatch rdf:resource="https://isl.ics.forth.gr/parthenos_vocabularies/Concept/32557"/>
    <skos:narrowMatch rdf:resource="https://isl.ics.forth.gr/parthenos_vocabularies/Concept/32820"/>
    <skos:narrowMatch rdf:resource="https://isl.ics.forth.gr/parthenos_vocabularies/Concept/32330"/>
    <skos:narrowMatch rdf:resource="https://isl.ics.forth.gr/parthenos_vocabularies/Concept/32336"/>
    <skos:narrowMatch rdf:resource="https://isl.ics.forth.gr/parthenos_vocabularies/Concept/32552"/>
    <skos:narrowMatch rdf:resource="https://isl.ics.forth.gr/parthenos_vocabularies/Concept/32721"/>
    <skos:prefLabel xml:lang="de">Gebaute Umgebung</skos:prefLabel>
    <skos:narrowMatch rdf:resource="https://isl.ics.forth.gr/parthenos_vocabularies/Concept/32930"/>
    <skos:narrowMatch rdf:resource="https://isl.ics.forth.gr/parthenos_vocabularies/Concept/32911"/>
    <skos:narrowMatch rdf:resource="https://isl.ics.forth.gr/parthenos_vocabularies/Concept/32520"/>
    <skos:narrowMatch rdf:resource="https://isl.ics.forth.gr/parthenos_vocabularies/Concept/32880"/>
    <skos:narrowMatch rdf:resource="https://isl.ics.forth.gr/parthenos_vocabularies/Concept/32840"/>
    <skos:narrowMatch rdf:resource="https://isl.ics.forth.gr/parthenos_vocabularies/Concept/32771"/>
    <skos:narrowMatch rdf:resource="https://isl.ics.forth.gr/parthenos_vocabularies/Concept/32948"/>
    <skos:narrowMatch rdf:resource="https://isl.ics.forth.gr/parthenos_vocabularies/Concept/32517"/>
    <skos:narrowMatch rdf:resource="https://isl.ics.forth.gr/parthenos_vocabularies/Concept/32986"/>
    <skos:narrowMatch rdf:resource="https://isl.ics.forth.gr/parthenos_vocabularies/Concept/32906"/>
    <skos:narrowMatch rdf:resource="https://isl.ics.forth.gr/parthenos_vocabularies/Concept/32679"/>
    <skos:narrowMatch rdf:resource="https://isl.ics.forth.gr/parthenos_vocabularies/Concept/32261"/>
    <skos:narrowMatch rdf:resource="https://isl.ics.forth.gr/parthenos_vocabularies/Concept/32710"/>
    <skos:narrowMatch rdf:resource="https://isl.ics.forth.gr/parthenos_vocabularies/Concept/32464"/>
    <skos:narrowMatch rdf:resource="https://isl.ics.forth.gr/parthenos_vocabularies/Concept/32369"/>
    <skos:narrowMatch rdf:resource="https://isl.ics.forth.gr/parthenos_vocabularies/Concept/32784"/>
    <skos:narrowMatch rdf:resource="https://isl.ics.forth.gr/parthenos_vocabularies/Concept/32876"/>
    <skos:narrowMatch rdf:resource="https://isl.ics.forth.gr/parthenos_vocabularies/Concept/32453"/>
    <skos:narrowMatch rdf:resource="https://isl.ics.forth.gr/parthenos_vocabularies/Concept/32378"/>
    <skos:narrowMatch rdf:resource="https://isl.ics.forth.gr/parthenos_vocabularies/Concept/32262"/>
    <skos:narrowMatch rdf:resource="https://isl.ics.forth.gr/parthenos_vocabularies/Concept/32775"/>
    <skos:narrowMatch rdf:resource="https://isl.ics.forth.gr/parthenos_vocabularies/Concept/32337"/>
    <skos:narrowMatch rdf:resource="https://isl.ics.forth.gr/parthenos_vocabularies/Concept/32647"/>
    <skos:narrowMatch rdf:resource="https://isl.ics.forth.gr/parthenos_vocabularies/Concept/32253"/>
    <skos:narrowMatch rdf:resource="https://isl.ics.forth.gr/parthenos_vocabularies/Concept/32333"/>
    <skos:narrowMatch rdf:resource="https://isl.ics.forth.gr/parthenos_vocabularies/Concept/32314"/>
    <skos:narrowMatch rdf:resource="https://isl.ics.forth.gr/parthenos_vocabularies/Concept/32613"/>
    <skos:narrowMatch rdf:resource="https://isl.ics.forth.gr/parthenos_vocabularies/Concept/32423"/>
    <skos:narrowMatch rdf:resource="https://isl.ics.forth.gr/parthenos_vocabularies/Concept/32638"/>
    <skos:narrowMatch rdf:resource="https://isl.ics.forth.gr/parthenos_vocabularies/Concept/32866"/>
    <skos:narrowMatch rdf:resource="https://isl.ics.forth.gr/parthenos_vocabularies/Concept/32812"/>
    <skos:narrowMatch rdf:resource="https://isl.ics.forth.gr/parthenos_vocabularies/Concept/32946"/>
    <skos:narrowMatch rdf:resource="https://isl.ics.forth.gr/parthenos_vocabularies/Concept/32301"/>
    <skos:narrowMatch rdf:resource="https://isl.ics.forth.gr/parthenos_vocabularies/Concept/32748"/>
    <skos:narrowMatch rdf:resource="https://isl.ics.forth.gr/parthenos_vocabularies/Concept/32684"/>
    <skos:narrowMatch rdf:resource="https://isl.ics.forth.gr/parthenos_vocabularies/Concept/32993"/>
    <skos:narrowMatch rdf:resource="https://isl.ics.forth.gr/parthenos_vocabularies/Concept/32963"/>
    <skos:narrowMatch rdf:resource="https://isl.ics.forth.gr/parthenos_vocabularies/Concept/32607"/>
    <skos:narrowMatch rdf:resource="https://isl.ics.forth.gr/parthenos_vocabularies/Concept/32804"/>
    <skos:narrowMatch rdf:resource="https://isl.ics.forth.gr/parthenos_vocabularies/Concept/32290"/>
    <skos:narrowMatch rdf:resource="https://isl.ics.forth.gr/parthenos_vocabularies/Concept/32470"/>
    <dcterms:dateSubmitted>2015-08-13T07:18:40Z</dcterms:dateSubmitted>
    <skos:narrowMatch rdf:resource="https://isl.ics.forth.gr/parthenos_vocabularies/Concept/32836"/>
    <skos:narrowMatch rdf:resource="https://isl.ics.forth.gr/parthenos_vocabularies/Concept/32275"/>
    <skos:narrowMatch rdf:resource="https://isl.ics.forth.gr/parthenos_vocabularies/Concept/32226"/>
    <skos:narrowMatch rdf:resource="https://isl.ics.forth.gr/parthenos_vocabularies/Concept/32641"/>
    <skos:narrowMatch rdf:resource="https://isl.ics.forth.gr/parthenos_vocabularies/Concept/32968"/>
    <skos:narrowMatch rdf:resource="https://isl.ics.forth.gr/parthenos_vocabularies/Concept/32568"/>
    <skos:narrowMatch rdf:resource="https://isl.ics.forth.gr/parthenos_vocabularies/Concept/32826"/>
    <skos:narrowMatch rdf:resource="https://isl.ics.forth.gr/parthenos_vocabularies/Concept/32651"/>
    <skos:narrowMatch rdf:resource="https://isl.ics.forth.gr/parthenos_vocabularies/Concept/32980"/>
    <skos:narrowMatch rdf:resource="https://isl.ics.forth.gr/parthenos_vocabularies/Concept/32845"/>
    <skos:narrowMatch rdf:resource="https://isl.ics.forth.gr/parthenos_vocabularies/Concept/32579"/>
    <skos:narrowMatch rdf:resource="https://isl.ics.forth.gr/parthenos_vocabularies/Concept/32553"/>
    <skos:narrowMatch rdf:resource="https://isl.ics.forth.gr/parthenos_vocabularies/Concept/32528"/>
    <skos:narrowMatch rdf:resource="https://isl.ics.forth.gr/parthenos_vocabularies/Concept/32418"/>
    <skos:narrowMatch rdf:resource="https://isl.ics.forth.gr/parthenos_vocabularies/Concept/32843"/>
    <skos:narrowMatch rdf:resource="https://isl.ics.forth.gr/parthenos_vocabularies/Concept/32319"/>
    <skos:narrowMatch rdf:resource="https://isl.ics.forth.gr/parthenos_vocabularies/Concept/32858"/>
    <skos:narrowMatch rdf:resource="https://isl.ics.forth.gr/parthenos_vocabularies/Concept/32718"/>
    <skos:narrowMatch rdf:resource="https://isl.ics.forth.gr/parthenos_vocabularies/Concept/32949"/>
    <skos:narrowMatch rdf:resource="https://isl.ics.forth.gr/parthenos_vocabularies/Concept/32958"/>
    <skos:narrowMatch rdf:resource="https://isl.ics.forth.gr/parthenos_vocabularies/Concept/32419"/>
    <skos:narrowMatch rdf:resource="https://isl.ics.forth.gr/parthenos_vocabularies/Concept/32674"/>
    <skos:narrowMatch rdf:resource="https://isl.ics.forth.gr/parthenos_vocabularies/Concept/32427"/>
    <skos:narrowMatch rdf:resource="https://isl.ics.forth.gr/parthenos_vocabularies/Concept/32766"/>
    <skos:narrowMatch rdf:resource="https://isl.ics.forth.gr/parthenos_vocabularies/Concept/32971"/>
    <skos:narrowMatch rdf:resource="https://isl.ics.forth.gr/parthenos_vocabularies/Concept/32368"/>
    <skos:narrowMatch rdf:resource="https://isl.ics.forth.gr/parthenos_vocabularies/Concept/32630"/>
    <skos:narrowMatch rdf:resource="https://isl.ics.forth.gr/parthenos_vocabularies/Concept/32382"/>
    <skos:narrowMatch rdf:resource="https://isl.ics.forth.gr/parthenos_vocabularies/Concept/32915"/>
    <skos:narrowMatch rdf:resource="https://isl.ics.forth.gr/parthenos_vocabularies/Concept/32776"/>
    <skos:narrowMatch rdf:resource="https://isl.ics.forth.gr/parthenos_vocabularies/Concept/32367"/>
    <skos:narrowMatch rdf:resource="https://isl.ics.forth.gr/parthenos_vocabularies/Concept/32698"/>
    <skos:narrowMatch rdf:resource="https://isl.ics.forth.gr/parthenos_vocabularies/Concept/32795"/>
    <skos:narrowMatch rdf:resource="https://isl.ics.forth.gr/parthenos_vocabularies/Concept/32283"/>
    <skos:narrowMatch rdf:resource="https://isl.ics.forth.gr/parthenos_vocabularies/Concept/32480"/>
    <skos:narrowMatch rdf:resource="https://isl.ics.forth.gr/parthenos_vocabularies/Concept/32408"/>
    <skos:narrowMatch rdf:resource="https://isl.ics.forth.gr/parthenos_vocabularies/Concept/32483"/>
    <skos:narrowMatch rdf:resource="https://isl.ics.forth.gr/parthenos_vocabularies/Concept/32208"/>
    <skos:narrowMatch rdf:resource="https://isl.ics.forth.gr/parthenos_vocabularies/Concept/32565"/>
    <skos:narrowMatch rdf:resource="https://isl.ics.forth.gr/parthenos_vocabularies/Concept/32462"/>
    <skos:narrowMatch rdf:resource="https://isl.ics.forth.gr/parthenos_vocabularies/Concept/32238"/>
    <skos:narrowMatch rdf:resource="https://isl.ics.forth.gr/parthenos_vocabularies/Concept/32363"/>
    <skos:narrowMatch rdf:resource="https://isl.ics.forth.gr/parthenos_vocabularies/Concept/32918"/>
    <skos:narrowMatch rdf:resource="https://isl.ics.forth.gr/parthenos_vocabularies/Concept/32206"/>
    <skos:narrowMatch rdf:resource="https://isl.ics.forth.gr/parthenos_vocabularies/Concept/32972"/>
    <skos:narrowMatch rdf:resource="https://isl.ics.forth.gr/parthenos_vocabularies/Concept/32910"/>
    <skos:narrowMatch rdf:resource="https://isl.ics.forth.gr/parthenos_vocabularies/Concept/32645"/>
    <skos:narrowMatch rdf:resource="https://isl.ics.forth.gr/parthenos_vocabularies/Concept/32886"/>
    <skos:narrowMatch rdf:resource="https://isl.ics.forth.gr/parthenos_vocabularies/Concept/32312"/>
    <skos:narrowMatch rdf:resource="https://isl.ics.forth.gr/parthenos_vocabularies/Concept/32704"/>
    <skos:narrowMatch rdf:resource="https://isl.ics.forth.gr/parthenos_vocabularies/Concept/32767"/>
    <skos:narrowMatch rdf:resource="https://isl.ics.forth.gr/parthenos_vocabularies/Concept/32296"/>
    <skos:narrowMatch rdf:resource="https://isl.ics.forth.gr/parthenos_vocabularies/Concept/32481"/>
    <skos:narrowMatch rdf:resource="https://isl.ics.forth.gr/parthenos_vocabularies/Concept/32381"/>
    <skos:narrowMatch rdf:resource="https://isl.ics.forth.gr/parthenos_vocabularies/Concept/32403"/>
    <skos:narrowMatch rdf:resource="https://isl.ics.forth.gr/parthenos_vocabularies/Concept/32472"/>
    <skos:narrowMatch rdf:resource="https://isl.ics.forth.gr/parthenos_vocabularies/Concept/32287"/>
    <skos:narrowMatch rdf:resource="https://isl.ics.forth.gr/parthenos_vocabularies/Concept/32239"/>
    <skos:narrowMatch rdf:resource="https://isl.ics.forth.gr/parthenos_vocabularies/Concept/32756"/>
    <skos:scopeNote xml:lang="de">Dieser Term klassifiziert Strukturen, einfach oder komplex, unabhängig von ihrer Größe, Dauer der Konstruktion oder Nutzung, die im Boden befestigt oder eingebettet sind und die nicht ohne irreversible Schäden bewegt werden können.</skos:scopeNote>
    <skos:narrowMatch rdf:resource="https://isl.ics.forth.gr/parthenos_vocabularies/Concept/32825"/>
    <skos:narrowMatch rdf:resource="https://isl.ics.forth.gr/parthenos_vocabularies/Concept/32627"/>
    <skos:narrowMatch rdf:resource="https://isl.ics.forth.gr/parthenos_vocabularies/Concept/32362"/>
    <skos:narrowMatch rdf:resource="https://isl.ics.forth.gr/parthenos_vocabularies/Concept/32962"/>
    <skos:narrowMatch rdf:resource="https://isl.ics.forth.gr/parthenos_vocabularies/Concept/32521"/>
    <skos:narrowMatch rdf:resource="https://isl.ics.forth.gr/parthenos_vocabularies/Concept/32650"/>
    <skos:narrowMatch rdf:resource="https://isl.ics.forth.gr/parthenos_vocabularies/Concept/32218"/>
    <skos:narrowMatch rdf:resource="https://isl.ics.forth.gr/parthenos_vocabularies/Concept/32259"/>
    <skos:narrowMatch rdf:resource="https://isl.ics.forth.gr/parthenos_vocabularies/Concept/32236"/>
    <skos:narrowMatch rdf:resource="https://isl.ics.forth.gr/parthenos_vocabularies/Concept/32473"/>
    <skos:narrowMatch rdf:resource="https://isl.ics.forth.gr/parthenos_vocabularies/Concept/32424"/>
    <skos:narrowMatch rdf:resource="https://isl.ics.forth.gr/parthenos_vocabularies/Concept/32762"/>
    <skos:narrowMatch rdf:resource="https://isl.ics.forth.gr/parthenos_vocabularies/Concept/32793"/>
    <skos:narrowMatch rdf:resource="https://isl.ics.forth.gr/parthenos_vocabularies/Concept/32245"/>
    <skos:narrowMatch rdf:resource="https://isl.ics.forth.gr/parthenos_vocabularies/Concept/32660"/>
    <skos:narrowMatch rdf:resource="https://isl.ics.forth.gr/parthenos_vocabularies/Concept/32643"/>
    <skos:narrowMatch rdf:resource="https://isl.ics.forth.gr/parthenos_vocabularies/Concept/32781"/>
    <skos:narrowMatch rdf:resource="https://isl.ics.forth.gr/parthenos_vocabularies/Concept/32377"/>
    <skos:narrowMatch rdf:resource="https://isl.ics.forth.gr/parthenos_vocabularies/Concept/32944"/>
    <skos:narrowMatch rdf:resource="https://isl.ics.forth.gr/parthenos_vocabularies/Concept/32874"/>
    <skos:narrowMatch rdf:resource="https://isl.ics.forth.gr/parthenos_vocabularies/Concept/32315"/>
    <skos:narrowMatch rdf:resource="https://isl.ics.forth.gr/parthenos_vocabularies/Concept/32321"/>
    <skos:narrowMatch rdf:resource="https://isl.ics.forth.gr/parthenos_vocabularies/Concept/32768"/>
    <skos:narrowMatch rdf:resource="https://isl.ics.forth.gr/parthenos_vocabularies/Concept/32902"/>
    <rdfs:type rdf:resource="http://www.w3.org/2004/02/skos/core#Concept"/>
    <skos:narrowMatch rdf:resource="https://isl.ics.forth.gr/parthenos_vocabularies/Concept/32302"/>
    <skos:narrowMatch rdf:resource="https://isl.ics.forth.gr/parthenos_vocabularies/Concept/32922"/>
    <skos:narrowMatch rdf:resource="https://isl.ics.forth.gr/parthenos_vocabularies/Concept/32957"/>
    <skos:narrowMatch rdf:resource="https://isl.ics.forth.gr/parthenos_vocabularies/Concept/32360"/>
    <skos:narrowMatch rdf:resource="https://isl.ics.forth.gr/parthenos_vocabularies/Concept/32580"/>
    <skos:narrowMatch rdf:resource="https://isl.ics.forth.gr/parthenos_vocabularies/Concept/32631"/>
    <skos:narrowMatch rdf:resource="https://isl.ics.forth.gr/parthenos_vocabularies/Concept/32251"/>
    <skos:narrowMatch rdf:resource="https://isl.ics.forth.gr/parthenos_vocabularies/Concept/32561"/>
    <skos:narrowMatch rdf:resource="https://isl.ics.forth.gr/parthenos_vocabularies/Concept/32513"/>
    <skos:narrowMatch rdf:resource="https://isl.ics.forth.gr/parthenos_vocabularies/Concept/32755"/>
    <skos:narrowMatch rdf:resource="https://isl.ics.forth.gr/parthenos_vocabularies/Concept/32291"/>
    <skos:narrowMatch rdf:resource="https://isl.ics.forth.gr/parthenos_vocabularies/Concept/32350"/>
    <skos:narrowMatch rdf:resource="https://isl.ics.forth.gr/parthenos_vocabularies/Concept/32220"/>
    <skos:narrowMatch rdf:resource="https://isl.ics.forth.gr/parthenos_vocabularies/Concept/32499"/>
    <skos:narrowMatch rdf:resource="https://isl.ics.forth.gr/parthenos_vocabularies/Concept/32822"/>
    <skos:narrowMatch rdf:resource="https://isl.ics.forth.gr/parthenos_vocabularies/Concept/32867"/>
    <skos:narrowMatch rdf:resource="https://isl.ics.forth.gr/parthenos_vocabularies/Concept/32863"/>
    <skos:narrowMatch rdf:resource="https://isl.ics.forth.gr/parthenos_vocabularies/Concept/32857"/>
    <skos:narrowMatch rdf:resource="https://isl.ics.forth.gr/parthenos_vocabularies/Concept/32973"/>
    <skos:narrowMatch rdf:resource="https://isl.ics.forth.gr/parthenos_vocabularies/Concept/32882"/>
    <skos:narrowMatch rdf:resource="https://isl.ics.forth.gr/parthenos_vocabularies/Concept/32272"/>
    <skos:narrowMatch rdf:resource="https://isl.ics.forth.gr/parthenos_vocabularies/Concept/32270"/>
    <skos:narrowMatch rdf:resource="https://isl.ics.forth.gr/parthenos_vocabularies/Concept/32797"/>
    <skos:narrowMatch rdf:resource="https://isl.ics.forth.gr/parthenos_vocabularies/Concept/32358"/>
    <skos:narrowMatch rdf:resource="https://isl.ics.forth.gr/parthenos_vocabularies/Concept/32501"/>
    <skos:narrowMatch rdf:resource="https://isl.ics.forth.gr/parthenos_vocabularies/Concept/32746"/>
    <skos:narrowMatch rdf:resource="https://isl.ics.forth.gr/parthenos_vocabularies/Concept/32666"/>
    <skos:narrowMatch rdf:resource="https://isl.ics.forth.gr/parthenos_vocabularies/Concept/32846"/>
    <skos:narrowMatch rdf:resource="https://isl.ics.forth.gr/parthenos_vocabularies/Concept/32452"/>
    <skos:narrowMatch rdf:resource="https://isl.ics.forth.gr/parthenos_vocabularies/Concept/32334"/>
    <skos:narrowMatch rdf:resource="https://isl.ics.forth.gr/parthenos_vocabularies/Concept/32791"/>
    <skos:narrowMatch rdf:resource="https://isl.ics.forth.gr/parthenos_vocabularies/Concept/32624"/>
    <skos:narrowMatch rdf:resource="https://isl.ics.forth.gr/parthenos_vocabularies/Concept/32371"/>
    <skos:narrowMatch rdf:resource="https://isl.ics.forth.gr/parthenos_vocabularies/Concept/32533"/>
    <skos:narrowMatch rdf:resource="https://isl.ics.forth.gr/parthenos_vocabularies/Concept/32289"/>
    <skos:narrowMatch rdf:resource="https://isl.ics.forth.gr/parthenos_vocabularies/Concept/32899"/>
    <skos:prefLabel xml:lang="el">δομημένο περιβάλλον</skos:prefLabel>
    <dcterms:creator xml:lang="en">BBT maintenance WG</dcterms:creator>
    <skos:prefLabel xml:lang="en">built environment</skos:prefLabel>
    <skos:narrowMatch rdf:resource="https://isl.ics.forth.gr/parthenos_vocabularies/Concept/32299"/>
    <skos:narrowMatch rdf:resource="https://isl.ics.forth.gr/parthenos_vocabularies/Concept/32416"/>
    <skos:narrowMatch rdf:resource="https://isl.ics.forth.gr/parthenos_vocabularies/Concept/32923"/>
    <skos:narrowMatch rdf:resource="https://isl.ics.forth.gr/parthenos_vocabularies/Concept/32583"/>
    <skos:narrowMatch rdf:resource="https://isl.ics.forth.gr/parthenos_vocabularies/Concept/32258"/>
    <skos:narrowMatch rdf:resource="https://isl.ics.forth.gr/parthenos_vocabularies/Concept/32740"/>
    <skos:narrowMatch rdf:resource="https://isl.ics.forth.gr/parthenos_vocabularies/Concept/32697"/>
    <skos:narrowMatch rdf:resource="https://isl.ics.forth.gr/parthenos_vocabularies/Concept/32893"/>
    <skos:narrowMatch rdf:resource="https://isl.ics.forth.gr/parthenos_vocabularies/Concept/32844"/>
    <skos:narrowMatch rdf:resource="https://isl.ics.forth.gr/parthenos_vocabularies/Concept/32434"/>
    <skos:narrowMatch rdf:resource="https://isl.ics.forth.gr/parthenos_vocabularies/Concept/32543"/>
    <skos:narrowMatch rdf:resource="https://isl.ics.forth.gr/parthenos_vocabularies/Concept/32653"/>
    <skos:narrowMatch rdf:resource="https://isl.ics.forth.gr/parthenos_vocabularies/Concept/32320"/>
    <skos:notation>000018</skos:notation>
    <skos:narrowMatch rdf:resource="https://isl.ics.forth.gr/parthenos_vocabularies/Concept/32671"/>
    <skos:narrowMatch rdf:resource="https://isl.ics.forth.gr/parthenos_vocabularies/Concept/32989"/>
    <skos:narrowMatch rdf:resource="https://isl.ics.forth.gr/parthenos_vocabularies/Concept/32800"/>
    <skos:broader rdf:resource="https://vocabs.dariah.eu/bbt/Concept/000004"/>
    <skos:narrowMatch rdf:resource="https://isl.ics.forth.gr/parthenos_vocabularies/Concept/32774"/>
    <skos:narrowMatch rdf:resource="https://isl.ics.forth.gr/parthenos_vocabularies/Concept/32410"/>
    <skos:narrowMatch rdf:resource="https://isl.ics.forth.gr/parthenos_vocabularies/Concept/32554"/>
    <skos:narrowMatch rdf:resource="https://isl.ics.forth.gr/parthenos_vocabularies/Concept/32878"/>
    <skos:narrowMatch rdf:resource="https://isl.ics.forth.gr/parthenos_vocabularies/Concept/32450"/>
    <skos:narrowMatch rdf:resource="https://isl.ics.forth.gr/parthenos_vocabularies/Concept/32300"/>
    <skos:narrowMatch rdf:resource="https://isl.ics.forth.gr/parthenos_vocabularies/Concept/32955"/>
    <skos:narrowMatch rdf:resource="https://isl.ics.forth.gr/parthenos_vocabularies/Concept/32782"/>
    <skos:narrowMatch rdf:resource="https://isl.ics.forth.gr/parthenos_vocabularies/Concept/32924"/>
    <skos:narrowMatch rdf:resource="https://isl.ics.forth.gr/parthenos_vocabularies/Concept/32921"/>
    <skos:narrowMatch rdf:resource="https://isl.ics.forth.gr/parthenos_vocabularies/Concept/32507"/>
    <skos:narrowMatch rdf:resource="https://isl.ics.forth.gr/parthenos_vocabularies/Concept/32913"/>
    <skos:scopeNote xml:lang="en">This term classifies structures, simple or complex, regardless of their size, duration of construction or use, that are attached or embedded in the ground and cannot be moved without irreversible damage.</skos:scopeNote>
    <skos:narrowMatch rdf:resource="https://isl.ics.forth.gr/parthenos_vocabularies/Concept/32274"/>
    <skos:narrowMatch rdf:resource="https://isl.ics.forth.gr/parthenos_vocabularies/Concept/32484"/>
    <skos:narrowMatch rdf:resource="https://isl.ics.forth.gr/parthenos_vocabularies/Concept/32717"/>
    <skos:narrowMatch rdf:resource="https://isl.ics.forth.gr/parthenos_vocabularies/Concept/32798"/>
    <skos:narrowMatch rdf:resource="https://isl.ics.forth.gr/parthenos_vocabularies/Concept/32487"/>
    <skos:narrowMatch rdf:resource="https://isl.ics.forth.gr/parthenos_vocabularies/Concept/32652"/>
    <skos:narrowMatch rdf:resource="https://isl.ics.forth.gr/parthenos_vocabularies/Concept/32702"/>
    <skos:narrowMatch rdf:resource="https://isl.ics.forth.gr/parthenos_vocabularies/Concept/32514"/>
    <skos:narrowMatch rdf:resource="https://isl.ics.forth.gr/parthenos_vocabularies/Concept/32625"/>
    <skos:narrowMatch rdf:resource="https://isl.ics.forth.gr/parthenos_vocabularies/Concept/32325"/>
    <skos:narrowMatch rdf:resource="https://isl.ics.forth.gr/parthenos_vocabularies/Concept/32304"/>
    <skos:narrowMatch rdf:resource="https://isl.ics.forth.gr/parthenos_vocabularies/Concept/32789"/>
    <skos:narrowMatch rdf:resource="https://isl.ics.forth.gr/parthenos_vocabularies/Concept/32855"/>
    <skos:narrowMatch rdf:resource="https://isl.ics.forth.gr/parthenos_vocabularies/Concept/32399"/>
    <skos:narrowMatch rdf:resource="https://isl.ics.forth.gr/parthenos_vocabularies/Concept/32929"/>
    <skos:narrowMatch rdf:resource="https://isl.ics.forth.gr/parthenos_vocabularies/Concept/32386"/>
    <skos:narrowMatch rdf:resource="https://isl.ics.forth.gr/parthenos_vocabularies/Concept/32979"/>
    <skos:narrowMatch rdf:resource="https://isl.ics.forth.gr/parthenos_vocabularies/Concept/32229"/>
    <skos:narrowMatch rdf:resource="https://isl.ics.forth.gr/parthenos_vocabularies/Concept/32566"/>
    <skos:narrowMatch rdf:resource="https://isl.ics.forth.gr/parthenos_vocabularies/Concept/32582"/>
    <skos:narrowMatch rdf:resource="https://isl.ics.forth.gr/parthenos_vocabularies/Concept/32551"/>
    <skos:narrowMatch rdf:resource="https://isl.ics.forth.gr/parthenos_vocabularies/Concept/32816"/>
    <skos:narrowMatch rdf:resource="https://isl.ics.forth.gr/parthenos_vocabularies/Concept/32897"/>
    <skos:narrowMatch rdf:resource="https://isl.ics.forth.gr/parthenos_vocabularies/Concept/32937"/>
    <skos:narrowMatch rdf:resource="https://isl.ics.forth.gr/parthenos_vocabularies/Concept/32279"/>
    <skos:narrowMatch rdf:resource="https://isl.ics.forth.gr/parthenos_vocabularies/Concept/32542"/>
    <skos:narrowMatch rdf:resource="https://isl.ics.forth.gr/parthenos_vocabularies/Concept/32364"/>
    <skos:narrowMatch rdf:resource="https://isl.ics.forth.gr/parthenos_vocabularies/Concept/32390"/>
    <skos:narrowMatch rdf:resource="https://isl.ics.forth.gr/parthenos_vocabularies/Concept/32852"/>
    <rdf:type rdf:resource="http://www.w3.org/2004/02/skos/core#Concept"/>
    <skos:narrowMatch rdf:resource="https://isl.ics.forth.gr/parthenos_vocabularies/Concept/32581"/>
    <skos:narrowMatch rdf:resource="https://isl.ics.forth.gr/parthenos_vocabularies/Concept/32861"/>
    <skos:narrowMatch rdf:resource="https://isl.ics.forth.gr/parthenos_vocabularies/Concept/32211"/>
    <skos:narrowMatch rdf:resource="https://isl.ics.forth.gr/parthenos_vocabularies/Concept/32720"/>
    <skos:narrowMatch rdf:resource="https://isl.ics.forth.gr/parthenos_vocabularies/Concept/32207"/>
    <skos:narrowMatch rdf:resource="https://isl.ics.forth.gr/parthenos_vocabularies/Concept/32537"/>
    <skos:narrowMatch rdf:resource="https://isl.ics.forth.gr/parthenos_vocabularies/Concept/32668"/>
    <skos:narrowMatch rdf:resource="https://isl.ics.forth.gr/parthenos_vocabularies/Concept/32688"/>
    <skos:narrowMatch rdf:resource="https://isl.ics.forth.gr/parthenos_vocabularies/Concept/32655"/>
    <skos:narrowMatch rdf:resource="https://isl.ics.forth.gr/parthenos_vocabularies/Concept/32477"/>
    <skos:narrowMatch rdf:resource="https://isl.ics.forth.gr/parthenos_vocabularies/Concept/32475"/>
    <skos:narrowMatch rdf:resource="https://isl.ics.forth.gr/parthenos_vocabularies/Concept/32230"/>
    <skos:scopeNote xml:lang="fr">Ce terme désigne toute structure, simple ou complexe, quelle que soit sa taille, sa durée de construction ou son utilisation, attachée au sol ou enfouie et qui ne peut être déplacée sans dommage irréversible.</skos:scopeNote>
    <skos:narrowMatch rdf:resource="https://isl.ics.forth.gr/parthenos_vocabularies/Concept/32200"/>
    <skos:narrowMatch rdf:resource="https://isl.ics.forth.gr/parthenos_vocabularies/Concept/32347"/>
    <skos:narrowMatch rdf:resource="https://isl.ics.forth.gr/parthenos_vocabularies/Concept/32677"/>
    <skos:narrowMatch rdf:resource="https://isl.ics.forth.gr/parthenos_vocabularies/Concept/32596"/>
    <skos:narrowMatch rdf:resource="https://isl.ics.forth.gr/parthenos_vocabularies/Concept/32619"/>
    <skos:narrowMatch rdf:resource="https://isl.ics.forth.gr/parthenos_vocabularies/Concept/32588"/>
    <skos:narrowMatch rdf:resource="https://isl.ics.forth.gr/parthenos_vocabularies/Concept/32731"/>
    <skos:narrowMatch rdf:resource="https://isl.ics.forth.gr/parthenos_vocabularies/Concept/32678"/>
    <skos:narrowMatch rdf:resource="https://isl.ics.forth.gr/parthenos_vocabularies/Concept/32525"/>
    <skos:narrowMatch rdf:resource="https://isl.ics.forth.gr/parthenos_vocabularies/Concept/32997"/>
    <skos:narrowMatch rdf:resource="https://isl.ics.forth.gr/parthenos_vocabularies/Concept/32355"/>
    <skos:narrowMatch rdf:resource="https://isl.ics.forth.gr/parthenos_vocabularies/Concept/32442"/>
    <skos:narrowMatch rdf:resource="https://isl.ics.forth.gr/parthenos_vocabularies/Concept/32681"/>
    <skos:narrowMatch rdf:resource="https://isl.ics.forth.gr/parthenos_vocabularies/Concept/32222"/>
    <skos:narrowMatch rdf:resource="https://isl.ics.forth.gr/parthenos_vocabularies/Concept/32617"/>
    <skos:note xml:lang="en">Narrower term examples: "single built works", "complexes", "infrastructure", "residential areas"</skos:note>
    <skos:narrowMatch rdf:resource="https://isl.ics.forth.gr/parthenos_vocabularies/Concept/32615"/>
    <skos:narrowMatch rdf:resource="https://isl.ics.forth.gr/parthenos_vocabularies/Concept/32235"/>
    <skos:narrowMatch rdf:resource="https://isl.ics.forth.gr/parthenos_vocabularies/Concept/32633"/>
    <skos:narrowMatch rdf:resource="https://isl.ics.forth.gr/parthenos_vocabularies/Concept/32877"/>
    <skos:narrowMatch rdf:resource="https://isl.ics.forth.gr/parthenos_vocabularies/Concept/32380"/>
    <skos:narrowMatch rdf:resource="https://isl.ics.forth.gr/parthenos_vocabularies/Concept/32584"/>
    <skos:narrowMatch rdf:resource="http://www.eionet.europa.eu/gemet/concept/13136"/>
    <skos:narrowMatch rdf:resource="https://isl.ics.forth.gr/parthenos_vocabularies/Concept/32841"/>
    <skos:narrowMatch rdf:resource="https://isl.ics.forth.gr/parthenos_vocabularies/Concept/32714"/>
    <skos:narrowMatch rdf:resource="https://isl.ics.forth.gr/parthenos_vocabularies/Concept/32444"/>
    <skos:narrowMatch rdf:resource="https://isl.ics.forth.gr/parthenos_vocabularies/Concept/32526"/>
    <skos:narrowMatch rdf:resource="https://isl.ics.forth.gr/parthenos_vocabularies/Concept/32837"/>
    <skos:narrowMatch rdf:resource="https://isl.ics.forth.gr/parthenos_vocabularies/Concept/32310"/>
    <skos:narrowMatch rdf:resource="https://isl.ics.forth.gr/parthenos_vocabularies/Concept/32657"/>
    <skos:narrowMatch rdf:resource="https://isl.ics.forth.gr/parthenos_vocabularies/Concept/32950"/>
    <skos:narrowMatch rdf:resource="https://isl.ics.forth.gr/parthenos_vocabularies/Concept/32662"/>
    <skos:narrowMatch rdf:resource="https://isl.ics.forth.gr/parthenos_vocabularies/Concept/32352"/>
    <skos:narrowMatch rdf:resource="https://isl.ics.forth.gr/parthenos_vocabularies/Concept/32415"/>
    <skos:narrowMatch rdf:resource="https://isl.ics.forth.gr/parthenos_vocabularies/Concept/32240"/>
    <skos:narrowMatch rdf:resource="https://isl.ics.forth.gr/parthenos_vocabularies/Concept/32559"/>
    <skos:narrowMatch rdf:resource="https://isl.ics.forth.gr/parthenos_vocabularies/Concept/32639"/>
    <skos:narrowMatch rdf:resource="https://isl.ics.forth.gr/parthenos_vocabularies/Concept/32898"/>
    <skos:narrowMatch rdf:resource="https://isl.ics.forth.gr/parthenos_vocabularies/Concept/32818"/>
    <skos:narrowMatch rdf:resource="https://isl.ics.forth.gr/parthenos_vocabularies/Concept/32664"/>
    <skos:narrowMatch rdf:resource="https://isl.ics.forth.gr/parthenos_vocabularies/Concept/32292"/>
    <skos:narrowMatch rdf:resource="https://isl.ics.forth.gr/parthenos_vocabularies/Concept/32422"/>
    <skos:narrowMatch rdf:resource="https://isl.ics.forth.gr/parthenos_vocabularies/Concept/32437"/>
    <skos:narrowMatch rdf:resource="https://isl.ics.forth.gr/parthenos_vocabularies/Concept/32327"/>
    <skos:narrowMatch rdf:resource="https://isl.ics.forth.gr/parthenos_vocabularies/Concept/32359"/>
    <skos:narrowMatch rdf:resource="https://isl.ics.forth.gr/parthenos_vocabularies/Concept/32392"/>
    <skos:narrowMatch rdf:resource="https://isl.ics.forth.gr/parthenos_vocabularies/Concept/32421"/>
    <skos:prefLabel xml:lang="fr">environnement bâti</skos:prefLabel>
    <skos:narrowMatch rdf:resource="https://isl.ics.forth.gr/parthenos_vocabularies/Concept/32393"/>
    <skos:narrowMatch rdf:resource="https://isl.ics.forth.gr/parthenos_vocabularies/Concept/32496"/>
    <skos:narrowMatch rdf:resource="https://isl.ics.forth.gr/parthenos_vocabularies/Concept/32875"/>
    <skos:narrowMatch rdf:resource="https://isl.ics.forth.gr/parthenos_vocabularies/Concept/32609"/>
    <skos:narrowMatch rdf:resource="https://isl.ics.forth.gr/parthenos_vocabularies/Concept/32715"/>
    <dcterms:modified>2019-04-10T10:55:26Z</dcterms:modified>
    <skos:narrowMatch rdf:resource="https://isl.ics.forth.gr/parthenos_vocabularies/Concept/32412"/>
    <skos:narrowMatch rdf:resource="https://isl.ics.forth.gr/parthenos_vocabularies/Concept/32832"/>
    <skos:narrowMatch rdf:resource="https://isl.ics.forth.gr/parthenos_vocabularies/Concept/32233"/>
    <skos:narrowMatch rdf:resource="https://isl.ics.forth.gr/parthenos_vocabularies/Concept/32939"/>
    <skos:narrowMatch rdf:resource="https://isl.ics.forth.gr/parthenos_vocabularies/Concept/32831"/>
    <skos:scopeNote xml:lang="el">Η ιεραρχία περιλαμβάνει τύπους υλικών αντικειμένων που αποτελούν προϊόντα της ανθρώπινης δραστηριότητας, με αισθητική, πολιτιστική, ιστορική, επιστημονική, ή άλλου είδους χρηστική αξία, που εκ κατασκευής ή και μέσω συλλογής διαμορφώνονται σε φορητές λειτουργικές οντότητες.</skos:scopeNote>
    <skos:narrowMatch rdf:resource="https://isl.ics.forth.gr/parthenos_vocabularies/Concept/32454"/>
    <skos:narrowMatch rdf:resource="https://isl.ics.forth.gr/parthenos_vocabularies/Concept/32646"/>
    <skos:narrowMatch rdf:resource="https://isl.ics.forth.gr/parthenos_vocabularies/Concept/32712"/>
    <skos:narrowMatch rdf:resource="https://isl.ics.forth.gr/parthenos_vocabularies/Concept/32938"/>
    <skos:narrowMatch rdf:resource="https://isl.ics.forth.gr/parthenos_vocabularies/Concept/32247"/>
    <skos:narrowMatch rdf:resource="https://isl.ics.forth.gr/parthenos_vocabularies/Concept/32398"/>
    <skos:narrowMatch rdf:resource="https://isl.ics.forth.gr/parthenos_vocabularies/Concept/32562"/>
    <skos:narrowMatch rdf:resource="https://isl.ics.forth.gr/parthenos_vocabularies/Concept/32707"/>
    <skos:narrowMatch rdf:resource="https://isl.ics.forth.gr/parthenos_vocabularies/Concept/32429"/>
    <skos:narrowMatch rdf:resource="https://isl.ics.forth.gr/parthenos_vocabularies/Concept/32892"/>
    <skos:narrowMatch rdf:resource="https://isl.ics.forth.gr/parthenos_vocabularies/Concept/32375"/>
    <skos:narrowMatch rdf:resource="https://isl.ics.forth.gr/parthenos_vocabularies/Concept/32945"/>
    <skos:narrowMatch rdf:resource="https://isl.ics.forth.gr/parthenos_vocabularies/Concept/32982"/>
    <skos:narrowMatch rdf:resource="https://isl.ics.forth.gr/parthenos_vocabularies/Concept/32344"/>
    <skos:narrowMatch rdf:resource="https://isl.ics.forth.gr/parthenos_vocabularies/Concept/32842"/>
    <skos:narrowMatch rdf:resource="https://isl.ics.forth.gr/parthenos_vocabularies/Concept/32384"/>
    <skos:narrowMatch rdf:resource="https://isl.ics.forth.gr/parthenos_vocabularies/Concept/32754"/>
    <skos:narrowMatch rdf:resource="https://isl.ics.forth.gr/parthenos_vocabularies/Concept/32870"/>
    <skos:narrowMatch rdf:resource="https://isl.ics.forth.gr/parthenos_vocabularies/Concept/32527"/>
    <skos:narrowMatch rdf:resource="https://isl.ics.forth.gr/parthenos_vocabularies/Concept/32695"/>
    <skos:narrowMatch rdf:resource="https://isl.ics.forth.gr/parthenos_vocabularies/Concept/32640"/>
    <skos:narrowMatch rdf:resource="https://isl.ics.forth.gr/parthenos_vocabularies/Concept/32457"/>
    <skos:narrowMatch rdf:resource="https://isl.ics.forth.gr/parthenos_vocabularies/Concept/32871"/>
    <skos:narrowMatch rdf:resource="https://isl.ics.forth.gr/parthenos_vocabularies/Concept/32576"/>
    <skos:narrowMatch rdf:resource="https://isl.ics.forth.gr/parthenos_vocabularies/Concept/32474"/>
    <skos:narrowMatch rdf:resource="https://isl.ics.forth.gr/parthenos_vocabularies/Concept/32293"/>
    <skos:narrowMatch rdf:resource="https://isl.ics.forth.gr/parthenos_vocabularies/Concept/32297"/>
    <skos:narrowMatch rdf:resource="https://isl.ics.forth.gr/parthenos_vocabularies/Concept/32286"/>
    <skos:narrowMatch rdf:resource="https://isl.ics.forth.gr/parthenos_vocabularies/Concept/32757"/>
    <skos:narrowMatch rdf:resource="https://isl.ics.forth.gr/parthenos_vocabularies/Concept/32570"/>
    <skos:narrowMatch rdf:resource="https://isl.ics.forth.gr/parthenos_vocabularies/Concept/32879"/>
    <skos:narrowMatch rdf:resource="https://isl.ics.forth.gr/parthenos_vocabularies/Concept/32996"/>
    <skos:narrowMatch rdf:resource="https://isl.ics.forth.gr/parthenos_vocabularies/Concept/32644"/>
    <skos:narrowMatch rdf:resource="https://isl.ics.forth.gr/parthenos_vocabularies/Concept/32663"/>
    <skos:narrowMatch rdf:resource="https://isl.ics.forth.gr/parthenos_vocabularies/Concept/32765"/>
    <skos:narrowMatch rdf:resource="https://isl.ics.forth.gr/parthenos_vocabularies/Concept/32605"/>
    <skos:narrowMatch rdf:resource="https://isl.ics.forth.gr/parthenos_vocabularies/Concept/32263"/>
    <skos:narrowMatch rdf:resource="https://isl.ics.forth.gr/parthenos_vocabularies/Concept/32808"/>
    <skos:narrowMatch rdf:resource="https://isl.ics.forth.gr/parthenos_vocabularies/Concept/32942"/>
    <skos:narrowMatch rdf:resource="https://isl.ics.forth.gr/parthenos_vocabularies/Concept/32402"/>
    <skos:narrowMatch rdf:resource="https://isl.ics.forth.gr/parthenos_vocabularies/Concept/32709"/>
    <skos:narrowMatch rdf:resource="https://isl.ics.forth.gr/parthenos_vocabularies/Concept/32469"/>
    <skos:narrowMatch rdf:resource="https://isl.ics.forth.gr/parthenos_vocabularies/Concept/32366"/>
    <skos:narrowMatch rdf:resource="https://isl.ics.forth.gr/parthenos_vocabularies/Concept/32372"/>
    <skos:narrowMatch rdf:resource="http://www.eionet.europa.eu/gemet/concept/13193"/>
    <skos:narrowMatch rdf:resource="https://isl.ics.forth.gr/parthenos_vocabularies/Concept/32869"/>
    <skos:narrowMatch rdf:resource="https://isl.ics.forth.gr/parthenos_vocabularies/Concept/32353"/>
    <skos:narrowMatch rdf:resource="https://isl.ics.forth.gr/parthenos_vocabularies/Concept/32778"/>
    <skos:narrowMatch rdf:resource="https://isl.ics.forth.gr/parthenos_vocabularies/Concept/32833"/>
    <skos:narrowMatch rdf:resource="https://isl.ics.forth.gr/parthenos_vocabularies/Concept/32491"/>
    <skos:narrowMatch rdf:resource="https://isl.ics.forth.gr/parthenos_vocabularies/Concept/32745"/>
    <skos:narrowMatch rdf:resource="https://isl.ics.forth.gr/parthenos_vocabularies/Concept/32374"/>
    <skos:narrowMatch rdf:resource="https://isl.ics.forth.gr/parthenos_vocabularies/Concept/32889"/>
    <skos:narrowMatch rdf:resource="https://isl.ics.forth.gr/parthenos_vocabularies/Concept/32425"/>
    <skos:narrowMatch rdf:resource="https://isl.ics.forth.gr/parthenos_vocabularies/Concept/32920"/>
    <skos:narrowMatch rdf:resource="https://isl.ics.forth.gr/parthenos_vocabularies/Concept/32799"/>
    <skos:narrowMatch rdf:resource="https://isl.ics.forth.gr/parthenos_vocabularies/Concept/32356"/>
    <skos:narrowMatch rdf:resource="https://isl.ics.forth.gr/parthenos_vocabularies/Concept/32433"/>
    <skos:narrowMatch rdf:resource="https://isl.ics.forth.gr/parthenos_vocabularies/Concept/32904"/>
    <skos:narrowMatch rdf:resource="https://isl.ics.forth.gr/parthenos_vocabularies/Concept/32810"/>
    <skos:narrowMatch rdf:resource="https://isl.ics.forth.gr/parthenos_vocabularies/Concept/32787"/>
    <skos:exactMatch rdf:resource="https://humanitiesthesaurus.academyofathens.gr/dyas-resource/Concept/23"/>
    <skos:narrowMatch rdf:resource="https://isl.ics.forth.gr/parthenos_vocabularies/Concept/32636"/>
    <skos:narrowMatch rdf:resource="https://isl.ics.forth.gr/parthenos_vocabularies/Concept/32998"/>
    <skos:narrowMatch rdf:resource="https://isl.ics.forth.gr/parthenos_vocabularies/Concept/32522"/>
    <skos:narrowMatch rdf:resource="https://isl.ics.forth.gr/parthenos_vocabularies/Concept/32732"/>
    <skos:narrowMatch rdf:resource="https://isl.ics.forth.gr/parthenos_vocabularies/Concept/32851"/>
    <skos:narrowMatch rdf:resource="https://isl.ics.forth.gr/parthenos_vocabularies/Concept/32900"/>
    <skos:narrowMatch rdf:resource="https://isl.ics.forth.gr/parthenos_vocabularies/Concept/32575"/>
    <skos:narrowMatch rdf:resource="https://isl.ics.forth.gr/parthenos_vocabularies/Concept/32439"/>
    <skos:narrowMatch rdf:resource="https://isl.ics.forth.gr/parthenos_vocabularies/Concept/32648"/>
    <skos:narrowMatch rdf:resource="https://isl.ics.forth.gr/parthenos_vocabularies/Concept/32219"/>
    <skos:narrowMatch rdf:resource="https://isl.ics.forth.gr/parthenos_vocabularies/Concept/32821"/>
    <skos:narrowMatch rdf:resource="https://isl.ics.forth.gr/parthenos_vocabularies/Concept/32626"/>
    <skos:narrowMatch rdf:resource="https://isl.ics.forth.gr/parthenos_vocabularies/Concept/32919"/>
    <skos:narrowMatch rdf:resource="https://isl.ics.forth.gr/parthenos_vocabularies/Concept/32659"/>
    <skos:narrowMatch rdf:resource="https://isl.ics.forth.gr/parthenos_vocabularies/Concept/32237"/>
    <skos:narrowMatch rdf:resource="https://isl.ics.forth.gr/parthenos_vocabularies/Concept/32216"/>
    <skos:narrowMatch rdf:resource="https://isl.ics.forth.gr/parthenos_vocabularies/Concept/32467"/>
    <skos:narrowMatch rdf:resource="https://isl.ics.forth.gr/parthenos_vocabularies/Concept/32943"/>
    <skos:narrowMatch rdf:resource="https://isl.ics.forth.gr/parthenos_vocabularies/Concept/32492"/>
    <skos:narrowMatch rdf:resource="https://isl.ics.forth.gr/parthenos_vocabularies/Concept/32531"/>
    <skos:narrowMatch rdf:resource="https://isl.ics.forth.gr/parthenos_vocabularies/Concept/32711"/>
    <skos:narrowMatch rdf:resource="https://isl.ics.forth.gr/parthenos_vocabularies/Concept/32966"/>
    <skos:narrowMatch rdf:resource="https://isl.ics.forth.gr/parthenos_vocabularies/Concept/32535"/>
    <skos:narrowMatch rdf:resource="https://isl.ics.forth.gr/parthenos_vocabularies/Concept/32476"/>
    <skos:narrowMatch rdf:resource="https://isl.ics.forth.gr/parthenos_vocabularies/Concept/32772"/>
    <skos:narrowMatch rdf:resource="https://isl.ics.forth.gr/parthenos_vocabularies/Concept/32737"/>
    <skos:narrowMatch rdf:resource="https://isl.ics.forth.gr/parthenos_vocabularies/Concept/32459"/>
    <skos:narrowMatch rdf:resource="https://isl.ics.forth.gr/parthenos_vocabularies/Concept/32379"/>
    <skos:narrowMatch rdf:resource="https://isl.ics.forth.gr/parthenos_vocabularies/Concept/32223"/>
    <skos:narrowMatch rdf:resource="https://isl.ics.forth.gr/parthenos_vocabularies/Concept/32349"/>
    <skos:narrowMatch rdf:resource="https://isl.ics.forth.gr/parthenos_vocabularies/Concept/32204"/>
    <skos:narrowMatch rdf:resource="https://isl.ics.forth.gr/parthenos_vocabularies/Concept/32672"/>
    <skos:narrowMatch rdf:resource="https://isl.ics.forth.gr/parthenos_vocabularies/Concept/32981"/>
    <skos:narrowMatch rdf:resource="https://isl.ics.forth.gr/parthenos_vocabularies/Concept/32744"/>
    <skos:narrowMatch rdf:resource="https://isl.ics.forth.gr/parthenos_vocabularies/Concept/32599"/>
    <skos:narrowMatch rdf:resource="https://isl.ics.forth.gr/parthenos_vocabularies/Concept/32683"/>
    <skos:narrowMatch rdf:resource="https://isl.ics.forth.gr/parthenos_vocabularies/Concept/32313"/>
    <skos:narrowMatch rdf:resource="https://isl.ics.forth.gr/parthenos_vocabularies/Concept/32790"/>
    <skos:narrowMatch rdf:resource="https://isl.ics.forth.gr/parthenos_vocabularies/Concept/32409"/>
    <skos:narrowMatch rdf:resource="https://isl.ics.forth.gr/parthenos_vocabularies/Concept/32252"/>
    <skos:narrowMatch rdf:resource="https://isl.ics.forth.gr/parthenos_vocabularies/Concept/32331"/>
    <skos:narrowMatch rdf:resource="https://isl.ics.forth.gr/parthenos_vocabularies/Concept/32339"/>
    <skos:narrowMatch rdf:resource="https://isl.ics.forth.gr/parthenos_vocabularies/Concept/32201"/>
    <skos:narrowMatch rdf:resource="https://isl.ics.forth.gr/parthenos_vocabularies/Concept/32680"/>
    <skos:narrowMatch rdf:resource="https://isl.ics.forth.gr/parthenos_vocabularies/Concept/32761"/>
    <skos:narrowMatch rdf:resource="https://isl.ics.forth.gr/parthenos_vocabularies/Concept/32860"/>
    <skos:narrowMatch rdf:resource="https://isl.ics.forth.gr/parthenos_vocabularies/Concept/32610"/>
    <skos:narrowMatch rdf:resource="https://isl.ics.forth.gr/parthenos_vocabularies/Concept/32839"/>
    <skos:narrowMatch rdf:resource="https://isl.ics.forth.gr/parthenos_vocabularies/Concept/32977"/>
    <skos:narrowMatch rdf:resource="https://isl.ics.forth.gr/parthenos_vocabularies/Concept/32632"/>
    <skos:narrowMatch rdf:resource="https://isl.ics.forth.gr/parthenos_vocabularies/Concept/32221"/>
    <skos:narrowMatch rdf:resource="https://isl.ics.forth.gr/parthenos_vocabularies/Concept/32621"/>
    <skos:narrowMatch rdf:resource="https://isl.ics.forth.gr/parthenos_vocabularies/Concept/32807"/>
    <skos:exactMatch rdf:resource="http://thesauri.dainst.org/_233a3677"/>
    <skos:narrowMatch rdf:resource="https://isl.ics.forth.gr/parthenos_vocabularies/Concept/32460"/>
    <skos:narrowMatch rdf:resource="https://isl.ics.forth.gr/parthenos_vocabularies/Concept/32267"/>
    <skos:narrowMatch rdf:resource="https://isl.ics.forth.gr/parthenos_vocabularies/Concept/32608"/>
    <skos:narrowMatch rdf:resource="https://isl.ics.forth.gr/parthenos_vocabularies/Concept/32865"/>
    <skos:narrowMatch rdf:resource="https://isl.ics.forth.gr/parthenos_vocabularies/Concept/32465"/>
    <skos:narrowMatch rdf:resource="https://isl.ics.forth.gr/parthenos_vocabularies/Concept/32502"/>
    <skos:narrowMatch rdf:resource="https://isl.ics.forth.gr/parthenos_vocabularies/Concept/32578"/>
    <skos:narrowMatch rdf:resource="https://isl.ics.forth.gr/parthenos_vocabularies/Concept/32404"/>
    <skos:narrowMatch rdf:resource="https://isl.ics.forth.gr/parthenos_vocabularies/Concept/32572"/>
    <skos:narrowMatch rdf:resource="https://isl.ics.forth.gr/parthenos_vocabularies/Concept/32779"/>
    <skos:narrowMatch rdf:resource="https://isl.ics.forth.gr/parthenos_vocabularies/Concept/32228"/>
    <skos:narrowMatch rdf:resource="https://isl.ics.forth.gr/parthenos_vocabularies/Concept/32308"/>
    <skos:narrowMatch rdf:resource="https://isl.ics.forth.gr/parthenos_vocabularies/Concept/32725"/>
    <skos:narrowMatch rdf:resource="https://isl.ics.forth.gr/parthenos_vocabularies/Concept/32824"/>
    <skos:narrowMatch rdf:resource="https://isl.ics.forth.gr/parthenos_vocabularies/Concept/32212"/>
    <skos:narrowMatch rdf:resource="https://isl.ics.forth.gr/parthenos_vocabularies/Concept/32903"/>
    <skos:narrowMatch rdf:resource="https://isl.ics.forth.gr/parthenos_vocabularies/Concept/32203"/>
    <skos:narrowMatch rdf:resource="https://isl.ics.forth.gr/parthenos_vocabularies/Concept/32814"/>
    <skos:narrowMatch rdf:resource="https://isl.ics.forth.gr/parthenos_vocabularies/Concept/32995"/>
    <skos:narrowMatch rdf:resource="https://isl.ics.forth.gr/parthenos_vocabularies/Concept/32742"/>
    <skos:narrowMatch rdf:resource="https://isl.ics.forth.gr/parthenos_vocabularies/Concept/32511"/>
    <skos:narrowMatch rdf:resource="https://isl.ics.forth.gr/parthenos_vocabularies/Concept/32343"/>
    <skos:narrowMatch rdf:resource="https://isl.ics.forth.gr/parthenos_vocabularies/Concept/32303"/>
    <skos:narrowMatch rdf:resource="https://isl.ics.forth.gr/parthenos_vocabularies/Concept/32738"/>
    <skos:narrowMatch rdf:resource="https://isl.ics.forth.gr/parthenos_vocabularies/Concept/32873"/>
    <skos:narrowMatch rdf:resource="https://isl.ics.forth.gr/parthenos_vocabularies/Concept/32323"/>
    <skos:narrowMatch rdf:resource="https://isl.ics.forth.gr/parthenos_vocabularies/Concept/32700"/>
    <skos:narrowMatch rdf:resource="https://isl.ics.forth.gr/parthenos_vocabularies/Concept/32612"/>
    <skos:narrowMatch rdf:resource="https://isl.ics.forth.gr/parthenos_vocabularies/Concept/32438"/>
    <skos:narrowMatch rdf:resource="https://isl.ics.forth.gr/parthenos_vocabularies/Concept/32656"/>
  </rdf:Description>
  <rdf:Description rdf:about="https://vocabs.dariah.eu/bbt/Facet/000006">
    <skos:scopeNote xml:lang="el">Το θέμα αυτό περιλαμβάνει αντικείμενα, η ουσία των οποίων μένει αμετάβλητη ανεξάρτητα από τον φορέα στον οποίο εμφανίζονται κάθε φορά. Προκύπτουν από την ανθρωπινή δραστηριότητα με ή χωρίς τη μεσολάβηση μηχανικών ή ηλεκτρονικών μέσων (έννοιες, σκέψεις στην πρώτη περίπτωση ή ψηφιακές φωτογραφίες, μετρήσεις γεωμετρικών κ.α. μεγεθών στη δεύτερη). 
Παρά το γεγονός ότι τα αντικείμενα αυτά εκδηλώνονται μέσω της χρήσης της ύλης, η τελευταία δεν παίζει κανένα ρόλο στον προσδιορισμό της ταυτότητάς τους. Εφόσον, λοιπόν, τα νοητικά αντικείμενα έχουν την ιδιότητα να εμφανίζονται μέσω της χρήσης της ύλης, (χαρτί, ηλεκτρονικά μέσα, πίνακες, φωτογραφίες, μνήμη κτλ.) μπορεί να υλοποιούνται σε περισσοτέρους από έναν φορείς ταυτόχρονα, χωρίς αυτό να μεταβάλλει ή να τροποποιεί την ταυτότητά τους. Ενώ, όμως, ο φορέας και η συγκεκριμένη εμφάνιση του νοητικού αντικείμενου μέσω υλικών στοιχείων δεν παίζει κανένα ρόλο στον προσδιορισμό του, οποιαδήποτε αλλαγή, μεταβολή ή τροποποίηση του ίδιου του νοητικού αντικειμένου (αφαίρεση ενός τμήματός του, αναθεώρησή του κτλ) επιφέρει αλλαγή στον προσδιορισμό της ταυτότητάς του.

Τα νοητικά αντικείμενα υφίστανται, στο βαθμό που υφίσταται ένας τουλάχιστον φορέας, στον οποίο εκδηλώνονται (συμπεριλαμβανομένης και της ανθρώπινης μνήμης). Η ύπαρξή τους τερματίζεται, όταν εξαφανίζεται και ο τελευταίος φορέας, στον οποίο εμφανίζονται, ή όταν καταστρέφεται η μνήμη στην οποία έχουν καταγραφεί.</skos:scopeNote>
    <skos:prefLabel xml:lang="de">Konzeptionelle Objekte</skos:prefLabel>
    <skos:member rdf:resource="https://vocabs.dariah.eu/bbt/Concept/000006"/>
    <skos:scopeNote xml:lang="en">This facet comprises types of objects whose essence remains the same regardless of the carrier. They are products of the human activity supported by the use of technical or electronic devices (digital photos, geometric measurements etc.) or without it (concepts, thoughts). The fact that they are materially produced does not determine their identity. Conceptual objects have the ability to exist on more than one particular carrier at the same time (paper, electronic signals, photos, human memories etc.), without the latter changing or altering their identity. On the contrary, any alteration of the conceptual object itself (removal of a part, revision etc.) changes the definition of its identity. Conceptual objects exist as long as they can be found on at least one carrier (human memory included). Their existence ends when the last carrier and the last memory are lost.</skos:scopeNote>
    <skos:member rdf:resource="https://vocabs.dariah.eu/bbt/Concept/000022"/>
    <skos:inScheme rdf:resource="https://vocabs.dariah.eu/bbt/ConceptScheme/Backbone_Thesaurus"/>
    <rdf:type rdf:resource="https://vocabs.dariah.eu/bbt/Facet"/>
    <skos:prefLabel xml:lang="el">Νοητικά Αντικείμενα</skos:prefLabel>
    <skos:member rdf:resource="https://vocabs.dariah.eu/bbt/Concept/000024"/>
    <skos:scopeNote xml:lang="fr">Cette facette désigne les objets dont l’essence reste la même quel qu’en soit le support. Ce sont des produits de l’activité humaine qui s’appuient sur l’utilisation de procédés techniques ou électroniques (photo numérique, mesures géométriques) or non (concepts, pensée). Le fait qu’ils soient matériels ne détermine pas leur identité. Les objets conceptuels ont la capacité à exister sur plus d’un seul support en même temps (photos, mémoire humaine, papier, signaux électroniques) sans que cela change leur identité. Au contraire toute modification de l’objet conceptuel (révision, recadrage) change la définition de son identité.
Les objets conceptuels existent tant qu’on peut les trouver sur au moins un support (y compris la mémoire humaine). Leur existence se termine quand le dernier support et la dernière mémoire sont perdus.</skos:scopeNote>
    <skos:member rdf:resource="https://vocabs.dariah.eu/bbt/Concept/000021"/>
    <dcterms:creator xml:lang="en">BBT maintenance WG</dcterms:creator>
    <skos:prefLabel xml:lang="fr">Objets conceptuels</skos:prefLabel>
    <skos:scopeNote xml:lang="de">Diese Facette beinhaltet Objektklassen, deren Essenz unabhängig von ihrem Trägerobjekt sind. Sie sind Produkte menschlicher Aktivität, die mit Hilfe technischer oder elektronischer Geräte (Digitalfotos, geometrische Messgeräte usw.) oder ohne solche (Konzepte, Gedanken, Ideen) entstehen. Ihre materielle Ausführung bestimmt nicht ihre Identität. Konzeptionelle Objekte können auf mehr als einem bestimmten Träger gleichzeitig bestehen (Papier, elektronische Signale, Fotos, menschliche Erinnerung usw.), ohne dass sich ihr Inhalt oder ihre Identität verändern. Im Gegenteil, bewirkt jede Veränderung des konzeptionellen Objektes (Entfernung von Teilen des Objektes, Überarbeitung eines Konzeptes usw.) eine Veränderung in der Definition seiner Identität. Konzeptionelle Objekte existieren so lange sie auf wenigstens einem Träger (inkl. menschlicher Erinnerung) nachgewiesen werden können. Ihre Existenz endet wenn der letzte Träger und die letzte Erinnerung daran verloren sind.</skos:scopeNote>
    <skos:prefLabel xml:lang="en">Conceptual Objects</skos:prefLabel>
    <rdf:type rdf:resource="http://www.w3.org/2004/02/skos/core#Collection"/>
    <skos:member rdf:resource="https://vocabs.dariah.eu/bbt/Concept/000023"/>
  </rdf:Description>
  <rdf:Description rdf:about="https://vocabs.dariah.eu/bbt/Concept/000008">
    <dcterms:creator xml:lang="en">BBT maintenance WG</dcterms:creator>
    <skos:prefLabel xml:lang="el">ρόλοι</skos:prefLabel>
    <dcterms:dateSubmitted>2015-08-13T07:33:06Z</dcterms:dateSubmitted>
    <skos:scopeNote xml:lang="de">Dieser Term umfasst Typen von Haltungen und/oder sozialen Verhaltensweisen, die von einer Person erwartet werden und aus der Beziehung dieses Individuums zu anderen Personen und sozialen Gruppen resultieren oder durch diese erworben werden.</skos:scopeNote>
    <skos:notation>000008</skos:notation>
    <skos:scopeNote xml:lang="el">Ο όρος περιγράφει attitudes and/or social behaviors that are expected of a person and which result from or are acquired through the relation of that person with other individuals or social groups.</skos:scopeNote>
    <skos:narrower rdf:resource="https://vocabs.dariah.eu/bbt/Concept/000025"/>
    <rdf:type rdf:resource="http://www.w3.org/2004/02/skos/core#Concept"/>
    <skos:prefLabel xml:lang="en">roles</skos:prefLabel>
    <skos:narrower rdf:resource="https://vocabs.dariah.eu/bbt/Concept/000026"/>
    <skos:prefLabel xml:lang="de">Rollen</skos:prefLabel>
    <skos:exactMatch rdf:resource="http://thesauri.dainst.org/_9a41616f"/>
    <skos:scopeNote xml:lang="en">This term classifies attitudes and/or social behaviors that are expected of a person and which result from or are acquired through the relation of that person with other individuals or social groups.</skos:scopeNote>
    <skos:scopeNote xml:lang="fr">Ce terme désigne les types de conduites ou comportements sociaux qui sont attendus d’une personne et qui résultent de ou sont acquis par la relation de cette personne avec d’autres individus ou groupes sociaux.</skos:scopeNote>
    <dcterms:modified>2020-01-21T08:13:54Z</dcterms:modified>
    <skos:exactMatch rdf:resource="http://w3id.org/lob/concept/3417"/>
    <skos:topConceptOf rdf:resource="https://vocabs.dariah.eu/bbt/ConceptScheme/Backbone_Thesaurus"/>
    <rdfs:type rdf:resource="http://www.w3.org/2004/02/skos/core#Concept"/>
    <skos:prefLabel xml:lang="fr">rôles</skos:prefLabel>
  </rdf:Description>
  <rdf:Description rdf:about="https://vocabs.dariah.eu/bbt/Facet/000005">
    <skos:prefLabel xml:lang="de">Epochentypen</skos:prefLabel>
    <dcterms:creator xml:lang="en">BBT maintenance WG</dcterms:creator>
    <skos:prefLabel xml:lang="fr">Types d'Époques</skos:prefLabel>
    <skos:scopeNote xml:lang="en">This facet comprises types of cultural, social, intellectual phenomena consistent with each other thus creating intelligible unities. These types of phenomena are spatially and temporally limited and their consistency relies on the appearance of at least one qualitative element that links them in a unity. The spatial and temporal restriction is a formal feature of the facet “types of epochs”. That means that the facet “types of epochs” has no reference to specific realizations of these types of phenomena. Consequently, this facet does not include time periods such as the Renaissance or the Roman period, or the period of the Balkan wars etc., but the types of their categorization, i.e. the abstract concepts by virtue of which it is possible to conceive the cultural, social and intellectual phenomena as coherent.</skos:scopeNote>
    <rdf:type rdf:resource="http://www.w3.org/2004/02/skos/core#Collection"/>
    <skos:prefLabel xml:lang="en">Types of Epochs</skos:prefLabel>
    <skos:scopeNote xml:lang="fr">Cette facette désigne les types de phénomènes culturels, sociaux ou intellectuels cohérents entre eux et créant ainsi des unités intelligibles. Ces types de phénomènes sont limités dans le temps et l'espace et leur cohérence dépend de l'émergence d'au moins un élément qualitatif qui les relie en une unité. La limite spatio-temporelle est une caractéristique formelle de la facette "type d'époques". Cela signifie que la facette "types d'époques" ne se réfère pas aux réalisations particulières de ces types de phénomènes. Par conséquent, cette facette n'inclut pas des périodes comme la Renaissance ou l'époque romaine, ou la période des guerres des Balkans, etc. mais les formes de leur catégorisation c'est à dire les concepts abstraits par lesquels il est possible de concevoir le phénomène culturel, social et intellectuel comme cohérent.</skos:scopeNote>
    <skos:scopeNote xml:lang="el">Περιλαμβάνει τύπους πολιτισμικών, κοινωνικών, διανοητικών φαινομένων που χαρακτηρίζονται από συνοχή δημιουργώντας νοητές ενότητες. Η συνοχή αυτή συγκροτείται λόγω της παρουσίασης ενός τουλάχιστον ποιοτικού στοιχείου που εμφανίζουν σύνολα φαινόμενων χωροχρονικά οριοθετημένων. Η χωροχρονική οριοθέτηση αποτελεί μορφικό χαρακτηριστικό του θέματος «Εποχές», δεν αναφέρεται δηλαδή σε συγκεκριμένες πραγματώσεις του θέματος αυτού. Κατά συνέπεια, στο θέμα αυτό δεν περιλαμβάνονται τα στιγμιότυπα εποχώνόπως η Αναγέννηση ή η Ρωμαϊκή περίοδος, ή η περίοδος των βαλκανικών πολέμων κτλ., αλλά οι τύποι κατηγοριοποίησής τους, δηλαδή οι αφηρημένες έννοιες, βάσει των οποίων είναι δυνατός ο εν γένει προσδιορισμός της συνοχής στην εμφάνιση πολιτισμικών, κοινωνικών και διανοητικών φαινομένων.</skos:scopeNote>
    <skos:member rdf:resource="https://vocabs.dariah.eu/bbt/Concept/000005"/>
    <rdf:type rdf:resource="https://vocabs.dariah.eu/bbt/Facet"/>
    <skos:scopeNote xml:lang="de">Diese Facette beinhaltet Typen von kulturellen, sozialen, intellektuellen Phänomenen, die untereinander konsistent sind und somit verständliche Einheiten bilden. Diese Typen von Phänomenen sind räumlich und zeitlich begrenzt und ihre Konsistenz beruht auf dem Auftreten wenigstens eines qualitativen Elements, welches sie zu einer Einheit verbindet. Die räumliche und zeitliche Beschränkung ist ein formales Merkmal der Facette "Epochentypen". Dies bedeutet, dass die Facette "Epochentypen" keinerlei Referenz zu spezifischen Realisierungen dieser Arten von Phänomenen besitzt. Folglich schließt diese Facette keine Zeiträume wie die Renaissance oder die römische Periode, oder die Periode der Balkankriege usw. ein, sondern umfasst die Arten ihrer Kategorisierungen, d. h. die abstrakten Konzepte aufgrund derer es möglich ist, die kulturelle, soziale und intellektuelle Phänomene zu verstehen.</skos:scopeNote>
    <skos:inScheme rdf:resource="https://vocabs.dariah.eu/bbt/ConceptScheme/Backbone_Thesaurus"/>
    <skos:prefLabel xml:lang="el">Εποχές</skos:prefLabel>
  </rdf:Description>
  <rdf:Description rdf:about="https://vocabs.dariah.eu/bbt/Concept/0000052">
    <skos:broader rdf:resource="https://vocabs.dariah.eu/bbt/Concept/0000049"/>
    <skos:notation>0000052</skos:notation>
    <skos:prefLabel xml:lang="en">3d-volumes</skos:prefLabel>
    <dcterms:dateSubmitted>2020-01-21T08:13:55Z</dcterms:dateSubmitted>
    <skos:scopeNote xml:lang="en">This term characterizes physical features or material objects extending in three dimensions/ defined along three axes of a Euclidean space . They can –but need not –be solid and can be reduced to three dimensional polyhedra. 

NOTE: The kind of Physical feature, Built environment or Geopolitical unit providing the geometric extent -i.e. the bed of a lake filled with water, the volume occupied by a building, or the Exclusive Economic Zone of a sovereign state represented in terms of a 3D volume -can be specified by coordinating this term with the suitable feature type, such as “surface areas of Physical features/ Built environments/ Geopolitical units”.</skos:scopeNote>
    <rdf:type rdf:resource="http://www.w3.org/2004/02/skos/core#Concept"/>
    <dcterms:creator xml:lang="en">BBT maintenance WG</dcterms:creator>
  </rdf:Description>
  <rdf:Description rdf:about="https://vocabs.dariah.eu/bbt/Concept/000017">
    <skos:note xml:lang="en">Narrower term examples:"stelae", "anvils"</skos:note>
    <skos:exactMatch rdf:resource="http://w3id.org/lob/concept/2277"/>
    <skos:scopeNote xml:lang="el">Η ιεραρχία περιλαμβάνει τύπους υλικών αντικειμένων που αποτελούν προϊόντα της ανθρώπινης δραστηριότητας, με αισθητική, πολιτιστική, ιστορική, επιστημονική, ή άλλου είδους χρηστική αξία, που εκ κατασκευής ή και μέσω συλλογής διαμορφώνονται σε φορητές λειτουργικές οντότητες.</skos:scopeNote>
    <skos:broader rdf:resource="https://vocabs.dariah.eu/bbt/Concept/000004"/>
    <skos:scopeNote xml:lang="de">Dieser Term beinhaltet materielle Objekte, die aus menschlichen Anstrengungen entstehen und die einen ästhetischen, kulturellen, historischen, wissenschaftlichen oder utilitaristischen Wert haben sowie von Anfang an/ursprünglich oder durch Sammeln tragbare funktionale Einheiten sind.</skos:scopeNote>
    <skos:scopeNote xml:lang="fr">Ce terme désigne les objets matériels résultant de l’action de l’homme qui ont une valeur esthétique, culturelle, historique, scientifique ou utilitaire et sont par nature ou par collection des entités fonctionnelles portables.</skos:scopeNote>
    <rdf:type rdf:resource="http://www.w3.org/2004/02/skos/core#Concept"/>
    <skos:prefLabel xml:lang="el">κινητά αντικείμενα</skos:prefLabel>
    <dcterms:creator xml:lang="en">BBT maintenance WG</dcterms:creator>
    <skos:prefLabel xml:lang="fr">objets mobiles</skos:prefLabel>
    <dcterms:modified>2019-04-10T10:55:16Z</dcterms:modified>
    <skos:prefLabel xml:lang="de">Mobile Objekte</skos:prefLabel>
    <rdfs:type rdf:resource="http://www.w3.org/2004/02/skos/core#Concept"/>
    <skos:notation>000017</skos:notation>
    <dcterms:dateSubmitted>2015-08-13T07:18:40Z</dcterms:dateSubmitted>
    <skos:prefLabel xml:lang="en">mobile objects</skos:prefLabel>
    <skos:exactMatch rdf:resource="https://humanitiesthesaurus.academyofathens.gr/dyas-resource/Concept/24"/>
    <skos:exactMatch rdf:resource="http://thesauri.dainst.org/_ad8ec5e3"/>
    <skos:scopeNote xml:lang="en">This term classifies material things that result from human endeavor, have aesthetic, cultural, historical, scientific, or other utilitarian value, and are by design or through collecting portable functional entities.</skos:scopeNote>
  </rdf:Description>
  <rdf:Description rdf:about="https://vocabs.dariah.eu/bbt/Concept/000006">
    <skos:prefLabel xml:lang="en">conceptual objects</skos:prefLabel>
    <skos:narrowMatch rdf:resource="https://isl.ics.forth.gr/parthenos_vocabularies/Concept/32999"/>
    <dcterms:creator xml:lang="en">BBT maintenance WG</dcterms:creator>
    <skos:topConceptOf rdf:resource="https://vocabs.dariah.eu/bbt/ConceptScheme/Backbone_Thesaurus"/>
    <skos:narrowMatch rdf:resource="https://isl.ics.forth.gr/parthenos_vocabularies/Concept/5859"/>
    <skos:narrowMatch rdf:resource="https://isl.ics.forth.gr/parthenos_vocabularies/Concept/5863"/>
    <skos:narrowMatch rdf:resource="https://isl.ics.forth.gr/parthenos_vocabularies/Concept/5829"/>
    <skos:prefLabel xml:lang="fr">objets conceptuels</skos:prefLabel>
    <skos:narrower rdf:resource="https://vocabs.dariah.eu/bbt/Concept/000022"/>
    <skos:prefLabel xml:lang="de">Konzeptionelle Objekte</skos:prefLabel>
    <skos:narrower rdf:resource="https://vocabs.dariah.eu/bbt/Concept/000024"/>
    <rdf:type rdf:resource="http://www.w3.org/2004/02/skos/core#Concept"/>
    <dcterms:dateSubmitted>2015-08-13T07:33:06Z</dcterms:dateSubmitted>
    <skos:prefLabel xml:lang="el">νοητικά αντικείμενα</skos:prefLabel>
    <dcterms:modified>2019-04-10T11:11:38Z</dcterms:modified>
    <skos:scopeNote xml:lang="fr">Ce terme désigne les objets dont l’essence reste la même quel qu’en soit le support. Ce sont des produits de l’activité humaine qui s’appuient sur l’utilisation de procédés techniques ou électroniques (photo numérique, mesures géométriques) or non (concepts, pensée). Le fait qu’ils soient matériels ne détermine pas leur identité. Les objets conceptuels ont la capacité à exister sur plus d’un seul support en même temps (photos, mémoire humaine, papier, signaux électroniques) sans que cela change leur identité. Au contraire toute modification de l’objet conceptuel (révision, recadrage) change la définition de son identité.
Les objets conceptuels existent tant qu’on peut les trouver sur au moins un support (y compris la mémoire humaine). Leur existence se termine quand le dernier support et la dernière mémoire sont perdus.</skos:scopeNote>
    <skos:narrower rdf:resource="https://vocabs.dariah.eu/bbt/Concept/000021"/>
    <skos:scopeNote xml:lang="en">This term classifies objects whose essence remains the same regardless of the carrier. They are products of the human activity supported by the use of technical or electronic devices (digital photos, geometric measurements etc.) or without it (concepts, thoughts). The fact that they are materially produced does not determine their identity. Conceptual objects have the ability to exist on more than one particular carrier at the same time (paper, electronic signals, photos, human memories etc.), without the latter changing or altering their identity. On the contrary, any alteration of the conceptual object itself (removal of a part, revision etc.) changes the definition of its identity. Conceptual objects exist as long as they can be found on at least one carrier (human memory included). Their existence ends when the last carrier and the last memory are lost.</skos:scopeNote>
    <skos:exactMatch rdf:resource="http://thesauri.dainst.org/_588a9c73"/>
    <rdfs:type rdf:resource="http://www.w3.org/2004/02/skos/core#Concept"/>
    <skos:scopeNote xml:lang="de">Dieser Term beinhaltet Objektklassen, deren Essenz unabhängig von ihrem Trägerobjekt sind. Sie sind Produkte menschlicher Aktivität, die mit Hilfe technischer oder elektronischer Geräte (Digitalfotos, geometrische Messgeräte usw.) oder ohne solche (Konzepte, Gedanken, Ideen) entstehen. Ihre materielle Ausführung bestimmt nicht ihre Identität. Konzeptionelle Objekte können auf mehr als einem bestimmten Träger gleichzeitig bestehen (Papier, elektronische Signale, Fotos, menschliche Erinnerung usw.), ohne dass sich ihr Inhalt oder ihre Identität verändern. Im Gegenteil, bewirkt jede Veränderung des konzeptionellen Objektes (Entfernung von Teilen des Objektes, Überarbeitung eines Konzeptes usw.) eine Veränderung in der Definition seiner Identität. Konzeptionelle Objekte existieren so lange sie auf wenigstens einem Träger (inkl. menschlicher Erinnerung) nachgewiesen werden können. Ihre Existenz endet wenn der letzte Träger und die letzte Erinnerung daran verloren sind.</skos:scopeNote>
    <skos:scopeNote xml:lang="el">Ο όρος περιγράφει αντικείμενα, η ουσία των οποίων μένει αμετάβλητη ανεξάρτητα από τον φορέα στον οποίο εμφανίζονται κάθε φορά. Προκύπτουν από την ανθρωπινή δραστηριότητα με ή χωρίς τη μεσολάβηση μηχανικών ή ηλεκτρονικών μέσων (έννοιες, σκέψεις στην πρώτη περίπτωση ή ψηφιακές φωτογραφίες, μετρήσεις γεωμετρικών κ.α. μεγεθών στη δεύτερη). 
Παρά το γεγονός ότι τα αντικείμενα αυτά εκδηλώνονται μέσω της χρήσης της ύλης, η τελευταία δεν παίζει κανένα ρόλο στον προσδιορισμό της ταυτότητάς τους. Εφόσον, λοιπόν, τα νοητικά αντικείμενα έχουν την ιδιότητα να εμφανίζονται μέσω της χρήσης της ύλης, (χαρτί, ηλεκτρονικά μέσα, πίνακες, φωτογραφίες, μνήμη κτλ.) μπορεί να υλοποιούνται σε περισσοτέρους από έναν φορείς ταυτόχρονα, χωρίς αυτό να μεταβάλλει ή να τροποποιεί την ταυτότητά τους. Ενώ, όμως, ο φορέας και η συγκεκριμένη εμφάνιση του νοητικού αντικείμενου μέσω υλικών στοιχείων δεν παίζει κανένα ρόλο στον προσδιορισμό του, οποιαδήποτε αλλαγή, μεταβολή ή τροποποίηση του ίδιου του νοητικού αντικειμένου (αφαίρεση ενός τμήματός του, αναθεώρησή του κτλ) επιφέρει αλλαγή στον προσδιορισμό της ταυτότητάς του.

Τα νοητικά αντικείμενα υφίστανται, στο βαθμό που υφίσταται ένας τουλάχιστον φορέας, στον οποίο εκδηλώνονται (συμπεριλαμβανομένης και της ανθρώπινης μνήμης). Η ύπαρξή τους τερματίζεται, όταν εξαφανίζεται και ο τελευταίος φορέας, στον οποίο εμφανίζονται, ή όταν καταστρέφεται η μνήμη στην οποία έχουν καταγραφεί.</skos:scopeNote>
    <skos:notation>000006</skos:notation>
    <skos:narrower rdf:resource="https://vocabs.dariah.eu/bbt/Concept/000023"/>
  </rdf:Description>
  <rdf:Description rdf:about="https://vocabs.dariah.eu/bbt/Concept/000003">
    <skos:scopeNote xml:lang="de">Dieser Term beinhaltet Typen physischer Substanzen, die Komponenten materieller Objekte sind oder zu dessen Herstellung genutzt werden, deren individuelle Substanz in Bezug auf die Funktion der Objekte (z. B. Gold, Wasser, Ziegel usw.) jedoch keine Rolle spielt. Die Facette kann Rohmaterialien, bearbeitete oder unbearbeitete Materialien, sowie modifizierte und zu Objekten inkorporierte Materialien beinhalten. Ihr Hauptmerkmal ist, dass sie nicht individualisiert werden können, d. h. sie bilden keine unabhängigen "Einheiten" mit klaren und deutlichen Grenzen oder Rollen in Bezug auf andere Einheiten der gleichen oder anderen Art.</skos:scopeNote>
    <skos:prefLabel xml:lang="en">materials</skos:prefLabel>
    <skos:narrowMatch rdf:resource="http://www.eionet.europa.eu/gemet/concept/5184"/>
    <skos:narrowMatch rdf:resource="http://www.eionet.europa.eu/gemet/concept/11793"/>
    <skos:notation>000003</skos:notation>
    <skos:narrowMatch rdf:resource="http://www.eionet.europa.eu/gemet/concept/11792"/>
    <skos:scopeNote xml:lang="el">Ο όρος περιγράφει υλικές υποστάσεις που αποτελούν συστατικά υλικών αντικειμένων ή που χρησιμοποιούνται στην κατασκευή τους, χωρίς η ατομική τους υπόσταση να παίζει ρόλο στη λειτουργία του αντικειμένου (π.χ. χρυσός, νερό, τούβλα κ.ά.). Τα υλικά μπορεί να περιλαμβάνουν καθαρές πρώτες ύλες, επεξεργασμένες ή ανεπεξέργαστές, αλλά και υλικά που έχουν μορφοποιηθεί και ενσωματωθεί σε αντικείμενα. Χαρακτηριστικό γνώρισμα των υλικών είναι ότι δεν μπορούν να εξατομικευτούν, να αποτελέσουν δηλαδή διακριτές «μονάδες», με σαφή και διακριτά όρια ή ρόλο σε σχέση με άλλες μονάδες του ίδιου ή διαφορετικού είδους.</skos:scopeNote>
    <skos:exactMatch rdf:resource="http://thesauri.dainst.org/_06103ab8"/>
    <skos:narrowMatch rdf:resource="http://www.eionet.europa.eu/gemet/concept/5912"/>
    <skos:prefLabel xml:lang="fr">matériaux</skos:prefLabel>
    <rdf:type rdf:resource="http://www.w3.org/2004/02/skos/core#Concept"/>
    <skos:prefLabel xml:lang="el">υλικά</skos:prefLabel>
    <skos:scopeNote xml:lang="en">This term classifies physical substances that  are constituents of material objects or are used in their construction, but whose individual substance is not a factor in the objects’ function (e.g. gold, water, bricks, etc.) The term may include pure raw materials, processed or unprocessed, and also materials that have been modelled and are incorporated into objects. Their main attribute is that they cannot be individualized, that is, they cannot be distinct "units" with clear and distinct boundaries or roles in respect to other units of the same or different kind.</skos:scopeNote>
    <rdfs:type rdf:resource="http://www.w3.org/2004/02/skos/core#Concept"/>
    <skos:narrowMatch rdf:resource="http://www.eionet.europa.eu/gemet/concept/5978"/>
    <skos:narrowMatch rdf:resource="http://www.eionet.europa.eu/gemet/concept/7401"/>
    <skos:narrowMatch rdf:resource="http://www.eionet.europa.eu/gemet/concept/4519"/>
    <skos:prefLabel xml:lang="de">Materialien</skos:prefLabel>
    <skos:narrowMatch rdf:resource="http://www.eionet.europa.eu/gemet/concept/4493"/>
    <skos:topConceptOf rdf:resource="https://vocabs.dariah.eu/bbt/ConceptScheme/Backbone_Thesaurus"/>
    <dcterms:creator xml:lang="en">BBT maintenance WG</dcterms:creator>
    <dcterms:dateSubmitted>2015-08-13T07:33:06Z</dcterms:dateSubmitted>
    <skos:narrowMatch rdf:resource="http://www.eionet.europa.eu/gemet/concept/52"/>
    <skos:narrowMatch rdf:resource="http://www.eionet.europa.eu/gemet/concept/2643"/>
    <skos:narrowMatch rdf:resource="http://www.eionet.europa.eu/gemet/concept/11791"/>
    <skos:exactMatch rdf:resource="https://humanitiesthesaurus.academyofathens.gr/dyas-resource/Concept/18"/>
    <skos:narrowMatch rdf:resource="http://www.eionet.europa.eu/gemet/concept/14619"/>
    <skos:narrowMatch rdf:resource="http://www.eionet.europa.eu/gemet/concept/6918"/>
    <skos:scopeNote xml:lang="fr">Ce terme désigne les types de substances physiques qui composent les objets matériels ou sont utilisées dans leur fabrication mais dont la substance individuelle n'est pas un facteur déterminant de la fonction de l'objet (par exemple, or, eau, brique etc.). La facette peut inclure les matières premières, transformées ou non, mais aussi les matériaux qui ont été façonnés et intégrés dans des objets. Leur attribut principal est qu'ils ne peuvent pas être individualisés c'est à dire qu'ils ne sont pas des unités aux frontières ou aux rôles clairs et distincts par rapport à des unités d'une nature identique ou différente.</skos:scopeNote>
    <skos:exactMatch rdf:resource="http://w3id.org/lob/concept/2281"/>
    <skos:narrowMatch rdf:resource="http://www.eionet.europa.eu/gemet/concept/4839"/>
    <dcterms:modified>2019-04-10T11:15:09Z</dcterms:modified>
    <skos:narrowMatch rdf:resource="http://www.eionet.europa.eu/gemet/concept/4523"/>
    <skos:narrowMatch rdf:resource="http://www.eionet.europa.eu/gemet/concept/5756"/>
  </rdf:Description>
  <rdf:Description rdf:about="https://vocabs.dariah.eu/bbt/Concept/000021">
    <skos:prefLabel xml:lang="el">συμβολικά αντικείμενα</skos:prefLabel>
    <skos:prefLabel xml:lang="de">Symbolische Objekte</skos:prefLabel>
    <skos:prefLabel xml:lang="en">symbolic objects</skos:prefLabel>
    <skos:scopeNote xml:lang="fr">Ce terme désigne les symboles identifiables et/ou les agrégations de symboles qui ont une structure objectivement reconnaissable et qui sont documentés comme des unités (ensembles de signes). Les objets symboliques peuvent servir à désigner ou à communiquer un contenu propositionnel mais ne dépendent pas de ce qu’ils désignent ou communiquent. Ils peuvent exister sur un ou plusieurs supports sans que cela leur retire ou ajoute à leur identité de symbole. Le fait d’être objectivement reconnaissables et documentés comme unités rend les objets symboliques indépendants de leur support matériel et de leur contenu symbolique. En conséquence ils peuvent avoir ou non une signification spécifique.</skos:scopeNote>
    <skos:exactMatch rdf:resource="https://humanitiesthesaurus.academyofathens.gr/dyas-resource/Concept/22"/>
    <rdfs:type rdf:resource="http://www.w3.org/2004/02/skos/core#Concept"/>
    <skos:note xml:lang="en">Narrower term examples: "information objects ","structural parts of information objects"</skos:note>
    <skos:narrowMatch rdf:resource="https://isl.ics.forth.gr/parthenos_vocabularies/Concept/33000"/>
    <skos:scopeNote xml:lang="en">This term classifies identifiable symbols and/or any aggregation of symbols, that have an objectively recognizable structure and that are documented as single units (sets or arrays of signs). Symbolic objects may serve to designate something, or to communicate some propositional content, but they don’t depend on what they designate or communicate. They can exist on one or more carriers simultaneously without this feature adding to or removing from the identity of the symbols. Being objectively recognizable and documented as single units, symbolic objects are independent of the material carrier and the symbolized content as well. Consequently symbolic objects may or may not have a specific meaning.</skos:scopeNote>
    <skos:broader rdf:resource="https://vocabs.dariah.eu/bbt/Concept/000006"/>
    <dcterms:modified>2019-04-10T10:55:11Z</dcterms:modified>
    <dcterms:creator xml:lang="en">BBT maintenance WG</dcterms:creator>
    <rdf:type rdf:resource="http://www.w3.org/2004/02/skos/core#Concept"/>
    <skos:exactMatch rdf:resource="http://w3id.org/lob/concept/3431"/>
    <skos:prefLabel xml:lang="fr">objets symboliques</skos:prefLabel>
    <skos:narrowMatch rdf:resource="https://isl.ics.forth.gr/parthenos_vocabularies/Concept/26978"/>
    <skos:notation>000021</skos:notation>
    <dcterms:dateSubmitted>2015-08-13T07:18:40Z</dcterms:dateSubmitted>
    <skos:scopeNote xml:lang="de">Dieser Term umfasst identifizierbare Symbole oder Ansammlungen von Symbolen, die eine objektiv erkennbare Struktur haben und als einzelne Elemente (Satz oder Anordnung von Zeichen) dokumentiert sind. Symbolische Objekte mögen dazu dienen, etwas zu be-/kennzeichnen oder einen bestimmten Inhalt auszudrücken, sind aber unabhängig von dem was sie ausdrücken oder kennzeichnen. Sie können auf einem oder mehreren Trägern gleichzeitig existieren, ohne dass die Träger die Identität der symbolischen Objekte verändern. Da sie objektiv erkennbar und als einzelne Elemente dokumentiert sind, sind symbolische Objekte unabhängig sowohl von ihrem materiellen Träger als auch von dem symbolisierten Inhalt. Folglich können symbolische Objekte eine spezifische Bedeutung haben, müssen aber nicht.</skos:scopeNote>
    <skos:exactMatch rdf:resource="http://thesauri.dainst.org/_598f0dfd"/>
    <skos:scopeNote xml:lang="el">Η ιεραρχία αυτή περιλαμβάνει σύμβολα ή πεπερασμένα σύνολα τύπων συμβόλων, τα οποία είναι αντικειμενικά αναγνωρίσιμα και θεωρούνται ολοκληρωμένες λειτουργικά μονάδες (σειρές ή διατάξεις συμβόλων). Η λειτουργία των συμβολικών αντικειμένων έγκειται στο ότι μπορεί να δηλώνουν κάτι ή να κοινοποιούν κάποιο περιεχόμενο, αλλά τα ίδια τα συμβολικά αντικείμενα είναι ανεξάρτητα από αυτό που δηλώνουν ή κοινοποιούν. Επιπλέον, μπορεί να εκφέρονται από διαφόρους υλικούς φορείς ταυτόχρονα χωρίς αυτό να προσθέτει ή να αφαιρεί κάτι στον προσδιορισμό της ταυτότητας των συμβόλων. Εφόσον λοιπόν τα συμβολικά αντικείμενα είναι αντικειμενικά αναγνωρίσιμα και συνιστούν λειτουργικά ολοκληρωμένες μονάδες (σειρές ή διατάξεις συμβόλων), είναι ανεξάρτητα τόσο από τον υλικό φορέα, από τον οποίο εκφέρονται κάθε φορά, όσο και από το συμβολιζόμενο περιεχόμενο, στο οποίο μπορεί να αναφέρονται και άρα είναι πιθανόν να μην έχουν τα ίδια κάθε φορά κάποιο αναγνωρίσιμο νόημα.</skos:scopeNote>
  </rdf:Description>
  <rdf:Description rdf:about="https://vocabs.dariah.eu/bbt/Concept/000012">
    <skos:prefLabel xml:lang="en">intentional destructions</skos:prefLabel>
    <rdf:type rdf:resource="http://www.w3.org/2004/02/skos/core#Concept"/>
    <dcterms:dateSubmitted>2015-08-13T07:18:40Z</dcterms:dateSubmitted>
    <skos:scopeNote xml:lang="fr">Ce terme désigne les activités intentionnelles menées dans le but de mettre fin à l’existence d’une entité ou d’une situation.</skos:scopeNote>
    <skos:narrowMatch rdf:resource="https://ark.frantiq.fr/ark:/26678/pcrtzwxWSKXL5O"/>
    <dcterms:creator xml:lang="en">BBT maintenance WG</dcterms:creator>
    <skos:exactMatch rdf:resource="https://humanitiesthesaurus.academyofathens.gr/dyas-resource/Concept/19"/>
    <skos:prefLabel xml:lang="fr">destructions volontaires</skos:prefLabel>
    <skos:scopeNote xml:lang="el">Η ιεραρχία αυτή περιλαμβάνει εμπρόθετες ενέργειες που αποσκοπούν στο τέλος της ύπαρξης καταστάσεων και οντοτήτων.</skos:scopeNote>
    <skos:broader rdf:resource="https://vocabs.dariah.eu/bbt/Concept/000001"/>
    <skos:scopeNote xml:lang="de">Dieser Term beinhaltet intentionelle Aktivitäten, die das Ende der Existenz von Entitäten oder Staatsangelegenheiten zum Ziel haben.</skos:scopeNote>
    <rdfs:type rdf:resource="http://www.w3.org/2004/02/skos/core#Concept"/>
    <skos:prefLabel xml:lang="el">εμπρόθετες καταστροφές</skos:prefLabel>
    <skos:prefLabel xml:lang="de">Intentionelle Zerstörung</skos:prefLabel>
    <skos:scopeNote xml:lang="en">This term classifies intentional activities aimed at causing the end of the existence of entities and states of affairs.</skos:scopeNote>
    <dcterms:modified>2019-04-10T10:55:23Z</dcterms:modified>
    <skos:notation>000012</skos:notation>
  </rdf:Description>
  <rdf:Description rdf:about="https://vocabs.dariah.eu/bbt/Concept/000016">
    <skos:scopeNote xml:lang="en">This term classifies changes in states of affairs, things and entities that result from natural phenomena and lead either to a) the creation of new states of affairs/things/entities or b) to the modification of already existing states of affairs/things/entities with the overall effect that their former identity is lost and they are transformed into new entities with a fundamentally different nature.</skos:scopeNote>
    <skos:prefLabel xml:lang="de">Genese</skos:prefLabel>
    <skos:prefLabel xml:lang="el">γενέσεις</skos:prefLabel>
    <rdfs:type rdf:resource="http://www.w3.org/2004/02/skos/core#Concept"/>
    <skos:exactMatch rdf:resource="https://humanitiesthesaurus.academyofathens.gr/dyas-resource/Concept/13"/>
    <skos:prefLabel xml:lang="en">geneses</skos:prefLabel>
    <rdf:type rdf:resource="http://www.w3.org/2004/02/skos/core#Concept"/>
    <skos:scopeNote xml:lang="de">Dieser Term beinhaltet Veränderungen in Zuständen, Dingen oder Entitäten, die aus Naturkatastrophen resultieren und entweder a) zur Herausbildung neuer Zustände/Dinge/Entitäten oder b) zur Modifikation bereits existierender Zustände/Dinge/Entitäten führen mit dem Effekt, dass ihre vorherige Identität verloren geht und sie sich in neue Entitäten mit fundamental neuen Grundzügen wandeln.</skos:scopeNote>
    <skos:prefLabel xml:lang="fr">genèses</skos:prefLabel>
    <dcterms:dateSubmitted>2015-08-13T07:18:40Z</dcterms:dateSubmitted>
    <dcterms:creator xml:lang="en">BBT maintenance WG</dcterms:creator>
    <skos:scopeNote xml:lang="el">Η ιεραρχία αυτή περιλαμβάνει αλλαγές καταστάσεων, πραγμάτων και οντοτήτων που αποδίδονται στην επενέργεια φυσικών αιτιών, τα οποία οδηγούν στη γένεση νέων ή στη μετατροπή της ταυτότητας των υπαρχόντων, με τρόπο ώστε να χάνεται η ταυτότητα των τελευταίων και να προκύπτει μια νέα οντότητα με θεμελιώδη διαφορετική φύση.</skos:scopeNote>
    <skos:exactMatch rdf:resource="http://thesauri.dainst.org/_2fe07279"/>
    <skos:narrowMatch rdf:resource="http://www.eionet.europa.eu/gemet/concept/812"/>
    <skos:scopeNote xml:lang="fr">Ce terme désigne les changements de situations, d'objets ou d’entités pouvant être attribués à l’activité de phénomènes naturels et dont l’effet est de mener soit à la création d’une nouvelle situation, objet ou entité soit à une modification de situation, d'objet ou d’entité telle l'identité antérieure est perdue et  transformée en nouvelle entité de nature fondamentalement différente.</skos:scopeNote>
    <skos:broader rdf:resource="https://vocabs.dariah.eu/bbt/Concept/000002"/>
    <skos:notation>000016</skos:notation>
    <dcterms:modified>2019-04-10T10:55:13Z</dcterms:modified>
  </rdf:Description>
  <rdf:Description rdf:about="https://vocabs.dariah.eu/bbt/Concept/000013">
    <rdf:type rdf:resource="http://www.w3.org/2004/02/skos/core#Concept"/>
    <dcterms:modified>2019-04-10T10:55:26Z</dcterms:modified>
    <dcterms:creator xml:lang="en">BBT maintenance WG</dcterms:creator>
    <skos:exactMatch rdf:resource="https://humanitiesthesaurus.academyofathens.gr/dyas-resource/Concept/21"/>
    <skos:prefLabel xml:lang="de">Funktionen</skos:prefLabel>
    <rdfs:type rdf:resource="http://www.w3.org/2004/02/skos/core#Concept"/>
    <skos:prefLabel xml:lang="el">λειτουργίες</skos:prefLabel>
    <skos:scopeNote xml:lang="fr">Ce terme désigne les activités qui sont les parties structurelles d’un système complexe et relativement stable de procédures permanentes et autonomes se répétant dans ce système et donc contribuant à sa préservation. Bien que ces fonctions fassent partie d'un système plus vaste, chacun d'entre elles est totalement distincte des autres. En tant que parties structurelles d'un système complexe, les fonctions sont des actions qui jouent un certain rôle au sein de ce système et visent à un objectif spécifique qu'elles doivent atteindre. A cet égard, l'objectif qu'une fonction doit atteindre ne peut être différent de celui pour laquelle elle est effectuée. Autrement dit, l'objectif d'une fonction est celui de son critère d'identité. Par conséquent, la notion de fonction est associée aux actions exécutées et à l'objectif visé de telle sorte que si un autre but est atteint en raison de facteurs extérieurs on parle d'une autre fonction ou activité.</skos:scopeNote>
    <dcterms:dateSubmitted>2015-08-13T07:18:40Z</dcterms:dateSubmitted>
    <skos:prefLabel xml:lang="en">functions</skos:prefLabel>
    <skos:broader rdf:resource="https://vocabs.dariah.eu/bbt/Concept/000001"/>
    <skos:scopeNote xml:lang="de">Dieser Term umfasst Aktivitäten, die strukturelle Bestandteile eines relativ stabilen komplexen Systems permanenter und in sich geschlossener Prozesse sind, welche sich innerhalb dieses Systems ständig wiederholen und so zu dessen Erhaltung beitragen. Obwohl Funktionen Teil eines weitergefassten Systems sind, ist jede Funktion völlig unabhängig von dem Rest. Als Teil eines komplexen Systems sind Funktionen als Aktionen zu beschreiben, welche eine bestimmte Rolle innerhalb dessen spielen und gewisse Ziele verfolgen, die sie erreichen müssen. In dieser Hinsicht ist es nicht möglich, dass der von einer Funktion verfolgte Zweck ein anderer ist, als jener für den diese Funktion ausgeführt wird. Der Zweck einer jeden Funktion ist demnach ihr Identitätsmerkmal. Folglich bezieht sich das Konzept der Funktion eindeutig auf die ausgeführte Aktion und auf das durch diese zu erreichende Ziel. Wenn aufgrund äußerer Faktoren ein anderes Ziel erreicht wird, muss daher von einer anderen Funktion oder Aktivität gesprochen werden.</skos:scopeNote>
    <skos:scopeNote xml:lang="el">Η ιεραρχία αυτή περιλαμβάνει ενέργειες που αποτελούν δομικά μέρη ενός σχετικά σταθερά διαρθρωμένου συστήματος (διαδικασιών, οργανισμών, μηχανισμών) μόνιμων και αλληλοεξαρτώμενων διεργασιών που επαναλαμβάνονται στο πλαίσιο αυτού του συστήματος και συντελούν έτσι στη διατήρησή του. Παρόλο που οι λειτουργίες είναι μέρη ενός ευρύτερου συστήματος, κάθε επιμέρους λειτουργία είναι απολύτως διακριτή από κάθε άλλη.Ως δομικά μέρη ενός διαρθρωμένου συστήματος, οι λειτουργίες είναι ενέργειες που έχουν ένα συγκεκριμένο ρόλο στο εσωτερικό του συστήματος και αποσκοπούν σε έναν ορισμένο σκοπό, τον οποίο πρέπει να εκπληρώσουν. Με αυτή την έννοια, δεν είναι δυνατόν ο σκοπός, τον οποίο εκπληρώνουν αυτές οι ενέργειες, να είναι διαφορετικός από τον σκοπό για τον οποίο επιτελούνται∙ με άλλα λόγια, ένα από τα κριτήρια ταυτότητας της λειτουργίας είναι ο σκοπός της.Η έννοια της λειτουργίας συνδέει, άρα, με μονοσήμαντο τρόπο τις σχέσεις των ενεργειών που επιτελούνται και του στόχου που επιτυγχάνουν οι ενέργειες αυτές, ώστε, όταν προκύψει από την παρεμβολή κάποιου άλλου τυχαίου παράγοντα ένας άλλος σκοπός από τον επιδιωκόμενο, να μιλάμε για άλλη λειτουργία ή για άλλη δραστηριότητα.Στον ορισμό της λειτουργίας δεν ενδιαφέρουν ούτε τα βήματα των δραστηριοτήτων για την εκπλήρωση ενός σκοπού, ούτε η μέθοδος, δηλαδή οι περιορισμοί που επιβάλλονται προκειμένου να επιτευχθεί ο σκοπός αυτός.</skos:scopeNote>
    <skos:exactMatch rdf:resource="http://thesauri.dainst.org/_e2eff393"/>
    <skos:prefLabel xml:lang="fr">fonctions</skos:prefLabel>
    <skos:notation>000013</skos:notation>
    <skos:scopeNote xml:lang="en">This term classifies activities that are structural parts of a relatively stable complex system of permanent and self-contained procedures that repeat themselves within this system and thus contribute to its preservation. Although functions are part of a wider system, each function is completely distinct from the rest. As structural parts of a complex system, functions are actions that play a certain role within a system and aim at a specific goal, which they must accomplish. In this respect it is not possible that the purpose which a certain function has to achieve is different from that for which the function is performed. In other words, the purpose of a function is one of its identity criteria. Consequently, the notion of the function univocally relates the actions performed and the target achieved by these actions in such a way that, if some other target is achieved due to external factors, we speak of a different function or activity.</skos:scopeNote>
    <skos:note xml:lang="en">Narrower term examples: "governance"</skos:note>
  </rdf:Description>
  <rdf:Description rdf:about="https://vocabs.dariah.eu/bbt/Concept/000011">
    <rdfs:type rdf:resource="http://www.w3.org/2004/02/skos/core#Concept"/>
    <skos:prefLabel xml:lang="en">human interactions</skos:prefLabel>
    <skos:prefLabel xml:lang="de">Menschliche Interaktionen</skos:prefLabel>
    <skos:prefLabel xml:lang="fr">interactions humaines</skos:prefLabel>
    <skos:notation>000011</skos:notation>
    <skos:scopeNote xml:lang="de">Dieser Term enthält intentionelle Aktivitäten, die durch wenigstens einen Akteur ausgeführt werden und das Erwirken oder Verändern von Phänomenen oder Sachverhalten auf sozialer, politischer, finanzieller, kultureller oder intellektueller Ebene zur Folge haben.</skos:scopeNote>
    <rdf:type rdf:resource="http://www.w3.org/2004/02/skos/core#Concept"/>
    <skos:scopeNote xml:lang="el">Η ιεραρχία αυτή περιλαμβάνει δραστηριότητες από έναν τουλάχιστον δράστη με σκοπό την εμφάνιση ή την αλλαγή φαινομένων ή/και καταστάσεων στο κοινωνικό, πολιτικό οικονομικό, πολιτισμικό και διανοητικό επίπεδο. Δεν πρόκειται για μεμονωμένες πράξεις, αλλά για σύνθετες ενέργειες ανεξαρτήτου κλίμακας.</skos:scopeNote>
    <skos:broader rdf:resource="https://vocabs.dariah.eu/bbt/Concept/000001"/>
    <skos:scopeNote xml:lang="fr">Ce terme désigne les activités menées par au moins un acteur causant ou changeant un phénomène ou une situation au niveau social, politique, financier, culturel ou intellectuel.</skos:scopeNote>
    <dcterms:creator xml:lang="en">BBT maintenance WG</dcterms:creator>
    <skos:scopeNote xml:lang="en">This term classifies intentional activities carried out by at least one actor causing or changing phenomena or states of affairs on the social, political, financial, cultural and intellectual level.</skos:scopeNote>
    <skos:narrowMatch rdf:resource="https://isl.ics.forth.gr/parthenos_vocabularies/Concept/5883"/>
    <skos:exactMatch rdf:resource="https://humanitiesthesaurus.academyofathens.gr/dyas-resource/Concept/20"/>
    <skos:note xml:lang="en">Narrower term examples: "social events, confrontations or conflicts", "political", "social and economic occurrences", "group management"</skos:note>
    <skos:prefLabel xml:lang="el">γεγονότα, συμβάντα</skos:prefLabel>
    <skos:exactMatch rdf:resource="http://thesauri.dainst.org/_4dc296b2"/>
    <dcterms:modified>2019-04-10T10:55:24Z</dcterms:modified>
    <dcterms:dateSubmitted>2015-08-13T07:18:40Z</dcterms:dateSubmitted>
  </rdf:Description>
  <rdf:Description rdf:about="https://vocabs.dariah.eu/bbt/Concept/000001">
    <skos:prefLabel xml:lang="fr">activités</skos:prefLabel>
    <skos:prefLabel xml:lang="en">activities</skos:prefLabel>
    <skos:scopeNote xml:lang="el">Ο όρος περιγράφει εμπρόθετες ενέργειες, οι οποίες οδηγούν στη διατήρηση, τη δημιουργία, την καταστροφή ή τη μεταβολή μιας κατάστασης ή μιας οντότητας (έμβιων όντων, πνευματικών προϊόντων, φυσικών στοιχείων, ομάδων, συγκροτημάτων, πολιτισμικών, κοινωνικών ή πνευματικών φαινομένων κτλ.), και οι οποίες τεκμηριώνονται.</skos:scopeNote>
    <skos:scopeNote xml:lang="fr">Ce terme désigne les types d'actions intentionnelles qui résultent en la conservation, création, production, modification ou destruction d’une entité (être vivant, objet conceptuel ou matériel, groupes, phénomènes sociaux, intellectuels, physiques etc.)</skos:scopeNote>
    <rdf:type rdf:resource="http://www.w3.org/2004/02/skos/core#Concept"/>
    <skos:narrower rdf:resource="https://vocabs.dariah.eu/bbt/Concept/000012"/>
    <skos:scopeNote xml:lang="en">This term classifies intentional actions that result in the preservation, creation, production, modification or destruction of an entity (living beings, conceptual/material objects, groups, social, intellectual, physical etc. phenomena).</skos:scopeNote>
    <rdfs:type rdf:resource="http://www.w3.org/2004/02/skos/core#Concept"/>
    <skos:narrowMatch rdf:resource="http://www.eionet.europa.eu/gemet/concept/1899"/>
    <dcterms:modified>2019-04-10T11:53:24Z</dcterms:modified>
    <skos:scopeNote xml:lang="de">Dieser Term beinhaltet Typen intentioneller Aktionen, die in der Erhaltung, Herstellung, Modifikation oder Zerstörung einer Entität (Lebewesen; konzeptionelle/materielle Objekte; Gruppen; soziale, intellektuelle, physische Phänomene usw.) resultieren.</skos:scopeNote>
    <skos:topConceptOf rdf:resource="https://vocabs.dariah.eu/bbt/ConceptScheme/Backbone_Thesaurus"/>
    <skos:narrower rdf:resource="https://vocabs.dariah.eu/bbt/Concept/000011"/>
    <skos:narrower rdf:resource="https://vocabs.dariah.eu/bbt/Concept/000010"/>
    <dcterms:creator xml:lang="en">BBT maintenance WG</dcterms:creator>
    <skos:prefLabel xml:lang="de">Aktivitäten</skos:prefLabel>
    <dcterms:dateSubmitted>2015-08-13T07:33:06Z</dcterms:dateSubmitted>
    <skos:narrowMatch rdf:resource="http://www.eionet.europa.eu/gemet/concept/1320"/>
    <skos:narrower rdf:resource="https://vocabs.dariah.eu/bbt/Concept/000013"/>
    <skos:narrowMatch rdf:resource="http://www.eionet.europa.eu/gemet/concept/1874"/>
    <skos:notation>000001</skos:notation>
    <skos:prefLabel xml:lang="el">δραστηριότητες</skos:prefLabel>
    <skos:exactMatch rdf:resource="http://thesauri.dainst.org/_e04cc3e7"/>
  </rdf:Description>
  <rdf:Description rdf:about="https://vocabs.dariah.eu/bbt/Concept/000005">
    <skos:scopeNote xml:lang="de">Dieser Term beinhaltet Typen von kulturellen, sozialen, intellektuellen Phänomenen, die untereinander konsistent sind und somit verständliche Einheiten bilden. Diese Typen von Phänomenen sind räumlich und zeitlich begrenzt und ihre Konsistenz beruht auf dem Auftreten wenigstens eines qualitativen Elements, welches sie zu einer Einheit verbindet. Die räumliche und zeitliche Beschränkung ist ein formales Merkmal der Facette "Epochentypen". Dies bedeutet, dass die Facette "Epochentypen" keinerlei Referenz zu spezifischen Realisierungen dieser Arten von Phänomenen besitzt. Folglich schließt diese Facette keine Zeiträume wie die Renaissance oder die römische Periode, oder die Periode der Balkankriege usw. ein, sondern umfasst die Arten ihrer Kategorisierungen, d. h. die abstrakten Konzepte aufgrund derer es möglich ist, die kulturelle, soziale und intellektuelle Phänomene zu verstehen.</skos:scopeNote>
    <skos:prefLabel xml:lang="el">εποχές</skos:prefLabel>
    <skos:note xml:lang="en">Narrower term examples: "geological epochs", "epochs of Art", "epochs of technology"</skos:note>
    <skos:prefLabel xml:lang="fr">types d'époques</skos:prefLabel>
    <rdfs:type rdf:resource="http://www.w3.org/2004/02/skos/core#Concept"/>
    <dcterms:modified>2019-04-10T11:16:38Z</dcterms:modified>
    <skos:scopeNote xml:lang="fr">Ce terme désigne les types de phénomènes culturels, sociaux ou intellectuels cohérents entre eux et créant ainsi des unités intelligibles. Ces types de phénomènes sont limités dans le temps et l'espace et leur cohérence dépend de l'émergence d'au moins un élément qualitatif qui les relie en une unité. La limite spatio-temporelle est une caractéristique formelle de la facette "type d'époques". Cela signifie que la facette "types d'époques" ne se réfère pas aux réalisations particulières de ces types de phénomènes. Par conséquent, cette facette n'inclut pas des périodes comme la Renaissance ou l'époque romaine, ou la période des guerres des Balkans, etc. mais les formes de leur catégorisation c'est à dire les concepts abstraits par lesquels il est possible de concevoir le phénomène culturel, social et intellectuel comme cohérent.</skos:scopeNote>
    <skos:prefLabel xml:lang="en">types of epochs</skos:prefLabel>
    <rdf:type rdf:resource="http://www.w3.org/2004/02/skos/core#Concept"/>
    <dcterms:dateSubmitted>2015-08-13T07:33:06Z</dcterms:dateSubmitted>
    <skos:notation>000005</skos:notation>
    <skos:scopeNote xml:lang="en">This term classifies cultural, social, intellectual phenomena consistent with each other thus creating intelligible unities. These phenomena are spatially and temporally limited and their consistency relies on the appearance of at least one qualitative element that links them in a unity. The spatial and temporal restriction is a formal feature of the facet “types of epochs”. That means that this term has no reference to specific realizations of these types of phenomena. Consequently, this term does not include time periods such as the Renaissance or the Roman period, or the period of the Balkan wars etc., but their categorization, i.e. the abstract concepts by virtue of which it is possible to conceive the cultural, social and intellectual phenomena as coherent.</skos:scopeNote>
    <skos:topConceptOf rdf:resource="https://vocabs.dariah.eu/bbt/ConceptScheme/Backbone_Thesaurus"/>
    <skos:prefLabel xml:lang="de">Epochentypen</skos:prefLabel>
    <dcterms:creator xml:lang="en">BBT maintenance WG</dcterms:creator>
    <skos:scopeNote xml:lang="el">Περιλαμβάνει τύπους πολιτισμικών, κοινωνικών, διανοητικών φαινομένων που χαρακτηρίζονται από συνοχή δημιουργώντας νοητές ενότητες. Η συνοχή αυτή συγκροτείται λόγω της παρουσίασης ενός τουλάχιστον ποιοτικού στοιχείου που εμφανίζουν σύνολα φαινόμενων χωροχρονικά οριοθετημένων. Η χωροχρονική οριοθέτηση αποτελεί μορφικό χαρακτηριστικό του θέματος «Εποχές», δεν αναφέρεται δηλαδή σε συγκεκριμένες πραγματώσεις του θέματος αυτού. Κατά συνέπεια, στο θέμα αυτό δεν περιλαμβάνονται τα στιγμιότυπα εποχώνόπως η Αναγέννηση ή η Ρωμαϊκή περίοδος, ή η περίοδος των βαλκανικών πολέμων κτλ., αλλά οι τύποι κατηγοριοποίησής τους, δηλαδή οι αφηρημένες έννοιες, βάσει των οποίων είναι δυνατός ο εν γένει προσδιορισμός της συνοχής στην εμφάνιση πολιτισμικών, κοινωνικών και διανοητικών φαινομένων.</skos:scopeNote>
    <skos:exactMatch rdf:resource="https://humanitiesthesaurus.academyofathens.gr/dyas-resource/Concept/30"/>
  </rdf:Description>
  <rdf:Description rdf:about="https://vocabs.dariah.eu/bbt/Concept/000023">
    <dcterms:dateSubmitted>2015-08-13T07:18:40Z</dcterms:dateSubmitted>
    <skos:prefLabel xml:lang="fr">méthodes</skos:prefLabel>
    <skos:broader rdf:resource="https://vocabs.dariah.eu/bbt/Concept/000006"/>
    <dcterms:creator xml:lang="en">BBT maintenance WG</dcterms:creator>
    <skos:narrowMatch rdf:resource="https://isl.ics.forth.gr/parthenos_vocabularies/Concept/30492"/>
    <skos:narrowMatch rdf:resource="http://www.eionet.europa.eu/gemet/concept/210"/>
    <skos:scopeNote xml:lang="en">This term classifies systems of specifications, restrictions and regulations about the design (this involves setting the principles, specifying the requirements and the means for achieving the desired result, estimating the consequences and the expected outcome) and/or the performance of the necessary activities (application of the selected principles and rules, provision and activation of the means and requirements for the realization of the chosen goals,  re-estimation of the consequences) in order to achieve certain results of a specific type.</skos:scopeNote>
    <skos:narrowMatch rdf:resource="https://isl.ics.forth.gr/parthenos_vocabularies/Concept/5828"/>
    <skos:prefLabel xml:lang="de">Methoden</skos:prefLabel>
    <rdfs:type rdf:resource="http://www.w3.org/2004/02/skos/core#Concept"/>
    <skos:scopeNote xml:lang="el">Η ιεραρχία αυτή περιλαμβάνει συστήματα κάποιων προδιαγραφών, περιορισμών και κανόνων που αφορούν στον σχεδιασμό (υιοθέτηση αρχών, επιλογή προϋποθέσεων, όρων και μέσων για την επίτευξη του επιθυμητού αποτελέσματος, υπολογισμός των συνεπειών και των αναμενόμενων αποτελεσμάτων) και/ή στην εκτέλεση (εφαρμογή των αρχών και των κανόνων, εφοδιασμός και ενεργοποίηση των μέσων και των όρων για την πραγματοποίηση ενός σκοπού, επανεξέταση των συνεπειών) των απαραίτητων ενεργειών, προκειμένου να επιτευχθεί ένα αποτέλεσμα ορισμένου είδους.</skos:scopeNote>
    <skos:exactMatch rdf:resource="http://thesauri.dainst.org/_39260fea"/>
    <skos:exactMatch rdf:resource="http://w3id.org/lob/concept/2283"/>
    <skos:prefLabel xml:lang="el">μέθοδοι</skos:prefLabel>
    <skos:notation>000023</skos:notation>
    <skos:narrowMatch rdf:resource="https://isl.ics.forth.gr/parthenos_vocabularies/Concept/5886"/>
    <skos:scopeNote xml:lang="de">Dieser Term klassifiziert Systeme von Vorgaben, Beschränkungen und Regulierungen zur Entwicklung (Festlegen von Grundlagen, Spezifizierung von Anforderungen und von Mitteln, um das Resultat zu erzielen, die Konsequenzen und das Ergebnis einzuschätzen), Planung und/oder Durchführung von Aktivitäten, die zur Erzielung bestimmter Resultate nötig sind (Anwendung der ausgewählten Grundlagen und Regeln, Bereitstellung und Anwendung der Mittel für die Realisierung der gesteckten Ziele, Neubewertung der Konsequenzen).</skos:scopeNote>
    <skos:narrowMatch rdf:resource="https://ark.frantiq.fr/ark:/26678/pcrtlpADryiiAo"/>
    <skos:exactMatch rdf:resource="https://humanitiesthesaurus.academyofathens.gr/dyas-resource/Concept/31"/>
    <rdf:type rdf:resource="http://www.w3.org/2004/02/skos/core#Concept"/>
    <skos:prefLabel xml:lang="en">methods</skos:prefLabel>
    <skos:note xml:lang="en">Narrower term examples: "procedures","techniques"</skos:note>
    <dcterms:modified>2019-04-10T10:55:16Z</dcterms:modified>
    <skos:scopeNote xml:lang="fr">Ce terme désigne les systèmes de spécifications, restrictions et régulations pour la conception et/ou la réalisation d’activités nécessaires dans le but d’obtenir certains résultats d’un type particulier. La conception implique de poser les principes, de spécifier les exigences et les moyens pour obtenir le résultat voulu, d'estimer les conséquences et le résultat final. Les activités nécessaires impliquent l’application de principes et de règles, la fourniture et la mise en œuvre de moyens et exigences pour la réalisation des objectifs, la réévaluation des conséquences.</skos:scopeNote>
  </rdf:Description>
  <rdf:Description rdf:about="https://vocabs.dariah.eu/bbt/Concept/0000049">
    <skos:topConceptOf rdf:resource="https://vocabs.dariah.eu/bbt/ConceptScheme/Backbone_Thesaurus"/>
    <rdfs:type rdf:resource="http://www.w3.org/2004/02/skos/core#Concept"/>
    <skos:exactMatch rdf:resource="http://w3id.org/lob/concept/2270"/>
    <dcterms:dateSubmitted>2020-01-21T08:13:53Z</dcterms:dateSubmitted>
    <skos:narrower rdf:resource="https://vocabs.dariah.eu/bbt/Concept/0000053"/>
    <skos:narrower rdf:resource="https://vocabs.dariah.eu/bbt/Concept/0000050"/>
    <rdf:type rdf:resource="http://www.w3.org/2004/02/skos/core#Concept"/>
    <skos:notation>0000049</skos:notation>
    <dcterms:modified>2020-01-21T08:29:34Z</dcterms:modified>
    <skos:narrower rdf:resource="https://vocabs.dariah.eu/bbt/Concept/0000051"/>
    <skos:scopeNote xml:lang="en">This term classifies kinds of designations and definitions of spatial extents based on either geometric expressions or spatial properties of observable features -like mountains, lakes, buildings, cities, etc. -and social constructs -referring to the spatial extent of of territories that fall within the jurisdiction of some geopolitical or other administrative unit.

NOTE: The terms listed as Geometric extents can be coordinated with the suitable type of phenomenal place, in the sense of CRMgeo, classified accordingly under Physical Features, Built Environment or Geopolitical Units.</skos:scopeNote>
    <skos:narrower rdf:resource="https://vocabs.dariah.eu/bbt/Concept/0000052"/>
    <skos:prefLabel xml:lang="en">geometric extents</skos:prefLabel>
    <dcterms:creator xml:lang="en">BBT maintenance WG</dcterms:creator>
  </rdf:Description>
  <rdf:Description rdf:about="https://vocabs.dariah.eu/bbt/Concept/000025">
    <skos:scopeNote xml:lang="fr">Ce terme désigne les rôles officiels attribués à des personnes ou à des groupes sociaux leur accordant des droits et leur donnant des obligations en relation avec soit le fonctionnement de ces droits et/ou soit l’accomplissement de devoirs d’administration et de direction de corps institutionnels. Ces propriétés sont reconnues institutionnellement et socialement et n’ont de sens que dans le contexte d’une communauté organisée.</skos:scopeNote>
    <skos:exactMatch rdf:resource="http://thesauri.dainst.org/_67a3acdc"/>
    <skos:scopeNote xml:lang="el">Η ιεραρχία περιλαμβάνει τύπους θεσμοθετημένων ιδιοτήτων προσώπων ή κοινωνικών ομάδων που υπαγορεύουν δικαιώματα ή/ και υποχρεώσεις σε σχέση με τη λειτουργία των δικαιωμάτων αυτών ή/ και την άσκηση καθηκόντων διοίκησης και διαχείρισης θεσμικών οργάνων. Οι ιδιότητες αυτές είναι θεσμικά και κοινωνικά αναγνωρισμένες και αποκτούν νόημα μόνο στο πλαίσιο μίας οργανωμένης κοινότητας.</skos:scopeNote>
    <dcterms:dateSubmitted>2015-08-13T07:18:40Z</dcterms:dateSubmitted>
    <dcterms:creator xml:lang="en">BBT maintenance WG</dcterms:creator>
    <skos:prefLabel xml:lang="el">αξιώματα</skos:prefLabel>
    <rdf:type rdf:resource="http://www.w3.org/2004/02/skos/core#Concept"/>
    <skos:broader rdf:resource="https://vocabs.dariah.eu/bbt/Concept/000008"/>
    <skos:notation>000025</skos:notation>
    <skos:exactMatch rdf:resource="https://humanitiesthesaurus.academyofathens.gr/dyas-resource/Concept/34"/>
    <skos:prefLabel xml:lang="de">Ämter</skos:prefLabel>
    <dcterms:modified>2020-01-21T08:13:54Z</dcterms:modified>
    <rdfs:type rdf:resource="http://www.w3.org/2004/02/skos/core#Concept"/>
    <skos:prefLabel xml:lang="fr">rôles officiels</skos:prefLabel>
    <skos:scopeNote xml:lang="de">Dieser Term umfasst offizielle Funktionen, die einem Individuum oder einer sozialen Gruppe zugesprochen werden. Solche Funktionen gewähren den Trägern Rechte und/oder schreiben Pflichten bezüglich der Ausübung dieser Rechte und/oder der Ausübung der administrativen und organisatorischen Aufgaben von institutionellen Einrichtungen vor. Diese Funktionen sind entweder institutionell oder sozial anerkannt und erhalten ihren Sinngehalt ausschließlich in dem Kontext einer organisierten Gesellschaft.</skos:scopeNote>
    <skos:scopeNote xml:lang="en">This term classifies official roles attributed to individuals, which grant them rights and/or dictate obligations in relation to exerting these rights and/or to performing of administrative and management duties of institutional bodies. These properties are institutionally and socially recognized and acquire meaning only in the context of an organized community.</skos:scopeNote>
    <skos:prefLabel xml:lang="en">offices</skos:prefLabel>
  </rdf:Description>
  <rdf:Description rdf:about="https://vocabs.dariah.eu/bbt/Concept/000007">
    <dcterms:dateSubmitted>2015-08-13T07:33:06Z</dcterms:dateSubmitted>
    <rdf:type rdf:resource="http://www.w3.org/2004/02/skos/core#Concept"/>
    <dcterms:creator xml:lang="en">BBT maintenance WG</dcterms:creator>
    <skos:scopeNote xml:lang="de">Unter diesem Term werden Beziehungen jeglicher Art klassifiziert (ökonomisch, religiös, athletisch, politisch, national usw.), welche aus gemeinsamen Handlungen mindestens zweier Individuen entstehen. Diese Beziehungen sollten auf der Annahme gemeinsamer Glaubensgrundsätze, Traditionen, Objektive und/oder Handlungen wie auch organisatorischer Merkmale beruhen.</skos:scopeNote>
    <dcterms:modified>2019-04-10T11:17:02Z</dcterms:modified>
    <skos:scopeNote xml:lang="en">This term classifies relations of whatever character (economic, religious, athletic, political, national etc.) that arise from the joint actions of at least two people. These relations should be based on the adoption of common beliefs, traditions, objectives and/or actions as well as showing organizational features.</skos:scopeNote>
    <skos:topConceptOf rdf:resource="https://vocabs.dariah.eu/bbt/ConceptScheme/Backbone_Thesaurus"/>
    <skos:narrowMatch rdf:resource="https://isl.ics.forth.gr/parthenos_vocabularies/Concept/5829"/>
    <skos:prefLabel xml:lang="en">groups and collectivities</skos:prefLabel>
    <skos:narrowMatch rdf:resource="https://humanitiesthesaurus.academyofathens.gr/dyas-resource/Concept/2253"/>
    <skos:prefLabel xml:lang="fr">groupes et collectivités</skos:prefLabel>
    <skos:exactMatch rdf:resource="https://humanitiesthesaurus.academyofathens.gr/dyas-resource/Concept/26"/>
    <skos:prefLabel xml:lang="de">Gruppen und Vereinigungen</skos:prefLabel>
    <skos:notation>000007</skos:notation>
    <skos:note xml:lang="en">Narrower term examples: "ethnicities", "political parties", "artistic groups", "groups of demonstrators".</skos:note>
    <skos:scopeNote xml:lang="fr">Ce terme désigne les relations de toute nature (économique, religieuse, sportives, politiques, nationale etc.) qui émanent de l’action conjuguée d’au moins deux personnes. Ces relations doivent être fondées sur l’adhésion à des croyances, traditions, objectifs et/ou actions communes et présenter également des caractéristiques organisationnelles.</skos:scopeNote>
    <skos:scopeNote xml:lang="el">Ο όρος περιγράφει σχέσεις οποιουδήποτε χαρακτήρα (οικονομικού, θρησκευτικού, αθλητικού, πολιτικού, εθνικού κτλ.) ως αποτέλεσμα κοινών ενεργειών δύο τουλάχιστον ατόμων. Οι σχέσεις αυτές θα πρέπει να στηρίζονται στην υιοθέτηση κοινών πεποιθήσεων ή/και στόχων ή/και δράσεων και να παρουσιάζουν οργανωτικά χαρακτηριστικά.</skos:scopeNote>
    <rdfs:type rdf:resource="http://www.w3.org/2004/02/skos/core#Concept"/>
    <skos:prefLabel xml:lang="el">συλλογικότητες και ομάδες</skos:prefLabel>
  </rdf:Description>
  <rdf:Description rdf:about="https://vocabs.dariah.eu/bbt/Facet/000003">
    <skos:prefLabel xml:lang="fr">Matériaux</skos:prefLabel>
    <rdf:type rdf:resource="http://www.w3.org/2004/02/skos/core#Collection"/>
    <skos:scopeNote xml:lang="en">This facet comprises types of physical substances that are constituents of material objects or are used in their construction, but whose individual substance is not a factor in the objects’ function (eg gold, water, bricks, etc.) The facet may include pure raw materials, processed or unprocessed, and also materials that have been modelled and are incorporated into objects. Their main attribute is that they cannot be individualized, that is, they cannot be distinct "units" with clear and distinct boundaries or roles in respect to other units of the same or different kind.</skos:scopeNote>
    <skos:prefLabel xml:lang="en">Materials</skos:prefLabel>
    <skos:scopeNote xml:lang="fr">Cette facette désigne les types de substances physiques qui composent les objets matériels ou sont utilisées dans leur fabrication mais dont la substance individuelle n'est pas un facteur déterminant de la fonction de l'objet (par exemple, or, eau, brique etc.). La facette peut inclure les matières premières, transformées ou non, mais aussi les matériaux qui ont été façonnés et intégrés dans des objets. Leur attribut principal est qu'ils ne peuvent pas être individualisés c'est à dire qu'ils ne sont pas des unités aux frontières ou aux rôles clairs et distincts par rapport à des unités d'une nature identique ou différente.</skos:scopeNote>
    <skos:inScheme rdf:resource="https://vocabs.dariah.eu/bbt/ConceptScheme/Backbone_Thesaurus"/>
    <skos:prefLabel xml:lang="de">Materialien</skos:prefLabel>
    <skos:scopeNote xml:lang="el">Το θέμα αυτό περιλαμβάνει υλικές υποστάσεις που αποτελούν συστατικά υλικών αντικειμένων ή που χρησιμοποιούνται στην κατασκευή τους, χωρίς η ατομική τους υπόσταση να παίζει ρόλο στη λειτουργία του αντικειμένου (π.χ. χρυσός, νερό, τούβλα κ.ά.). Τα υλικά μπορεί να περιλαμβάνουν καθαρές πρώτες ύλες, επεξεργασμένες ή ανεπεξέργαστές, αλλά και υλικά που έχουν μορφοποιηθεί και ενσωματωθεί σε αντικείμενα. Χαρακτηριστικό γνώρισμα των υλικών είναι ότι δεν μπορούν να εξατομικευτούν, να αποτελέσουν δηλαδή διακριτές «μονάδες», με σαφή και διακριτά όρια ή ρόλο σε σχέση με άλλες μονάδες του ίδιου ή διαφορετικού είδους.</skos:scopeNote>
    <skos:member rdf:resource="https://vocabs.dariah.eu/bbt/Concept/000003"/>
    <dcterms:creator xml:lang="en">BBT maintenance WG</dcterms:creator>
    <skos:scopeNote xml:lang="de">Diese Facette beinhaltet Typen physischer Substanzen, die Komponenten materieller Objekte sind oder zu dessen Herstellung genutzt werden, deren individuelle Substanz in Bezug auf die Funktion der Objekte (z. B. Gold, Wasser, Ziegel usw.) jedoch keine Rolle spielt. Die Facette kann Rohmaterialien, bearbeitete oder unbearbeitete Materialien, sowie modifizierte und zu Objekten inkorporierte Materialien beinhalten. Ihr Hauptmerkmal ist, dass sie nicht individualisiert werden können, d. h. sie bilden keine unabhängigen "Einheiten" mit klaren und deutlichen Grenzen oder Rollen in Bezug auf andere Einheiten der gleichen oder anderen Art.</skos:scopeNote>
    <rdf:type rdf:resource="https://vocabs.dariah.eu/bbt/Facet"/>
    <skos:prefLabel xml:lang="el">Υλικά</skos:prefLabel>
  </rdf:Description>
  <rdf:Description rdf:about="https://vocabs.dariah.eu/bbt/Concept/000002">
    <dcterms:dateSubmitted>2015-08-13T07:33:06Z</dcterms:dateSubmitted>
    <skos:scopeNote xml:lang="de">Diese Term beinhaltet Typen von Veränderungen von Sachverhalten, Dingen und Entitäten, die eine natürliche Ursache haben (z. B. Erdbeben, Fluten).</skos:scopeNote>
    <skos:prefLabel xml:lang="en">natural processes</skos:prefLabel>
    <skos:topConceptOf rdf:resource="https://vocabs.dariah.eu/bbt/ConceptScheme/Backbone_Thesaurus"/>
    <rdf:type rdf:resource="http://www.w3.org/2004/02/skos/core#Concept"/>
    <dcterms:creator xml:lang="en">BBT maintenance WG</dcterms:creator>
    <skos:prefLabel xml:lang="el">φυσικές μεταβολές</skos:prefLabel>
    <skos:prefLabel xml:lang="fr">processus naturel</skos:prefLabel>
    <dcterms:modified>2019-04-10T11:14:33Z</dcterms:modified>
    <skos:exactMatch rdf:resource="http://thesauri.dainst.org/_e140fe64"/>
    <skos:prefLabel xml:lang="de">Natürliche Prozesse</skos:prefLabel>
    <skos:narrower rdf:resource="https://vocabs.dariah.eu/bbt/Concept/000015"/>
    <skos:scopeNote xml:lang="el">Ο όρος περιγράφει αλλαγές καταστάσεων, πραγμάτων και οντοτήτων που αποδίδονται στην επενέργεια φυσικών αιτιών (σεισμών, πλημμύρων κτλ.).</skos:scopeNote>
    <skos:narrower rdf:resource="https://vocabs.dariah.eu/bbt/Concept/000016"/>
    <skos:notation>000002</skos:notation>
    <skos:scopeNote xml:lang="fr">Ce terme désigne tous les types de changements de situations, d'objets ou d’entités résultant d’un phénomène naturel, par exemple tremblements de terre, inondations.</skos:scopeNote>
    <rdfs:type rdf:resource="http://www.w3.org/2004/02/skos/core#Concept"/>
    <skos:scopeNote xml:lang="en">This term classifies changes in states of affairs, things and entities that result from natural phenomena (e.g. earthquakes, floods).</skos:scopeNote>
  </rdf:Description>
  <rdf:Description rdf:about="https://vocabs.dariah.eu/bbt/Facet/000009">
    <skos:prefLabel xml:lang="el">Γεωπολιτικές Μονάδες</skos:prefLabel>
    <skos:scopeNote xml:lang="el">Το θέμα αυτό περιλαμβάνει τύπους διοικητικών διαιρέσεων τους οποίους εφαρμόζει ένα κράτος ή άλλο κρατικό ή πολιτικό μόρφωμα στην επικράτεια δικαιοδοσίας του. Εγγενή χαρακτηριστικά των τύπων αυτών αποτελούν, μεταξύ άλλων, η εδαφική έκταση στην οποία υλοποιούνται/ ασκούνται, η χρονική διάρκεια που είναι σε ισχύ, οι φορείς άσκησης εξουσίας που έχουν στη διάθεσή τους και ο βαθμός αυτονομίας τους σε θέματα διοίκησης και εκμετάλλευσης των πόρων τους.</skos:scopeNote>
    <skos:scopeNote xml:lang="en">This facet comprises types of administrative divisions used by a state or other sovereign or political structure within the boundaries of its jurisdiction. Intrinsic features of these units include, among others, the extent of the area over which they are applied/exercised, the chronological extent during which they are in force, their governing bodies and the degree of autonomy they are granted in relation to managing and exploiting of their resources.</skos:scopeNote>
    <skos:member rdf:resource="https://vocabs.dariah.eu/bbt/Concept/000009"/>
    <rdf:type rdf:resource="http://www.w3.org/2004/02/skos/core#Collection"/>
    <skos:prefLabel xml:lang="de">Geopolitische Einheiten</skos:prefLabel>
    <skos:scopeNote xml:lang="fr">Cette facette désigne les types de divisions administratives utilisées par un État ou toute autre structure politique souveraine au sein de ses limites de juridiction. Les caractéristiques intrinsèques de ses unités incluent, entre autres, l'étendue de la zone sur laquelle elles sont appliquées/exercées, l'étendue chronologique pendant laquelle elles sont en vigueur, leurs corps gouvernants et le degré d'autonomie qui leur est attribué par rapport à la gestion et à l'exploitation de leurs ressources.</skos:scopeNote>
    <skos:prefLabel xml:lang="en">Geopolitical Units</skos:prefLabel>
    <rdf:type rdf:resource="https://vocabs.dariah.eu/bbt/Facet"/>
    <skos:scopeNote xml:lang="de">Diese Facette beinhaltet Typen von administrativen Einheiten, die von staatlichen oder anderen souveränen/unabhängigen oder politischen Körperschaften innerhalb der Grenzen ihrer Jurisdiktion genutzt werden. Wesentliche Eigenschaften dieser Einheiten sind u. a. ihre geographische Ausdehnung, ihre chronologische Ausdehnung, ihre Regierungsgremien und der Grad ihrer Autonomie, die ihnen in Bezug auf die Verwaltung ihrer Ressourcen zugesprochen sind.</skos:scopeNote>
    <dcterms:creator xml:lang="en">BBT maintenance WG</dcterms:creator>
    <skos:prefLabel xml:lang="fr">Unités Géopolitiques</skos:prefLabel>
    <skos:inScheme rdf:resource="https://vocabs.dariah.eu/bbt/ConceptScheme/Backbone_Thesaurus"/>
  </rdf:Description>
  <rdf:Description rdf:about="https://vocabs.dariah.eu/bbt/Concept/000020">
    <dcterms:creator xml:lang="en">BBT maintenance WG</dcterms:creator>
    <skos:prefLabel xml:lang="el">δομικά μέρη υλικών αντικειμένων</skos:prefLabel>
    <skos:scopeNote xml:lang="de">Diese Hierarchie beinhaltet Objekte, die eigens als Teil eines komplexen Objektes hergestellt werden. Die Komponenten sind in Bezug auf das komplexe Objekt, zu dem sie gehören, autonom. Trotz ihrer Autonomie sind sie jedoch in ihrer Funktion nicht unabhängig, sondern sind strukturelle Teile des Objektes, d. h. sie haben eine spezifische Funktion innerhalb des Moduls, zu dem sie gehören und welches sie bilden.
Notiz: Die strukturellen Elemente der materiellen Objekte werden nicht als Narrower Terms des komplexen Objektes, zu welchem sie gehören, betrachtet.</skos:scopeNote>
    <skos:broader rdf:resource="https://vocabs.dariah.eu/bbt/Concept/000004"/>
    <dcterms:modified>2019-04-10T10:55:21Z</dcterms:modified>
    <skos:exactMatch rdf:resource="http://thesauri.dainst.org/_6a93899c"/>
    <skos:scopeNote xml:lang="el">Η ιεραρχία αυτή περιλαμβάνει τύπους αντικειμένων, τα οποία είναι κατασκευασμένα ώστε να μπορούν να αποτελούν μέρη ενός σύνθετου υλικού αντικειμένου. Αυτά τα αντικείμενα διαθέτουν αυτοτέλεια σε σχέση με τη σύνθετη ενότητα του ανάλογου τύπου αντικειμένου, στο οποίο προβλέπεται να προστεθούν. Παρά την αυτοτέλειά τους, όμως, δεν είναι ανεξάρτητα ως προς την προβλεπόμενη λειτουργία τους, αλλά αποτελούν δομικά μέρη του αντικειμένου, έχουν δηλαδή μια συγκεκριμένη λειτουργία στο πλαίσιο της ενότητας στην οποία ανήκουν και την οποία σχηματίζουν.

Σημείωση: Τα δομικά μέρη των υλικών αντικειμένων δε θεωρούνται στενότεροι όροι του συνόλου στο οποίο ανήκουν.</skos:scopeNote>
    <rdf:type rdf:resource="http://www.w3.org/2004/02/skos/core#Concept"/>
    <skos:note xml:lang="en">Narrower term examples: "strings", "bases (object components)"</skos:note>
    <skos:prefLabel xml:lang="de">Objektkomponenten</skos:prefLabel>
    <skos:exactMatch rdf:resource="https://humanitiesthesaurus.academyofathens.gr/dyas-resource/Concept/17"/>
    <skos:prefLabel xml:lang="fr">partie structurelle d'entités matérielle</skos:prefLabel>
    <dcterms:dateSubmitted>2015-08-13T07:18:40Z</dcterms:dateSubmitted>
    <skos:prefLabel xml:lang="en">structural parts of material objects</skos:prefLabel>
    <skos:scopeNote xml:lang="en">This class classifies objects especially constructed to be parts of a complex material object. These objects have autonomy in relation to the complex object of the appropriate type, to which they are intended to be added. Despite their autonomy, however, they are not independent in terms of their intended function, but are structural parts of the object, ie they have a specific function within the module to which they belong and which they form. Note: The structural parts of the material things are not considered narrower terms of the aggregation to which they belong.</skos:scopeNote>
    <skos:scopeNote xml:lang="fr">Ce terme désigne les objets spécialement construits pour faire partie d’une entité matérielle complexe. Ces objets sont autonomes par rapport à une entité complexe donnée à laquelle ils sont destinés à être ajoutés. Cependant, en dépit de leur caractère autonome, ils ne sont pas indépendants du point de vue de leur fonction prévue mais sont des parties structurelles de l'objet, ils ont donc une fonction spécifique au sein du module auquel ils appartiennent et qu'ils constituent. Attention : les parties structurelles d’entités matérielles ne sont pas considérées comme des termes spécifique de l’entité matérielle à laquelle elle sont agrégées.</skos:scopeNote>
    <skos:notation>000020</skos:notation>
    <rdfs:type rdf:resource="http://www.w3.org/2004/02/skos/core#Concept"/>
  </rdf:Description>
  <rdf:Description rdf:about="https://vocabs.dariah.eu/bbt/Facet/0000049">
    <skos:inScheme rdf:resource="https://vocabs.dariah.eu/bbt/ConceptScheme/Backbone_Thesaurus"/>
    <rdf:type rdf:resource="http://www.w3.org/2004/02/skos/core#Collection"/>
    <skos:member rdf:resource="https://vocabs.dariah.eu/bbt/Concept/0000049"/>
    <skos:member rdf:resource="https://vocabs.dariah.eu/bbt/Concept/0000051"/>
    <skos:member rdf:resource="https://vocabs.dariah.eu/bbt/Concept/0000050"/>
    <rdf:type rdf:resource="https://vocabs.dariah.eu/bbt/Facet"/>
    <skos:scopeNote xml:lang="en">This facet comprises kinds of designations and definitions of spatial extents based on either geometric expressions or spatial properties of observable features -like mountains, lakes, buildings, cities, etc. -and social constructs -referring to the spatial extent of of territories that fall within the jurisdiction of some geopolitical or other administrative unit.

NOTE: The terms and hierarchies of this facet can be coordinated with the suitable type of phenomenal place, in the sense of CRMgeo, [1] classified accordingly under Physical Features, Built Environment or Geopolitical Units. 

[1] Hiebel, G.H, Doerr, M. (2013). An ontological spatio-temporal refinement for the CIDOC CRM and GIS standards. 19th Annual meeting of the European Association of Archaeologists (EAA2013) 2013, Pilsen, Czech Republic, 4-8 September 2013, p. 20.</skos:scopeNote>
    <skos:prefLabel xml:lang="en">Geometric Extents</skos:prefLabel>
    <dcterms:creator xml:lang="en">BBT maintenance WG</dcterms:creator>
    <skos:member rdf:resource="https://vocabs.dariah.eu/bbt/Concept/0000052"/>
    <skos:member rdf:resource="https://vocabs.dariah.eu/bbt/Concept/0000053"/>
  </rdf:Description>
  <rdf:Description rdf:about="https://vocabs.dariah.eu/bbt/Facet/000007">
    <rdf:type rdf:resource="http://www.w3.org/2004/02/skos/core#Collection"/>
    <skos:prefLabel xml:lang="en">Groups and Collectivities</skos:prefLabel>
    <skos:scopeNote xml:lang="de">Unter dieser Facette werden Beziehungen jeglicher Art klassifiziert (ökonomisch, religiös, athletisch, politisch, national usw.), welche aus gemeinsamen Handlungen mindestens zweier Individuen entstehen. Diese Beziehungen sollten auf der Annahme gemeinsamer Glaubensgrundsätze, Traditionen, Objektive und/oder Handlungen wie auch organisatorischer Merkmale beruhen.</skos:scopeNote>
    <skos:scopeNote xml:lang="el">Το θέμα αυτό περιλαμβάνει σχέσεις οποιουδήποτε χαρακτήρα (οικονομικού, θρησκευτικού, αθλητικού, πολιτικού, εθνικού κτλ.) ως αποτέλεσμα κοινών ενεργειών δύο τουλάχιστον ατόμων. Οι σχέσεις αυτές θα πρέπει να στηρίζονται στην υιοθέτηση κοινών πεποιθήσεων ή/και στόχων ή/και δράσεων και να παρουσιάζουν οργανωτικά χαρακτηριστικά.</skos:scopeNote>
    <dcterms:creator xml:lang="en">BBT maintenance WG</dcterms:creator>
    <skos:scopeNote xml:lang="fr">Cette facette désigne les relations de toute nature (économique, religieuse, sportives, politiques, nationale etc.) qui émanent de l’action conjuguée d’au moins deux personnes. Ces relations doivent être fondées sur l’adhésion à des croyances, traditions, objectifs et/ou actions communes et présenter également des caractéristiques organisationnelles.</skos:scopeNote>
    <skos:prefLabel xml:lang="de">Gruppen und Vereinigungen</skos:prefLabel>
    <skos:inScheme rdf:resource="https://vocabs.dariah.eu/bbt/ConceptScheme/Backbone_Thesaurus"/>
    <skos:member rdf:resource="https://vocabs.dariah.eu/bbt/Concept/000007"/>
    <rdf:type rdf:resource="https://vocabs.dariah.eu/bbt/Facet"/>
    <skos:prefLabel xml:lang="el">Συλλογικότητες και Ομάδες</skos:prefLabel>
    <skos:prefLabel xml:lang="fr">Groupes et Collectivités</skos:prefLabel>
    <skos:scopeNote xml:lang="en">This facet comprises relations of whatever character (economic, religious, athletic, political, national etc.) that arise from the joint actions of at least two people. These relations should be based on the adoption of common beliefs, traditions, objectives and/or actions as well as showing organizational features.</skos:scopeNote>
  </rdf:Description>
  <rdf:Description rdf:about="https://vocabs.dariah.eu/bbt/Concept/000010">
    <skos:broader rdf:resource="https://vocabs.dariah.eu/bbt/Concept/000001"/>
    <skos:narrowMatch rdf:resource="http://www.eionet.europa.eu/gemet/concept/429"/>
    <dcterms:dateSubmitted>2015-08-13T07:18:40Z</dcterms:dateSubmitted>
    <skos:scopeNote xml:lang="fr">Ce terme désigne les secteurs d’activité professionnelle ou potentiellement professionnelle socialement et/ou légalement reconnus sur la base de critères d’auto-cohérence, d'efficacité des pratiques employées, de l’adoption de méthodes communes et de la capacité de transfert de connaissances et d’expertise à ces secteurs professionnels. Chaque secteur inclut des types d’activités qui se réfèrent à une certaine unité d'action potentiellement caractéristique d'une certaine professionnalisation ou spécialisation. Cette spécialisation peut concerner la production ou la modification d'objets matériels, la conception ou la compréhension d'activités ou de phénomènes, la fourniture ou le transfert de services, de connaissances et de savoir-faire et la création d'oeuvres et de phénomènes à valeur esthétique.
Note : il est important de préciser qu'un terme classé dans la hiérarchie "disciplines" ne doit pas être confondu avec l’acteur qui la pratique, le résultat de cette activité ou la méthode employée pour obtenir ce résultat. L'acteur comme "cause efficiente", le résultat comme "cause finale" et la méthode comme ensemble de règles et de contraintes que l'acteur suit pour mener à bien une action sont des termes différents appartenant à différentes facettes et hiérarchies. Pour déterminer les activités à classer dans la hiérarchie "disciplines" il ne faut pas confondre l'histoire d'une discipline particulière, c'est à dire l'environnement spatio-temporel dans lequel cette discipline est apparue et a été perçue avec le type d'activités caractéristiques de cette discipline.</skos:scopeNote>
    <skos:narrowMatch rdf:resource="https://ark.frantiq.fr/ark:/26678/pcrtvun1g7PPLq"/>
    <skos:exactMatch rdf:resource="https://humanitiesthesaurus.academyofathens.gr/dyas-resource/Concept/33"/>
    <skos:prefLabel xml:lang="de">Disziplinen</skos:prefLabel>
    <skos:exactMatch rdf:resource="https://isl.ics.forth.gr/parthenos_vocabularies/Concept/5827"/>
    <skos:scopeNote xml:lang="en">This term classifies professional or potentially professional areas of employment, that are socially and/ or legally recognized on the basis of the criteria of self-coherence, the efficacy of the practices they employ, the adoption of common methods and the ability to transfer knowledge and expertise in the relevant professional sector. Each sector includes types of activities that point to a certain unity of action characteristic of some sort of professional or potentially potential specialization. The specialization may relate to the production or modification of material objects, the conception and understanding of activities or phenomena, the provision /transfer of services, knowledge and know-how and the creation of works and phenomena with aesthetic value. Note: It is important to clarify that the terms classified in the “disciplines” term  should not be confused with the actor who performs an act or the results of his activity or the method used in order to achieve this result. The actor as “the efficient cause”, the result as “the final cause” and the method as the sum of the rules and constraints that an actor follows in order to perform an act, are different terms which belong to different facets and hierarchies. When determining the activities classified in the “Disciplines” hierarchy we should not confuse the history of a specific discipline ie the specific temporal and spatial environment in which this discipline appeared and was perceived with the type of activities characterizing this discipline.</skos:scopeNote>
    <skos:prefLabel xml:lang="el">τομείς απασχόλησης</skos:prefLabel>
    <skos:prefLabel xml:lang="en">disciplines</skos:prefLabel>
    <skos:scopeNote xml:lang="de">Dieser Term umfasst professionelle oder potentiell professionelle Berufszweige, die auf der Grundlage folgender Kriterien gesellschaftlich und/oder rechtlich anerkannt sind: Selbstkohärenz, Effizienz der angewendeten Praktiken, Anwendung gemeinsamer Methoden und die Fähigkeit, Wissen und Kompetenz in die entsprechenden Forschungsfelder zu übertragen. Jeder Bereich beinhaltet Handlungen, die auf Aktivitäten mit bestimmten Charakteristika von professionellen oder potentiell professionellen Spezialisierungen hinführen. Diese Spezialisierungen können mit der Produktion oder Modifikation von materiellen Objekten, mit der Konzeption und dem Verständnis von Aktivitäten oder Phänomenen, mit der Bereitstellung/Transfer von Dienstleistungen, Wissen, Fachwissen und mit dem Erschaffen von Werken und Phänomenen mit ästhetischem Wert in Verbindung stehen.
Notiz: Die in diesem Term aufgeführten Begriffe, sollten nicht mit den charakteristischen Tätigkeiten des ausführenden Akteurs oder mit dem Ergebnis seiner Handlung oder mit der verwendeten Methode verwechselt werden. Bei dem Akteur als „effiziente Ursache“, dem Ergebnis als „die letzte Ursache“ und der Methode als die Summe der Regeln und Beschränkungen, die ein Akteur folgt, um eine Tätigkeit auszuführen, handelt es sich um andere Begriffe, die zu anderen Facetten und Hierarchien gehören. Bei der Bestimmung der in der Hierarchie „Disziplinen“ klassifizierten Aktivitäten sollte die Geschichte einer bestimmten Disziplin, d. h. der spezifische zeitliche und räumliche Kontext in welchem diese Disziplin entstand, mit den diese Disziplin charakterisierenden Arten von Aktivitäten, nicht verwechselt werden.</skos:scopeNote>
    <dcterms:creator xml:lang="en">BBT maintenance WG</dcterms:creator>
    <rdfs:type rdf:resource="http://www.w3.org/2004/02/skos/core#Concept"/>
    <skos:notation>000010</skos:notation>
    <dcterms:modified>2019-04-10T10:55:20Z</dcterms:modified>
    <skos:note xml:lang="en">Narrower term examples: "construction of material objects and installations", "conception and comprehension of phenomena", "provision of knowledge and expertise",  "production of works and/or phenomena of aesthetic value"</skos:note>
    <rdf:type rdf:resource="http://www.w3.org/2004/02/skos/core#Concept"/>
    <skos:exactMatch rdf:resource="http://thesauri.dainst.org/_6e11e02c"/>
    <skos:narrowMatch rdf:resource="https://ark.frantiq.fr/ark:/26678/pcrtBjGEQJB8ga"/>
    <skos:prefLabel xml:lang="fr">disciplines</skos:prefLabel>
    <skos:scopeNote xml:lang="el">Περιλαμβάνει τομείς επαγγελματικής ή δυνάμει επαγγελματικής απασχόλησης, κοινωνικά ή/και νομικά αποδεκτής βάσει των κριτηρίων της αυτοτέλειας του κάθε τομέα, της αποτελεσματικότητας της πρακτικής που εφαρμόζει, της υιοθέτησης κοινών μεθόδων και της δυνατότητας μεταβίβασης της γνώσης και της τεχνογνωσίας του εκάστοτε επαγγελματικού τομέα. Ο κάθε τομέας περιέχει τύπους ενεργειών που δημιουργούν ενότητες, οι οποίες εκφράζουν μια μορφή επαγγελματικής ή δυνάμει επαγγελματικής εξειδίκευσης. Η εξειδίκευση αυτή μπορεί να αφορά στην κατασκευή ή αλλαγή υλικών αντικειμένων, στη σύλληψη και κατανόηση ενεργειών ή φαινομένων, στην παροχή, στη μεταφορά/ μεταβίβαση υπηρεσιών, γνώσης και τεχνογνωσίας και στην παραγωγή έργων και φαινομένων με αισθητική αξία. Γενικές παρατηρήσεις: α) Θα πρέπει να είναι απολύτως σαφές ότι οι όροι τους οποίους προσδιορίζουμε στην ιεραρχία αυτή αφορούν τύπους ενεργειών και δεν πρέπει να συγχέονται ούτε με τον δράστη, ούτε με το αποτέλεσμα της ενέργειας, ούτε με τη διαδικασία που οδηγεί στο συγκεκριμένο αποτέλεσμα. Ο δράστης, ως το ποιητικό αίτιο, το αποτέλεσμα ως το τελικό αίτιο και η διαδικασία ως το σύνολο των περιορισμών και κανόνων, η εφαρμογή των οποίων κρίνεται ότι οδηγεί σε ένα συγκεκριμένο αποτέλεσμα, αποτελούν ξεχωριστούς όρους που ανήκουν σε διαφορετικές ιεραρχίες και θέματα. β) Στον προσδιορισμό δραστηριοτήτων και την κατάταξή τους στους αντίστοιχους ειδικότερους όρους, θα πρέπει να μην συγχέουμε την ιστορία ενός τομέα απασχόλησης, δηλαδή το συγκεκριμένο πλαίσιο στο οποίο ο τομέας αυτός εμφανίζεται και προσλαμβάνεται, με τον τύπο των ενεργειών που χαρακτηρίζουν τον τομέα αυτόν.</skos:scopeNote>
  </rdf:Description>
  <rdf:Description rdf:about="https://vocabs.dariah.eu/bbt/Concept/000026">
    <skos:scopeNote xml:lang="el">Η ιεραρχία περιλαμβάνει τύπους στάσεων ή/ και συμπεριφορών που χαρακτηρίζουν τις διαπροσωπικές σχέσεις ατόμων που συνδέονται με δεσμούς αίματος, γάμου, υιοθεσίας ή αναδοχής. Περιλαμβάνει επίσης τύπους στάσεων ή/ και συμπεριφορών ατόμων που συνδέονται, μεταξύ άλλων, με θρησκευτικές, πνευματικές ή φιλικές σχέσεις ή σχέσεις αντιπαλότητας ή/ και ανταγωνισμού.</skos:scopeNote>
    <skos:broader rdf:resource="https://vocabs.dariah.eu/bbt/Concept/000008"/>
    <skos:prefLabel xml:lang="el">ρόλοι διαπροσωπικών σχέσεων</skos:prefLabel>
    <skos:notation>000026</skos:notation>
    <dcterms:dateSubmitted>2015-08-13T07:18:40Z</dcterms:dateSubmitted>
    <skos:exactMatch rdf:resource="https://humanitiesthesaurus.academyofathens.gr/dyas-resource/Concept/35"/>
    <dcterms:modified>2019-04-10T10:55:12Z</dcterms:modified>
    <skos:prefLabel xml:lang="fr">rôles dans les relations interpersonnelle</skos:prefLabel>
    <rdf:type rdf:resource="http://www.w3.org/2004/02/skos/core#Concept"/>
    <skos:scopeNote xml:lang="fr">Ce terme désigne les conduites et/ou comportements qui caractérisent les relations interpersonnelles de personnes liées par la parenté, le mariage ou l’adoption. Il inclut les les conduites et/ou comportements de personnes liées par des relations religieuses, spirituelles, amicales, de rivalité et/ou antagonistes.</skos:scopeNote>
    <skos:scopeNote xml:lang="de">Dieser Term klassifiziert Haltungen und/oder Verhaltensweisen, die zwischenmenschliche Beziehungen von Personen charakterisieren, die durch Verwandtschaft, Heirat oder Adoption miteinander verbunden sind. Außerdem beinhaltet er Typen von Handlungen und/oder Verhaltensweisen von Personen, die durch religiöse, spirituelle, freundschaftliche, feindliche und /oder antagonistische Beziehungen miteinander verbunden sind.</skos:scopeNote>
    <dcterms:creator xml:lang="en">BBT maintenance WG</dcterms:creator>
    <rdfs:type rdf:resource="http://www.w3.org/2004/02/skos/core#Concept"/>
    <skos:scopeNote xml:lang="en">This term classifies attitudes and/ or behaviors that characterize the interpersonal relations of people who are linked through kinship, marriage or adoption. It also comprises the types of attitudes and/ or behaviors of people linked through religious, spiritual, friendly, rivalrous and/ or antagonistic relations.</skos:scopeNote>
    <skos:prefLabel xml:lang="de">Rollen zwischenmenschlicher Beziehungen</skos:prefLabel>
    <skos:prefLabel xml:lang="en">roles of interpersonal relations</skos:prefLabel>
  </rdf:Description>
  <rdf:Description rdf:about="https://vocabs.dariah.eu/bbt/Facet/">
    <rdfs:subClassOf rdf:resource="http://www.w3.org/2004/02/skos/core#Collection"/>
    <skos:scopeNote>grouping of concepts of the same inherent category</skos:scopeNote>
  </rdf:Description>
  <rdf:Description rdf:about="https://vocabs.dariah.eu/bbt/Concept/0000053">
    <skos:scopeNote xml:lang="en">This term classifies one-dimensional shapes on a surface that are either straight or curved and can be defined by a connected series of unique x,y coordinate pairs/points forming a continuous path. The said points are all contained in it [2]. Linear extents can be used to show the geometry of linear features such as roads, rivers, contours, footpaths, flight paths and so on. 
[1] https://docs.qgis.org/2.8/en/docs/gentle_gis_introduction/vector_data.html#figure-geometry-polyline   
[2] https://en.wikipedia.org/wiki/Line_(geometry)

NOTE: The kind of Physical feature, Built environment or Geopolitical unit -or part thereof, f.i. a mountain range, a road, a borders between two countries -providing the linear extent can be specified by coordinating this term with the suitable feature type, such as “linear extents of Physical features/ Built environments/ Geopolitical units”.</skos:scopeNote>
    <skos:prefLabel xml:lang="en">linear extent</skos:prefLabel>
    <skos:broader rdf:resource="https://vocabs.dariah.eu/bbt/Concept/0000049"/>
    <dcterms:creator xml:lang="en">BBT maintenance WG</dcterms:creator>
    <rdf:type rdf:resource="http://www.w3.org/2004/02/skos/core#Concept"/>
    <skos:notation>0000053</skos:notation>
    <dcterms:dateSubmitted>2020-01-21T08:29:34Z</dcterms:dateSubmitted>
  </rdf:Description>
  <rdf:Description rdf:about="https://vocabs.dariah.eu/bbt/Facet/000008">
    <skos:scopeNote xml:lang="en">This facet comprises the types of attitudes and/or social behaviors that are expected of a person and which result from or are acquired through the relation of that person with other individuals or social groups.</skos:scopeNote>
    <skos:inScheme rdf:resource="https://vocabs.dariah.eu/bbt/ConceptScheme/Backbone_Thesaurus"/>
    <rdf:type rdf:resource="http://www.w3.org/2004/02/skos/core#Collection"/>
    <skos:member rdf:resource="https://vocabs.dariah.eu/bbt/Concept/000008"/>
    <skos:member rdf:resource="https://vocabs.dariah.eu/bbt/Concept/000026"/>
    <dcterms:creator xml:lang="en">BBT maintenance WG</dcterms:creator>
    <skos:prefLabel xml:lang="el">Ρόλοι</skos:prefLabel>
    <skos:scopeNote xml:lang="de">Diese Facette umfasst Typen von Haltungen und/oder sozialen Verhaltensweisen, die von einer Person erwartet werden und aus der Beziehung dieses Individuums zu anderen Personen und sozialen Gruppen resultieren oder durch diese erworben werden.</skos:scopeNote>
    <skos:prefLabel xml:lang="de">Rollen</skos:prefLabel>
    <skos:prefLabel xml:lang="en">Roles</skos:prefLabel>
    <skos:scopeNote xml:lang="fr">Cette facette désigne les types de conduites ou comportements sociaux qui sont attendus d’une personne et qui résultent de ou sont acquis par la relation de cette personne avec d’autres individus ou groupes sociaux.</skos:scopeNote>
    <rdf:type rdf:resource="https://vocabs.dariah.eu/bbt/Facet"/>
    <skos:scopeNote xml:lang="el">Το θέμα περιλαμβάνει τύπους στάσεων ή/και κοινωνικών συμπεριφορών που αναμένονται από ένα πρόσωπο και που προκύπτουν ή αποκτώνται από τη σχέση του με άλλα πρόσωπα ή κοινωνικές ομάδες.</skos:scopeNote>
    <skos:member rdf:resource="https://vocabs.dariah.eu/bbt/Concept/000025"/>
    <skos:prefLabel xml:lang="fr">Rôles</skos:prefLabel>
  </rdf:Description>
  <rdf:Description rdf:about="https://vocabs.dariah.eu/bbt/Concept/0000050">
    <skos:broader rdf:resource="https://vocabs.dariah.eu/bbt/Concept/0000049"/>
    <skos:notation>0000050</skos:notation>
    <rdf:type rdf:resource="http://www.w3.org/2004/02/skos/core#Concept"/>
    <dcterms:dateSubmitted>2020-01-21T08:13:54Z</dcterms:dateSubmitted>
    <skos:prefLabel xml:lang="en">points</skos:prefLabel>
    <skos:scopeNote xml:lang="en">This term classifies zero-dimensional geometric primitives, representing the position [1] of the centroid of a particular feature, on a given surface –irrespective of its actual spatial extent –depending on the scale of the representation (the smaller the scale, the more likely it is for a feature to be thus represented), convenience and the type of feature the points stand for [2]. 

[1] The OpenGIS; Abstract Specification; Topic 5: Features 
[2] https://docs.qgis.org/2.8/en/docs/gentle_gis_introduction/vector_data.html#figure-geometry-point

NOTE: The terms listed as points can be coordinated with the suitable type of phenomenal place -in the sense of CRMgeo [1] -classified under the hierarchies of Physical Features, Built Environment or Geopolitical Units.</skos:scopeNote>
    <dcterms:creator xml:lang="en">BBT maintenance WG</dcterms:creator>
  </rdf:Description>
  <rdf:Description rdf:about="https://vocabs.dariah.eu/bbt/Concept/0000051">
    <skos:prefLabel xml:lang="en">surface areas</skos:prefLabel>
    <skos:notation>0000051</skos:notation>
    <dcterms:creator xml:lang="en">BBT maintenance WG</dcterms:creator>
    <skos:scopeNote xml:lang="en">The term classifies quantities expressing the extent of a two dimensional feature, figure or shape defined by a connected sequence of x,y coordinate pairs/points, where the first and last coordinate pair/points are the same and all others are unique, thus forming a polygon. The latter can have a shared geometry, i.e. boundaries that are in common with a neighboring polygon.  Surface areas can be seen as contiguous projections onto some reference space. Examples of such areas are enclosed spaces like dams, islands, country boundaries and so on.

NOTE: The kind of Physical feature, Built environment or Geopolitical unit providing the geometric extent -i.e. a lake, a stadium, a prefecture -can be specified by coordinating this term with the suitable feature type, such as “surface areas of Physical features/ Built environments/ Geopolitical units”.</skos:scopeNote>
    <dcterms:dateSubmitted>2020-01-21T08:13:54Z</dcterms:dateSubmitted>
    <rdf:type rdf:resource="http://www.w3.org/2004/02/skos/core#Concept"/>
    <skos:broader rdf:resource="https://vocabs.dariah.eu/bbt/Concept/0000049"/>
  </rdf:Description>
</rdf:RDF>
