@prefix skos: <http://www.w3.org/2004/02/skos/core#> .
@prefix dc: <http://purl.org/dc/terms/> .
@prefix xsd: <http://www.w3.org/2001/XMLSchema#> .
@prefix dc11: <http://purl.org/dc/elements/1.1/> .
@prefix ns0: <https://vocabs.acdh.oeaw.ac.at/schema#> .
@prefix rdfs: <http://www.w3.org/2000/01/rdf-schema#> .

<https://vocabs.acdh.oeaw.ac.at/dhataxonomy/dhaTaxonomyScheme>
  skos:hasTopConcept <https://vocabs.acdh.oeaw.ac.at/dhataxonomy/Concept54>, <https://vocabs.acdh.oeaw.ac.at/dhataxonomy/Concept18>, <https://vocabs.acdh.oeaw.ac.at/dhataxonomy/Concept70>, <https://vocabs.acdh.oeaw.ac.at/dhataxonomy/Concept3>, <https://vocabs.acdh.oeaw.ac.at/dhataxonomy/Concept14>, <https://vocabs.acdh.oeaw.ac.at/dhataxonomy/Concept61>, <https://vocabs.acdh.oeaw.ac.at/dhataxonomy/Concept23>, <https://vocabs.acdh.oeaw.ac.at/dhataxonomy/Concept34>, <https://vocabs.acdh.oeaw.ac.at/dhataxonomy/Concept36>, <https://vocabs.acdh.oeaw.ac.at/dhataxonomy/Concept42>, <https://vocabs.acdh.oeaw.ac.at/dhataxonomy/Concept68>, <https://vocabs.acdh.oeaw.ac.at/dhataxonomy/Concept19>, <https://vocabs.acdh.oeaw.ac.at/dhataxonomy/Concept43>, <https://vocabs.acdh.oeaw.ac.at/dhataxonomy/Concept32>, <https://vocabs.acdh.oeaw.ac.at/dhataxonomy/Concept55>, <https://vocabs.acdh.oeaw.ac.at/dhataxonomy/Concept9>, <https://vocabs.acdh.oeaw.ac.at/dhataxonomy/Concept37>, <https://vocabs.acdh.oeaw.ac.at/dhataxonomy/Concept22>, <https://vocabs.acdh.oeaw.ac.at/dhataxonomy/Concept16>, <https://vocabs.acdh.oeaw.ac.at/dhataxonomy/Concept33>, <https://vocabs.acdh.oeaw.ac.at/dhataxonomy/Concept59>, <https://vocabs.acdh.oeaw.ac.at/dhataxonomy/Concept48>, <https://vocabs.acdh.oeaw.ac.at/dhataxonomy/Concept44>, <https://vocabs.acdh.oeaw.ac.at/dhataxonomy/Concept65>, <https://vocabs.acdh.oeaw.ac.at/dhataxonomy/Concept10>, <https://vocabs.acdh.oeaw.ac.at/dhataxonomy/Concept12>, <https://vocabs.acdh.oeaw.ac.at/dhataxonomy/Concept31>, <https://vocabs.acdh.oeaw.ac.at/dhataxonomy/Concept74>, <https://vocabs.acdh.oeaw.ac.at/dhataxonomy/Concept29>, <https://vocabs.acdh.oeaw.ac.at/dhataxonomy/Concept1>, <https://vocabs.acdh.oeaw.ac.at/dhataxonomy/Concept8>, <https://vocabs.acdh.oeaw.ac.at/dhataxonomy/Concept57>, <https://vocabs.acdh.oeaw.ac.at/dhataxonomy/Concept67>, <https://vocabs.acdh.oeaw.ac.at/dhataxonomy/Concept21>, <https://vocabs.acdh.oeaw.ac.at/dhataxonomy/Concept63>, <https://vocabs.acdh.oeaw.ac.at/dhataxonomy/Concept46>, <https://vocabs.acdh.oeaw.ac.at/dhataxonomy/Concept39>, <https://vocabs.acdh.oeaw.ac.at/dhataxonomy/Concept6>, <https://vocabs.acdh.oeaw.ac.at/dhataxonomy/Concept5>, <https://vocabs.acdh.oeaw.ac.at/dhataxonomy/Concept45>, <https://vocabs.acdh.oeaw.ac.at/dhataxonomy/Concept17>, <https://vocabs.acdh.oeaw.ac.at/dhataxonomy/Concept26>, <https://vocabs.acdh.oeaw.ac.at/dhataxonomy/Concept35>, <https://vocabs.acdh.oeaw.ac.at/dhataxonomy/Concept40>, <https://vocabs.acdh.oeaw.ac.at/dhataxonomy/Concept64>, <https://vocabs.acdh.oeaw.ac.at/dhataxonomy/Concept47>, <https://vocabs.acdh.oeaw.ac.at/dhataxonomy/Concept7>, <https://vocabs.acdh.oeaw.ac.at/dhataxonomy/Concept71>, <https://vocabs.acdh.oeaw.ac.at/dhataxonomy/Concept25>, <https://vocabs.acdh.oeaw.ac.at/dhataxonomy/Concept30>, <https://vocabs.acdh.oeaw.ac.at/dhataxonomy/Concept69>, <https://vocabs.acdh.oeaw.ac.at/dhataxonomy/Concept4>, <https://vocabs.acdh.oeaw.ac.at/dhataxonomy/Concept60>, <https://vocabs.acdh.oeaw.ac.at/dhataxonomy/Concept50>, <https://vocabs.acdh.oeaw.ac.at/dhataxonomy/Concept72>, <https://vocabs.acdh.oeaw.ac.at/dhataxonomy/Concept73>, <https://vocabs.acdh.oeaw.ac.at/dhataxonomy/Concept62>, <https://vocabs.acdh.oeaw.ac.at/dhataxonomy/Concept52>, <https://vocabs.acdh.oeaw.ac.at/dhataxonomy/Concept28>, <https://vocabs.acdh.oeaw.ac.at/dhataxonomy/Concept51>, <https://vocabs.acdh.oeaw.ac.at/dhataxonomy/Concept2>, <https://vocabs.acdh.oeaw.ac.at/dhataxonomy/Concept58>, <https://vocabs.acdh.oeaw.ac.at/dhataxonomy/Concept27>, <https://vocabs.acdh.oeaw.ac.at/dhataxonomy/Concept38>, <https://vocabs.acdh.oeaw.ac.at/dhataxonomy/Concept11>, <https://vocabs.acdh.oeaw.ac.at/dhataxonomy/Concept41>, <https://vocabs.acdh.oeaw.ac.at/dhataxonomy/Concept20>, <https://vocabs.acdh.oeaw.ac.at/dhataxonomy/Concept15>, <https://vocabs.acdh.oeaw.ac.at/dhataxonomy/Concept49>, <https://vocabs.acdh.oeaw.ac.at/dhataxonomy/Concept56>, <https://vocabs.acdh.oeaw.ac.at/dhataxonomy/Concept13>, <https://vocabs.acdh.oeaw.ac.at/dhataxonomy/Concept53>, <https://vocabs.acdh.oeaw.ac.at/dhataxonomy/Concept24>, <https://vocabs.acdh.oeaw.ac.at/dhataxonomy/Concept66> ;
  ns0:hasMetadataCreator "Ksenia Zaytseva" ;
  ns0:hasOwner "ACDH-OEAW"@en ;
  dc:publisher "ACDH-OEAW" ;
  dc:rightsHolder "ACDH-OEAW" ;
  ns0:hasTitle "DHA Taxonomy"@en ;
  ns0:hasCreatedStartDate "Thu Oct 01 00:00:00 CEST 2015"^^xsd:date ;
  dc11:subject "Computational methods in humanities"@en, "Cultural analytics"@en, "Text technologies"@en ;
  dc:license "https://creativecommons.org/licenses/by/4.0/" ;
  ns0:creator "ACDH-OEAW Team"@en ;
  a skos:ConceptScheme ;
  ns0:hasURL <https://vocabs.acdh.oeaw.ac.at/dhataxonomy/en> ;
  dc11:description "DHA taxonomy is a knowledge organization system designed to describe subjects, resources and tools within activities of Digital Humanities Austria."@en ;
  dc11:format "application/rdf+xml" ;
  ns0:hasFormat "application/rdf+xml" ;
  rdfs:label "DHA Taxonomy"@en ;
  dc11:language "English"@en ;
  ns0:isNewVersionOf <https://arche.acdh.oeaw.ac.at/browser/> ;
  ns0:hasRightsHolder "ACDH-OEAW"@en ;
  ns0:hasIdentifier <https://vocabs.acdh.oeaw.ac.at/dhataxonomy/dhaTaxonomyScheme> ;
  ns0:hasLanguage "English"@en ;
  ns0:hasDescription "DHA taxonomy is a knowledge organization system designed to describe subjects, resources and tools within activities of Digital Humanities Austria."@en ;
  ns0:hasLicense "https://creativecommons.org/licenses/by/4.0/" ;
  ns0:hasLifeCycleStatus "completed"@en ;
  dc11:title "DHA Taxonomy"@en ;
  ns0:hasCreatedEndDate "Tue Apr 03 00:00:00 CEST 2018"^^xsd:date ;
  dc11:relation "http://www.digital-humanities.at/en" ;
  dc:issued "Tue Apr 03 00:00:00 CEST 2018"^^xsd:date ;
  ns0:hasAccessRestriction "public"@en ;
  ns0:hasLicensor "ACDH-OEAW"@en ;
  ns0:hasRelatedDiscipline "Digital Humanities" ;
  dc:modified "Tue Apr 03 00:00:00 CEST 2018"^^xsd:date ;
  dc:created "Thu Oct 01 00:00:00 CEST 2015"^^xsd:date ;
  dc11:creator "ACDH-OEAW Team"@en ;
  dc:contributor "DHA consortium" .

<https://vocabs.acdh.oeaw.ac.at/dhataxonomy/Concept48.07>
  skos:definition "process of grouping together the different inflected forms of a word to its canonical form so that they can be analysed as a single item"@en ;
  dc:created "Thu Oct 01 00:00:00 CEST 2015"^^xsd:date ;
  skos:prefLabel "lemmatisation"@en ;
  dc:modified "Mon Jun 20 00:00:00 CEST 2016"^^xsd:date ;
  a skos:Concept ;
  skos:notation "48.07"^^xsd:int ;
  skos:broader <https://vocabs.acdh.oeaw.ac.at/dhataxonomy/Concept48> ;
  skos:inScheme <https://vocabs.acdh.oeaw.ac.at/dhataxonomy/dhaTaxonomyScheme> ;
  dc11:source "based on: Wikipedia contributors, \"Lemmatisation,\" Wikipedia, The Free Encyclopedia, https://en.wikipedia.org/w/index.php?title=Lemmatisation&oldid=692695396 (accessed February 28, 2016)."@en .

<https://vocabs.acdh.oeaw.ac.at/dhataxonomy/Concept3.03>
  dc:created "Thu Oct 01 00:00:00 CEST 2015"^^xsd:date ;
  skos:inScheme <https://vocabs.acdh.oeaw.ac.at/dhataxonomy/dhaTaxonomyScheme> ;
  skos:altLabel "Friend Of A Friend"@en ;
  dc:modified "Mon Jun 20 00:00:00 CEST 2016"^^xsd:date ;
  dc11:source "Wikipedia contributors, \"FOAF (ontology),\" Wikipedia, The Free Encyclopedia, https://en.wikipedia.org/w/index.php?title=FOAF_(ontology)&oldid=703222322 (accessed February 28, 2016)."@en ;
  skos:broader <https://vocabs.acdh.oeaw.ac.at/dhataxonomy/Concept3> ;
  a skos:Concept ;
  skos:notation "3.03"^^xsd:int ;
  skos:prefLabel "FOAF"@en ;
  skos:definition "a machine-readable ontology describing persons, their activities and their relations to other people and objects"@en .

<https://vocabs.acdh.oeaw.ac.at/dhataxonomy/Concept14>
  dc:modified "Mon Jun 20 00:00:00 CEST 2016"^^xsd:date ;
  dc11:source "psychology. Oxford Dictionaries. Oxford University Press. http://www.oxforddictionaries.com/definition/english/psychology (accessed February 28, 2016)."@en ;
  a skos:Concept ;
  dc:created "Thu Oct 01 00:00:00 CEST 2015"^^xsd:date ;
  skos:inScheme <https://vocabs.acdh.oeaw.ac.at/dhataxonomy/dhaTaxonomyScheme> ;
  skos:topConceptOf <https://vocabs.acdh.oeaw.ac.at/dhataxonomy/dhaTaxonomyScheme> ;
  skos:prefLabel "psychology"@en ;
  skos:definition "the scientific study of the human mind and its functions"@en ;
  skos:notation "14"^^xsd:int .

<https://vocabs.acdh.oeaw.ac.at/dhataxonomy/Concept23>
  dc11:source "Wikipedia contributors, \"Media studies,\" Wikipedia, The Free Encyclopedia, https://en.wikipedia.org/w/index.php?title=Media_studies&oldid=710007026 (accessed April 4, 2016)."@en ;
  skos:notation "23"^^xsd:int ;
  skos:prefLabel "media studies"@en ;
  skos:inScheme <https://vocabs.acdh.oeaw.ac.at/dhataxonomy/dhaTaxonomyScheme> ;
  dc:created "Thu Oct 01 00:00:00 CEST 2015"^^xsd:date ;
  skos:topConceptOf <https://vocabs.acdh.oeaw.ac.at/dhataxonomy/dhaTaxonomyScheme> ;
  dc:modified "Mon Jun 20 00:00:00 CEST 2016"^^xsd:date ;
  a skos:Concept ;
  skos:definition "a discipline and field of study that deals with the content, history, and effects of various media; in particular, the mass media"@en .

<https://vocabs.acdh.oeaw.ac.at/dhataxonomy/Concept62>
  dc:created "Thu Oct 01 00:00:00 CEST 2015"^^xsd:date ;
  a skos:Concept ;
  dc11:creator "ACDH-OEAW Team"@en ;
  dc:modified "Mon Jun 20 00:00:00 CEST 2016"^^xsd:date ;
  skos:definition "teaching materials in DH domain"@en ;
  skos:inScheme <https://vocabs.acdh.oeaw.ac.at/dhataxonomy/dhaTaxonomyScheme> ;
  skos:topConceptOf <https://vocabs.acdh.oeaw.ac.at/dhataxonomy/dhaTaxonomyScheme> ;
  skos:notation "62"^^xsd:int ;
  skos:prefLabel "teaching"@en .

<https://vocabs.acdh.oeaw.ac.at/dhataxonomy/Concept40.02>
  dc11:source "based on Wikipedia contributors, \"Ontology engineering,\" Wikipedia, The Free Encyclopedia, https://en.wikipedia.org/w/index.php?title=Ontology_engineering&oldid=685693548 (accessed February 28, 2016)."@en ;
  skos:prefLabel "ontology"@en ;
  dc:created "Thu Oct 01 00:00:00 CEST 2015"^^xsd:date ;
  skos:inScheme <https://vocabs.acdh.oeaw.ac.at/dhataxonomy/dhaTaxonomyScheme> ;
  a skos:Concept ;
  skos:broader <https://vocabs.acdh.oeaw.ac.at/dhataxonomy/Concept40> ;
  skos:definition "formal representations of a set of concepts within a domain and the relationships between those concepts"@en ;
  dc:modified "Mon Jun 20 00:00:00 CEST 2016"^^xsd:date ;
  skos:notation "40.02"^^xsd:int .

<https://vocabs.acdh.oeaw.ac.at/dhataxonomy/Concept27>
  skos:inScheme <https://vocabs.acdh.oeaw.ac.at/dhataxonomy/dhaTaxonomyScheme> ;
  skos:notation "27"^^xsd:int ;
  skos:topConceptOf <https://vocabs.acdh.oeaw.ac.at/dhataxonomy/dhaTaxonomyScheme> ;
  dc11:source "lexicography. Oxford Dictionaries. Oxford University Press. http://www.oxforddictionaries.com/definition/english/lexicography (accessed February 28, 2016)."@en ;
  dc:created "Thu Oct 01 00:00:00 CEST 2015"^^xsd:date ;
  skos:definition "the activity or occupation of compiling dictionaries"@en ;
  dc:modified "Mon Jun 20 00:00:00 CEST 2016"^^xsd:date ;
  a skos:Concept ;
  skos:prefLabel "lexicography"@en .

<https://vocabs.acdh.oeaw.ac.at/dhataxonomy/Concept17>
  skos:prefLabel "education"@en ;
  skos:definition "the process of facilitating learning, or the acquisition of knowledge, skills, values, beliefs, and habits"@en ;
  dc11:source "Wikipedia contributors, \"Education,\" Wikipedia, The Free Encyclopedia, https://en.wikipedia.org/w/index.php?title=Education&oldid=713401365 (accessed April 4, 2016)."@en ;
  skos:topConceptOf <https://vocabs.acdh.oeaw.ac.at/dhataxonomy/dhaTaxonomyScheme> ;
  skos:notation "17"^^xsd:int ;
  dc:created "Thu Oct 01 00:00:00 CEST 2015"^^xsd:date ;
  a skos:Concept ;
  dc:modified "Mon Jun 20 00:00:00 CEST 2016"^^xsd:date ;
  skos:inScheme <https://vocabs.acdh.oeaw.ac.at/dhataxonomy/dhaTaxonomyScheme> .

<https://vocabs.acdh.oeaw.ac.at/dhataxonomy/Concept4>
  skos:topConceptOf <https://vocabs.acdh.oeaw.ac.at/dhataxonomy/dhaTaxonomyScheme> ;
  a skos:Concept ;
  skos:definition "a protocol for exposing and collecting descriptions (metadata) of archival objects (or any digital objects)"@en ;
  skos:prefLabel "OAI-PMH"@en ;
  dc11:creator "ACDH-OEAW Team"@en ;
  skos:notation "4"^^xsd:int ;
  dc:modified "Mon Jun 20 00:00:00 CEST 2016"^^xsd:date ;
  skos:altLabel "Open Archives Initiative Protocol for Metadata Harvesting"@en ;
  dc:created "Thu Oct 01 00:00:00 CEST 2015"^^xsd:date ;
  skos:inScheme <https://vocabs.acdh.oeaw.ac.at/dhataxonomy/dhaTaxonomyScheme> .

<https://vocabs.acdh.oeaw.ac.at/dhataxonomy/Concept71>
  a skos:Concept ;
  skos:definition "books, articles, journals, technical reports, documentation etc. informing on DH topics"@en ;
  dc:modified "Mon Jun 20 00:00:00 CEST 2016"^^xsd:date ;
  dc11:creator "ACDH-OEAW Team"@en ;
  skos:notation "71"^^xsd:int ;
  skos:prefLabel "type_reading"@en ;
  dc:created "Thu Oct 01 00:00:00 CEST 2015"^^xsd:date ;
  skos:inScheme <https://vocabs.acdh.oeaw.ac.at/dhataxonomy/dhaTaxonomyScheme> ;
  skos:topConceptOf <https://vocabs.acdh.oeaw.ac.at/dhataxonomy/dhaTaxonomyScheme> .

<https://vocabs.acdh.oeaw.ac.at/dhataxonomy/Concept33>
  skos:notation "33"^^xsd:int ;
  a skos:Concept ;
  skos:definition "a digital representation of acoustic signals"@en ;
  dc11:creator "ACDH-OEAW Team"@en ;
  dc:modified "Mon Jun 20 00:00:00 CEST 2016"^^xsd:date ;
  skos:prefLabel "audio recording"@en ;
  skos:inScheme <https://vocabs.acdh.oeaw.ac.at/dhataxonomy/dhaTaxonomyScheme> ;
  skos:topConceptOf <https://vocabs.acdh.oeaw.ac.at/dhataxonomy/dhaTaxonomyScheme> ;
  dc:created "Thu Oct 01 00:00:00 CEST 2015"^^xsd:date .

<https://vocabs.acdh.oeaw.ac.at/dhataxonomy/Concept40.03>
  dc11:source "based on Wikipedia contributors, \"Controlled vocabulary,\" Wikipedia, The Free Encyclopedia, https://en.wikipedia.org/w/index.php?title=Controlled_vocabulary&oldid=704734498 (accessed February 28, 2016)."@en ;
  dc:created "Thu Oct 01 00:00:00 CEST 2015"^^xsd:date ;
  a skos:Concept ;
  dc:modified "Mon Jun 20 00:00:00 CEST 2016"^^xsd:date ;
  skos:broader <https://vocabs.acdh.oeaw.ac.at/dhataxonomy/Concept40> ;
  skos:definition "list of words or phrases used to classify units of information"@en ;
  skos:notation "40.03"^^xsd:int ;
  skos:prefLabel "vocabulary"@en ;
  skos:inScheme <https://vocabs.acdh.oeaw.ac.at/dhataxonomy/dhaTaxonomyScheme> .

<https://vocabs.acdh.oeaw.ac.at/dhataxonomy/Concept39.01>
  a skos:Concept ;
  dc:modified "Mon Jun 20 00:00:00 CEST 2016"^^xsd:date ;
  skos:broader <https://vocabs.acdh.oeaw.ac.at/dhataxonomy/Concept39> ;
  dc:created "Thu Oct 01 00:00:00 CEST 2015"^^xsd:date ;
  skos:prefLabel "corpus"@en ;
  skos:notation "39.01"^^xsd:int ;
  skos:inScheme <https://vocabs.acdh.oeaw.ac.at/dhataxonomy/dhaTaxonomyScheme> ;
  dc11:source "Wikipedia contributors, \"Text corpus,\" Wikipedia, The Free Encyclopedia, https://en.wikipedia.org/w/index.php?title=Text_corpus&oldid=701487841(accessed February 28, 2016)."@en ;
  skos:definition "large and structured set of texts electronically stored and processed"@en .

<https://vocabs.acdh.oeaw.ac.at/dhataxonomy/Concept32>
  skos:notation "32"^^xsd:int ;
  a skos:Concept ;
  skos:prefLabel "history studies"@en ;
  dc:modified "Mon Jun 20 00:00:00 CEST 2016"^^xsd:date ;
  dc11:source "based on history. Oxford Dictionaries. Oxford University Press. http://www.oxforddictionaries.com/definition/english/history (accessed February 28, 2016)."@en ;
  dc:created "Thu Oct 01 00:00:00 CEST 2015"^^xsd:date ;
  skos:topConceptOf <https://vocabs.acdh.oeaw.ac.at/dhataxonomy/dhaTaxonomyScheme> ;
  skos:inScheme <https://vocabs.acdh.oeaw.ac.at/dhataxonomy/dhaTaxonomyScheme> ;
  skos:definition "the study of past events, particularly in human affairs"@en .

<https://vocabs.acdh.oeaw.ac.at/dhataxonomy/Concept48.03>
  skos:notation "48.03"^^xsd:int ;
  skos:definition "process of classification of individual tokens in a text as belonging to a particular part of speech or word class"@en ;
  skos:inScheme <https://vocabs.acdh.oeaw.ac.at/dhataxonomy/dhaTaxonomyScheme> ;
  skos:broader <https://vocabs.acdh.oeaw.ac.at/dhataxonomy/Concept48> ;
  dc11:creator "ACDH-OEAW Team"@en ;
  a skos:Concept ;
  dc:modified "Mon Jun 20 00:00:00 CEST 2016"^^xsd:date ;
  skos:prefLabel "pos-tagging"@en ;
  dc:created "Thu Oct 01 00:00:00 CEST 2015"^^xsd:date .

<https://vocabs.acdh.oeaw.ac.at/dhataxonomy/Collection01>
  a skos:Collection ;
  skos:member <https://vocabs.acdh.oeaw.ac.at/dhataxonomy/Concept3.04>, <https://vocabs.acdh.oeaw.ac.at/dhataxonomy/Concept2.02>, <https://vocabs.acdh.oeaw.ac.at/dhataxonomy/Concept7>, <https://vocabs.acdh.oeaw.ac.at/dhataxonomy/Concept3.02>, <https://vocabs.acdh.oeaw.ac.at/dhataxonomy/Concept2.01>, <https://vocabs.acdh.oeaw.ac.at/dhataxonomy/Concept6.01>, <https://vocabs.acdh.oeaw.ac.at/dhataxonomy/Concept1>, <https://vocabs.acdh.oeaw.ac.at/dhataxonomy/Concept7.01>, <https://vocabs.acdh.oeaw.ac.at/dhataxonomy/Concept3.01>, <https://vocabs.acdh.oeaw.ac.at/dhataxonomy/Concept2>, <https://vocabs.acdh.oeaw.ac.at/dhataxonomy/Concept5>, <https://vocabs.acdh.oeaw.ac.at/dhataxonomy/Concept6>, <https://vocabs.acdh.oeaw.ac.at/dhataxonomy/Concept7.03>, <https://vocabs.acdh.oeaw.ac.at/dhataxonomy/Concept7.02>, <https://vocabs.acdh.oeaw.ac.at/dhataxonomy/Concept3.03>, <https://vocabs.acdh.oeaw.ac.at/dhataxonomy/Concept4>, <https://vocabs.acdh.oeaw.ac.at/dhataxonomy/Concept3>, <https://vocabs.acdh.oeaw.ac.at/dhataxonomy/Concept7.04> ;
  skos:scopeNote "This group comprises the concepts related to Formats, Protocols and Standards accepted and used in Digital Humanities community."@en ;
  dc:created "Tue Apr 03 00:00:00 CEST 2018"^^xsd:date ;
  skos:prefLabel "Formats, Protocols, Standards"@en ;
  dc11:title "Formats, Protocols, Standards"@en ;
  dc11:creator "ACDH-OEAW Team"@en ;
  dc:modified "Tue Apr 03 00:00:00 CEST 2018"^^xsd:date .

<https://vocabs.acdh.oeaw.ac.at/dhataxonomy/Concept7.04>
  dc:modified "Mon Jun 20 00:00:00 CEST 2016"^^xsd:date ;
  skos:altLabel "Search/Retrieve via URL / Context Query Language"@en ;
  a skos:Concept ;
  skos:definition "protocol for querying structured data stores, using Context Query Language as query language and XML-based return format; mainly used in library systems"@en ;
  skos:prefLabel "SRU/CQL"@en ;
  dc11:creator "ACDH-OEAW Team"@en ;
  skos:broader <https://vocabs.acdh.oeaw.ac.at/dhataxonomy/Concept7> ;
  skos:inScheme <https://vocabs.acdh.oeaw.ac.at/dhataxonomy/dhaTaxonomyScheme> ;
  skos:notation "7.04"^^xsd:int ;
  dc:created "Thu Oct 01 00:00:00 CEST 2015"^^xsd:date .

<https://vocabs.acdh.oeaw.ac.at/dhataxonomy/Concept48>
  skos:altLabel "Natural Language Processing"@en ;
  skos:narrower <https://vocabs.acdh.oeaw.ac.at/dhataxonomy/Concept48.06>, <https://vocabs.acdh.oeaw.ac.at/dhataxonomy/Concept48.01>, <https://vocabs.acdh.oeaw.ac.at/dhataxonomy/Concept48.04>, <https://vocabs.acdh.oeaw.ac.at/dhataxonomy/Concept48.05>, <https://vocabs.acdh.oeaw.ac.at/dhataxonomy/Concept48.02>, <https://vocabs.acdh.oeaw.ac.at/dhataxonomy/Concept48.03>, <https://vocabs.acdh.oeaw.ac.at/dhataxonomy/Concept48.07> ;
  dc:created "Thu Oct 01 00:00:00 CEST 2015"^^xsd:date ;
  skos:definition "tools and methods to process (analyse, enrich, transform) language resources"@en ;
  a skos:Concept ;
  skos:topConceptOf <https://vocabs.acdh.oeaw.ac.at/dhataxonomy/dhaTaxonomyScheme> ;
  skos:inScheme <https://vocabs.acdh.oeaw.ac.at/dhataxonomy/dhaTaxonomyScheme> ;
  skos:notation "48"^^xsd:int ;
  dc11:creator "ACDH-OEAW Team"@en ;
  dc:modified "Mon Jun 20 00:00:00 CEST 2016"^^xsd:date ;
  skos:prefLabel "NLP"@en .

<https://vocabs.acdh.oeaw.ac.at/dhataxonomy/Concept7>
  skos:prefLabel "query language"@en ;
  skos:narrower <https://vocabs.acdh.oeaw.ac.at/dhataxonomy/Concept7.04>, <https://vocabs.acdh.oeaw.ac.at/dhataxonomy/Concept7.01>, <https://vocabs.acdh.oeaw.ac.at/dhataxonomy/Concept7.03>, <https://vocabs.acdh.oeaw.ac.at/dhataxonomy/Concept7.02> ;
  skos:definition "formalised system of signs for retrieving information from structured data stores (databases)"@en ;
  a skos:Concept ;
  dc:modified "Mon Jun 20 00:00:00 CEST 2016"^^xsd:date ;
  dc:created "Thu Oct 01 00:00:00 CEST 2015"^^xsd:date ;
  dc11:source "based on Wikipedia contributors, \"Query language,\" Wikipedia, The Free Encyclopedia, https://en.wikipedia.org/w/index.php?title=Query_language&oldid=708613942 (accessed June 13, 2016)."@en ;
  skos:notation "7"^^xsd:int ;
  skos:topConceptOf <https://vocabs.acdh.oeaw.ac.at/dhataxonomy/dhaTaxonomyScheme> ;
  skos:inScheme <https://vocabs.acdh.oeaw.ac.at/dhataxonomy/dhaTaxonomyScheme> .

<https://vocabs.acdh.oeaw.ac.at/dhataxonomy/Concept53>
  a skos:Concept ;
  skos:notation "53"^^xsd:int ;
  dc11:creator "ACDH-OEAW Team"@en ;
  skos:definition "tool for viewing and modifying digital objects"@en ;
  skos:prefLabel "editor"@en ;
  dc:modified "Mon Jun 20 00:00:00 CEST 2016"^^xsd:date ;
  skos:narrower <https://vocabs.acdh.oeaw.ac.at/dhataxonomy/Concept53.01> ;
  skos:inScheme <https://vocabs.acdh.oeaw.ac.at/dhataxonomy/dhaTaxonomyScheme> ;
  skos:topConceptOf <https://vocabs.acdh.oeaw.ac.at/dhataxonomy/dhaTaxonomyScheme> ;
  dc:created "Thu Oct 01 00:00:00 CEST 2015"^^xsd:date .

<https://vocabs.acdh.oeaw.ac.at/dhataxonomy/Concept6.01>
  dc:created "Thu Oct 01 00:00:00 CEST 2015"^^xsd:date ;
  skos:altLabel "Component MetaData Infrastructure"@en ;
  skos:inScheme <https://vocabs.acdh.oeaw.ac.at/dhataxonomy/dhaTaxonomyScheme> ;
  skos:notation "6.01"^^xsd:int ;
  a skos:Concept ;
  dc:modified "Mon Jun 20 00:00:00 CEST 2016"^^xsd:date ;
  skos:broader <https://vocabs.acdh.oeaw.ac.at/dhataxonomy/Concept6> ;
  dc11:source "based on \"Component Metadata.\" CLARIN ERIC. Accessed June 13, 2016. https://www.clarin.eu/content/component-metadata."@en ;
  skos:definition "a framework to describe and reuse metadata schemas, based on the idea of reusable components and concept-based semantic interoperability"@en ;
  skos:prefLabel "CMDI"@en .

<https://vocabs.acdh.oeaw.ac.at/dhataxonomy/Concept70>
  skos:inScheme <https://vocabs.acdh.oeaw.ac.at/dhataxonomy/dhaTaxonomyScheme> ;
  skos:definition "a formal endeavor to ensure that digital information of continuing value remains accessible and usable"@en ;
  skos:notation "70"^^xsd:int ;
  dc11:source "Wikipedia contributors, \"Digital preservation,\" Wikipedia, The Free Encyclopedia, https://en.wikipedia.org/w/index.php?title=Digital_preservation&oldid=823615256 (accessed February 8, 2018)."@en ;
  dc:modified "Tue Apr 03 00:00:00 CEST 2018"^^xsd:date ;
  dc:created "Tue Apr 03 00:00:00 CEST 2018"^^xsd:date ;
  skos:prefLabel "digital preservation"@en ;
  skos:topConceptOf <https://vocabs.acdh.oeaw.ac.at/dhataxonomy/dhaTaxonomyScheme> ;
  a skos:Concept .

<https://vocabs.acdh.oeaw.ac.at/dhataxonomy/Concept39.05>
  skos:inScheme <https://vocabs.acdh.oeaw.ac.at/dhataxonomy/dhaTaxonomyScheme> ;
  dc11:source "Wikipedia contributors, \"Historical language,\" Wikipedia, The Free Encyclopedia, https://en.wikipedia.org/w/index.php?title=Historical_language&oldid=688305297 (accessed February 8, 2018)."@en ;
  skos:prefLabel "historical language"@en ;
  skos:notation "39.05"^^xsd:int ;
  dc:created "Tue Apr 03 00:00:00 CEST 2018"^^xsd:date ;
  dc:modified "Tue Apr 03 00:00:00 CEST 2018"^^xsd:date ;
  skos:definition "a language that is spoken in a historical period, but that is distinct from its modern form; that is, it is a form of language historically attested to from the past which has evolved into more modern forms"@en ;
  skos:broader <https://vocabs.acdh.oeaw.ac.at/dhataxonomy/Concept39> ;
  a skos:Concept .

<https://vocabs.acdh.oeaw.ac.at/dhataxonomy/Collection05>
  skos:member <https://vocabs.acdh.oeaw.ac.at/dhataxonomy/Concept66>, <https://vocabs.acdh.oeaw.ac.at/dhataxonomy/Concept63>, <https://vocabs.acdh.oeaw.ac.at/dhataxonomy/Concept66.01>, <https://vocabs.acdh.oeaw.ac.at/dhataxonomy/Concept66.05>, <https://vocabs.acdh.oeaw.ac.at/dhataxonomy/Concept56.01>, <https://vocabs.acdh.oeaw.ac.at/dhataxonomy/Concept66.02>, <https://vocabs.acdh.oeaw.ac.at/dhataxonomy/Concept68>, <https://vocabs.acdh.oeaw.ac.at/dhataxonomy/Concept58>, <https://vocabs.acdh.oeaw.ac.at/dhataxonomy/Concept66.03>, <https://vocabs.acdh.oeaw.ac.at/dhataxonomy/Concept60>, <https://vocabs.acdh.oeaw.ac.at/dhataxonomy/Concept66.04>, <https://vocabs.acdh.oeaw.ac.at/dhataxonomy/Concept64>, <https://vocabs.acdh.oeaw.ac.at/dhataxonomy/Concept65>, <https://vocabs.acdh.oeaw.ac.at/dhataxonomy/Concept56>, <https://vocabs.acdh.oeaw.ac.at/dhataxonomy/Concept57>, <https://vocabs.acdh.oeaw.ac.at/dhataxonomy/Concept59.01>, <https://vocabs.acdh.oeaw.ac.at/dhataxonomy/Concept59>, <https://vocabs.acdh.oeaw.ac.at/dhataxonomy/Concept70>, <https://vocabs.acdh.oeaw.ac.at/dhataxonomy/Concept67.01>, <https://vocabs.acdh.oeaw.ac.at/dhataxonomy/Concept69>, <https://vocabs.acdh.oeaw.ac.at/dhataxonomy/Concept62>, <https://vocabs.acdh.oeaw.ac.at/dhataxonomy/Concept61>, <https://vocabs.acdh.oeaw.ac.at/dhataxonomy/Concept67>, <https://vocabs.acdh.oeaw.ac.at/dhataxonomy/Concept55> ;
  dc:modified "Tue Apr 03 00:00:00 CEST 2018"^^xsd:date ;
  skos:scopeNote "This group comprises topics of research, discussion and application within digital humanities community."@en ;
  skos:prefLabel "Topics"@en ;
  dc11:title "Topics"@en ;
  dc11:creator "ACDH-OEAW Team"@en ;
  dc:created "Tue Apr 03 00:00:00 CEST 2018"^^xsd:date ;
  a skos:Collection .

<https://vocabs.acdh.oeaw.ac.at/dhataxonomy/Concept51.01>
  dc11:source "based on Wikipedia contributors, \"Graph theory,\" Wikipedia, The Free Encyclopedia, https://en.wikipedia.org/w/index.php?title=Graph_theory&oldid=725036230 (accessed June 13, 2016)."@en ;
  dc:created "Thu Oct 01 00:00:00 CEST 2015"^^xsd:date ;
  skos:broader <https://vocabs.acdh.oeaw.ac.at/dhataxonomy/Concept51> ;
  dc:modified "Mon Jun 20 00:00:00 CEST 2016"^^xsd:date ;
  skos:prefLabel "graph"@en ;
  skos:notation "51.01"^^xsd:int ;
  skos:definition "(mathematical) structure representing objects (nodes) and relations between them (edges)"@en ;
  skos:inScheme <https://vocabs.acdh.oeaw.ac.at/dhataxonomy/dhaTaxonomyScheme> ;
  a skos:Concept .

<https://vocabs.acdh.oeaw.ac.at/dhataxonomy/Concept2.01>
  dc11:source "Maarten Van Gompel, \"FoLiA Format for Linguistic Annotation.\" FoLiA. Accessed June 13, 2016. https://proycon.github.io/folia/."@en ;
  skos:altLabel "Format for Linguistic Annotation"@en ;
  skos:notation "2.01"^^xsd:int ;
  skos:prefLabel "Folia"@en ;
  dc:created "Thu Oct 01 00:00:00 CEST 2015"^^xsd:date ;
  skos:broader <https://vocabs.acdh.oeaw.ac.at/dhataxonomy/Concept2> ;
  dc:modified "Mon Jun 20 00:00:00 CEST 2016"^^xsd:date ;
  a skos:Concept ;
  skos:inScheme <https://vocabs.acdh.oeaw.ac.at/dhataxonomy/dhaTaxonomyScheme> ;
  skos:definition "an XML-based annotation format, suitable for the representation of linguistically annotated language resources"@en .

<https://vocabs.acdh.oeaw.ac.at/dhataxonomy/Concept59>
  dc11:source "based on Wikipedia contributors, \"Semantic Web,\" Wikipedia, The Free Encyclopedia, https://en.wikipedia.org/w/index.php?title=Semantic_Web&oldid=724047432 (accessed June 13, 2016); Berners-Lee, Tim; James Hendler; Ora Lassila. \"The Semantic Web\". Scientific American Magazine. May 2001. Accessed March 26, 2008."@en ;
  skos:prefLabel "Semantic web"@en ;
  dc:created "Thu Oct 01 00:00:00 CEST 2015"^^xsd:date ;
  skos:inScheme <https://vocabs.acdh.oeaw.ac.at/dhataxonomy/dhaTaxonomyScheme> ;
  skos:narrower <https://vocabs.acdh.oeaw.ac.at/dhataxonomy/Concept59.01> ;
  skos:notation "59"^^xsd:int ;
  a skos:Concept ;
  skos:definition "extension of the web, a common framework that allows data to be shared and reused across application, enterprise, and community boundaries"@en ;
  skos:topConceptOf <https://vocabs.acdh.oeaw.ac.at/dhataxonomy/dhaTaxonomyScheme> ;
  dc:modified "Mon Jun 20 00:00:00 CEST 2016"^^xsd:date .

<https://vocabs.acdh.oeaw.ac.at/dhataxonomy/Concept7.03>
  skos:prefLabel "CQP/CQL"@en ;
  skos:definition "query language used to search corpus"@en ;
  dc:created "Thu Oct 01 00:00:00 CEST 2015"^^xsd:date ;
  skos:inScheme <https://vocabs.acdh.oeaw.ac.at/dhataxonomy/dhaTaxonomyScheme> ;
  skos:altLabel "Corpus Query Language"@en ;
  skos:notation "7.03"^^xsd:int ;
  a skos:Concept ;
  dc11:creator "ACDH-OEAW Team"@en ;
  skos:broader <https://vocabs.acdh.oeaw.ac.at/dhataxonomy/Concept7> ;
  dc:modified "Mon Jun 20 00:00:00 CEST 2016"^^xsd:date .

<https://vocabs.acdh.oeaw.ac.at/dhataxonomy/Concept74>
  skos:topConceptOf <https://vocabs.acdh.oeaw.ac.at/dhataxonomy/dhaTaxonomyScheme> ;
  dc:created "Thu Oct 01 00:00:00 CEST 2015"^^xsd:date ;
  skos:notation "74"^^xsd:int ;
  skos:definition "processing instructions that can be executed on a computer (scripts, command-line tools, programs)"@en ;
  a skos:Concept ;
  dc11:creator "ACDH-OEAW Team"@en ;
  skos:prefLabel "type_software"@en ;
  dc:modified "Mon Jun 20 00:00:00 CEST 2016"^^xsd:date ;
  skos:inScheme <https://vocabs.acdh.oeaw.ac.at/dhataxonomy/dhaTaxonomyScheme> .

<https://vocabs.acdh.oeaw.ac.at/dhataxonomy/Concept3.04>
  skos:notation "3.04"^^xsd:int ;
  skos:altLabel "Comité international pour la documentation: Conceptual Reference Model"@en ;
  dc11:source "based on \"The CIDOC CRM.\" The CIDOC CRM. Accessed June 13, 2016. http://www.cidoc-crm.org/."@en ;
  skos:prefLabel "CIDOC CRM"@en ;
  dc:modified "Mon Jun 20 00:00:00 CEST 2016"^^xsd:date ;
  skos:broader <https://vocabs.acdh.oeaw.ac.at/dhataxonomy/Concept3> ;
  dc:created "Thu Oct 01 00:00:00 CEST 2015"^^xsd:date ;
  skos:inScheme <https://vocabs.acdh.oeaw.ac.at/dhataxonomy/dhaTaxonomyScheme> ;
  skos:definition "a machine-readable ontology that provides definitions and a formal structure for describing general (top-level) concepts and relationships; used mainly in cultural heritage domain"@en ;
  a skos:Concept .

<https://vocabs.acdh.oeaw.ac.at/dhataxonomy/Concept28>
  skos:definition "the scientific study of language and its structure"@en ;
  skos:prefLabel "linguistics"@en ;
  skos:inScheme <https://vocabs.acdh.oeaw.ac.at/dhataxonomy/dhaTaxonomyScheme> ;
  skos:notation "28"^^xsd:int ;
  dc11:source "linguistics. Oxford Dictionaries. Oxford University Press. http://www.oxforddictionaries.com/definition/english/linguistics (accessed February 28, 2016)."@en ;
  a skos:Concept ;
  dc:modified "Mon Jun 20 00:00:00 CEST 2016"^^xsd:date ;
  dc:created "Thu Oct 01 00:00:00 CEST 2015"^^xsd:date ;
  skos:narrower <https://vocabs.acdh.oeaw.ac.at/dhataxonomy/Concept28.01>, <https://vocabs.acdh.oeaw.ac.at/dhataxonomy/Concept28.02> ;
  skos:topConceptOf <https://vocabs.acdh.oeaw.ac.at/dhataxonomy/dhaTaxonomyScheme> .

<https://vocabs.acdh.oeaw.ac.at/dhataxonomy/Concept41>
  skos:notation "41"^^xsd:int ;
  dc11:source "Wikipedia contributors, \"Optical character recognition,\" Wikipedia, The Free Encyclopedia, https://en.wikipedia.org/w/index.php?title=Optical_character_recognition&oldid=706482815 (accessed February 28, 2016)."@en ;
  skos:topConceptOf <https://vocabs.acdh.oeaw.ac.at/dhataxonomy/dhaTaxonomyScheme> ;
  skos:definition "mechanical or electronic conversion of images of typed, handwritten or printed text into machine-encoded text"@en ;
  skos:inScheme <https://vocabs.acdh.oeaw.ac.at/dhataxonomy/dhaTaxonomyScheme> ;
  skos:altLabel "OCR"@en ;
  skos:prefLabel "Optical Character Recognition"@en ;
  a skos:Concept ;
  dc:modified "Mon Jun 20 00:00:00 CEST 2016"^^xsd:date ;
  dc:created "Thu Oct 01 00:00:00 CEST 2015"^^xsd:date .

<https://vocabs.acdh.oeaw.ac.at/dhataxonomy/Concept3.02>
  dc:modified "Mon Jun 20 00:00:00 CEST 2016"^^xsd:date ;
  skos:broader <https://vocabs.acdh.oeaw.ac.at/dhataxonomy/Concept3> ;
  skos:definition "a group of W3C specifications designed as a metadata data model to provide interoperability between applications that exchange machine-understandable information on the Web. It is used as a general method for conceptual description or modeling of information."@en ;
  dc11:source "based on Wikipedia contributors, \"Resource Description Framework,\" Wikipedia, The Free Encyclopedia, https://en.wikipedia.org/w/index.php?title=Resource_Description_Framework&oldid=722184246 (accessed June 13, 2016)."@en ;
  a skos:Concept ;
  skos:inScheme <https://vocabs.acdh.oeaw.ac.at/dhataxonomy/dhaTaxonomyScheme> ;
  skos:notation "3.02"^^xsd:int ;
  skos:prefLabel "RDF"@en ;
  dc:created "Thu Oct 01 00:00:00 CEST 2015"^^xsd:date ;
  skos:altLabel "Resource Description Framework"@en .

<https://vocabs.acdh.oeaw.ac.at/dhataxonomy/Collection02>
  skos:member <https://vocabs.acdh.oeaw.ac.at/dhataxonomy/Concept11>, <https://vocabs.acdh.oeaw.ac.at/dhataxonomy/Concept28>, <https://vocabs.acdh.oeaw.ac.at/dhataxonomy/Concept13>, <https://vocabs.acdh.oeaw.ac.at/dhataxonomy/Concept12>, <https://vocabs.acdh.oeaw.ac.at/dhataxonomy/Concept15>, <https://vocabs.acdh.oeaw.ac.at/dhataxonomy/Concept21>, <https://vocabs.acdh.oeaw.ac.at/dhataxonomy/Concept20>, <https://vocabs.acdh.oeaw.ac.at/dhataxonomy/Concept25>, <https://vocabs.acdh.oeaw.ac.at/dhataxonomy/Concept8>, <https://vocabs.acdh.oeaw.ac.at/dhataxonomy/Concept10>, <https://vocabs.acdh.oeaw.ac.at/dhataxonomy/Concept16>, <https://vocabs.acdh.oeaw.ac.at/dhataxonomy/Concept31>, <https://vocabs.acdh.oeaw.ac.at/dhataxonomy/Concept30>, <https://vocabs.acdh.oeaw.ac.at/dhataxonomy/Concept28.01>, <https://vocabs.acdh.oeaw.ac.at/dhataxonomy/Concept28.02>, <https://vocabs.acdh.oeaw.ac.at/dhataxonomy/Concept24>, <https://vocabs.acdh.oeaw.ac.at/dhataxonomy/Concept26>, <https://vocabs.acdh.oeaw.ac.at/dhataxonomy/Concept22>, <https://vocabs.acdh.oeaw.ac.at/dhataxonomy/Concept19>, <https://vocabs.acdh.oeaw.ac.at/dhataxonomy/Concept32>, <https://vocabs.acdh.oeaw.ac.at/dhataxonomy/Concept14>, <https://vocabs.acdh.oeaw.ac.at/dhataxonomy/Concept9>, <https://vocabs.acdh.oeaw.ac.at/dhataxonomy/Concept17>, <https://vocabs.acdh.oeaw.ac.at/dhataxonomy/Concept18>, <https://vocabs.acdh.oeaw.ac.at/dhataxonomy/Concept23>, <https://vocabs.acdh.oeaw.ac.at/dhataxonomy/Concept29>, <https://vocabs.acdh.oeaw.ac.at/dhataxonomy/Concept27> ;
  a skos:Collection ;
  skos:prefLabel "Disciplines"@en ;
  dc11:title "Disciplines"@en ;
  dc:created "Tue Apr 03 00:00:00 CEST 2018"^^xsd:date ;
  skos:scopeNote "This group comprises the disciplines that are part of digital humanities research."@en ;
  dc:modified "Tue Apr 03 00:00:00 CEST 2018"^^xsd:date ;
  dc11:creator "ACDH-OEAW Team"@en .

<https://vocabs.acdh.oeaw.ac.at/dhataxonomy/Concept46>
  a skos:Concept ;
  skos:definition "system or procedure automatically expressing text from one language in another language"@en ;
  dc11:creator "ACDH-OEAW Team"@en ;
  skos:notation "46"^^xsd:int ;
  dc:modified "Mon Jun 20 00:00:00 CEST 2016"^^xsd:date ;
  dc:created "Thu Oct 01 00:00:00 CEST 2015"^^xsd:date ;
  skos:topConceptOf <https://vocabs.acdh.oeaw.ac.at/dhataxonomy/dhaTaxonomyScheme> ;
  skos:prefLabel "machine translation"@en ;
  skos:inScheme <https://vocabs.acdh.oeaw.ac.at/dhataxonomy/dhaTaxonomyScheme> .

<https://vocabs.acdh.oeaw.ac.at/dhataxonomy/Concept49>
  skos:prefLabel "Social network analysis"@en ;
  skos:notation "49"^^xsd:int ;
  dc:modified "Mon Jun 20 00:00:00 CEST 2016"^^xsd:date ;
  skos:definition "a set of methods used to investigate relationships and  interactions of individual actors and/or groups"@en ;
  skos:topConceptOf <https://vocabs.acdh.oeaw.ac.at/dhataxonomy/dhaTaxonomyScheme> ;
  dc:created "Thu Oct 01 00:00:00 CEST 2015"^^xsd:date ;
  dc11:source "based on Wikipedia contributors, \"Social network analysis,\" Wikipedia, The Free Encyclopedia, https://en.wikipedia.org/w/index.php?title=Social_network_analysis&oldid=702459164 (accessed February 28, 2016)."@en ;
  skos:inScheme <https://vocabs.acdh.oeaw.ac.at/dhataxonomy/dhaTaxonomyScheme> ;
  a skos:Concept .

<https://vocabs.acdh.oeaw.ac.at/dhataxonomy/Concept73>
  dc11:creator "ACDH-OEAW Team"@en ;
  skos:definition "online resources (both static and dynamic or interactive) that can be explored or downloaded and used for further research; e.g. datasets, digital editions, web applications, catalogues, registries, processing services, etc."@en ;
  skos:notation "73"^^xsd:int ;
  skos:prefLabel "type_resource"@en ;
  a skos:Concept ;
  dc:modified "Mon Jun 20 00:00:00 CEST 2016"^^xsd:date ;
  skos:inScheme <https://vocabs.acdh.oeaw.ac.at/dhataxonomy/dhaTaxonomyScheme> ;
  skos:topConceptOf <https://vocabs.acdh.oeaw.ac.at/dhataxonomy/dhaTaxonomyScheme> ;
  dc:created "Thu Oct 01 00:00:00 CEST 2015"^^xsd:date .

<https://vocabs.acdh.oeaw.ac.at/dhataxonomy/Concept67>
  skos:prefLabel "data management"@en ;
  dc:modified "Tue Apr 03 00:00:00 CEST 2018"^^xsd:date ;
  dc:created "Tue Apr 03 00:00:00 CEST 2018"^^xsd:date ;
  skos:topConceptOf <https://vocabs.acdh.oeaw.ac.at/dhataxonomy/dhaTaxonomyScheme> ;
  a skos:Concept ;
  skos:inScheme <https://vocabs.acdh.oeaw.ac.at/dhataxonomy/dhaTaxonomyScheme> ;
  skos:notation "67"^^xsd:int ;
  dc11:source "Wikipedia contributors, \"Data management,\" Wikipedia, The Free Encyclopedia, https://en.wikipedia.org/w/index.php?title=Data_management&oldid=819356963 (accessed February 8, 2018)."@en ;
  skos:narrower <https://vocabs.acdh.oeaw.ac.at/dhataxonomy/Concept67.01> ;
  skos:definition "data management comprises all the disciplines related to managing data as a valuable resource"@en .

<https://vocabs.acdh.oeaw.ac.at/dhataxonomy/Concept2>
  dc:created "Thu Oct 01 00:00:00 CEST 2015"^^xsd:date ;
  dc11:creator "ACDH-OEAW Team"@en ;
  a skos:Concept ;
  skos:definition "the representation of printed texts in digital format"@en ;
  skos:topConceptOf <https://vocabs.acdh.oeaw.ac.at/dhataxonomy/dhaTaxonomyScheme> ;
  skos:prefLabel "text encoding"@en ;
  skos:inScheme <https://vocabs.acdh.oeaw.ac.at/dhataxonomy/dhaTaxonomyScheme> ;
  dc:modified "Mon Jun 20 00:00:00 CEST 2016"^^xsd:date ;
  skos:narrower <https://vocabs.acdh.oeaw.ac.at/dhataxonomy/Concept2.02>, <https://vocabs.acdh.oeaw.ac.at/dhataxonomy/Concept2.01> ;
  skos:notation "2"^^xsd:int .

<https://vocabs.acdh.oeaw.ac.at/dhataxonomy/Concept47>
  dc11:source "GIS. Oxford Dictionaries. Oxford University Press. http://www.oxforddictionaries.com/definition/english/gis (accessed February 28, 2016)."@en ;
  skos:altLabel "Geographic Information System"@en ;
  a skos:Concept ;
  dc:modified "Mon Jun 20 00:00:00 CEST 2016"^^xsd:date ;
  skos:prefLabel "GIS"@en ;
  skos:definition "system for storing and manipulating geographical information"@en ;
  dc:created "Thu Oct 01 00:00:00 CEST 2015"^^xsd:date ;
  skos:notation "47"^^xsd:int ;
  skos:topConceptOf <https://vocabs.acdh.oeaw.ac.at/dhataxonomy/dhaTaxonomyScheme> ;
  skos:inScheme <https://vocabs.acdh.oeaw.ac.at/dhataxonomy/dhaTaxonomyScheme> .

<https://vocabs.acdh.oeaw.ac.at/dhataxonomy/Concept7.01>
  a skos:Concept ;
  skos:definition "query language for manipulating and retrieving data stored in relational databases"@en ;
  dc:modified "Mon Jun 20 00:00:00 CEST 2016"^^xsd:date ;
  skos:notation "7.01"^^xsd:int ;
  skos:prefLabel "SQL"@en ;
  dc11:source "based on Wikipedia contributors, \"SQL,\" Wikipedia, The Free Encyclopedia, https://en.wikipedia.org/w/index.php?title=SQL&oldid=724471814 (accessed June 13, 2016)."@en ;
  skos:altLabel "Structured Query Language"@en ;
  skos:inScheme <https://vocabs.acdh.oeaw.ac.at/dhataxonomy/dhaTaxonomyScheme> ;
  skos:broader <https://vocabs.acdh.oeaw.ac.at/dhataxonomy/Concept7> ;
  dc:created "Thu Oct 01 00:00:00 CEST 2015"^^xsd:date .

<https://vocabs.acdh.oeaw.ac.at/dhataxonomy/Concept35>
  skos:inScheme <https://vocabs.acdh.oeaw.ac.at/dhataxonomy/dhaTaxonomyScheme> ;
  dc11:creator "ACDH-OEAW Team"@en ;
  skos:definition "a digital representation of objects in a three-dimensional space"@en ;
  skos:prefLabel "3D"@en ;
  dc:modified "Mon Jun 20 00:00:00 CEST 2016"^^xsd:date ;
  dc:created "Thu Oct 01 00:00:00 CEST 2015"^^xsd:date ;
  skos:topConceptOf <https://vocabs.acdh.oeaw.ac.at/dhataxonomy/dhaTaxonomyScheme> ;
  skos:notation "35"^^xsd:int ;
  a skos:Concept .

<https://vocabs.acdh.oeaw.ac.at/dhataxonomy/Collection04>
  skos:member <https://vocabs.acdh.oeaw.ac.at/dhataxonomy/Concept45>, <https://vocabs.acdh.oeaw.ac.at/dhataxonomy/Concept48.02>, <https://vocabs.acdh.oeaw.ac.at/dhataxonomy/Concept48.05>, <https://vocabs.acdh.oeaw.ac.at/dhataxonomy/Concept41>, <https://vocabs.acdh.oeaw.ac.at/dhataxonomy/Concept48.04>, <https://vocabs.acdh.oeaw.ac.at/dhataxonomy/Concept48.01>, <https://vocabs.acdh.oeaw.ac.at/dhataxonomy/Concept44>, <https://vocabs.acdh.oeaw.ac.at/dhataxonomy/Concept46>, <https://vocabs.acdh.oeaw.ac.at/dhataxonomy/Concept48.06>, <https://vocabs.acdh.oeaw.ac.at/dhataxonomy/Concept48>, <https://vocabs.acdh.oeaw.ac.at/dhataxonomy/Concept52>, <https://vocabs.acdh.oeaw.ac.at/dhataxonomy/Concept49>, <https://vocabs.acdh.oeaw.ac.at/dhataxonomy/Concept54>, <https://vocabs.acdh.oeaw.ac.at/dhataxonomy/Concept50>, <https://vocabs.acdh.oeaw.ac.at/dhataxonomy/Concept48.03>, <https://vocabs.acdh.oeaw.ac.at/dhataxonomy/Concept53>, <https://vocabs.acdh.oeaw.ac.at/dhataxonomy/Concept47>, <https://vocabs.acdh.oeaw.ac.at/dhataxonomy/Concept43>, <https://vocabs.acdh.oeaw.ac.at/dhataxonomy/Concept53.01>, <https://vocabs.acdh.oeaw.ac.at/dhataxonomy/Concept51.01>, <https://vocabs.acdh.oeaw.ac.at/dhataxonomy/Concept48.07>, <https://vocabs.acdh.oeaw.ac.at/dhataxonomy/Concept51>, <https://vocabs.acdh.oeaw.ac.at/dhataxonomy/Concept42>, <https://vocabs.acdh.oeaw.ac.at/dhataxonomy/Concept45.01> ;
  dc11:title "Tools and Services"@en ;
  a skos:Collection ;
  dc11:creator "ACDH-OEAW Team"@en ;
  dc:created "Tue Apr 03 00:00:00 CEST 2018"^^xsd:date ;
  skos:prefLabel "Tools and Services"@en ;
  dc:modified "Tue Apr 03 00:00:00 CEST 2018"^^xsd:date ;
  skos:scopeNote "This group comprises  the tool and services used in digital humanities field."@en .

<https://vocabs.acdh.oeaw.ac.at/dhataxonomy/Concept37>
  dc11:source "based on map. Oxford Dictionaries. Oxford University Press. http://www.oxforddictionaries.com/definition/english/map (accessed February 28, 2016)."@en ;
  dc:modified "Mon Jun 20 00:00:00 CEST 2016"^^xsd:date ;
  skos:prefLabel "map"@en ;
  a skos:Concept ;
  skos:definition "schematic representation of an area of land or sea showing physical features, cities, roads, etc."@en ;
  dc:created "Thu Oct 01 00:00:00 CEST 2015"^^xsd:date ;
  skos:inScheme <https://vocabs.acdh.oeaw.ac.at/dhataxonomy/dhaTaxonomyScheme> ;
  skos:topConceptOf <https://vocabs.acdh.oeaw.ac.at/dhataxonomy/dhaTaxonomyScheme> ;
  skos:notation "37"^^xsd:int .

<https://vocabs.acdh.oeaw.ac.at/dhataxonomy/Concept38>
  dc11:source "based on image. Oxford Dictionaries. Oxford University Press. http://www.oxforddictionaries.com/definition/english/image (accessed February 28, 2016)."@en ;
  skos:prefLabel "image"@en ;
  a skos:Concept ;
  skos:topConceptOf <https://vocabs.acdh.oeaw.ac.at/dhataxonomy/dhaTaxonomyScheme> ;
  skos:definition "a two-dimensional visual representation of something"@en ;
  dc:modified "Mon Jun 20 00:00:00 CEST 2016"^^xsd:date ;
  skos:notation "38"^^xsd:int ;
  dc:created "Thu Oct 01 00:00:00 CEST 2015"^^xsd:date ;
  skos:inScheme <https://vocabs.acdh.oeaw.ac.at/dhataxonomy/dhaTaxonomyScheme> .

<https://vocabs.acdh.oeaw.ac.at/dhataxonomy/Concept3.01>
  skos:inScheme <https://vocabs.acdh.oeaw.ac.at/dhataxonomy/dhaTaxonomyScheme> ;
  skos:notation "3.01"^^xsd:int ;
  dc11:source "based on Wikipedia contributors, \"Simple Knowledge Organization System,\" Wikipedia, The Free Encyclopedia, https://en.wikipedia.org/w/index.php?title=Simple_Knowledge_Organization_System&oldid=703222387 (accessed February 28, 2016)."@en ;
  skos:prefLabel "SKOS"@en ;
  skos:definition "a W3C recommendation format designed for the representation of thesauri, classification schemes, taxonomies, subject-heading systems, or any other type of structured controlled vocabulary"@en ;
  dc:modified "Mon Jun 20 00:00:00 CEST 2016"^^xsd:date ;
  skos:broader <https://vocabs.acdh.oeaw.ac.at/dhataxonomy/Concept3> ;
  dc:created "Thu Oct 01 00:00:00 CEST 2015"^^xsd:date ;
  skos:altLabel "Simple Knowledge Organisation System"@en ;
  a skos:Concept .

<https://vocabs.acdh.oeaw.ac.at/dhataxonomy/Concept58>
  skos:notation "58"^^xsd:int ;
  dc:created "Thu Oct 01 00:00:00 CEST 2015"^^xsd:date ;
  skos:topConceptOf <https://vocabs.acdh.oeaw.ac.at/dhataxonomy/dhaTaxonomyScheme> ;
  skos:definition "learning conducted via electronic media, typically on the Internet"@en ;
  skos:inScheme <https://vocabs.acdh.oeaw.ac.at/dhataxonomy/dhaTaxonomyScheme> ;
  skos:prefLabel "e-learning"@en ;
  dc11:source "e-learning. Oxford Dictionaries. Oxford University Press. http://www.oxforddictionaries.com/definition/english/e-learning (accessed February 28, 2016)."@en ;
  a skos:Concept ;
  dc:modified "Mon Jun 20 00:00:00 CEST 2016"^^xsd:date .

<https://vocabs.acdh.oeaw.ac.at/dhataxonomy/Concept60>
  dc11:source "based Wikipedia contributors, \"Open access,\" Wikipedia, The Free Encyclopedia, https://en.wikipedia.org/w/index.php?title=Open_access&oldid=705203639 (accessed February 28, 2016)."@en ;
  dc:created "Thu Oct 01 00:00:00 CEST 2015"^^xsd:date ;
  skos:notation "60"^^xsd:int ;
  dc:modified "Mon Jun 20 00:00:00 CEST 2016"^^xsd:date ;
  skos:inScheme <https://vocabs.acdh.oeaw.ac.at/dhataxonomy/dhaTaxonomyScheme> ;
  skos:definition "resources (both research outputs and research data) that are free of all restrictions on access and free of many restrictions on use"@en ;
  skos:topConceptOf <https://vocabs.acdh.oeaw.ac.at/dhataxonomy/dhaTaxonomyScheme> ;
  a skos:Concept ;
  skos:prefLabel "open access"@en .

<https://vocabs.acdh.oeaw.ac.at/dhataxonomy/Concept30>
  skos:inScheme <https://vocabs.acdh.oeaw.ac.at/dhataxonomy/dhaTaxonomyScheme> ;
  skos:topConceptOf <https://vocabs.acdh.oeaw.ac.at/dhataxonomy/dhaTaxonomyScheme> ;
  a skos:Concept ;
  dc:created "Thu Oct 01 00:00:00 CEST 2015"^^xsd:date ;
  skos:definition "the study of contemporary (especially mass) culture"@en ;
  dc:modified "Mon Jun 20 00:00:00 CEST 2016"^^xsd:date ;
  skos:notation "30"^^xsd:int ;
  dc11:source "cultural studies. Oxford Dictionaries. Oxford University Press. http://www.oxforddictionaries.com/definition/english/cultural-studies (accessed February 28, 2016)."@en ;
  skos:prefLabel "cultural studies"@en .

<https://vocabs.acdh.oeaw.ac.at/dhataxonomy/Concept66.03>
  dc11:source "based on ARIADNE. Accessed June 13, 2016. http://www.ariadne-infrastructure.eu/."@en ;
  skos:definition "research infrastructure that brings together and integrates existing archaeological research data infrastructures"@en ;
  a skos:Concept ;
  skos:inScheme <https://vocabs.acdh.oeaw.ac.at/dhataxonomy/dhaTaxonomyScheme> ;
  skos:altLabel "Advanced Research Infrastructure for Archaeological Dataset Networking in Europe"@en ;
  dc:created "Thu Oct 01 00:00:00 CEST 2015"^^xsd:date ;
  skos:notation "66.03"^^xsd:int ;
  skos:prefLabel "ARIADNE"@en ;
  dc:modified "Mon Jun 20 00:00:00 CEST 2016"^^xsd:date ;
  skos:broader <https://vocabs.acdh.oeaw.ac.at/dhataxonomy/Concept66> .

<https://vocabs.acdh.oeaw.ac.at/dhataxonomy/Concept40>
  skos:prefLabel "semantic resource"@en ;
  dc11:creator "ACDH-OEAW Team"@en ;
  skos:notation "40"^^xsd:int ;
  dc:created "Thu Oct 01 00:00:00 CEST 2015"^^xsd:date ;
  skos:inScheme <https://vocabs.acdh.oeaw.ac.at/dhataxonomy/dhaTaxonomyScheme> ;
  skos:topConceptOf <https://vocabs.acdh.oeaw.ac.at/dhataxonomy/dhaTaxonomyScheme> ;
  a skos:Concept ;
  skos:definition "a machine-readable data-set conveying structured information about concepts and their relations to each other used as a basic building block of the semantic web"@en ;
  skos:narrower <https://vocabs.acdh.oeaw.ac.at/dhataxonomy/Concept40.02>, <https://vocabs.acdh.oeaw.ac.at/dhataxonomy/Concept40.04>, <https://vocabs.acdh.oeaw.ac.at/dhataxonomy/Concept40.03>, <https://vocabs.acdh.oeaw.ac.at/dhataxonomy/Concept40.01> ;
  dc:modified "Mon Jun 20 00:00:00 CEST 2016"^^xsd:date .

<https://vocabs.acdh.oeaw.ac.at/dhataxonomy/Concept11>
  skos:topConceptOf <https://vocabs.acdh.oeaw.ac.at/dhataxonomy/dhaTaxonomyScheme> ;
  skos:inScheme <https://vocabs.acdh.oeaw.ac.at/dhataxonomy/dhaTaxonomyScheme> ;
  a skos:Concept ;
  dc11:source "based on Wikipedia contributors, \"Gender studies,\" Wikipedia, The Free Encyclopedia, https://en.wikipedia.org/w/index.php?title=Gender_studies&oldid=833509786 (accessed April 3, 2018)."@en ;
  dc:modified "Tue Apr 03 00:00:00 CEST 2018"^^xsd:date ;
  skos:definition "an interdisciplinary field and academic studies devoted to gender identity and gendered representation as central categories of analysis, including women's studies (concerning women, feminism, gender, and politics), men's studies and LGBT studies."@en ;
  skos:prefLabel "gender studies"@en ;
  dc:created "Thu Oct 01 00:00:00 CEST 2015"^^xsd:date ;
  skos:notation "11"^^xsd:int .

<https://vocabs.acdh.oeaw.ac.at/dhataxonomy/Concept8>
  dc:created "Thu Oct 01 00:00:00 CEST 2015"^^xsd:date ;
  skos:notation "8"^^xsd:int ;
  skos:topConceptOf <https://vocabs.acdh.oeaw.ac.at/dhataxonomy/dhaTaxonomyScheme> ;
  dc11:source "Wikipedia contributors, \"Musicology,\" Wikipedia, The Free Encyclopedia, https://en.wikipedia.org/w/index.php?title=Musicology&oldid=711823687 (accessed April 4, 2016)."@en ;
  dc:modified "Mon Jun 20 00:00:00 CEST 2016"^^xsd:date ;
  skos:definition "the scholarly analysis of, and research on, music, a part of humanities."@en ;
  a skos:Concept ;
  skos:prefLabel "musicology"@en ;
  skos:inScheme <https://vocabs.acdh.oeaw.ac.at/dhataxonomy/dhaTaxonomyScheme> .

<https://vocabs.acdh.oeaw.ac.at/dhataxonomy/Collection03>
  skos:member <https://vocabs.acdh.oeaw.ac.at/dhataxonomy/Concept39.04>, <https://vocabs.acdh.oeaw.ac.at/dhataxonomy/Concept39.05>, <https://vocabs.acdh.oeaw.ac.at/dhataxonomy/Concept39>, <https://vocabs.acdh.oeaw.ac.at/dhataxonomy/Concept36>, <https://vocabs.acdh.oeaw.ac.at/dhataxonomy/Concept33>, <https://vocabs.acdh.oeaw.ac.at/dhataxonomy/Concept40.02>, <https://vocabs.acdh.oeaw.ac.at/dhataxonomy/Concept40.03>, <https://vocabs.acdh.oeaw.ac.at/dhataxonomy/Concept39.03>, <https://vocabs.acdh.oeaw.ac.at/dhataxonomy/Concept39.01>, <https://vocabs.acdh.oeaw.ac.at/dhataxonomy/Concept34>, <https://vocabs.acdh.oeaw.ac.at/dhataxonomy/Concept39.02>, <https://vocabs.acdh.oeaw.ac.at/dhataxonomy/Concept38>, <https://vocabs.acdh.oeaw.ac.at/dhataxonomy/Concept40.01>, <https://vocabs.acdh.oeaw.ac.at/dhataxonomy/Concept40>, <https://vocabs.acdh.oeaw.ac.at/dhataxonomy/Concept40.04>, <https://vocabs.acdh.oeaw.ac.at/dhataxonomy/Concept37>, <https://vocabs.acdh.oeaw.ac.at/dhataxonomy/Concept35> ;
  a skos:Collection ;
  skos:scopeNote "This group comprises  the resources used in digital humanities field."@en ;
  dc:created "Tue Apr 03 00:00:00 CEST 2018"^^xsd:date ;
  dc:modified "Tue Apr 03 00:00:00 CEST 2018"^^xsd:date ;
  dc11:creator "ACDH-OEAW Team"@en ;
  dc11:title "Resources"@en ;
  skos:prefLabel "Resources"@en .

<https://vocabs.acdh.oeaw.ac.at/dhataxonomy/Concept45.01>
  skos:broader <https://vocabs.acdh.oeaw.ac.at/dhataxonomy/Concept45> ;
  dc:created "Thu Oct 01 00:00:00 CEST 2015"^^xsd:date ;
  skos:inScheme <https://vocabs.acdh.oeaw.ac.at/dhataxonomy/dhaTaxonomyScheme> ;
  skos:prefLabel "metasearch"@en ;
  skos:notation "45.01"^^xsd:int ;
  dc11:creator "ACDH-OEAW Team"@en ;
  dc:modified "Mon Jun 20 00:00:00 CEST 2016"^^xsd:date ;
  skos:definition "services that allows to query multiple search services and aggregates the multiple results to one result set"@en ;
  skos:altLabel "aggregator"@en ;
  a skos:Concept .

<https://vocabs.acdh.oeaw.ac.at/dhataxonomy/Concept28.01>
  skos:definition "the branch of linguistics concerned with analysis of corpora as a means of studying language"@en ;
  skos:broader <https://vocabs.acdh.oeaw.ac.at/dhataxonomy/Concept28> ;
  dc:created "Thu Oct 01 00:00:00 CEST 2015"^^xsd:date ;
  skos:inScheme <https://vocabs.acdh.oeaw.ac.at/dhataxonomy/dhaTaxonomyScheme> ;
  skos:prefLabel "corpus linguistics"@en ;
  a skos:Concept ;
  skos:notation "28.01"^^xsd:int ;
  dc11:source "corpus linguistics. Oxford Dictionaries. Oxford University Press. http://www.oxforddictionaries.com/definition/english/corpus-linguistics (accessed February 28, 2016)."@en ;
  dc:modified "Mon Jun 20 00:00:00 CEST 2016"^^xsd:date .

<https://vocabs.acdh.oeaw.ac.at/dhataxonomy/Concept52>
  dc11:source "Wikipedia contributors, \"Annotation,\" Wikipedia, The Free Encyclopedia, https://en.wikipedia.org/w/index.php?title=Annotation&oldid=696830730 (accessed February 28, 2016)."@en ;
  dc:created "Thu Oct 01 00:00:00 CEST 2015"^^xsd:date ;
  skos:inScheme <https://vocabs.acdh.oeaw.ac.at/dhataxonomy/dhaTaxonomyScheme> ;
  skos:prefLabel "annotation"@en ;
  skos:definition "metadata (e.g. a comment, explanation, presentational markup) attached to text, image, or other data, both manual and automatic"@en ;
  skos:topConceptOf <https://vocabs.acdh.oeaw.ac.at/dhataxonomy/dhaTaxonomyScheme> ;
  a skos:Concept ;
  skos:notation "52"^^xsd:int ;
  dc:modified "Mon Jun 20 00:00:00 CEST 2016"^^xsd:date .

<https://vocabs.acdh.oeaw.ac.at/dhataxonomy/Concept31>
  skos:topConceptOf <https://vocabs.acdh.oeaw.ac.at/dhataxonomy/dhaTaxonomyScheme> ;
  a skos:Concept ;
  skos:inScheme <https://vocabs.acdh.oeaw.ac.at/dhataxonomy/dhaTaxonomyScheme> ;
  dc:created "Thu Oct 01 00:00:00 CEST 2015"^^xsd:date ;
  dc:modified "Mon Jun 20 00:00:00 CEST 2016"^^xsd:date ;
  skos:definition "the study, evaluation, and interpretation of literature"@en ;
  skos:prefLabel "literary studies"@en ;
  dc11:source "based on Wikipedia contributors, \"Literary criticism,\" Wikipedia, The Free Encyclopedia, https://en.wikipedia.org/w/index.php?title=Literary_criticism&oldid=704327390 (accessed February 28, 2016)."@en ;
  skos:notation "31"^^xsd:int .

<https://vocabs.acdh.oeaw.ac.at/dhataxonomy/Concept19>
  skos:topConceptOf <https://vocabs.acdh.oeaw.ac.at/dhataxonomy/dhaTaxonomyScheme> ;
  skos:inScheme <https://vocabs.acdh.oeaw.ac.at/dhataxonomy/dhaTaxonomyScheme> ;
  skos:definition "both the process and the product of planning, designing, and constructing buildings and other physical structures"@en ;
  skos:notation "19"^^xsd:int ;
  skos:prefLabel "architecture"@en ;
  a skos:Concept ;
  dc11:source "Wikipedia contributors, \"Architecture,\" Wikipedia, The Free Encyclopedia, https://en.wikipedia.org/w/index.php?title=Architecture&oldid=712664162 (accessed April 4, 2016)."@en ;
  dc:modified "Mon Jun 20 00:00:00 CEST 2016"^^xsd:date ;
  dc:created "Thu Oct 01 00:00:00 CEST 2015"^^xsd:date .

<https://vocabs.acdh.oeaw.ac.at/dhataxonomy/Concept64>
  skos:definition "publicly funded, publicly accountable institutions collecting and presenting cultural heritage materials"@en ;
  skos:inScheme <https://vocabs.acdh.oeaw.ac.at/dhataxonomy/dhaTaxonomyScheme> ;
  skos:altLabel "galleries, libraries, archives, and museums"@en ;
  dc:created "Thu Oct 01 00:00:00 CEST 2015"^^xsd:date ;
  skos:prefLabel "GLAM"@en ;
  dc:modified "Mon Jun 20 00:00:00 CEST 2016"^^xsd:date ;
  dc11:source "based on Wikipedia contributors, \"GLAM (industry sector),\" Wikipedia, The Free Encyclopedia, https://en.wikipedia.org/w/index.php?title=GLAM_(industry_sector)&oldid=699993792 (accessed February 28, 2016)."@en ;
  a skos:Concept ;
  skos:notation "64"^^xsd:int ;
  skos:topConceptOf <https://vocabs.acdh.oeaw.ac.at/dhataxonomy/dhaTaxonomyScheme> .

<https://vocabs.acdh.oeaw.ac.at/dhataxonomy/Concept56>
  skos:notation "56"^^xsd:int ;
  a skos:Concept ;
  dc:modified "Mon Jun 20 00:00:00 CEST 2016"^^xsd:date ;
  dc:created "Thu Oct 01 00:00:00 CEST 2015"^^xsd:date ;
  dc11:source "based on Wikipedia contributors, \"Semantic interoperability,\" Wikipedia, The Free Encyclopedia, https://en.wikipedia.org/w/index.php?title=Semantic_interoperability&oldid=706040693 (accessed February 28, 2016)."@en ;
  skos:topConceptOf <https://vocabs.acdh.oeaw.ac.at/dhataxonomy/dhaTaxonomyScheme> ;
  skos:inScheme <https://vocabs.acdh.oeaw.ac.at/dhataxonomy/dhaTaxonomyScheme> ;
  skos:narrower <https://vocabs.acdh.oeaw.ac.at/dhataxonomy/Concept56.01> ;
  skos:definition "ability of information systems to exchange data with unambiguous, shared meaning"@en ;
  skos:prefLabel "semantic interoperability"@en .

<https://vocabs.acdh.oeaw.ac.at/dhataxonomy/Concept13>
  a skos:Concept ;
  dc11:source "Wikipedia contributors, \"Theology,\" Wikipedia, The Free Encyclopedia, https://en.wikipedia.org/w/index.php?title=Theology&oldid=712002093 (accessed April 4, 2016)."@en ;
  skos:notation "13"^^xsd:int ;
  dc:modified "Mon Jun 20 00:00:00 CEST 2016"^^xsd:date ;
  skos:prefLabel "theology"@en ;
  skos:definition "the critical study of concepts of God and of the nature of religious ideas."@en ;
  dc:created "Thu Oct 01 00:00:00 CEST 2015"^^xsd:date ;
  skos:inScheme <https://vocabs.acdh.oeaw.ac.at/dhataxonomy/dhaTaxonomyScheme> ;
  skos:topConceptOf <https://vocabs.acdh.oeaw.ac.at/dhataxonomy/dhaTaxonomyScheme> .

<https://vocabs.acdh.oeaw.ac.at/dhataxonomy/Concept45>
  dc:created "Thu Oct 01 00:00:00 CEST 2015"^^xsd:date ;
  dc11:creator "ACDH-OEAW Team"@en ;
  a skos:Concept ;
  skos:prefLabel "search service"@en ;
  skos:topConceptOf <https://vocabs.acdh.oeaw.ac.at/dhataxonomy/dhaTaxonomyScheme> ;
  skos:narrower <https://vocabs.acdh.oeaw.ac.at/dhataxonomy/Concept45.01> ;
  skos:inScheme <https://vocabs.acdh.oeaw.ac.at/dhataxonomy/dhaTaxonomyScheme> ;
  skos:notation "45"^^xsd:int ;
  dc:modified "Mon Jun 20 00:00:00 CEST 2016"^^xsd:date ;
  skos:definition "service that allows to query a specific set of information resources"@en .

<https://vocabs.acdh.oeaw.ac.at/dhataxonomy/Concept39.04>
  skos:definition "a structured list of words or multi-word expressions providing reference information about their meaning, translations in other languages, pronunciation, origin, usage etc."@en ;
  skos:altLabel "dictionary"@en ;
  skos:notation "39.04"^^xsd:int ;
  skos:inScheme <https://vocabs.acdh.oeaw.ac.at/dhataxonomy/dhaTaxonomyScheme> ;
  skos:broader <https://vocabs.acdh.oeaw.ac.at/dhataxonomy/Concept39> ;
  skos:prefLabel "lexical resource"@en ;
  dc11:creator "ACDH-OEAW Team"@en ;
  a skos:Concept ;
  dc:modified "Mon Jun 20 00:00:00 CEST 2016"^^xsd:date ;
  dc:created "Thu Oct 01 00:00:00 CEST 2015"^^xsd:date .

<https://vocabs.acdh.oeaw.ac.at/dhataxonomy/Concept7.02>
  dc:created "Thu Oct 01 00:00:00 CEST 2015"^^xsd:date ;
  skos:altLabel "SPARQL Protocol and RDF Query Language"@en ;
  skos:broader <https://vocabs.acdh.oeaw.ac.at/dhataxonomy/Concept7> ;
  skos:notation "7.02"^^xsd:int ;
  skos:prefLabel "SPARQL"@en ;
  dc:modified "Mon Jun 20 00:00:00 CEST 2016"^^xsd:date ;
  skos:definition "query language for manipulating and retrieving data stored in RDF format"@en ;
  dc11:source "based on Wikipedia contributors, \"SPARQL,\" Wikipedia, The Free Encyclopedia, https://en.wikipedia.org/w/index.php?title=SPARQL&oldid=723415025 (accessed June 13, 2016)."@en ;
  a skos:Concept ;
  skos:inScheme <https://vocabs.acdh.oeaw.ac.at/dhataxonomy/dhaTaxonomyScheme> .

<https://vocabs.acdh.oeaw.ac.at/dhataxonomy/Concept65>
  dc:modified "Mon Jun 20 00:00:00 CEST 2016"^^xsd:date ;
  dc11:source "Wikipedia contributors, \"Cultural heritage,\" Wikipedia, The Free Encyclopedia, https://en.wikipedia.org/w/index.php?title=Cultural_heritage&oldid=703905866 (accessed February 29, 2016)."@en ;
  skos:definition "legacy of physical artifacts and intangible attributes of a group or society that are inherited from past generations, maintained in the present and bestowed for the benefit of future generations"@en ;
  dc:created "Thu Oct 01 00:00:00 CEST 2015"^^xsd:date ;
  skos:topConceptOf <https://vocabs.acdh.oeaw.ac.at/dhataxonomy/dhaTaxonomyScheme> ;
  skos:notation "65"^^xsd:int ;
  a skos:Concept ;
  skos:prefLabel "cultural heritage"@en ;
  skos:inScheme <https://vocabs.acdh.oeaw.ac.at/dhataxonomy/dhaTaxonomyScheme> .

<https://vocabs.acdh.oeaw.ac.at/dhataxonomy/Concept61>
  skos:definition "software free for use, distribution and improvements"@en ;
  a skos:Concept ;
  dc11:creator "ACDH-OEAW Team"@en ;
  skos:topConceptOf <https://vocabs.acdh.oeaw.ac.at/dhataxonomy/dhaTaxonomyScheme> ;
  skos:prefLabel "open source"@en ;
  skos:inScheme <https://vocabs.acdh.oeaw.ac.at/dhataxonomy/dhaTaxonomyScheme> ;
  skos:notation "61"^^xsd:int ;
  dc:created "Thu Oct 01 00:00:00 CEST 2015"^^xsd:date ;
  dc:modified "Mon Jun 20 00:00:00 CEST 2016"^^xsd:date .

<https://vocabs.acdh.oeaw.ac.at/dhataxonomy/Concept66.04>
  skos:prefLabel "DARIAH"@en ;
  dc:created "Thu Oct 01 00:00:00 CEST 2015"^^xsd:date ;
  skos:inScheme <https://vocabs.acdh.oeaw.ac.at/dhataxonomy/dhaTaxonomyScheme> ;
  skos:altLabel "Digital Research Infrastructure for the Arts and Humanities"@en ;
  skos:broader <https://vocabs.acdh.oeaw.ac.at/dhataxonomy/Concept66> ;
  skos:notation "66.04"^^xsd:int ;
  skos:definition "pan-european infrastructure for arts and humanities scholars working with computational methods"@en ;
  dc:modified "Mon Jun 20 00:00:00 CEST 2016"^^xsd:date ;
  dc11:source "based on DARIAH. Accessed June 13, 2016. https://dariah.eu/about/dariah-in-a-nutshell.html."@en ;
  a skos:Concept .

<https://vocabs.acdh.oeaw.ac.at/dhataxonomy/Concept28.02>
  skos:prefLabel "morphology"@en ;
  skos:inScheme <https://vocabs.acdh.oeaw.ac.at/dhataxonomy/dhaTaxonomyScheme> ;
  dc:created "Thu Oct 01 00:00:00 CEST 2015"^^xsd:date ;
  dc11:source "morphology. Oxford Dictionaries. Oxford University Press. http://www.oxforddictionaries.com/definition/english/morphology (accessed February 28, 2016)."@en ;
  a skos:Concept ;
  dc:modified "Mon Jun 20 00:00:00 CEST 2016"^^xsd:date ;
  skos:definition "the study of the forms of words"@en ;
  skos:broader <https://vocabs.acdh.oeaw.ac.at/dhataxonomy/Concept28> ;
  skos:notation "28.02"^^xsd:int .

<https://vocabs.acdh.oeaw.ac.at/dhataxonomy/Concept55>
  skos:definition "the body of terms used with a particular technical application in a subject of study, profession, etc."@en ;
  dc:created "Thu Nov 10 00:00:00 CET 2016"^^xsd:date ;
  skos:inScheme <https://vocabs.acdh.oeaw.ac.at/dhataxonomy/dhaTaxonomyScheme> ;
  skos:notation "55"^^xsd:int ;
  skos:topConceptOf <https://vocabs.acdh.oeaw.ac.at/dhataxonomy/dhaTaxonomyScheme> ;
  dc11:source "terminology. Oxford Dictionaries. Oxford University Press. https://en.oxforddictionaries.com/definition/terminology (accessed April 3, 2018)."@en ;
  skos:prefLabel "terminology"@en ;
  dc:modified "Tue Apr 03 00:00:00 CEST 2018"^^xsd:date ;
  a skos:Concept .

<https://vocabs.acdh.oeaw.ac.at/dhataxonomy/Concept36>
  dc11:source "geodata. Oxford Dictionaries. Oxford University Press. http://www.oxforddictionaries.com/definition/english/geodata (accessed February 28, 2016)."@en ;
  skos:definition "computerized geographical data"@en ;
  skos:prefLabel "geodata"@en ;
  a skos:Concept ;
  dc:modified "Mon Jun 20 00:00:00 CEST 2016"^^xsd:date ;
  dc:created "Thu Oct 01 00:00:00 CEST 2015"^^xsd:date ;
  skos:notation "36"^^xsd:int ;
  skos:topConceptOf <https://vocabs.acdh.oeaw.ac.at/dhataxonomy/dhaTaxonomyScheme> ;
  skos:inScheme <https://vocabs.acdh.oeaw.ac.at/dhataxonomy/dhaTaxonomyScheme> .

<https://vocabs.acdh.oeaw.ac.at/dhataxonomy/Concept43>
  dc11:creator "ACDH-OEAW Team"@en ;
  dc:modified "Mon Jun 20 00:00:00 CEST 2016"^^xsd:date ;
  a skos:Concept ;
  skos:notation "43"^^xsd:int ;
  dc:created "Thu Oct 01 00:00:00 CEST 2015"^^xsd:date ;
  skos:inScheme <https://vocabs.acdh.oeaw.ac.at/dhataxonomy/dhaTaxonomyScheme> ;
  skos:prefLabel "repository"@en ;
  skos:topConceptOf <https://vocabs.acdh.oeaw.ac.at/dhataxonomy/dhaTaxonomyScheme> ;
  skos:definition "service for depositing/preserving (and optionally presenting) resources"@en .

<https://vocabs.acdh.oeaw.ac.at/dhataxonomy/Concept21>
  dc:modified "Mon Jun 20 00:00:00 CEST 2016"^^xsd:date ;
  skos:inScheme <https://vocabs.acdh.oeaw.ac.at/dhataxonomy/dhaTaxonomyScheme> ;
  skos:notation "21"^^xsd:int ;
  skos:prefLabel "methods and statistics"@en ;
  skos:topConceptOf <https://vocabs.acdh.oeaw.ac.at/dhataxonomy/dhaTaxonomyScheme> ;
  a skos:Concept ;
  dc:created "Thu Oct 01 00:00:00 CEST 2015"^^xsd:date ;
  dc11:source "statistics. Oxford Dictionaries. Oxford University Press. http://www.oxforddictionaries.com/definition/english/statistics (accessed February 28, 2016)."@en ;
  skos:definition "the practice or science of collecting and analysing numerical data in large quantities"@en .

<https://vocabs.acdh.oeaw.ac.at/dhataxonomy/Concept50>
  skos:altLabel "Virtual research environment"@en ;
  skos:notation "50"^^xsd:int ;
  skos:inScheme <https://vocabs.acdh.oeaw.ac.at/dhataxonomy/dhaTaxonomyScheme> ;
  skos:definition "application integrating access to resources and a number of specialized functions, tailored to specific research methods, allowing collaborative work"@en ;
  dc11:creator "ACDH-OEAW Team"@en ;
  dc:created "Thu Oct 01 00:00:00 CEST 2015"^^xsd:date ;
  dc:modified "Mon Jun 20 00:00:00 CEST 2016"^^xsd:date ;
  a skos:Concept ;
  skos:prefLabel "VRE"@en ;
  skos:topConceptOf <https://vocabs.acdh.oeaw.ac.at/dhataxonomy/dhaTaxonomyScheme> .

<https://vocabs.acdh.oeaw.ac.at/dhataxonomy/Concept56.01>
  skos:definition "process of establishing pairwise semantic equivalencies (or other semantic relations) between distinct knowledge representations"@en ;
  skos:notation "56.01"^^xsd:int ;
  dc:created "Thu Oct 01 00:00:00 CEST 2015"^^xsd:date ;
  skos:inScheme <https://vocabs.acdh.oeaw.ac.at/dhataxonomy/dhaTaxonomyScheme> ;
  a skos:Concept ;
  skos:prefLabel "schema mapping"@en ;
  dc11:creator "ACDH-OEAW Team"@en ;
  skos:broader <https://vocabs.acdh.oeaw.ac.at/dhataxonomy/Concept56> ;
  dc:modified "Mon Jun 20 00:00:00 CEST 2016"^^xsd:date .

<https://vocabs.acdh.oeaw.ac.at/dhataxonomy/Collection06>
  a skos:Collection ;
  dc:modified "Tue Apr 03 00:00:00 CEST 2018"^^xsd:date ;
  dc11:title "Type"@en ;
  skos:prefLabel "Type"@en ;
  skos:scopeNote "This group contains resource type for an internal bibliography of digital humanities resources."@en ;
  dc11:creator "ACDH-OEAW Team"@en ;
  skos:member <https://vocabs.acdh.oeaw.ac.at/dhataxonomy/Concept72>, <https://vocabs.acdh.oeaw.ac.at/dhataxonomy/Concept73>, <https://vocabs.acdh.oeaw.ac.at/dhataxonomy/Concept74>, <https://vocabs.acdh.oeaw.ac.at/dhataxonomy/Concept71> ;
  dc:created "Tue Apr 03 00:00:00 CEST 2018"^^xsd:date .

<https://vocabs.acdh.oeaw.ac.at/dhataxonomy/Concept10>
  skos:prefLabel "political science"@en ;
  dc11:source "political science. Oxford Dictionaries. Oxford University Press. http://www.oxforddictionaries.com/definition/english/political-science (accessed February 28, 2016)."@en ;
  skos:topConceptOf <https://vocabs.acdh.oeaw.ac.at/dhataxonomy/dhaTaxonomyScheme> ;
  skos:inScheme <https://vocabs.acdh.oeaw.ac.at/dhataxonomy/dhaTaxonomyScheme> ;
  skos:definition "the branch of knowledge that deals with the state and systems of government"@en ;
  dc:created "Thu Oct 01 00:00:00 CEST 2015"^^xsd:date ;
  dc:modified "Mon Jun 20 00:00:00 CEST 2016"^^xsd:date ;
  a skos:Concept ;
  skos:notation "10"^^xsd:int .

<https://vocabs.acdh.oeaw.ac.at/dhataxonomy/Concept39.03>
  a skos:Concept ;
  dc11:creator "ACDH-OEAW Team"@en ;
  skos:broader <https://vocabs.acdh.oeaw.ac.at/dhataxonomy/Concept39> ;
  dc:modified "Mon Jun 20 00:00:00 CEST 2016"^^xsd:date ;
  skos:prefLabel "historical text"@en ;
  skos:notation "39.03"^^xsd:int ;
  skos:definition "any text created in the past"@en ;
  dc:created "Thu Oct 01 00:00:00 CEST 2015"^^xsd:date ;
  skos:inScheme <https://vocabs.acdh.oeaw.ac.at/dhataxonomy/dhaTaxonomyScheme> .

<https://vocabs.acdh.oeaw.ac.at/dhataxonomy/Concept63>
  skos:topConceptOf <https://vocabs.acdh.oeaw.ac.at/dhataxonomy/dhaTaxonomyScheme> ;
  dc11:creator "ACDH-OEAW Team"@en ;
  skos:inScheme <https://vocabs.acdh.oeaw.ac.at/dhataxonomy/dhaTaxonomyScheme> ;
  a skos:Concept ;
  skos:notation "63"^^xsd:int ;
  skos:prefLabel "programming"@en ;
  skos:definition "information about programming guides, tutorials, documentation"@en ;
  dc:created "Thu Oct 01 00:00:00 CEST 2015"^^xsd:date ;
  dc:modified "Mon Jun 20 00:00:00 CEST 2016"^^xsd:date .

<https://vocabs.acdh.oeaw.ac.at/dhataxonomy/Concept16>
  skos:topConceptOf <https://vocabs.acdh.oeaw.ac.at/dhataxonomy/dhaTaxonomyScheme> ;
  skos:inScheme <https://vocabs.acdh.oeaw.ac.at/dhataxonomy/dhaTaxonomyScheme> ;
  a skos:Concept ;
  skos:definition "the branch of knowledge concerned with the production, consumption, and transfer of wealth"@en ;
  skos:prefLabel "economics"@en ;
  skos:notation "16"^^xsd:int ;
  dc:modified "Mon Jun 20 00:00:00 CEST 2016"^^xsd:date ;
  dc:created "Thu Oct 01 00:00:00 CEST 2015"^^xsd:date ;
  dc11:source "economics. Oxford Dictionaries. Oxford University Press. http://www.oxforddictionaries.com/definition/english/economics (accessed February 28, 2016)."@en .

<https://vocabs.acdh.oeaw.ac.at/dhataxonomy/Concept66>
  skos:prefLabel "research infrastructure"@en ;
  skos:narrower <https://vocabs.acdh.oeaw.ac.at/dhataxonomy/Concept66.04>, <https://vocabs.acdh.oeaw.ac.at/dhataxonomy/Concept66.01>, <https://vocabs.acdh.oeaw.ac.at/dhataxonomy/Concept66.03>, <https://vocabs.acdh.oeaw.ac.at/dhataxonomy/Concept66.05>, <https://vocabs.acdh.oeaw.ac.at/dhataxonomy/Concept66.02> ;
  dc11:source "based on \"WHAT ARE RIs ?\" Research Infrastructures. Accessed June 13, 2016. http://ec.europa.eu/research/infrastructures/index_en.cfm?pg=what."@en ;
  dc:created "Thu Oct 01 00:00:00 CEST 2015"^^xsd:date ;
  skos:inScheme <https://vocabs.acdh.oeaw.ac.at/dhataxonomy/dhaTaxonomyScheme> ;
  skos:topConceptOf <https://vocabs.acdh.oeaw.ac.at/dhataxonomy/dhaTaxonomyScheme> ;
  a skos:Concept ;
  skos:definition "facilities, resources and related services used by the scientific community to conduct research"@en ;
  skos:notation "66"^^xsd:int ;
  dc:modified "Mon Jun 20 00:00:00 CEST 2016"^^xsd:date .

<https://vocabs.acdh.oeaw.ac.at/dhataxonomy/Concept48.01>
  skos:prefLabel "tokenisation"@en ;
  dc:created "Thu Oct 01 00:00:00 CEST 2015"^^xsd:date ;
  a skos:Concept ;
  skos:definition "process of breaking a stream of text up into words, phrases, symbols, or other meaningful elements called tokens"@en ;
  dc11:source "Wikipedia contributors, \"Tokenization (lexical analysis),\" Wikipedia, The Free Encyclopedia, https://en.wikipedia.org/w/index.php?title=Tokenization_(lexical_analysis)&oldid=637328355 (accessed February 28, 2016)."@en ;
  skos:notation "48.01"^^xsd:int ;
  skos:broader <https://vocabs.acdh.oeaw.ac.at/dhataxonomy/Concept48> ;
  dc:modified "Mon Jun 20 00:00:00 CEST 2016"^^xsd:date ;
  skos:inScheme <https://vocabs.acdh.oeaw.ac.at/dhataxonomy/dhaTaxonomyScheme> .

<https://vocabs.acdh.oeaw.ac.at/dhataxonomy/Concept44>
  a skos:Concept ;
  skos:prefLabel "sentiment analysis"@en ;
  dc11:source "based on sentiment analysis. Oxford Dictionaries. Oxford University Press. http://www.oxforddictionaries.com/definition/english/sentiment-analysis (accessed February 28, 2016)."@en ;
  skos:notation "44"^^xsd:int ;
  skos:definition "procedure of computationally identifying and categorizing opinions expressed in a piece of text"@en ;
  dc:modified "Mon Jun 20 00:00:00 CEST 2016"^^xsd:date ;
  dc:created "Thu Oct 01 00:00:00 CEST 2015"^^xsd:date ;
  skos:topConceptOf <https://vocabs.acdh.oeaw.ac.at/dhataxonomy/dhaTaxonomyScheme> ;
  skos:inScheme <https://vocabs.acdh.oeaw.ac.at/dhataxonomy/dhaTaxonomyScheme> .

<https://vocabs.acdh.oeaw.ac.at/dhataxonomy/Concept34>
  dc11:creator "ACDH-OEAW Team"@en ;
  skos:prefLabel "video recording"@en ;
  skos:topConceptOf <https://vocabs.acdh.oeaw.ac.at/dhataxonomy/dhaTaxonomyScheme> ;
  skos:inScheme <https://vocabs.acdh.oeaw.ac.at/dhataxonomy/dhaTaxonomyScheme> ;
  dc:created "Thu Oct 01 00:00:00 CEST 2015"^^xsd:date ;
  skos:definition "a digital representation of visual and acoustic signals"@en ;
  dc:modified "Mon Jun 20 00:00:00 CEST 2016"^^xsd:date ;
  skos:notation "34"^^xsd:int ;
  a skos:Concept .

<https://vocabs.acdh.oeaw.ac.at/dhataxonomy/Concept53.01>
  dc11:creator "ACDH-OEAW Team"@en ;
  skos:definition "digital tool with special functionalities for viewing and authoring data in XML"@en ;
  skos:notation "53.01"^^xsd:int ;
  skos:inScheme <https://vocabs.acdh.oeaw.ac.at/dhataxonomy/dhaTaxonomyScheme> ;
  dc:created "Thu Oct 01 00:00:00 CEST 2015"^^xsd:date ;
  skos:prefLabel "xml-editor"@en ;
  skos:broader <https://vocabs.acdh.oeaw.ac.at/dhataxonomy/Concept53> ;
  dc:modified "Mon Jun 20 00:00:00 CEST 2016"^^xsd:date ;
  a skos:Concept .

<https://vocabs.acdh.oeaw.ac.at/dhataxonomy/Concept54>
  skos:inScheme <https://vocabs.acdh.oeaw.ac.at/dhataxonomy/dhaTaxonomyScheme> ;
  skos:topConceptOf <https://vocabs.acdh.oeaw.ac.at/dhataxonomy/dhaTaxonomyScheme> ;
  skos:prefLabel "crowdsourcing"@en ;
  dc:created "Thu Oct 01 00:00:00 CEST 2015"^^xsd:date ;
  skos:notation "54"^^xsd:int ;
  dc:modified "Mon Jun 20 00:00:00 CEST 2016"^^xsd:date ;
  a skos:Concept ;
  dc11:source "based on Wikipedia contributors, \"Crowdsourcing,\" Wikipedia, The Free Encyclopedia, https://en.wikipedia.org/w/index.php?title=Crowdsourcing&oldid=707269325 (accessed February 28, 2016)."@en ;
  skos:definition "practice of solving a given (data processing) task by contributions from a large group of people via the Internet"@en .

<https://vocabs.acdh.oeaw.ac.at/dhataxonomy/Concept18>
  skos:notation "18"^^xsd:int ;
  skos:topConceptOf <https://vocabs.acdh.oeaw.ac.at/dhataxonomy/dhaTaxonomyScheme> ;
  skos:inScheme <https://vocabs.acdh.oeaw.ac.at/dhataxonomy/dhaTaxonomyScheme> ;
  a skos:Concept ;
  skos:prefLabel "communication studies"@en ;
  skos:definition "academic discipline that deals with processes of human communication"@en ;
  dc11:source "Wikipedia contributors, \"Communication studies,\" Wikipedia, The Free Encyclopedia, https://en.wikipedia.org/w/index.php?title=Communication_studies&oldid=705166533 (accessed February 28, 2016)."@en ;
  dc:created "Thu Oct 01 00:00:00 CEST 2015"^^xsd:date ;
  dc:modified "Mon Jun 20 00:00:00 CEST 2016"^^xsd:date .

<https://vocabs.acdh.oeaw.ac.at/dhataxonomy/Concept5>
  dc:created "Thu Oct 01 00:00:00 CEST 2015"^^xsd:date ;
  skos:inScheme <https://vocabs.acdh.oeaw.ac.at/dhataxonomy/dhaTaxonomyScheme> ;
  skos:topConceptOf <https://vocabs.acdh.oeaw.ac.at/dhataxonomy/dhaTaxonomyScheme> ;
  skos:notation "5"^^xsd:int ;
  skos:altLabel "Open Archival Information System"@en ;
  skos:definition "a system and a reference model for organisation of archival preservation and access to the digital information over the time"@en ;
  dc:modified "Mon Jun 20 00:00:00 CEST 2016"^^xsd:date ;
  a skos:Concept ;
  skos:prefLabel "OAIS"@en .

<https://vocabs.acdh.oeaw.ac.at/dhataxonomy/Concept9>
  skos:notation "9"^^xsd:int ;
  a skos:Concept ;
  dc:modified "Mon Jun 20 00:00:00 CEST 2016"^^xsd:date ;
  skos:definition "the scientific study of human society and social relationships"@en ;
  skos:prefLabel "social sciences"@en ;
  skos:inScheme <https://vocabs.acdh.oeaw.ac.at/dhataxonomy/dhaTaxonomyScheme> ;
  skos:topConceptOf <https://vocabs.acdh.oeaw.ac.at/dhataxonomy/dhaTaxonomyScheme> ;
  dc:created "Thu Oct 01 00:00:00 CEST 2015"^^xsd:date ;
  dc11:source "social science. Oxford Dictionaries. Oxford University Press. http://www.oxforddictionaries.com/definition/english/social-science (accessed February 28, 2016)."@en .

<https://vocabs.acdh.oeaw.ac.at/dhataxonomy/Concept72>
  skos:definition "groups of people such as organisations, research infrastructures, institutions, consortia, networks, etc."@en ;
  a skos:Concept ;
  dc11:creator "ACDH-OEAW Team"@en ;
  skos:notation "72"^^xsd:int ;
  dc:created "Thu Oct 01 00:00:00 CEST 2015"^^xsd:date ;
  skos:topConceptOf <https://vocabs.acdh.oeaw.ac.at/dhataxonomy/dhaTaxonomyScheme> ;
  skos:prefLabel "type_organisation"@en ;
  dc:modified "Mon Jun 20 00:00:00 CEST 2016"^^xsd:date ;
  skos:inScheme <https://vocabs.acdh.oeaw.ac.at/dhataxonomy/dhaTaxonomyScheme> .

<https://vocabs.acdh.oeaw.ac.at/dhataxonomy/Concept69>
  a skos:Concept ;
  skos:altLabel "biographies"@en ;
  skos:prefLabel "biographical data"@en ;
  dc11:source "based on Wikipedia contributors, \"Biography,\" Wikipedia, The Free Encyclopedia, https://en.wikipedia.org/w/index.php?title=Biography&oldid=832378964 (accessed April 3, 2018)."@en ;
  dc:created "Tue Apr 03 00:00:00 CEST 2018"^^xsd:date ;
  skos:topConceptOf <https://vocabs.acdh.oeaw.ac.at/dhataxonomy/dhaTaxonomyScheme> ;
  dc:modified "Tue Apr 03 00:00:00 CEST 2018"^^xsd:date ;
  skos:definition "a detailed description of a person's life that involves more than just the basic facts like education, work, relationships, and death; it portrays a person's experience of these life events"@en ;
  skos:notation "69"^^xsd:int ;
  skos:inScheme <https://vocabs.acdh.oeaw.ac.at/dhataxonomy/dhaTaxonomyScheme> .

<https://vocabs.acdh.oeaw.ac.at/dhataxonomy/Concept39.02>
  dc:created "Thu Oct 01 00:00:00 CEST 2015"^^xsd:date ;
  skos:definition "collections of texts (or just sentences) annotated with complete syntactic structure"@en ;
  skos:inScheme <https://vocabs.acdh.oeaw.ac.at/dhataxonomy/dhaTaxonomyScheme> ;
  a skos:Concept ;
  dc11:creator "ACDH-OEAW Team"@en ;
  dc:modified "Mon Jun 20 00:00:00 CEST 2016"^^xsd:date ;
  skos:notation "39.02"^^xsd:int ;
  skos:broader <https://vocabs.acdh.oeaw.ac.at/dhataxonomy/Concept39> ;
  skos:prefLabel "treebank"@en .

<https://vocabs.acdh.oeaw.ac.at/dhataxonomy/Concept12>
  skos:prefLabel "theatre studies"@en ;
  dc:created "Thu Oct 01 00:00:00 CEST 2015"^^xsd:date ;
  skos:inScheme <https://vocabs.acdh.oeaw.ac.at/dhataxonomy/dhaTaxonomyScheme> ;
  skos:topConceptOf <https://vocabs.acdh.oeaw.ac.at/dhataxonomy/dhaTaxonomyScheme> ;
  skos:notation "12"^^xsd:int ;
  skos:definition "the study of theatrical performance in relation to its literary, physical, psycho-biological, sociological, and historical contexts"@en ;
  dc:modified "Mon Jun 20 00:00:00 CEST 2016"^^xsd:date ;
  a skos:Concept ;
  dc11:source "Wikipedia contributors, \"Theatre studies,\" Wikipedia, The Free Encyclopedia, https://en.wikipedia.org/w/index.php?title=Theatre_studies&oldid=668409531 (accessed April 4, 2016)."@en .

<https://vocabs.acdh.oeaw.ac.at/dhataxonomy/Concept51>
  dc:created "Thu Oct 01 00:00:00 CEST 2015"^^xsd:date ;
  skos:inScheme <https://vocabs.acdh.oeaw.ac.at/dhataxonomy/dhaTaxonomyScheme> ;
  skos:definition "visual representation of data/information aimed at better ways of exploring the data"@en ;
  skos:narrower <https://vocabs.acdh.oeaw.ac.at/dhataxonomy/Concept51.01> ;
  skos:prefLabel "visualization"@en ;
  skos:topConceptOf <https://vocabs.acdh.oeaw.ac.at/dhataxonomy/dhaTaxonomyScheme> ;
  skos:notation "51"^^xsd:int ;
  dc:modified "Mon Jun 20 00:00:00 CEST 2016"^^xsd:date ;
  dc11:source "based on Wikipedia contributors, \"Data visualization,\" Wikipedia, The Free Encyclopedia, https://en.wikipedia.org/w/index.php?title=Data_visualization&oldid=706343042 (accessed February 28, 2016)."@en ;
  a skos:Concept .

<https://vocabs.acdh.oeaw.ac.at/dhataxonomy/Concept1>
  dc:created "Thu Oct 01 00:00:00 CEST 2015"^^xsd:date ;
  skos:prefLabel "XML"@en ;
  skos:altLabel "Extensible Markup Language"@en ;
  dc11:source "based on Wikipedia contributors, \"XML\", Wikipedia, The Free Encyclopedia, https://en.wikipedia.org/w/index.php?title=XML&oldid=724493259 (accessed June 13, 2016)."@en ;
  skos:notation "1"^^xsd:int ;
  dc:modified "Mon Jun 20 00:00:00 CEST 2016"^^xsd:date ;
  skos:inScheme <https://vocabs.acdh.oeaw.ac.at/dhataxonomy/dhaTaxonomyScheme> ;
  skos:definition "a W3C-standardised markup system that defines a set of rules for encoding digital documents"@en ;
  skos:topConceptOf <https://vocabs.acdh.oeaw.ac.at/dhataxonomy/dhaTaxonomyScheme> ;
  a skos:Concept .

<https://vocabs.acdh.oeaw.ac.at/dhataxonomy/Concept25>
  a skos:Concept ;
  skos:prefLabel "geography"@en ;
  dc:modified "Mon Jun 20 00:00:00 CEST 2016"^^xsd:date ;
  skos:notation "25"^^xsd:int ;
  skos:definition "the study of the physical features of the earth and its atmosphere, and of human activity as it affects and is affected by these"@en ;
  dc11:source "geography. Oxford Dictionaries. Oxford University Press. http://www.oxforddictionaries.com/definition/english/geography (accessed February 28, 2016)."@en ;
  skos:inScheme <https://vocabs.acdh.oeaw.ac.at/dhataxonomy/dhaTaxonomyScheme> ;
  skos:topConceptOf <https://vocabs.acdh.oeaw.ac.at/dhataxonomy/dhaTaxonomyScheme> ;
  dc:created "Thu Oct 01 00:00:00 CEST 2015"^^xsd:date .

<https://vocabs.acdh.oeaw.ac.at/dhataxonomy/Concept15>
  a skos:Concept ;
  dc:modified "Mon Jun 20 00:00:00 CEST 2016"^^xsd:date ;
  dc:created "Thu Oct 01 00:00:00 CEST 2015"^^xsd:date ;
  skos:notation "15"^^xsd:int ;
  dc11:source "demography. Oxford Dictionaries. Oxford University Press. http://www.oxforddictionaries.com/definition/english/demography (accessed February 28, 2016)."@en ;
  skos:definition "the study of statistics which illustrate the changing structure of human populations"@en ;
  skos:inScheme <https://vocabs.acdh.oeaw.ac.at/dhataxonomy/dhaTaxonomyScheme> ;
  skos:topConceptOf <https://vocabs.acdh.oeaw.ac.at/dhataxonomy/dhaTaxonomyScheme> ;
  skos:prefLabel "demography"@en .

<https://vocabs.acdh.oeaw.ac.at/dhataxonomy/Concept66.01>
  dc:created "Thu Oct 01 00:00:00 CEST 2015"^^xsd:date ;
  skos:broader <https://vocabs.acdh.oeaw.ac.at/dhataxonomy/Concept66> ;
  skos:altLabel "Pooling Activities, Resources and Tools for Heritage E-research Networking, Optimization and Synergies"@en ;
  skos:inScheme <https://vocabs.acdh.oeaw.ac.at/dhataxonomy/dhaTaxonomyScheme> ;
  skos:definition "European cluster infrastucture H2020 project that aims to pool and harmonize the activities in existing research infrastructures  and strengthen the cohesion of research in the broad sector of Linguistic Studies, Humanities, Cultural Heritage, History, Archaeology and related fields"@en ;
  skos:prefLabel "PARTHENOS"@en ;
  dc11:source "based on PARTHENOS. Accessed June 13, 2016. http://www.parthenos-project.eu/."@en ;
  a skos:Concept ;
  dc:modified "Mon Jun 20 00:00:00 CEST 2016"^^xsd:date ;
  skos:notation "66.01"^^xsd:int .

<https://vocabs.acdh.oeaw.ac.at/dhataxonomy/Concept57>
  skos:prefLabel "copyright and licensing"@en ;
  skos:definition "information about rights and conditions of use and distribution of resources"@en ;
  dc:created "Thu Oct 01 00:00:00 CEST 2015"^^xsd:date ;
  skos:inScheme <https://vocabs.acdh.oeaw.ac.at/dhataxonomy/dhaTaxonomyScheme> ;
  skos:notation "57"^^xsd:int ;
  skos:topConceptOf <https://vocabs.acdh.oeaw.ac.at/dhataxonomy/dhaTaxonomyScheme> ;
  a skos:Concept ;
  dc11:creator "ACDH-OEAW Team"@en ;
  dc:modified "Mon Jun 20 00:00:00 CEST 2016"^^xsd:date .

<https://vocabs.acdh.oeaw.ac.at/dhataxonomy/Concept3>
  skos:notation "3"^^xsd:int ;
  a skos:Concept ;
  skos:narrower <https://vocabs.acdh.oeaw.ac.at/dhataxonomy/Concept3.01>, <https://vocabs.acdh.oeaw.ac.at/dhataxonomy/Concept3.02>, <https://vocabs.acdh.oeaw.ac.at/dhataxonomy/Concept3.03>, <https://vocabs.acdh.oeaw.ac.at/dhataxonomy/Concept3.04> ;
  dc:modified "Mon Jun 20 00:00:00 CEST 2016"^^xsd:date ;
  skos:definition "machine-readable terminologies that define concepts and relationships used to describe and organize data on the web"@en ;
  skos:inScheme <https://vocabs.acdh.oeaw.ac.at/dhataxonomy/dhaTaxonomyScheme> ;
  dc11:source "based on \"Vocabularies.\" W3C. Accessed June 13, 2016. https://www.w3.org/standards/semanticweb/ontology."@en ;
  skos:topConceptOf <https://vocabs.acdh.oeaw.ac.at/dhataxonomy/dhaTaxonomyScheme> ;
  dc:created "Thu Oct 01 00:00:00 CEST 2015"^^xsd:date ;
  skos:prefLabel "semantic web vocabularies"@en .

<https://vocabs.acdh.oeaw.ac.at/dhataxonomy/Concept6>
  dc:modified "Mon Jun 20 00:00:00 CEST 2016"^^xsd:date ;
  skos:inScheme <https://vocabs.acdh.oeaw.ac.at/dhataxonomy/dhaTaxonomyScheme> ;
  dc11:source "based on metadata. Oxford Dictionaries. Oxford University Press. http://www.oxforddictionaries.com/definition/english/metadata (accessed February 28, 2016)."@en ;
  skos:definition "data about data, structured information that describes an information resource"@en ;
  skos:notation "6"^^xsd:int ;
  skos:topConceptOf <https://vocabs.acdh.oeaw.ac.at/dhataxonomy/dhaTaxonomyScheme> ;
  a skos:Concept ;
  dc:created "Thu Oct 01 00:00:00 CEST 2015"^^xsd:date ;
  skos:prefLabel "metadata"@en ;
  skos:narrower <https://vocabs.acdh.oeaw.ac.at/dhataxonomy/Concept6.01> .

<https://vocabs.acdh.oeaw.ac.at/dhataxonomy/Concept66.05>
  dc11:source "based on Europeana. Accessed June 13, 2016. http://www.europeana.eu/portal/."@en ;
  skos:definition "multi-lingual online collection of millions of digitised items from European museums, libraries, archives and multi-media collections"@en ;
  skos:prefLabel "Europeana"@en ;
  a skos:Concept ;
  skos:inScheme <https://vocabs.acdh.oeaw.ac.at/dhataxonomy/dhaTaxonomyScheme> ;
  skos:notation "66.05"^^xsd:int ;
  dc:created "Thu Oct 01 00:00:00 CEST 2015"^^xsd:date ;
  dc:modified "Mon Jun 20 00:00:00 CEST 2016"^^xsd:date ;
  skos:broader <https://vocabs.acdh.oeaw.ac.at/dhataxonomy/Concept66> .

<https://vocabs.acdh.oeaw.ac.at/dhataxonomy/Concept68>
  skos:definition "the process of converting information into a digital (i.e. computer-readable) format, in which the information is organized into bits"@en ;
  skos:inScheme <https://vocabs.acdh.oeaw.ac.at/dhataxonomy/dhaTaxonomyScheme> ;
  skos:prefLabel "digitisation"@en ;
  dc11:source "Wikipedia contributors, \"Digitization,\" Wikipedia, The Free Encyclopedia, https://en.wikipedia.org/w/index.php?title=Digitization&oldid=818105832 (accessed February 8, 2018)."@en ;
  skos:notation "68"^^xsd:int ;
  dc:modified "Tue Apr 03 00:00:00 CEST 2018"^^xsd:date ;
  dc:created "Tue Apr 03 00:00:00 CEST 2018"^^xsd:date ;
  skos:topConceptOf <https://vocabs.acdh.oeaw.ac.at/dhataxonomy/dhaTaxonomyScheme> ;
  a skos:Concept .

<https://vocabs.acdh.oeaw.ac.at/dhataxonomy/Concept40.04>
  a skos:Concept ;
  skos:broader <https://vocabs.acdh.oeaw.ac.at/dhataxonomy/Concept40> ;
  skos:prefLabel "knowledge base"@en ;
  skos:notation "40.04"^^xsd:int ;
  dc11:source "based on Wikipedia contributors, \"Knowledge base,\" Wikipedia, The Free Encyclopedia, https://en.wikipedia.org/w/index.php?title=Knowledge_base&oldid=718798303 (accessed June 13, 2016)."@en ;
  dc:modified "Mon Jun 20 00:00:00 CEST 2016"^^xsd:date ;
  skos:definition "complex information resource that consists of structured and unstructured data to be used in digital applications"@en ;
  dc:created "Thu Oct 01 00:00:00 CEST 2015"^^xsd:date ;
  skos:inScheme <https://vocabs.acdh.oeaw.ac.at/dhataxonomy/dhaTaxonomyScheme> .

<https://vocabs.acdh.oeaw.ac.at/dhataxonomy/Concept48.06>
  skos:broader <https://vocabs.acdh.oeaw.ac.at/dhataxonomy/Concept48> ;
  skos:notation "48.06"^^xsd:int ;
  dc:modified "Mon Jun 20 00:00:00 CEST 2016"^^xsd:date ;
  a skos:Concept ;
  dc11:source "Wikipedia contributors, \"Entity linking,\" Wikipedia, The Free Encyclopedia, https://en.wikipedia.org/w/index.php?title=Entity_linking&oldid=833222865 (accessed April 3, 2018)."@en ;
  dc:created "Thu Oct 01 00:00:00 CEST 2015"^^xsd:date ;
  skos:inScheme <https://vocabs.acdh.oeaw.ac.at/dhataxonomy/dhaTaxonomyScheme> ;
  skos:definition "task of determining the identity of entities mentioned in text that requires a knowldge base containing the netities to which entity mentions can be linked"@en ;
  skos:prefLabel "entity linking"@en ;
  skos:altLabel "Named Entity Linking"@en .

<https://vocabs.acdh.oeaw.ac.at/dhataxonomy/Concept66.02>
  dc:modified "Mon Jun 20 00:00:00 CEST 2016"^^xsd:date ;
  skos:inScheme <https://vocabs.acdh.oeaw.ac.at/dhataxonomy/dhaTaxonomyScheme> ;
  skos:notation "66.02"^^xsd:int ;
  a skos:Concept ;
  skos:altLabel "Common LAnguage Resources and Technology INfrastructure"@en ;
  skos:prefLabel "CLARIN"@en ;
  dc:created "Thu Oct 01 00:00:00 CEST 2015"^^xsd:date ;
  dc11:source "based on CLARIN. Accessed June 13, 2016.  https://www.clarin.eu/"@en ;
  skos:definition "European research infrastructure for the Humanities and Social Sciences, focusing on language resources (data and tools)"@en ;
  skos:broader <https://vocabs.acdh.oeaw.ac.at/dhataxonomy/Concept66> .

<https://vocabs.acdh.oeaw.ac.at/dhataxonomy/Concept24>
  skos:definition "the academic field of study that embraces Near Eastern and Far Eastern societies and cultures, languages, peoples, history and archaeology"@en ;
  a skos:Concept ;
  dc:modified "Mon Jun 20 00:00:00 CEST 2016"^^xsd:date ;
  skos:notation "24"^^xsd:int ;
  dc:created "Thu Oct 01 00:00:00 CEST 2015"^^xsd:date ;
  dc11:source "Wikipedia contributors, \"Oriental studies,\" Wikipedia, The Free Encyclopedia, https://en.wikipedia.org/w/index.php?title=Oriental_studies&oldid=706288051 (accessed February 28, 2016)."@en ;
  skos:prefLabel "oriental studies"@en ;
  skos:topConceptOf <https://vocabs.acdh.oeaw.ac.at/dhataxonomy/dhaTaxonomyScheme> ;
  skos:inScheme <https://vocabs.acdh.oeaw.ac.at/dhataxonomy/dhaTaxonomyScheme> .

<https://vocabs.acdh.oeaw.ac.at/dhataxonomy/Concept29>
  dc11:source "archaeology. Oxford Dictionaries. Oxford University Press. http://www.oxforddictionaries.com/definition/english/archaeology (accessed February 28, 2016)."@en ;
  skos:prefLabel "archaeology"@en ;
  dc:modified "Mon Jun 20 00:00:00 CEST 2016"^^xsd:date ;
  skos:notation "29"^^xsd:int ;
  a skos:Concept ;
  skos:inScheme <https://vocabs.acdh.oeaw.ac.at/dhataxonomy/dhaTaxonomyScheme> ;
  skos:topConceptOf <https://vocabs.acdh.oeaw.ac.at/dhataxonomy/dhaTaxonomyScheme> ;
  skos:definition "the study of human history and prehistory through the excavation of sites and the analysis of artefacts and other physical remains"@en ;
  dc:created "Thu Oct 01 00:00:00 CEST 2015"^^xsd:date .

<https://vocabs.acdh.oeaw.ac.at/dhataxonomy/Concept26>
  skos:notation "26"^^xsd:int ;
  dc11:source "Wikipedia contributors, \"Philosophy,\" Wikipedia, The Free Encyclopedia, https://en.wikipedia.org/w/index.php?title=Philosophy&oldid=712469925 (accessed April 4, 2016)."@en ;
  skos:definition "the study of general and fundamental problems concerning matters such as existence, knowledge, values, reason, mind, and language"@en ;
  skos:inScheme <https://vocabs.acdh.oeaw.ac.at/dhataxonomy/dhaTaxonomyScheme> ;
  skos:prefLabel "philosophy"@en ;
  a skos:Concept ;
  skos:topConceptOf <https://vocabs.acdh.oeaw.ac.at/dhataxonomy/dhaTaxonomyScheme> ;
  dc:created "Thu Oct 01 00:00:00 CEST 2015"^^xsd:date ;
  dc:modified "Mon Jun 20 00:00:00 CEST 2016"^^xsd:date .

<https://vocabs.acdh.oeaw.ac.at/dhataxonomy/Concept22>
  dc11:source "law. Oxford Dictionaries. Oxford University Press. http://www.oxforddictionaries.com/definition/english/law (accessed February 28, 2016)."@en ;
  skos:inScheme <https://vocabs.acdh.oeaw.ac.at/dhataxonomy/dhaTaxonomyScheme> ;
  skos:definition "systems of law as a subject of study or as the basis of the legal profession"@en ;
  dc:modified "Mon Jun 20 00:00:00 CEST 2016"^^xsd:date ;
  skos:prefLabel "law"@en ;
  dc:created "Thu Oct 01 00:00:00 CEST 2015"^^xsd:date ;
  skos:topConceptOf <https://vocabs.acdh.oeaw.ac.at/dhataxonomy/dhaTaxonomyScheme> ;
  a skos:Concept ;
  skos:notation "22"^^xsd:int .

<https://vocabs.acdh.oeaw.ac.at/dhataxonomy/Concept39>
  dc:modified "Mon Jun 20 00:00:00 CEST 2016"^^xsd:date ;
  skos:notation "39"^^xsd:int ;
  skos:narrower <https://vocabs.acdh.oeaw.ac.at/dhataxonomy/Concept39.02>, <https://vocabs.acdh.oeaw.ac.at/dhataxonomy/Concept39.05>, <https://vocabs.acdh.oeaw.ac.at/dhataxonomy/Concept39.01>, <https://vocabs.acdh.oeaw.ac.at/dhataxonomy/Concept39.04>, <https://vocabs.acdh.oeaw.ac.at/dhataxonomy/Concept39.03> ;
  dc:created "Thu Oct 01 00:00:00 CEST 2015"^^xsd:date ;
  skos:topConceptOf <https://vocabs.acdh.oeaw.ac.at/dhataxonomy/dhaTaxonomyScheme> ;
  a skos:Concept ;
  skos:inScheme <https://vocabs.acdh.oeaw.ac.at/dhataxonomy/dhaTaxonomyScheme> ;
  skos:prefLabel "language resource"@en ;
  dc11:source "Simons, G. F., and Bird, S. “Toward a Global Infrastructure for the Sustainability of Language Resources.” Proceedings of 22nd Pacific Asia Conference on Language, Information and Computation, 20–22 November 2008, Cebu City, Philippines. Accessed March 30, 2016. http://www-01.sil.org/~simonsg/preprint/PACLIC22.pdf."@en ;
  skos:definition "a language  resource  is  any  physical  or  digital  item  that  is  a  product  of  language  documentation,  description,  or  development  or  is  a  tool  that  specifically  supports  the creation and use of such products"@en .

<https://vocabs.acdh.oeaw.ac.at/dhataxonomy/Concept59.01>
  dc:modified "Mon Jun 20 00:00:00 CEST 2016"^^xsd:date ;
  skos:notation "59.01"^^xsd:int ;
  a skos:Concept ;
  dc:created "Thu Oct 01 00:00:00 CEST 2015"^^xsd:date ;
  dc11:source "Wikipedia contributors, \"Linked data,\" Wikipedia, The Free Encyclopedia, https://en.wikipedia.org/w/index.php?title=Linked_data&oldid=701965470 (accessed February 28, 2016)."@en ;
  skos:definition "method of publishing structured data so that it can be interlinked and become more useful through semantic queries"@en ;
  skos:prefLabel "Linked data"@en ;
  skos:broader <https://vocabs.acdh.oeaw.ac.at/dhataxonomy/Concept59> ;
  skos:inScheme <https://vocabs.acdh.oeaw.ac.at/dhataxonomy/dhaTaxonomyScheme> .

<https://vocabs.acdh.oeaw.ac.at/dhataxonomy/Concept42>
  skos:topConceptOf <https://vocabs.acdh.oeaw.ac.at/dhataxonomy/dhaTaxonomyScheme> ;
  a skos:Concept ;
  skos:inScheme <https://vocabs.acdh.oeaw.ac.at/dhataxonomy/dhaTaxonomyScheme> ;
  skos:notation "42"^^xsd:int ;
  dc11:source "Patrick Sahle. \"About a catalog of: Digital Scholarly Editions, v 3.0, Snapshot 2008ff.\" Scholarly Digital Editions. 2008. Accessed June 13, 2016. http://www.digitale-edition.de/vlet-about.html."@en ;
  dc:created "Thu Oct 01 00:00:00 CEST 2015"^^xsd:date ;
  dc:modified "Mon Jun 20 00:00:00 CEST 2016"^^xsd:date ;
  skos:prefLabel "digital edition"@en ;
  skos:definition "a scholarly edition is the critical representation of historical documents"@en .

<https://vocabs.acdh.oeaw.ac.at/dhataxonomy/Concept48.05>
  skos:notation "48.05"^^xsd:int ;
  skos:prefLabel "NER"@en ;
  skos:definition "process of identifying mentions of individuals/entities in a text"@en ;
  skos:inScheme <https://vocabs.acdh.oeaw.ac.at/dhataxonomy/dhaTaxonomyScheme> ;
  skos:altLabel "Named Entity Recognition"@en ;
  dc:modified "Mon Jun 20 00:00:00 CEST 2016"^^xsd:date ;
  a skos:Concept ;
  dc:created "Thu Oct 01 00:00:00 CEST 2015"^^xsd:date ;
  skos:broader <https://vocabs.acdh.oeaw.ac.at/dhataxonomy/Concept48> ;
  dc11:creator "ACDH-OEAW Team"@en .

<https://vocabs.acdh.oeaw.ac.at/dhataxonomy/Concept20>
  dc11:source "based on art history. Oxford Dictionaries. Oxford University Press. http://www.oxforddictionaries.com/definition/english/art-history (accessed February 28, 2016)."@en ;
  skos:inScheme <https://vocabs.acdh.oeaw.ac.at/dhataxonomy/dhaTaxonomyScheme> ;
  dc:created "Thu Oct 01 00:00:00 CEST 2015"^^xsd:date ;
  skos:prefLabel "art studies"@en ;
  skos:topConceptOf <https://vocabs.acdh.oeaw.ac.at/dhataxonomy/dhaTaxonomyScheme> ;
  a skos:Concept ;
  skos:definition "the academic study of the history and development of visual arts"@en ;
  skos:notation "20"^^xsd:int ;
  dc:modified "Mon Jun 20 00:00:00 CEST 2016"^^xsd:date .

<https://vocabs.acdh.oeaw.ac.at/dhataxonomy/Concept67.01>
  skos:broader <https://vocabs.acdh.oeaw.ac.at/dhataxonomy/Concept67> ;
  dc:modified "Tue Apr 03 00:00:00 CEST 2018"^^xsd:date ;
  skos:notation "67.01"^^xsd:int ;
  skos:definition "research data management concerns the organisation of data, from its entry to the research cycle through to the dissemination and archiving of valuable results"@en ;
  dc11:source "Whyte, A., Tedds, J. (2011). ‘Making the Case for Research Data Management’. DCC Briefing Papers. Edinburgh: Digital Curation Centre. Available online: http://www.dcc.ac.uk/resources/briefing-papers"@en ;
  skos:inScheme <https://vocabs.acdh.oeaw.ac.at/dhataxonomy/dhaTaxonomyScheme> ;
  a skos:Concept ;
  skos:prefLabel "research data management"@en ;
  dc:created "Tue Apr 03 00:00:00 CEST 2018"^^xsd:date .

<https://vocabs.acdh.oeaw.ac.at/dhataxonomy/Concept48.02>
  a skos:Concept ;
  skos:notation "48.02"^^xsd:int ;
  dc11:creator "ACDH-OEAW Team"@en ;
  dc:modified "Mon Jun 20 00:00:00 CEST 2016"^^xsd:date ;
  skos:broader <https://vocabs.acdh.oeaw.ac.at/dhataxonomy/Concept48> ;
  skos:prefLabel "tagging"@en ;
  skos:definition "the assignment of descriptive labels (from a defined vocabulary) to particular segments of text, such as (but not only) word-class identifiers to tokens"@en ;
  dc:created "Thu Oct 01 00:00:00 CEST 2015"^^xsd:date ;
  skos:inScheme <https://vocabs.acdh.oeaw.ac.at/dhataxonomy/dhaTaxonomyScheme> .

<https://vocabs.acdh.oeaw.ac.at/dhataxonomy/Concept2.02>
  dc11:source "\"TEI: Text Encoding Initiative.\" TEI: Text Encoding Initiative. Accessed June 13, 2016. http://www.tei-c.org/index.xml."@en ;
  skos:inScheme <https://vocabs.acdh.oeaw.ac.at/dhataxonomy/dhaTaxonomyScheme> ;
  dc:created "Thu Oct 01 00:00:00 CEST 2015"^^xsd:date ;
  skos:broader <https://vocabs.acdh.oeaw.ac.at/dhataxonomy/Concept2> ;
  skos:definition "a set of guidelines which specify encoding methods for machine-readable texts, chiefly in the humanities, social sciences and linguistics"@en ;
  a skos:Concept ;
  dc:modified "Mon Jun 20 00:00:00 CEST 2016"^^xsd:date ;
  skos:prefLabel "TEI"@en ;
  skos:altLabel "Text Encoding Initiative"@en ;
  skos:notation "2.02"^^xsd:int .

<https://vocabs.acdh.oeaw.ac.at/dhataxonomy/Concept48.04>
  skos:definition "process of analysing the syntactic structures of a written (natural language) text"@en ;
  dc11:creator "ACDH-OEAW Team"@en ;
  a skos:Concept ;
  dc:created "Thu Oct 01 00:00:00 CEST 2015"^^xsd:date ;
  skos:inScheme <https://vocabs.acdh.oeaw.ac.at/dhataxonomy/dhaTaxonomyScheme> ;
  skos:notation "48.04"^^xsd:int ;
  skos:prefLabel "parsing"@en ;
  skos:broader <https://vocabs.acdh.oeaw.ac.at/dhataxonomy/Concept48> ;
  dc:modified "Mon Jun 20 00:00:00 CEST 2016"^^xsd:date .

<https://vocabs.acdh.oeaw.ac.at/dhataxonomy/Concept40.01>
  skos:notation "40.01"^^xsd:int ;
  dc:modified "Mon Jun 20 00:00:00 CEST 2016"^^xsd:date ;
  a skos:Concept ;
  skos:definition "hierarchical classification of entities of interest"@en ;
  skos:broader <https://vocabs.acdh.oeaw.ac.at/dhataxonomy/Concept40> ;
  dc11:source "Wikipedia contributors, \"Corporate taxonomy,\" Wikipedia, The Free Encyclopedia, https://en.wikipedia.org/w/index.php?title=Corporate_taxonomy&oldid=702154777 (accessed February 28, 2016)."@en ;
  skos:prefLabel "taxonomy"@en ;
  skos:inScheme <https://vocabs.acdh.oeaw.ac.at/dhataxonomy/dhaTaxonomyScheme> ;
  dc:created "Thu Oct 01 00:00:00 CEST 2015"^^xsd:date .